<?xml version="1.0" encoding="UTF-8"?>
<rdf:RDF xmlns:foaf="http://xmlns.com/foaf/0.1/"
         xmlns:skos="http://www.w3.org/2004/02/skos/core#"
         xmlns:dc="http://purl.org/dc/elements/1.1/"
         xmlns:dct="http://purl.org/dc/terms/"
         xmlns:gml="http://www.opengis.net/gml"
         xmlns:rdf="http://www.w3.org/1999/02/22-rdf-syntax-ns#">
   <skos:ConceptScheme rdf:about="5cc12a4f-6784-372a-801a-09d227bc67c4:conceptscheme:1.0">
      <dc:identifier>5cc12a4f-6784-372a-801a-09d227bc67c4</dc:identifier>
      <dc:title>Australian Ocean Data Network analysis method register</dc:title>
      <dc:description>This register contains controlled vocabulary for analysis method and sample preparation that will ultimately be available in MCP metadata. The controlled vocabulary will be used by the faceted search on the AODN/IMOS portal.</dc:description>
      <dc:URI>http://vocab.aodn.org.au/Australian Ocean Data Network analysis method register/1.0</dc:URI>
      <dct:modified>2013-07-29</dct:modified>
      <dct:modified>2013-07-29</dct:modified>
      <dc:creator>
         <foaf:Organization>
            <foaf:name>eMarine Information Infrastructure</foaf:name>
         </foaf:Organization>
         <foaf:Organization>
            <foaf:name>eMarine Information Infrastructure</foaf:name>
         </foaf:Organization>
      </dc:creator>
      <dc:publisher>
         <foaf:Organization>
            <foaf:name>eMarine Information Infrastructure</foaf:name>
         </foaf:Organization>
      </dc:publisher>
      <dct:issued>2015-11-17T17:02:31</dct:issued>
   </skos:ConceptScheme>
   <skos:Concept rdf:about="5cc12a4f-6784-372a-801a-09d227bc67c4:concept:476">
      <skos:prefLabel xml:lang="en">filtration and acetone extraction</skos:prefLabel>
      <skos:inScheme rdf:resource="5cc12a4f-6784-372a-801a-09d227bc67c4:conceptscheme:1.0"/>
      <skos:definition xml:lang="en">Physical separation of the solid phase from a volume of water or air before the solid phase was mixed with acidified acetone to extract soluble compounds, usually plant pigments.</skos:definition>
      <skos:scopeNote xml:lang="en">filtration and acetone extraction: Physical separation of the solid phase from a volume of water or air before the solid phase was mixed with acidified acetone to extract soluble compounds, usually plant pigments.</skos:scopeNote>
   </skos:Concept>
   <skos:Concept rdf:about="5cc12a4f-6784-372a-801a-09d227bc67c4:concept:477">
      <skos:prefLabel xml:lang="en">high performance liquid chromatography (HPLC)</skos:prefLabel>
      <skos:inScheme rdf:resource="5cc12a4f-6784-372a-801a-09d227bc67c4:conceptscheme:1.0"/>
      <skos:definition xml:lang="en">A chromatographic technique for separating and analysing mixtures of substances, using a packed column containing microspheres coated with the stationary phase and where the mobile phase is pumped through the column with a high pressure pump. The emergence of each component of the sample under analysis from the column is monitored using one of a number of different detectors.</skos:definition>
      <skos:scopeNote xml:lang="en">high performance liquid chromatography (HPLC): A chromatographic technique for separating and analysing mixtures of substances, using a packed column containing microspheres coated with the stationary phase and where the mobile phase is pumped through the column with a high pressure pump. The emergence of each component of the sample under analysis from the column is monitored using one of a number of different detectors.</skos:scopeNote>
   </skos:Concept>
   <skos:Concept rdf:about="5cc12a4f-6784-372a-801a-09d227bc67c4:concept:479">
      <skos:prefLabel xml:lang="en">equilibration with air, drying</skos:prefLabel>
      <skos:inScheme rdf:resource="5cc12a4f-6784-372a-801a-09d227bc67c4:conceptscheme:1.0"/>
      <skos:definition xml:lang="en">The dissolved gas content of the sample (water or sediment incorporating pore water) was brought into equilibrium with a restricted volume of air which was subsequently dried and analysed, giving the composition of the sample dissolved gas phase.</skos:definition>
      <skos:scopeNote xml:lang="en">equilibration with air, drying: The dissolved gas content of the sample (water or sediment incorporating pore water) was brought into equilibrium with a restricted volume of air which was subsequently dried and analysed, giving the composition of the sample dissolved gas phase.</skos:scopeNote>
   </skos:Concept>
   <skos:Concept rdf:about="5cc12a4f-6784-372a-801a-09d227bc67c4:concept:480">
      <skos:prefLabel xml:lang="en">constant temperature non-dispersive infra-red gas analysis</skos:prefLabel>
      <skos:inScheme rdf:resource="5cc12a4f-6784-372a-801a-09d227bc67c4:conceptscheme:1.0"/>
      <skos:definition xml:lang="en">Measurement in an instrument that simultaneously determines CO2 and water vapour concentrations in a gas mixture by measuring infra-red absorption</skos:definition>
      <skos:scopeNote xml:lang="en">constant temperature non-dispersive infra-red gas analysis: Measurement in an instrument that simultaneously determines CO2 and water vapour concentrations in a gas mixture by measuring infra-red absorption</skos:scopeNote>
   </skos:Concept>
   <skos:Concept rdf:about="5cc12a4f-6784-372a-801a-09d227bc67c4:concept:578">
      <skos:prefLabel xml:lang="en">Hourly maximum</skos:prefLabel>
      <skos:inScheme rdf:resource="5cc12a4f-6784-372a-801a-09d227bc67c4:conceptscheme:1.0"/>
      <skos:definition xml:lang="en"/>
      <skos:scopeNote xml:lang="en">Hourly maximum</skos:scopeNote>
   </skos:Concept>
   <skos:Concept rdf:about="5cc12a4f-6784-372a-801a-09d227bc67c4:concept:579">
      <skos:prefLabel xml:lang="en">Hourly Mean</skos:prefLabel>
      <skos:inScheme rdf:resource="5cc12a4f-6784-372a-801a-09d227bc67c4:conceptscheme:1.0"/>
      <skos:definition xml:lang="en"/>
      <skos:scopeNote xml:lang="en">Hourly Mean</skos:scopeNote>
   </skos:Concept>
   <skos:Concept rdf:about="5cc12a4f-6784-372a-801a-09d227bc67c4:concept:580">
      <skos:prefLabel xml:lang="en">Hourly minimum</skos:prefLabel>
      <skos:inScheme rdf:resource="5cc12a4f-6784-372a-801a-09d227bc67c4:conceptscheme:1.0"/>
      <skos:definition xml:lang="en"/>
      <skos:scopeNote xml:lang="en">Hourly minimum</skos:scopeNote>
   </skos:Concept>
</rdf:RDF>