<?xml version="1.0" encoding="UTF-8"?>
<rdf:RDF xmlns:rdf="http://www.w3.org/1999/02/22-rdf-syntax-ns#" xmlns:owl="http://www.w3.org/2002/07/owl#" xmlns:cycAnnot="http://sw.cyc.com/CycAnnotations_v1#" xmlns:cyc="http://sw.cyc.com/concept/" xmlns:dbpedia="http://dbpedia.org/resource/" xmlns:ctag="http://commontag.org/ns#" xmlns:opencyc="http://sw.opencyc.org/concept/" xmlns:foaf="http://xmlns.com/foaf/0.1/" xmlns:csw="http://semantic-web.at/ontologies/csw.owl#" xmlns:rdfs="http://www.w3.org/2000/01/rdf-schema#" xmlns:skos="http://www.w3.org/2004/02/skos/core#" xmlns:xsd="http://www.w3.org/2001/XMLSchema#" xmlns:dc="http://purl.org/dc/elements/1.1/" xmlns:freebase="http://rdf.freebase.com/ns/" xmlns:dcterms="http://purl.org/dc/terms/" xmlns:tags="http://www.holygoat.co.uk/owl/redwood/0.1/tags/">
  <!-- RDF data export created by PoolParty. -->
  <!-- This file contains a hierarchical subtree of a SKOS thesaurus. -->
  <!-- Export date: Tue Jul 21 03:51:40 CEST 2015 -->
  <rdf:Description rdf:about="http://vocab.aodn.org.au/def/instrument/1">
    <csw:hierarchyRoot rdf:datatype="http://www.w3.org/2001/XMLSchema#boolean">true</csw:hierarchyRoot>
    <csw:hierarchyRootType rdf:resource="http://www.w3.org/2004/02/skos/core#ConceptScheme" />
    <rdf:type rdf:resource="http://www.w3.org/2004/02/skos/core#ConceptScheme" />
    <dcterms:title xml:lang="en">AODN instrument vocabulary</dcterms:title>
    <dcterms:description xml:lang="en">This register contains a controlled vocabulary for instruments that will ultimately be available in MCP metadata. The controlled vocabulary will be used by the faceted search on the AODN/IMOS portal.</dcterms:description>
    <dcterms:contributor>Natalia_Atkins</dcterms:contributor>
    <dcterms:publisher xml:lang="en">eMarine Information Infrastructure (eMII)</dcterms:publisher>
    <dcterms:subject xml:lang="en">instrument</dcterms:subject>
    <dcterms:creator xml:lang="en">Sebastien Mancini</dcterms:creator>
    <dcterms:created rdf:datatype="http://www.w3.org/2001/XMLSchema#dateTime">2012-12-10T00:00:00Z</dcterms:created>
    <dc:rights>Freely Available For Reuse</dc:rights>
    <skos:hasTopConcept rdf:resource="http://vocab.nerc.ac.uk/collection/L05/current/101" />
    <skos:hasTopConcept rdf:resource="http://vocab.nerc.ac.uk/collection/L05/current/102" />
    <skos:hasTopConcept rdf:resource="http://vocab.nerc.ac.uk/collection/L05/current/110" />
    <skos:hasTopConcept rdf:resource="http://vocab.nerc.ac.uk/collection/L05/current/111" />
    <skos:hasTopConcept rdf:resource="http://vocab.nerc.ac.uk/collection/L05/current/113" />
    <skos:hasTopConcept rdf:resource="http://vocab.nerc.ac.uk/collection/L05/current/114" />
    <skos:hasTopConcept rdf:resource="http://vocab.nerc.ac.uk/collection/L05/current/115" />
    <skos:hasTopConcept rdf:resource="http://vocab.nerc.ac.uk/collection/L05/current/122" />
    <skos:hasTopConcept rdf:resource="http://vocab.nerc.ac.uk/collection/L05/current/123" />
    <skos:hasTopConcept rdf:resource="http://vocab.nerc.ac.uk/collection/L05/current/130" />
    <skos:hasTopConcept rdf:resource="http://vocab.nerc.ac.uk/collection/L05/current/132" />
    <skos:hasTopConcept rdf:resource="http://vocab.nerc.ac.uk/collection/L05/current/133" />
    <skos:hasTopConcept rdf:resource="http://vocab.nerc.ac.uk/collection/L05/current/134" />
    <skos:hasTopConcept rdf:resource="http://vocab.nerc.ac.uk/collection/L05/current/181" />
    <skos:hasTopConcept rdf:resource="http://vocab.nerc.ac.uk/collection/L05/current/21" />
    <skos:hasTopConcept rdf:resource="http://vocab.nerc.ac.uk/collection/L05/current/22" />
    <skos:hasTopConcept rdf:resource="http://vocab.nerc.ac.uk/collection/L05/current/308" />
    <skos:hasTopConcept rdf:resource="http://vocab.nerc.ac.uk/collection/L05/current/350" />
    <skos:hasTopConcept rdf:resource="http://vocab.nerc.ac.uk/collection/L05/current/351" />
    <skos:hasTopConcept rdf:resource="http://vocab.nerc.ac.uk/collection/L05/current/369" />
    <skos:hasTopConcept rdf:resource="http://vocab.nerc.ac.uk/collection/L05/current/381" />
    <skos:hasTopConcept rdf:resource="http://vocab.nerc.ac.uk/collection/L05/current/382" />
    <skos:hasTopConcept rdf:resource="http://vocab.nerc.ac.uk/collection/L05/current/385" />
    <skos:hasTopConcept rdf:resource="http://vocab.nerc.ac.uk/collection/L05/current/FFES" />
    <skos:hasTopConcept rdf:resource="http://vocab.nerc.ac.uk/collection/L05/current/POS17" />
    <skos:hasTopConcept rdf:resource="http://vocab.nerc.ac.uk/collection/L05/current/WPS" />
    <skos:hasTopConcept rdf:resource="http://vocab.nerc.ac.uk/collection/L05/current/103" />
    <skos:hasTopConcept rdf:resource="http://vocab.nerc.ac.uk/collection/L05/current/121" />
    <skos:hasTopConcept rdf:resource="http://vocab.nerc.ac.uk/collection/L05/current/124" />
    <skos:hasTopConcept rdf:resource="http://vocab.nerc.ac.uk/collection/L05/current/135" />
    <skos:hasTopConcept rdf:resource="http://vocab.nerc.ac.uk/collection/L05/current/14" />
    <skos:hasTopConcept rdf:resource="http://vocab.nerc.ac.uk/collection/L05/current/151" />
    <skos:hasTopConcept rdf:resource="http://vocab.nerc.ac.uk/collection/L05/current/157" />
    <skos:hasTopConcept rdf:resource="http://vocab.nerc.ac.uk/collection/L05/current/180" />
    <skos:hasTopConcept rdf:resource="http://vocab.nerc.ac.uk/collection/L05/current/183" />
    <skos:hasTopConcept rdf:resource="http://vocab.nerc.ac.uk/collection/L05/current/185" />
    <skos:hasTopConcept rdf:resource="http://vocab.nerc.ac.uk/collection/L05/current/186" />
    <skos:hasTopConcept rdf:resource="http://vocab.nerc.ac.uk/collection/L05/current/23" />
    <skos:hasTopConcept rdf:resource="http://vocab.nerc.ac.uk/collection/L05/current/24" />
    <skos:hasTopConcept rdf:resource="http://vocab.nerc.ac.uk/collection/L05/current/30" />
    <skos:hasTopConcept rdf:resource="http://vocab.nerc.ac.uk/collection/L05/current/301" />
    <skos:hasTopConcept rdf:resource="http://vocab.nerc.ac.uk/collection/L05/current/303" />
    <skos:hasTopConcept rdf:resource="http://vocab.nerc.ac.uk/collection/L05/current/304" />
    <skos:hasTopConcept rdf:resource="http://vocab.nerc.ac.uk/collection/L05/current/305" />
    <skos:hasTopConcept rdf:resource="http://vocab.nerc.ac.uk/collection/L05/current/306" />
    <skos:hasTopConcept rdf:resource="http://vocab.nerc.ac.uk/collection/L05/current/31" />
    <skos:hasTopConcept rdf:resource="http://vocab.nerc.ac.uk/collection/L05/current/310" />
    <skos:hasTopConcept rdf:resource="http://vocab.nerc.ac.uk/collection/L05/current/311" />
    <skos:hasTopConcept rdf:resource="http://vocab.nerc.ac.uk/collection/L05/current/312" />
    <skos:hasTopConcept rdf:resource="http://vocab.nerc.ac.uk/collection/L05/current/33" />
    <skos:hasTopConcept rdf:resource="http://vocab.nerc.ac.uk/collection/L05/current/353" />
    <skos:hasTopConcept rdf:resource="http://vocab.nerc.ac.uk/collection/L05/current/355" />
    <skos:hasTopConcept rdf:resource="http://vocab.nerc.ac.uk/collection/L05/current/356" />
    <skos:hasTopConcept rdf:resource="http://vocab.nerc.ac.uk/collection/L05/current/377" />
    <skos:hasTopConcept rdf:resource="http://vocab.nerc.ac.uk/collection/L05/current/379" />
    <skos:hasTopConcept rdf:resource="http://vocab.nerc.ac.uk/collection/L05/current/383" />
    <skos:hasTopConcept rdf:resource="http://vocab.nerc.ac.uk/collection/L05/current/384" />
    <skos:hasTopConcept rdf:resource="http://vocab.nerc.ac.uk/collection/L05/current/388" />
    <skos:hasTopConcept rdf:resource="http://vocab.nerc.ac.uk/collection/L05/current/50" />
    <skos:hasTopConcept rdf:resource="http://vocab.nerc.ac.uk/collection/L05/current/51" />
    <skos:hasTopConcept rdf:resource="http://vocab.nerc.ac.uk/collection/L05/current/53" />
    <skos:hasTopConcept rdf:resource="http://vocab.nerc.ac.uk/collection/L05/current/54" />
    <skos:hasTopConcept rdf:resource="http://vocab.nerc.ac.uk/collection/L05/current/60" />
    <skos:hasTopConcept rdf:resource="http://vocab.nerc.ac.uk/collection/L05/current/61" />
    <skos:hasTopConcept rdf:resource="http://vocab.nerc.ac.uk/collection/L05/current/62" />
    <skos:hasTopConcept rdf:resource="http://vocab.nerc.ac.uk/collection/L05/current/63" />
    <skos:hasTopConcept rdf:resource="http://vocab.nerc.ac.uk/collection/L05/current/64" />
    <skos:hasTopConcept rdf:resource="http://vocab.nerc.ac.uk/collection/L05/current/65" />
    <skos:hasTopConcept rdf:resource="http://vocab.nerc.ac.uk/collection/L05/current/68" />
    <skos:hasTopConcept rdf:resource="http://vocab.nerc.ac.uk/collection/L05/current/69" />
    <skos:hasTopConcept rdf:resource="http://vocab.nerc.ac.uk/collection/L05/current/81" />
    <skos:hasTopConcept rdf:resource="http://vocab.nerc.ac.uk/collection/L05/current/82" />
    <skos:hasTopConcept rdf:resource="http://vocab.nerc.ac.uk/collection/L05/current/90" />
    <skos:hasTopConcept rdf:resource="http://vocab.nerc.ac.uk/collection/L05/current/91" />
    <skos:hasTopConcept rdf:resource="http://vocab.nerc.ac.uk/collection/L05/current/LAB02" />
    <skos:hasTopConcept rdf:resource="http://vocab.nerc.ac.uk/collection/L05/current/LAB05" />
    <skos:hasTopConcept rdf:resource="http://vocab.nerc.ac.uk/collection/L05/current/LAB06" />
    <skos:hasTopConcept rdf:resource="http://vocab.nerc.ac.uk/collection/L05/current/LAB07" />
    <skos:hasTopConcept rdf:resource="http://vocab.nerc.ac.uk/collection/L05/current/LAB08" />
    <skos:hasTopConcept rdf:resource="http://vocab.nerc.ac.uk/collection/L05/current/LAB09" />
    <skos:hasTopConcept rdf:resource="http://vocab.nerc.ac.uk/collection/L05/current/LAB10" />
    <skos:hasTopConcept rdf:resource="http://vocab.nerc.ac.uk/collection/L05/current/LAB11" />
    <skos:hasTopConcept rdf:resource="http://vocab.nerc.ac.uk/collection/L05/current/LAB15" />
    <skos:hasTopConcept rdf:resource="http://vocab.nerc.ac.uk/collection/L05/current/LAB16" />
    <skos:hasTopConcept rdf:resource="http://vocab.nerc.ac.uk/collection/L05/current/LAB17" />
    <skos:hasTopConcept rdf:resource="http://vocab.nerc.ac.uk/collection/L05/current/LAB18" />
    <skos:hasTopConcept rdf:resource="http://vocab.nerc.ac.uk/collection/L05/current/LAB19" />
    <skos:hasTopConcept rdf:resource="http://vocab.nerc.ac.uk/collection/L05/current/LAB20" />
    <skos:hasTopConcept rdf:resource="http://vocab.nerc.ac.uk/collection/L05/current/LAB21" />
    <skos:hasTopConcept rdf:resource="http://vocab.nerc.ac.uk/collection/L05/current/LAB22" />
    <skos:hasTopConcept rdf:resource="http://vocab.nerc.ac.uk/collection/L05/current/LAB25" />
    <skos:hasTopConcept rdf:resource="http://vocab.nerc.ac.uk/collection/L05/current/LAB37" />
    <skos:hasTopConcept rdf:resource="http://vocab.nerc.ac.uk/collection/L05/current/LAB39" />
    <skos:hasTopConcept rdf:resource="http://vocab.nerc.ac.uk/collection/L05/current/LAB40" />
    <dcterms:modified rdf:datatype="http://www.w3.org/2001/XMLSchema#dateTime">2015-07-10T05:35:02Z</dcterms:modified>
    <skos:hasTopConcept rdf:resource="http://vocab.nerc.ac.uk/collection/L05/current/POS03" />
    <skos:hasTopConcept rdf:resource="http://vocab.aodn.org.au/def/instrument/entity/361" />
    <skos:hasTopConcept rdf:resource="http://vocab.aodn.org.au/def/instrument/entity/363" />
    <skos:hasTopConcept rdf:resource="http://vocab.aodn.org.au/def/instrument/entity/365" />
  </rdf:Description>
  <rdf:Description rdf:about="http://vocab.nerc.ac.uk/collection/L05/current/LAB39">
    <rdf:type rdf:resource="http://www.w3.org/2004/02/skos/core#Concept" />
    <skos:prefLabel xml:lang="en">Geiger counters</skos:prefLabel>
    <skos:topConceptOf rdf:resource="http://vocab.aodn.org.au/def/instrument/1" />
    <skos:inScheme rdf:resource="http://vocab.aodn.org.au/def/instrument/1" />
    <dcterms:created rdf:datatype="http://www.w3.org/2001/XMLSchema#dateTime">2014-05-29T00:00:00Z</dcterms:created>
    <skos:definition xml:lang="en">Instruments that measure their distance above a specified elevation such as the sea surface or the seabed. Classification includes acoustic and pressure-based instruments that are designed to provide platform z co-ordinate spatial coverage in the atmosphere or a water body. It excludes remote sensing instruments such as LIDAR and satellite radar altimeters designed to map surface elevation.</skos:definition>
    <dc:source>(L051) SeaDataNet device categories</dc:source>
    <dc:publisher>British Oceanographic Data Centre (BODC)</dc:publisher>
  </rdf:Description>
  <rdf:Description rdf:about="http://vocab.nerc.ac.uk/collection/L05/current/LAB37">
    <rdf:type rdf:resource="http://www.w3.org/2004/02/skos/core#Concept" />
    <skos:prefLabel xml:lang="en">flow cytometers</skos:prefLabel>
    <skos:topConceptOf rdf:resource="http://vocab.aodn.org.au/def/instrument/1" />
    <skos:inScheme rdf:resource="http://vocab.aodn.org.au/def/instrument/1" />
    <dcterms:created rdf:datatype="http://www.w3.org/2001/XMLSchema#dateTime">2013-03-28T00:00:00Z</dcterms:created>
    <skos:definition xml:lang="en">Instruments that suspend cells in a stream of fluid past detection sensors whilst illuminating them with laser light. Used for cell counting sorting biomarker detection and protein engineering.</skos:definition>
    <dc:source>(L051) SeaDataNet device categories</dc:source>
    <dc:publisher>British Oceanographic Data Centre (BODC)</dc:publisher>
  </rdf:Description>
  <rdf:Description rdf:about="http://vocab.nerc.ac.uk/collection/L05/current/110">
    <rdf:type rdf:resource="http://www.w3.org/2004/02/skos/core#Concept" />
    <skos:prefLabel xml:lang="en">wave recorders</skos:prefLabel>
    <skos:topConceptOf rdf:resource="http://vocab.aodn.org.au/def/instrument/1" />
    <skos:inScheme rdf:resource="http://vocab.aodn.org.au/def/instrument/1" />
    <dcterms:created rdf:datatype="http://www.w3.org/2001/XMLSchema#dateTime">2013-03-28T00:00:00Z</dcterms:created>
    <skos:definition xml:lang="en">Instrument that measures water column surface wave parameters including height period direction and energy spectra.</skos:definition>
    <dc:source>(L051) SeaDataNet device categories</dc:source>
    <dc:publisher>British Oceanographic Data Centre (BODC)</dc:publisher>
    <skos:narrower rdf:resource="http://vocab.nerc.ac.uk/collection/L22/current/TOOL0268" />
    <skos:narrower rdf:resource="http://vocab.nerc.ac.uk/collection/L22/current/TOOL0696" />
    <skos:narrower rdf:resource="http://vocab.nerc.ac.uk/collection/L22/current/TOOL0710" />
    <skos:narrower rdf:resource="http://vocab.nerc.ac.uk/collection/L22/current/TOOL0729" />
    <skos:narrower rdf:resource="http://vocab.nerc.ac.uk/collection/L22/current/TOOL0733" />
    <skos:narrower rdf:resource="http://vocab.nerc.ac.uk/collection/L22/current/TOOL0781" />
    <skos:narrower rdf:resource="http://vocab.nerc.ac.uk/collection/L22/current/TOOL0898/" />
    <dcterms:modified rdf:datatype="http://www.w3.org/2001/XMLSchema#dateTime">2015-06-30T06:13:24Z</dcterms:modified>
    <dcterms:contributor>Natalia_Atkins</dcterms:contributor>
  </rdf:Description>
  <rdf:Description rdf:about="http://vocab.nerc.ac.uk/collection/L22/current/TOOL0733">
    <rdf:type rdf:resource="http://www.w3.org/2004/02/skos/core#Concept" />
    <skos:prefLabel xml:lang="en">Teledyne RDI Workhorse NEMO-WHSW600 Waves Processing Array</skos:prefLabel>
    <skos:inScheme rdf:resource="http://vocab.aodn.org.au/def/instrument/1" />
    <dcterms:created rdf:datatype="http://www.w3.org/2001/XMLSchema#dateTime">2014-07-16T00:00:00Z</dcterms:created>
    <skos:definition xml:lang="en">A module that may be attached to the Workhorse ADCP Waves Array to process the data and reduce it to a volume that can be transmitted in near real-time. The maximum working depth is 200m.  More information may be found in http://www.rdinstruments.com/datasheets/nemo_ds.pdf.</skos:definition>
    <dc:source>(L221) SeaVoX Device Catalogue</dc:source>
    <dc:publisher>British Oceanographic Data Centre (BODC)</dc:publisher>
  </rdf:Description>
  <rdf:Description rdf:about="http://vocab.nerc.ac.uk/collection/L22/current/TOOL0898/">
    <rdf:type rdf:resource="http://www.w3.org/2004/02/skos/core#Concept" />
    <skos:prefLabel xml:lang="en">Nortek acoustic wave and current profiler</skos:prefLabel>
    <skos:altLabel xml:lang="en">Nortek AWAC</skos:altLabel>
    <skos:inScheme rdf:resource="http://vocab.aodn.org.au/def/instrument/1" />
    <dcterms:created rdf:datatype="http://www.w3.org/2001/XMLSchema#dateTime">2015-06-03T00:00:00Z</dcterms:created>
    <skos:definition xml:lang="en">A family of instruments that simultaneously measure current profiles and wave height and direction designed for coastal monitoring.  It is available in three transmit frequencies: 1 MHz (range 30 m, cell size 0.25-4 m); 600 kHz (range 50 m, cell size 0.5-8 m), 400 kHz (range 100 m, cell size 1-8 m) and has  four beams, one vertical and the other three 120 degrees apart slanted at 25 degrees. Maximum number of cells is 128. Current speeds up to 10 m/s may be measured at an accuracy of 1% of measured value ±0.5cm/s. Temperature (embedded thermistor with 0.1C accuracy and 0.01C resolution), compass (magnetometer with 2 degrees accuracy and 0.1 degree resolution providing tilt less than 15 degrees), tilt (liquid level) and pressure (piezo resistive with accuracy of 0.5% (optional 0.1%) full scale - usually 100m - and resolution of 0.005% full scale) sensors are provided as standard.</skos:definition>
    <dc:publisher>British Oceanographic Data Centre (BODC)</dc:publisher>
    <dcterms:modified rdf:datatype="http://www.w3.org/2001/XMLSchema#dateTime">2015-06-30T06:19:13Z</dcterms:modified>
    <dcterms:contributor>Natalia_Atkins</dcterms:contributor>
  </rdf:Description>
  <rdf:Description rdf:about="http://vocab.nerc.ac.uk/collection/L22/current/TOOL0729">
    <rdf:type rdf:resource="http://www.w3.org/2004/02/skos/core#Concept" />
    <skos:prefLabel xml:lang="en">RBR TWR-2050 Submersible Tide and Wave Recorder</skos:prefLabel>
    <skos:inScheme rdf:resource="http://vocab.aodn.org.au/def/instrument/1" />
    <dcterms:created rdf:datatype="http://www.w3.org/2001/XMLSchema#dateTime">2014-07-14T00:00:00Z</dcterms:created>
    <skos:definition xml:lang="en">The TWR-2050P is a small, self-contained, submersible temperature, wave and depth recorder (sensors and data logger). It can be deployed for a period of up to three years and can collect more than 1,200,000 sets of samples. Data can be retained in memory for 20 years (even without batteries). Available in two casings, plastic and titanium, with depth ratings of 740m and 6600m respectively. The temperature channel of the TWR-2050 is calibrated to an accuracy of ± 0.002°C (ITS-90) over the range -5 to +35°C.  Typical drift has been measured to be 0.002°C per year. The thermistor may be external (&lt;3sec time constant) or internal (&lt;20sec time constant). A fast thermistor probe (0.095sec) is also available. The depth channel is calibrated to an accuracy of 0.05%fs  Ranges from 10m to 6,600m are available. Temperature and depth only sensors (TDR) and surface-mounted sensors (HT) are also available.</skos:definition>
    <dc:source>(L221) SeaVoX Device Catalogue</dc:source>
    <dc:publisher>British Oceanographic Data Centre (BODC)</dc:publisher>
  </rdf:Description>
  <rdf:Description rdf:about="http://vocab.nerc.ac.uk/collection/L22/current/TOOL0781">
    <rdf:type rdf:resource="http://www.w3.org/2004/02/skos/core#Concept" />
    <skos:prefLabel xml:lang="en">Datawell waverider buoy</skos:prefLabel>
    <skos:altLabel xml:lang="en">Datawell waverider</skos:altLabel>
    <skos:inScheme rdf:resource="http://vocab.aodn.org.au/def/instrument/1" />
    <dcterms:created rdf:datatype="http://www.w3.org/2001/XMLSchema#dateTime">2013-03-28T00:00:00Z</dcterms:created>
    <skos:definition xml:lang="en">A non-directional waverider system with an accelerometer mounted in a loose tethered buoy (0.7 or 0.9m in diameter) that measures the vertical accelerations of the buoy as it moves with the water surface.  The accelerations are integrated twice within the buoy and the displacement signal so obtained is then transmitted to a shore station where it is processed to provide wave data statistics.</skos:definition>
    <dc:source>(L221) SeaVoX Device Catalogue</dc:source>
    <dc:publisher>British Oceanographic Data Centre (BODC)</dc:publisher>
  </rdf:Description>
  <rdf:Description rdf:about="http://vocab.nerc.ac.uk/collection/L22/current/TOOL0696">
    <rdf:type rdf:resource="http://www.w3.org/2004/02/skos/core#Concept" />
    <skos:prefLabel xml:lang="en">Sea-Bird SBE 26plus SEAGAUGE Wave and Tide Recorder</skos:prefLabel>
    <skos:inScheme rdf:resource="http://vocab.aodn.org.au/def/instrument/1" />
    <dcterms:created rdf:datatype="http://www.w3.org/2001/XMLSchema#dateTime">2013-09-25T00:00:00Z</dcterms:created>
    <skos:definition xml:lang="en">The SBE 26 SEAGAUGE is a water level recorder with a Digiquartz pressure sensor, accurate clock, precision thermometer and optional conductivity sensor in a casing able to operate down to 600m. Pressure data are integrated to give sea level or are burst recorded at rates up to 4 Hz to measure characterise waves. The instrument offers improved temperature sensor accuracy (0.01C with 0.001C resolution or optionally 0.001C with 0.0001C resolution), data storage and operational functionality over the SBE-26. More information at http://www.seabird.com/products/spec_sheets/26plusdata.htm.</skos:definition>
    <dc:source>(L221) SeaVoX Device Catalogue</dc:source>
    <dc:publisher>British Oceanographic Data Centre (BODC)</dc:publisher>
    <skos:scopeNote xml:lang="en">manufacturer:Sea-Bird Electronics Inc.</skos:scopeNote>
  </rdf:Description>
  <rdf:Description rdf:about="http://vocab.nerc.ac.uk/collection/L22/current/TOOL0268">
    <rdf:type rdf:resource="http://www.w3.org/2004/02/skos/core#Concept" />
    <skos:prefLabel xml:lang="en">Datawell directional waverider buoy</skos:prefLabel>
    <skos:inScheme rdf:resource="http://vocab.aodn.org.au/def/instrument/1" />
    <dcterms:created rdf:datatype="http://www.w3.org/2001/XMLSchema#dateTime">2014-02-17T00:00:00Z</dcterms:created>
    <skos:definition xml:lang="en">A directional waverider buoy comprising a heave-pitch-roll sensor, two accelerometers and a 3-axis fluxgate compass in a 90cm diameter spherical buoy that measures waves using a translational principle so that horizontal motions rather than wave slopes are measured making the measurement independent of buoy roll motions. A single point rubber cord vertical mooring ensures adequate symmetrical horizontal buoy response to resolve small motions at low frequencies. Data are transmitted to a shore based station and/or an Argos satellite. Three versions of the buoy designated MkI, MkII and MkIII have been produced with evolving internal electronics but fundamentally the same design. More information may be found at http://www.bodc.ac.uk/data/documents/nodb/65329/</skos:definition>
    <dc:source>(L221) SeaVoX Device Catalogue</dc:source>
    <dc:publisher>British Oceanographic Data Centre (BODC)</dc:publisher>
    <skos:scopeNote xml:lang="en">manufacturer:Datawell</skos:scopeNote>
  </rdf:Description>
  <rdf:Description rdf:about="http://vocab.nerc.ac.uk/collection/L22/current/TOOL0710">
    <rdf:type rdf:resource="http://www.w3.org/2004/02/skos/core#Concept" />
    <skos:prefLabel xml:lang="en">TRIAXYS directional wave sensor</skos:prefLabel>
    <skos:inScheme rdf:resource="http://vocab.aodn.org.au/def/instrument/1" />
    <dcterms:created rdf:datatype="http://www.w3.org/2001/XMLSchema#dateTime">2014-07-14T00:00:00Z</dcterms:created>
    <skos:definition xml:lang="en">A sensor packaged in a small stainless steel box with a single connector for power and data that outputs fully processed wave data. Sampling is in bursts from 1-34 minutes with a sampling interval from 5-1440 minutes. It may be located anywhere on a floating platform and comprises three accelerometers and three rate sensors that measure displacement along the three orthogonal axes of the platform. Direction is measured using a gimballed fluxgate compass. Resolution is 0.01m for height, 0.1 second for period and one degree for direction. Accuracy is better than 2% for height and period and 3 degrees for direction. More information is available in http://axystechnologies.com/wp-content/uploads/2014/01/TRIAXYS-NW-Sensors-Digital-Layout.pdf.</skos:definition>
    <dc:source>(L221) SeaVoX Device Catalogue</dc:source>
    <dc:publisher>British Oceanographic Data Centre (BODC)</dc:publisher>
  </rdf:Description>
  <rdf:Description rdf:about="http://vocab.nerc.ac.uk/collection/L05/current/111">
    <rdf:type rdf:resource="http://www.w3.org/2004/02/skos/core#Concept" />
    <skos:prefLabel xml:lang="en">sea level recorders</skos:prefLabel>
    <skos:topConceptOf rdf:resource="http://vocab.aodn.org.au/def/instrument/1" />
    <skos:inScheme rdf:resource="http://vocab.aodn.org.au/def/instrument/1" />
    <dcterms:created rdf:datatype="http://www.w3.org/2001/XMLSchema#dateTime">2014-06-04T00:00:00Z</dcterms:created>
    <skos:definition xml:lang="en">Instrument that make smoothed measurements of the elevation of the sea surface relative to a fixed vertical datum</skos:definition>
    <dc:source>(L051) SeaDataNet device categories</dc:source>
    <dc:publisher>British Oceanographic Data Centre (BODC)</dc:publisher>
    <skos:narrower rdf:resource="http://vocab.nerc.ac.uk/collection/L22/current/TOOL0169" />
    <skos:narrower rdf:resource="http://vocab.nerc.ac.uk/collection/L22/current/TOOL0675" />
    <skos:narrower rdf:resource="http://vocab.nerc.ac.uk/collection/L22/current/TOOL0680" />
    <skos:narrower rdf:resource="http://vocab.nerc.ac.uk/collection/L22/current/TOOL0685" />
    <skos:narrower rdf:resource="http://vocab.nerc.ac.uk/collection/L22/current/TOOL0696" />
    <skos:narrower rdf:resource="http://vocab.nerc.ac.uk/collection/L22/current/TOOL0708" />
    <skos:narrower rdf:resource="http://vocab.nerc.ac.uk/collection/L22/current/TOOL0729" />
    <skos:narrower rdf:resource="http://vocab.nerc.ac.uk/collection/L22/current/TOOL0731" />
    <dcterms:modified rdf:datatype="http://www.w3.org/2001/XMLSchema#dateTime">2015-05-29T06:29:17Z</dcterms:modified>
    <skos:narrower rdf:resource="http://vocab.nerc.ac.uk/collection/L22/current/TOOL0809" />
  </rdf:Description>
  <rdf:Description rdf:about="http://vocab.nerc.ac.uk/collection/L22/current/TOOL0708">
    <rdf:type rdf:resource="http://www.w3.org/2004/02/skos/core#Concept" />
    <skos:prefLabel xml:lang="en">Heise Model DXD Digital Output Pressure Transducer</skos:prefLabel>
    <skos:inScheme rdf:resource="http://vocab.aodn.org.au/def/instrument/1" />
    <dcterms:created rdf:datatype="http://www.w3.org/2001/XMLSchema#dateTime">2014-07-11T00:00:00Z</dcterms:created>
    <skos:definition xml:lang="en">This is digital pressure transducer with an RS232 or RS485 interface in a stainless steel housing with an accuracy of 0.02% full scale. More information is available at http://www.heise.com/Products/pressure_transducers/upload/Heise-Bul-HTR-4-08-3.pdf.</skos:definition>
    <dc:source>(L221) SeaVoX Device Catalogue</dc:source>
    <dc:publisher>British Oceanographic Data Centre (BODC)</dc:publisher>
  </rdf:Description>
  <rdf:Description rdf:about="http://vocab.nerc.ac.uk/collection/L22/current/TOOL0169">
    <rdf:type rdf:resource="http://www.w3.org/2004/02/skos/core#Concept" />
    <skos:prefLabel xml:lang="en">RBR DR-1050 Depth recorder</skos:prefLabel>
    <skos:inScheme rdf:resource="http://vocab.aodn.org.au/def/instrument/1" />
    <dcterms:created rdf:datatype="http://www.w3.org/2001/XMLSchema#dateTime">2013-03-28T00:00:00Z</dcterms:created>
    <skos:definition xml:lang="en">The DR-1050 is a pressure recorder with possible ranges of 10, 20, 50, 100, 200, 500, 740, 1000, 2000, 4000, 6000 and 10000 dbar; an accuracy of 0.05% full scale; a resolution of &lt;0.001% full scale; and a time constant of &lt;10 msec.</skos:definition>
    <dc:source>(L221) SeaVoX Device Catalogue</dc:source>
    <dc:publisher>British Oceanographic Data Centre (BODC)</dc:publisher>
    <skos:scopeNote xml:lang="en">manufacturer: RBR</skos:scopeNote>
  </rdf:Description>
  <rdf:Description rdf:about="http://vocab.nerc.ac.uk/collection/L22/current/TOOL0731">
    <rdf:type rdf:resource="http://www.w3.org/2004/02/skos/core#Concept" />
    <skos:prefLabel xml:lang="en">ReefNet Sensus Ultra</skos:prefLabel>
    <skos:inScheme rdf:resource="http://vocab.aodn.org.au/def/instrument/1" />
    <dcterms:created rdf:datatype="http://www.w3.org/2001/XMLSchema#dateTime">2014-07-14T00:00:00Z</dcterms:created>
    <skos:definition xml:lang="en">The ReefNet Sensus Ultra is a compact temperature and depth logging sensor designed for use as a dive computer. Depths between 0 and 500 feet are measured with precision better than 0.5 inches of water, and accuracy of +/-12 inches. Temperature is measured between -20 degC and + 40 degC, with precision of 0.01 degC, and accuracy of +/-0.8 degC. Sampling interval is configurable from 1 second to over 18 hours, with storage capacity of one year at 60 second sampling resolution.</skos:definition>
    <dc:source>(L221) SeaVoX Device Catalogue</dc:source>
    <dc:publisher>British Oceanographic Data Centre (BODC)</dc:publisher>
  </rdf:Description>
  <rdf:Description rdf:about="http://vocab.nerc.ac.uk/collection/L22/current/TOOL0729">
    <rdf:type rdf:resource="http://www.w3.org/2004/02/skos/core#Concept" />
    <skos:prefLabel xml:lang="en">RBR TWR-2050 Submersible Tide and Wave Recorder</skos:prefLabel>
    <skos:inScheme rdf:resource="http://vocab.aodn.org.au/def/instrument/1" />
    <dcterms:created rdf:datatype="http://www.w3.org/2001/XMLSchema#dateTime">2014-07-14T00:00:00Z</dcterms:created>
    <skos:definition xml:lang="en">The TWR-2050P is a small, self-contained, submersible temperature, wave and depth recorder (sensors and data logger). It can be deployed for a period of up to three years and can collect more than 1,200,000 sets of samples. Data can be retained in memory for 20 years (even without batteries). Available in two casings, plastic and titanium, with depth ratings of 740m and 6600m respectively. The temperature channel of the TWR-2050 is calibrated to an accuracy of ± 0.002°C (ITS-90) over the range -5 to +35°C.  Typical drift has been measured to be 0.002°C per year. The thermistor may be external (&lt;3sec time constant) or internal (&lt;20sec time constant). A fast thermistor probe (0.095sec) is also available. The depth channel is calibrated to an accuracy of 0.05%fs  Ranges from 10m to 6,600m are available. Temperature and depth only sensors (TDR) and surface-mounted sensors (HT) are also available.</skos:definition>
    <dc:source>(L221) SeaVoX Device Catalogue</dc:source>
    <dc:publisher>British Oceanographic Data Centre (BODC)</dc:publisher>
  </rdf:Description>
  <rdf:Description rdf:about="http://vocab.nerc.ac.uk/collection/L22/current/TOOL0809">
    <owl:deprecated rdf:datatype="http://www.w3.org/2001/XMLSchema#boolean">true</owl:deprecated>
    <rdfs:label xml:lang="en">RBR TGR-2050 submersible tide gauge</rdfs:label>
    <rdf:type rdf:resource="http://www.w3.org/2004/02/skos/core#Concept" />
    <skos:prefLabel xml:lang="en">RBR TGR-2050 submersible tide gauge</skos:prefLabel>
    <skos:altLabel xml:lang="en">RBR TGR-2050 TG</skos:altLabel>
    <skos:inScheme rdf:resource="http://vocab.aodn.org.au/def/instrument/1" />
    <dcterms:created rdf:datatype="http://www.w3.org/2001/XMLSchema#dateTime">2013-03-28T00:00:00Z</dcterms:created>
    <skos:definition xml:lang="en">A small (265mm x 38mm OD) self-contained, submersible temperature and pressure logger designed to monitor tide levels without interference from wave action by averaging pressure data sampled at 4 Hz. This operating mode differentiates it from the similar TDR-2050. Temperature channel is calibrated to ±0.002C. Depth channel is calibrated to an accuracy of ±0.05% full scale.</skos:definition>
    <dc:source>(L221) SeaVoX Device Catalogue</dc:source>
    <dc:publisher>British Oceanographic Data Centre (BODC)</dc:publisher>
    <dcterms:modified rdf:datatype="http://www.w3.org/2001/XMLSchema#dateTime">2015-07-07T04:49:53Z</dcterms:modified>
    <dcterms:contributor>Natalia_Atkins</dcterms:contributor>
  </rdf:Description>
  <rdf:Description rdf:about="http://vocab.nerc.ac.uk/collection/L22/current/TOOL0675">
    <rdf:type rdf:resource="http://www.w3.org/2004/02/skos/core#Concept" />
    <skos:prefLabel xml:lang="en">WETLabs Water Quality Monitor</skos:prefLabel>
    <dcterms:created rdf:datatype="http://www.w3.org/2001/XMLSchema#dateTime">2014-04-01T00:00:00Z</dcterms:created>
    <skos:definition xml:lang="en">An instrument that incorporates WET Labs fluorometer-turbidity and Sea-Bird's CTD sensors, providing temperature, salinity, depth, dissolved oxygen, chlorophyll fluorescence, turbidity and backscattering data. It is designed for long-term deployment in coastal waters with protection against biofouling and fouling by sediment loads. More information is available at http://www.wetlabs.com/wqm.</skos:definition>
    <dc:source>(L221) SeaVoX Device Catalogue</dc:source>
    <dc:publisher>British Oceanographic Data Centre (BODC)</dc:publisher>
    <skos:inScheme rdf:resource="http://vocab.aodn.org.au/def/instrument/1" />
    <skos:scopeNote xml:lang="en">manufacture:WETLabs Inc.</skos:scopeNote>
  </rdf:Description>
  <rdf:Description rdf:about="http://vocab.nerc.ac.uk/collection/L22/current/TOOL0685">
    <rdf:type rdf:resource="http://www.w3.org/2004/02/skos/core#Concept" />
    <skos:prefLabel xml:lang="en">Aquatech AQUAlogger 520PT mini temperature and pressure logger</skos:prefLabel>
    <skos:inScheme rdf:resource="http://vocab.aodn.org.au/def/instrument/1" />
    <dcterms:created rdf:datatype="http://www.w3.org/2001/XMLSchema#dateTime">2014-06-04T00:00:00Z</dcterms:created>
    <skos:definition xml:lang="en">A miniature (200mm long, 32mm diameter) self-contained data logger incorporating a thermistor temperature sensor (resolution better that 0.007C, accuracy 0.05C) and a pressure sensor in a housing designed to operate at depths down to 1000m.  The type of pressure sensor fitted depends upon the maximum operating depth required with resolution and accuracy a function of the full-scale reading. The logger may be programmed to provide a wide variety of sampling regimes, including burst recording. More information may be found in http://www.aquatecgroup.com/images/manual_guides/bg%20-%20520.pdf.</skos:definition>
    <dc:source>(L221) SeaVoX Device Catalogue</dc:source>
    <dc:publisher>British Oceanographic Data Centre (BODC)</dc:publisher>
  </rdf:Description>
  <rdf:Description rdf:about="http://vocab.nerc.ac.uk/collection/L22/current/TOOL0696">
    <rdf:type rdf:resource="http://www.w3.org/2004/02/skos/core#Concept" />
    <skos:prefLabel xml:lang="en">Sea-Bird SBE 26plus SEAGAUGE Wave and Tide Recorder</skos:prefLabel>
    <skos:inScheme rdf:resource="http://vocab.aodn.org.au/def/instrument/1" />
    <dcterms:created rdf:datatype="http://www.w3.org/2001/XMLSchema#dateTime">2013-09-25T00:00:00Z</dcterms:created>
    <skos:definition xml:lang="en">The SBE 26 SEAGAUGE is a water level recorder with a Digiquartz pressure sensor, accurate clock, precision thermometer and optional conductivity sensor in a casing able to operate down to 600m. Pressure data are integrated to give sea level or are burst recorded at rates up to 4 Hz to measure characterise waves. The instrument offers improved temperature sensor accuracy (0.01C with 0.001C resolution or optionally 0.001C with 0.0001C resolution), data storage and operational functionality over the SBE-26. More information at http://www.seabird.com/products/spec_sheets/26plusdata.htm.</skos:definition>
    <dc:source>(L221) SeaVoX Device Catalogue</dc:source>
    <dc:publisher>British Oceanographic Data Centre (BODC)</dc:publisher>
    <skos:scopeNote xml:lang="en">manufacturer:Sea-Bird Electronics Inc.</skos:scopeNote>
  </rdf:Description>
  <rdf:Description rdf:about="http://vocab.nerc.ac.uk/collection/L22/current/TOOL0680">
    <rdf:type rdf:resource="http://www.w3.org/2004/02/skos/core#Concept" />
    <skos:prefLabel xml:lang="en">GE Druck RPT 350 Resonant Pressure Transducer</skos:prefLabel>
    <skos:inScheme rdf:resource="http://vocab.aodn.org.au/def/instrument/1" />
    <dcterms:created rdf:datatype="http://www.w3.org/2001/XMLSchema#dateTime">2013-10-15T00:00:00Z</dcterms:created>
    <skos:definition xml:lang="en">The GE Druck RPT350 Resonant Pressure Transducer, uses silicon technology to give high accuracy and stability with low manufacturing costs. It ranges from 35 to 3500 mbar abs.</skos:definition>
    <dc:source>(L221) SeaVoX Device Catalogue</dc:source>
    <dc:publisher>British Oceanographic Data Centre (BODC)</dc:publisher>
    <skos:scopeNote xml:lang="en">manufacturer:General Electric Company</skos:scopeNote>
  </rdf:Description>
  <rdf:Description rdf:about="http://vocab.nerc.ac.uk/collection/L05/current/113">
    <rdf:type rdf:resource="http://www.w3.org/2004/02/skos/core#Concept" />
    <skos:prefLabel xml:lang="en">fluorometers</skos:prefLabel>
    <skos:topConceptOf rdf:resource="http://vocab.aodn.org.au/def/instrument/1" />
    <skos:inScheme rdf:resource="http://vocab.aodn.org.au/def/instrument/1" />
    <dcterms:created rdf:datatype="http://www.w3.org/2001/XMLSchema#dateTime">2013-03-28T00:00:00Z</dcterms:created>
    <skos:definition xml:lang="en">Instrument that measures the amount of stimulated electromagnetic radiation produced by pulses of electromagnetic radiation emitted into the water column</skos:definition>
    <dc:source>(L051) SeaDataNet device categories</dc:source>
    <dc:publisher>British Oceanographic Data Centre (BODC)</dc:publisher>
    <skos:narrower rdf:resource="http://vocab.nerc.ac.uk/collection/L22/current/TOOL0215" />
    <skos:narrower rdf:resource="http://vocab.nerc.ac.uk/collection/L22/current/TOOL0673" />
    <skos:narrower rdf:resource="http://vocab.nerc.ac.uk/collection/L22/current/TOOL0674" />
    <skos:narrower rdf:resource="http://vocab.nerc.ac.uk/collection/L22/current/TOOL0675" />
    <skos:narrower rdf:resource="http://vocab.nerc.ac.uk/collection/L22/current/TOOL0720" />
  </rdf:Description>
  <rdf:Description rdf:about="http://vocab.nerc.ac.uk/collection/L22/current/TOOL0675">
    <rdf:type rdf:resource="http://www.w3.org/2004/02/skos/core#Concept" />
    <skos:prefLabel xml:lang="en">WETLabs Water Quality Monitor</skos:prefLabel>
    <dcterms:created rdf:datatype="http://www.w3.org/2001/XMLSchema#dateTime">2014-04-01T00:00:00Z</dcterms:created>
    <skos:definition xml:lang="en">An instrument that incorporates WET Labs fluorometer-turbidity and Sea-Bird's CTD sensors, providing temperature, salinity, depth, dissolved oxygen, chlorophyll fluorescence, turbidity and backscattering data. It is designed for long-term deployment in coastal waters with protection against biofouling and fouling by sediment loads. More information is available at http://www.wetlabs.com/wqm.</skos:definition>
    <dc:source>(L221) SeaVoX Device Catalogue</dc:source>
    <dc:publisher>British Oceanographic Data Centre (BODC)</dc:publisher>
    <skos:inScheme rdf:resource="http://vocab.aodn.org.au/def/instrument/1" />
    <skos:scopeNote xml:lang="en">manufacture:WETLabs Inc.</skos:scopeNote>
  </rdf:Description>
  <rdf:Description rdf:about="http://vocab.nerc.ac.uk/collection/L22/current/TOOL0215">
    <rdf:type rdf:resource="http://www.w3.org/2004/02/skos/core#Concept" />
    <skos:prefLabel xml:lang="en">WETLabs ECO-FLNTU combined fluorometer and turbidity sensor</skos:prefLabel>
    <dcterms:created rdf:datatype="http://www.w3.org/2001/XMLSchema#dateTime">2013-12-16T00:00:00Z</dcterms:created>
    <skos:definition xml:lang="en">The ECO-FLNTU combines the ECO fluorometer with an optical scattering measurement at 700nm for simultaneous determination of turbidity. The fluorometer can typically measure phytoplankton concentrations in the range 0.01-50 ug/l, with a sensitivity of 0.01 ug/l. The turbidity sensor can measure within the range 0.01-25 NTU, with a sensitivity of 0.01 NTU. The instrument is stable over a temperature range of 0-20 degC and is rated to a depth of 600 m as standard, with the option of a 'deep' instrument rated to 6000m.</skos:definition>
    <dc:source>(L221) SeaVoX Device Catalogue</dc:source>
    <dc:publisher>British Oceanographic Data Centre (BODC)</dc:publisher>
    <skos:inScheme rdf:resource="http://vocab.aodn.org.au/def/instrument/1" />
    <skos:scopeNote xml:lang="en">manufacture:WETLabs Inc.</skos:scopeNote>
  </rdf:Description>
  <rdf:Description rdf:about="http://vocab.nerc.ac.uk/collection/L22/current/TOOL0674">
    <rdf:type rdf:resource="http://www.w3.org/2004/02/skos/core#Concept" />
    <skos:prefLabel xml:lang="en">WETLabs ECO Triplet</skos:prefLabel>
    <dcterms:created rdf:datatype="http://www.w3.org/2001/XMLSchema#dateTime">2013-09-10T00:00:00Z</dcterms:created>
    <skos:definition xml:lang="en">A three-optical-sensor instrument that may carry any combination of fluorometers or single-wavelength scattering meters. The fluorometers are single wavelength sensors that can be configured for chlorophyll-a, CDOM, phycocyanin, phycoerythrin, fluorescein or rhodamine. Scattering meters measure optical scattering at blue, green or red wavelengths. More information may be found at http://www.wetlabs.com/eco-triplet.</skos:definition>
    <dc:source>(L221) SeaVoX Device Catalogue</dc:source>
    <dc:publisher>British Oceanographic Data Centre (BODC)</dc:publisher>
    <skos:inScheme rdf:resource="http://vocab.aodn.org.au/def/instrument/1" />
    <skos:scopeNote xml:lang="en">manufacture:WETLabs Inc.</skos:scopeNote>
  </rdf:Description>
  <rdf:Description rdf:about="http://vocab.nerc.ac.uk/collection/L22/current/TOOL0673">
    <rdf:type rdf:resource="http://www.w3.org/2004/02/skos/core#Concept" />
    <skos:prefLabel xml:lang="en">WETLabs ECO Puck Triple-Measurement Meter</skos:prefLabel>
    <dcterms:created rdf:datatype="http://www.w3.org/2001/XMLSchema#dateTime">2013-09-11T00:00:00Z</dcterms:created>
    <skos:definition xml:lang="en">A miniature version of the Environmental Characterisation Optics (ECO) sensors built for OEM applications, with the design specifically targeted at AUVs, gliders and profiling floats. The triplet version carries a fluorometer plus two other sensors that may be additional fluorometers, single-wavelength scattering meters (BB) or a volume scattering function meter (VSF). The fluorometers are single wavelength sensors that can be configured for chlorophyll-a, CDOM, phycocyanin, phycoerythrin, fluorescein or rhodamine. BB measures optical scattering at 117 degrees at 470, 532 or 650 nm wavelengths. VSF measures optical scattering at 100, 125 and 150 degrees. More information may be found at http://www.wetlabs.com/eco-puck.</skos:definition>
    <dc:source>(L221) SeaVoX Device Catalogue</dc:source>
    <dc:publisher>British Oceanographic Data Centre (BODC)</dc:publisher>
    <skos:inScheme rdf:resource="http://vocab.aodn.org.au/def/instrument/1" />
    <skos:scopeNote xml:lang="en">manufacture:WETLabs Inc.</skos:scopeNote>
  </rdf:Description>
  <rdf:Description rdf:about="http://vocab.nerc.ac.uk/collection/L22/current/TOOL0720">
    <rdf:type rdf:resource="http://www.w3.org/2004/02/skos/core#Concept" />
    <skos:prefLabel xml:lang="en">SMRU Ltd CTD/Fluorometer Satellite Relay Data Logger</skos:prefLabel>
    <skos:inScheme rdf:resource="http://vocab.aodn.org.au/def/instrument/1" />
    <dcterms:created rdf:datatype="http://www.w3.org/2001/XMLSchema#dateTime">2013-10-10T00:00:00Z</dcterms:created>
    <skos:definition xml:lang="en">A package comprising a Valeport CTD sensor head plus a customised Turner Cyclops-7 fluorometer combined with an RF unit and antenna suitable for transmission of data via the Argos satellite system. The unit contains an internal battery and a microprocessor that logs data and schedules the transfer of data. The package is designed for attachment to marine mammals and has an operational depth range of down to 2000 m. CTD accuracy is 0.005 C (temperature), 0.01 mS/cm (conductivity) and 2 dBar (pressure).  It is built and calibrated at Valeport Ltd, while SMRU Ltd, the commercial arm of the Sea Mammal Research Unit of the University of St Andrews, is responsible for its distribution, and for streaming and processing the data. More information is available at http://www.smru.st-and.ac.uk/Instrumentation/FluorometryTag/.</skos:definition>
    <dc:source>(L221) SeaVoX Device Catalogue</dc:source>
    <dc:publisher>British Oceanographic Data Centre (BODC)</dc:publisher>
    <skos:scopeNote xml:lang="en">manufacturer:SMRU Instrumentation</skos:scopeNote>
  </rdf:Description>
  <rdf:Description rdf:about="http://vocab.nerc.ac.uk/collection/L05/current/114">
    <rdf:type rdf:resource="http://www.w3.org/2004/02/skos/core#Concept" />
    <skos:prefLabel xml:lang="en">current meters</skos:prefLabel>
    <skos:topConceptOf rdf:resource="http://vocab.aodn.org.au/def/instrument/1" />
    <skos:inScheme rdf:resource="http://vocab.aodn.org.au/def/instrument/1" />
    <dcterms:created rdf:datatype="http://www.w3.org/2001/XMLSchema#dateTime">2013-03-28T00:00:00Z</dcterms:created>
    <skos:definition xml:lang="en">Instrument that measures current speed and direction at a single depth</skos:definition>
    <dc:source>(L051) SeaDataNet device categories</dc:source>
    <dc:publisher>British Oceanographic Data Centre (BODC)</dc:publisher>
    <skos:narrower rdf:resource="http://vocab.nerc.ac.uk/collection/L22/current/TOOL0089" />
    <skos:narrower rdf:resource="http://vocab.nerc.ac.uk/collection/L22/current/TOOL0121" />
    <skos:narrower rdf:resource="http://vocab.nerc.ac.uk/collection/L22/current/TOOL0476" />
    <skos:narrower rdf:resource="http://vocab.nerc.ac.uk/collection/L22/current/TOOL0477" />
  </rdf:Description>
  <rdf:Description rdf:about="http://vocab.nerc.ac.uk/collection/L22/current/TOOL0477">
    <rdf:type rdf:resource="http://www.w3.org/2004/02/skos/core#Concept" />
    <skos:prefLabel xml:lang="en">Nortek Aquadopp 6000 3D doppler current meter</skos:prefLabel>
    <skos:inScheme rdf:resource="http://vocab.aodn.org.au/def/instrument/1" />
    <dcterms:created rdf:datatype="http://www.w3.org/2001/XMLSchema#dateTime">2013-03-28T00:00:00Z</dcterms:created>
    <skos:definition xml:lang="en">The Nortek Aquadopp 6000 is a single-depth doppler current meter designed for deployment on deep water moorings, although it is also suitable for attachment to fixed structures. It features higher power and an increased signal-to-noise ratio compared with the standard (300 m depth rated) Aquadopp so that it can provide accurate current measurements in water with low concentrations of suspended particulate matter. Current velocity is derived from the Doppler shift measured by two or three 2MHz acoustic beams. It comes with compass, tilt, pressure and temperature sensors. It has a titanium casing rated to 6000 m and data are stored on an internal logger. It can be run in diagnostic mode when set to collect data at 1 Hz frequency in user specified intervals, which allows studies of mooring motion and the performance of other current meters to be conducted.</skos:definition>
    <dc:source>(L221) SeaVoX Device Catalogue</dc:source>
    <dc:publisher>British Oceanographic Data Centre (BODC)</dc:publisher>
    <skos:scopeNote xml:lang="en">manufacturer:Nortek</skos:scopeNote>
  </rdf:Description>
  <rdf:Description rdf:about="http://vocab.nerc.ac.uk/collection/L22/current/TOOL0121">
    <rdf:type rdf:resource="http://www.w3.org/2004/02/skos/core#Concept" />
    <skos:prefLabel xml:lang="en">Aanderaa RCM 7/8 Recording Current Meter</skos:prefLabel>
    <skos:inScheme rdf:resource="http://vocab.aodn.org.au/def/instrument/1" />
    <dcterms:created rdf:datatype="http://www.w3.org/2001/XMLSchema#dateTime">2014-04-01T00:00:00Z</dcterms:created>
    <skos:definition xml:lang="en">Family of self-recording paddle wheel current meters with different pressure cases that record the vector averaged speed and direction over a sampling interval. The paddle wheel rotor is magnetically coupled to an electronic counter. The meter has a balanced weight vane which aligns it with the current flow. For more details see http://www.bodc.ac.uk/data/documents/nodb/65611/.</skos:definition>
    <dc:source>(L221) SeaVoX Device Catalogue</dc:source>
    <dc:publisher>British Oceanographic Data Centre (BODC)</dc:publisher>
    <skos:scopeNote xml:lang="en">manufacturer:Aanderaa Data Instruments</skos:scopeNote>
  </rdf:Description>
  <rdf:Description rdf:about="http://vocab.nerc.ac.uk/collection/L22/current/TOOL0089">
    <rdf:type rdf:resource="http://www.w3.org/2004/02/skos/core#Concept" />
    <skos:prefLabel xml:lang="en">Nortek Aquadopp 3D doppler current meter</skos:prefLabel>
    <skos:inScheme rdf:resource="http://vocab.aodn.org.au/def/instrument/1" />
    <dcterms:created rdf:datatype="http://www.w3.org/2001/XMLSchema#dateTime">2013-03-28T00:00:00Z</dcterms:created>
    <skos:definition xml:lang="en">The Aquadopp is a single-depth doppler current meter designed both for real time data collection and self contained deployments logging internally. It comes with compass, tilt, pressure and temperature sensors. It can also be configured to measure surface wave height, period and direction concurrently. It has the unique feature of being run in diagnostic mode when set to collect data at 1 Hz frequency in user specified intervals. This allows studies of mooring motion and the performance of other current meters to be conducted. It can be set in various configurations with titanium housings for deployment at greater depths.</skos:definition>
    <dc:source>(L221) SeaVoX Device Catalogue</dc:source>
    <dc:publisher>British Oceanographic Data Centre (BODC)</dc:publisher>
    <skos:scopeNote xml:lang="en">manufacturer:Nortek</skos:scopeNote>
  </rdf:Description>
  <rdf:Description rdf:about="http://vocab.nerc.ac.uk/collection/L22/current/TOOL0476">
    <rdf:type rdf:resource="http://www.w3.org/2004/02/skos/core#Concept" />
    <skos:prefLabel xml:lang="en">Nortek Aquadopp 3000 3D doppler current meter</skos:prefLabel>
    <skos:inScheme rdf:resource="http://vocab.aodn.org.au/def/instrument/1" />
    <dcterms:created rdf:datatype="http://www.w3.org/2001/XMLSchema#dateTime">2013-03-28T00:00:00Z</dcterms:created>
    <skos:definition xml:lang="en">The Nortek Aquadopp 3000 is a single-depth doppler current meter designed for deployment in intermediate water depths down to 3000 m. It is suitable for use on moorings or fixed structures. It features higher power and an increased signal-to-noise ratio compared with the standard (300 m depth rated) Aquadopp so that it can provide accurate current measurements in water with low concentrations of suspended particulate matter. Current velocity is derived from the Doppler shift measured by two or three 2MHz acoustic beams. It comes with compass, tilt, pressure and temperature sensors. Data are stored on an internal data logger. It can be run in diagnostic mode when set to collect data at 1 Hz frequency in user specified intervals, which allows studies of mooring motion and the performance of other current meters to be conducted.</skos:definition>
    <dc:source>(L221) SeaVoX Device Catalogue</dc:source>
    <dc:publisher>British Oceanographic Data Centre (BODC)</dc:publisher>
    <skos:scopeNote xml:lang="en">manufacturer:Nortek</skos:scopeNote>
  </rdf:Description>
  <rdf:Description rdf:about="http://vocab.nerc.ac.uk/collection/L05/current/115">
    <rdf:type rdf:resource="http://www.w3.org/2004/02/skos/core#Concept" />
    <skos:prefLabel xml:lang="en">current profilers</skos:prefLabel>
    <skos:narrower rdf:resource="http://vocab.aodn.org.au/def/instrument/entity/37" />
    <skos:topConceptOf rdf:resource="http://vocab.aodn.org.au/def/instrument/1" />
    <dcterms:created rdf:datatype="http://www.w3.org/2001/XMLSchema#dateTime">2012-12-19T00:00:00Z</dcterms:created>
    <skos:definition xml:lang="en">Instrument that measures current speed and direction at multiple predetermined depths simultaneously</skos:definition>
    <dc:source>(L051) SeaDataNet device categories</dc:source>
    <dc:publisher>British Oceanographic Data Centre (BODC)</dc:publisher>
    <skos:narrower rdf:resource="http://vocab.nerc.ac.uk/collection/L22/current/TOOL0888/" />
    <skos:inScheme rdf:resource="http://vocab.aodn.org.au/def/instrument/1" />
    <dcterms:contributor>Natalia_Atkins</dcterms:contributor>
    <skos:narrower rdf:resource="http://vocab.nerc.ac.uk/collection/L22/current/TOOL0056" />
    <skos:narrower rdf:resource="http://vocab.nerc.ac.uk/collection/L22/current/TOOL0293" />
    <skos:narrower rdf:resource="http://vocab.nerc.ac.uk/collection/L22/current/TOOL0294" />
    <skos:narrower rdf:resource="http://vocab.nerc.ac.uk/collection/L22/current/TOOL0295" />
    <skos:narrower rdf:resource="http://vocab.nerc.ac.uk/collection/L22/current/TOOL0445" />
    <skos:narrower rdf:resource="http://vocab.nerc.ac.uk/collection/L22/current/TOOL0732" />
    <dcterms:modified rdf:datatype="http://www.w3.org/2001/XMLSchema#dateTime">2015-07-01T02:08:02Z</dcterms:modified>
    <skos:narrower rdf:resource="http://vocab.nerc.ac.uk/collection/L22/current/TOOL0898/" />
  </rdf:Description>
  <rdf:Description rdf:about="http://vocab.nerc.ac.uk/collection/L22/current/TOOL0732">
    <rdf:type rdf:resource="http://www.w3.org/2004/02/skos/core#Concept" />
    <skos:prefLabel xml:lang="en">Teledyne RDI Workhorse Quartermaster 150kHz ADCP</skos:prefLabel>
    <skos:inScheme rdf:resource="http://vocab.aodn.org.au/def/instrument/1" />
    <dcterms:created rdf:datatype="http://www.w3.org/2001/XMLSchema#dateTime">2014-07-16T00:00:00Z</dcterms:created>
    <skos:definition xml:lang="en">A 4-beam 150 KHz instrument designed for moored instrument applications at depths down to 1500m as standard or 3000m and 600m as options. Effective measurement range is 300m with up to 255 bins each 2-24m deep. Velocity accuracy is the greater of 1% or 0.5 cm/s.  More information is available at http://www.rdinstruments.com/datasheets/quartermaster_ds.pdf.</skos:definition>
    <dc:source>(L221) SeaVoX Device Catalogue</dc:source>
    <dc:publisher>British Oceanographic Data Centre (BODC)</dc:publisher>
  </rdf:Description>
  <rdf:Description rdf:about="http://vocab.nerc.ac.uk/collection/L22/current/TOOL0898/">
    <rdf:type rdf:resource="http://www.w3.org/2004/02/skos/core#Concept" />
    <skos:prefLabel xml:lang="en">Nortek acoustic wave and current profiler</skos:prefLabel>
    <skos:altLabel xml:lang="en">Nortek AWAC</skos:altLabel>
    <skos:inScheme rdf:resource="http://vocab.aodn.org.au/def/instrument/1" />
    <dcterms:created rdf:datatype="http://www.w3.org/2001/XMLSchema#dateTime">2015-06-03T00:00:00Z</dcterms:created>
    <skos:definition xml:lang="en">A family of instruments that simultaneously measure current profiles and wave height and direction designed for coastal monitoring.  It is available in three transmit frequencies: 1 MHz (range 30 m, cell size 0.25-4 m); 600 kHz (range 50 m, cell size 0.5-8 m), 400 kHz (range 100 m, cell size 1-8 m) and has  four beams, one vertical and the other three 120 degrees apart slanted at 25 degrees. Maximum number of cells is 128. Current speeds up to 10 m/s may be measured at an accuracy of 1% of measured value ±0.5cm/s. Temperature (embedded thermistor with 0.1C accuracy and 0.01C resolution), compass (magnetometer with 2 degrees accuracy and 0.1 degree resolution providing tilt less than 15 degrees), tilt (liquid level) and pressure (piezo resistive with accuracy of 0.5% (optional 0.1%) full scale - usually 100m - and resolution of 0.005% full scale) sensors are provided as standard.</skos:definition>
    <dc:publisher>British Oceanographic Data Centre (BODC)</dc:publisher>
    <dcterms:modified rdf:datatype="http://www.w3.org/2001/XMLSchema#dateTime">2015-06-30T06:19:13Z</dcterms:modified>
    <dcterms:contributor>Natalia_Atkins</dcterms:contributor>
  </rdf:Description>
  <rdf:Description rdf:about="http://vocab.nerc.ac.uk/collection/L22/current/TOOL0445">
    <rdf:type rdf:resource="http://www.w3.org/2004/02/skos/core#Concept" />
    <skos:prefLabel xml:lang="en">Teledyne RDI Broadband 150kHz ADCP</skos:prefLabel>
    <skos:inScheme rdf:resource="http://vocab.aodn.org.au/def/instrument/1" />
    <dcterms:created rdf:datatype="http://www.w3.org/2001/XMLSchema#dateTime">2014-02-06T00:00:00Z</dcterms:created>
    <skos:definition xml:lang="en">The RDI Broadband ADCP is designed for mooring deployment and has an operating frequency of 150 kHz. The instrument uses Doppler-technology to achieve accurate and non-intrusive measurements and it can come with pressure and temperature sensors. It can be used in real time measurement situations or can log to an internal recorder powered by internal batteries.</skos:definition>
    <dc:source>(L221) SeaVoX Device Catalogue</dc:source>
    <dc:publisher>British Oceanographic Data Centre (BODC)</dc:publisher>
    <skos:scopeNote xml:lang="en">manufacturer:Teledyne RD Instruments</skos:scopeNote>
  </rdf:Description>
  <rdf:Description rdf:about="http://vocab.aodn.org.au/def/instrument/entity/37">
    <rdf:type rdf:resource="http://www.w3.org/2004/02/skos/core#Concept" />
    <skos:prefLabel xml:lang="en">Nortek Continental</skos:prefLabel>
    <dcterms:created rdf:datatype="http://www.w3.org/2001/XMLSchema#dateTime">2013-03-28T00:00:00Z</dcterms:created>
    <skos:definition xml:lang="en">The Continental comes in two frequencies, the 190 kHz version that is used for maximum (vertical) profiling range and the 470 kHz unit that is mostly used in 2D horizontal applications due to the narrow beam width and long profiling range in shallow water. In either case, you get the full advantage of affordable prices, flexible hardware with extra sensor interfaces, titanium and plastic housings, and an excellent software suite to control the instrument in online or stand-alone applications. The Nortek power management is included in the Continental, allowing stand-alone deployments from 3–12 months definal on battery options and range requirements. All models come standard with compass, tilt, pressure, and temperature sensors and an internal recorder. Optional equipment includes larger recorders for longer deployment and external battery housings that do not interfere with the compass located in the low-profile Continental housing.</skos:definition>
    <dc:source>Australian Ocean Data Network instrument register</dc:source>
    <dc:publisher>eMarine Information Infrastructure (eMII)</dc:publisher>
    <skos:scopeNote xml:lang="en">manufacturer:Nortek</skos:scopeNote>
    <dcterms:creator xml:lang="en">Sebastien Mancini</dcterms:creator>
    <skos:inScheme rdf:resource="http://vocab.aodn.org.au/def/instrument/1" />
  </rdf:Description>
  <rdf:Description rdf:about="http://vocab.nerc.ac.uk/collection/L22/current/TOOL0056">
    <rdf:type rdf:resource="http://www.w3.org/2004/02/skos/core#Concept" />
    <skos:prefLabel xml:lang="en">Teledyne RDI Workhorse Long-Ranger ADCP</skos:prefLabel>
    <skos:inScheme rdf:resource="http://vocab.aodn.org.au/def/instrument/1" />
    <dcterms:created rdf:datatype="http://www.w3.org/2001/XMLSchema#dateTime">2013-03-28T00:00:00Z</dcterms:created>
    <skos:definition xml:lang="en">The Teledyne RDI Workhorse Long-Ranger acoustic doppler current profiler is a long-range and long-term self contained ADCP. It has a patented broadband signal (75 kHz) and a standard depth rating of 1500m. It operates effectively between temperatures of -5 DegC and 45 DegC and has a velocity accuracy of plus or minus 1%; plus or minus 5 mm per s</skos:definition>
    <dc:source>(L221) SeaVoX Device Catalogue</dc:source>
    <dc:publisher>British Oceanographic Data Centre (BODC)</dc:publisher>
    <skos:scopeNote xml:lang="en">manufacturer:Teledyne RD Instruments</skos:scopeNote>
  </rdf:Description>
  <rdf:Description rdf:about="http://vocab.nerc.ac.uk/collection/L22/current/TOOL0295">
    <rdf:type rdf:resource="http://www.w3.org/2004/02/skos/core#Concept" />
    <skos:prefLabel xml:lang="en">Teledyne RDI Workhorse Sentinel-300 ADCP</skos:prefLabel>
    <skos:inScheme rdf:resource="http://vocab.aodn.org.au/def/instrument/1" />
    <dcterms:created rdf:datatype="http://www.w3.org/2001/XMLSchema#dateTime">2013-03-28T00:00:00Z</dcterms:created>
    <skos:definition xml:lang="en">An ADCP designed for self-contained use on moorings or vessel mounting. It has a patented 300 kHz broadband signal and a standard depth rating of 200 metres. It operates effectively between temperatures of -5 to 45 DegC and a range of up to 165m with a depth cell size of 8m. Velocity accuracy is plus or minus 0.5% or 0.5 cm/sec.</skos:definition>
    <dc:source>(L221) SeaVoX Device Catalogue</dc:source>
    <dc:publisher>British Oceanographic Data Centre (BODC)</dc:publisher>
    <skos:scopeNote xml:lang="en">manufacturer:Teledyne RD Instruments</skos:scopeNote>
  </rdf:Description>
  <rdf:Description rdf:about="http://vocab.nerc.ac.uk/collection/L22/current/TOOL0294">
    <rdf:type rdf:resource="http://www.w3.org/2004/02/skos/core#Concept" />
    <skos:prefLabel xml:lang="en">Teledyne RDI Workhorse Sentinel-600 ADCP</skos:prefLabel>
    <skos:inScheme rdf:resource="http://vocab.aodn.org.au/def/instrument/1" />
    <dcterms:created rdf:datatype="http://www.w3.org/2001/XMLSchema#dateTime">2013-03-28T00:00:00Z</dcterms:created>
    <skos:definition xml:lang="en">An ADCP designed for self-contained use on moorings or vessel mounting. It has a patented 600 kHz broadband signal and a standard depth rating of 200 metres. It operates effectively between temperatures of -5 to 45 DegC and a range of up to 70m with a depth cell size of 4m.Velocity accuracy is plus or minus 0.3% or 0.3 cm/sec.</skos:definition>
    <dc:source>(L221) SeaVoX Device Catalogue</dc:source>
    <dc:publisher>British Oceanographic Data Centre (BODC)</dc:publisher>
    <skos:scopeNote xml:lang="en">manufacturer:Teledyne RD Instruments</skos:scopeNote>
  </rdf:Description>
  <rdf:Description rdf:about="http://vocab.nerc.ac.uk/collection/L22/current/TOOL0293">
    <rdf:type rdf:resource="http://www.w3.org/2004/02/skos/core#Concept" />
    <skos:prefLabel xml:lang="en">Teledyne RDI Workhorse Sentinel-1200 ADCP</skos:prefLabel>
    <skos:inScheme rdf:resource="http://vocab.aodn.org.au/def/instrument/1" />
    <dcterms:created rdf:datatype="http://www.w3.org/2001/XMLSchema#dateTime">2013-03-28T00:00:00Z</dcterms:created>
    <skos:definition xml:lang="en">An ADCP designed for self-contained use on moorings or vessel mounting. It has a patented 1200 kHz broadband signal and a standard depth rating of 200 metres. It operates effectively between temperatures of -5 to 45 DegC and a range of up to 20m with a depth cell size of 2m. Velocity accuracy is plus or minus  0.3% or 0.3 cm/sec.</skos:definition>
    <dc:source>(L221) SeaVoX Device Catalogue</dc:source>
    <dc:publisher>British Oceanographic Data Centre (BODC)</dc:publisher>
    <skos:scopeNote xml:lang="en">manufacturer:Teledyne RD Instruments</skos:scopeNote>
  </rdf:Description>
  <rdf:Description rdf:about="http://vocab.nerc.ac.uk/collection/L22/current/TOOL0888/">
    <rdf:type rdf:resource="http://www.w3.org/2004/02/skos/core#Concept" />
    <skos:prefLabel xml:lang="en">Nortek Aquadopp Doppler current profiler</skos:prefLabel>
    <skos:altLabel xml:lang="en">Aquadopp profiler</skos:altLabel>
    <skos:inScheme rdf:resource="http://vocab.aodn.org.au/def/instrument/1" />
    <dcterms:created rdf:datatype="http://www.w3.org/2001/XMLSchema#dateTime">2015-06-03T00:00:00Z</dcterms:created>
    <skos:definition xml:lang="en">A family of self-contained Doppler current profilers designed for deployment on the seabed, moorings, buoys or fixed structures.  A range of transducers - 400 kHz (60-90m range: 2-8m cell size), 600 kHz (30-40m range: 1-4m cell size), Z-cell 600 kHz, 1 MHz (12-20m range: 0.3-4m cell size), Z-cell 1MHz, 2 MHz (4-10m range:0.1-2m cell size) and side-looking.  Each transducer has 3 beams and the instrument has a maximum of 128 cells. Current speeds up to 10 m/s may be measured at an accuracy of 1% of measured value ±0.5cm/s. The standard depth rating is 300 m with 3000 m or 600m versions available. Temperature (embedded thermistor with 0.1C accuracy and 0.01C resolution), compass (magnetometer with 2 degrees accuracy and 0.1 degree resolution providing tilt less than 20 degrees), tilt (liquid level with 0.2 degree accuracy and 0.1 degree resolution) and pressure (piezo resistive with accuracy of 0.5% full scale - usually 100m - and resolution of 0.005% full scale) sensors are provided as standard.</skos:definition>
    <dc:publisher>British Oceanographic Data Centre (BODC)</dc:publisher>
    <dcterms:modified rdf:datatype="http://www.w3.org/2001/XMLSchema#dateTime">2015-07-01T02:07:35Z</dcterms:modified>
    <dcterms:contributor>Natalia_Atkins</dcterms:contributor>
  </rdf:Description>
  <rdf:Description rdf:about="http://vocab.nerc.ac.uk/collection/L05/current/82">
    <rdf:type rdf:resource="http://www.w3.org/2004/02/skos/core#Concept" />
    <skos:prefLabel xml:lang="en">in-situ incubators</skos:prefLabel>
    <skos:topConceptOf rdf:resource="http://vocab.aodn.org.au/def/instrument/1" />
    <skos:inScheme rdf:resource="http://vocab.aodn.org.au/def/instrument/1" />
    <dcterms:created rdf:datatype="http://www.w3.org/2001/XMLSchema#dateTime">2014-05-22T00:00:00Z</dcterms:created>
    <skos:definition xml:lang="en">A rig that allows water samples to be retained from where they were collected whilst physically separated from their surroundings.  Includes small-scale incubation rigs and mesocosms.</skos:definition>
    <dc:source>(L051) SeaDataNet device categories</dc:source>
    <dc:publisher>British Oceanographic Data Centre (BODC)</dc:publisher>
  </rdf:Description>
  <rdf:Description rdf:about="http://vocab.nerc.ac.uk/collection/L05/current/81">
    <rdf:type rdf:resource="http://www.w3.org/2004/02/skos/core#Concept" />
    <skos:prefLabel xml:lang="en">shipboard incubators</skos:prefLabel>
    <skos:topConceptOf rdf:resource="http://vocab.aodn.org.au/def/instrument/1" />
    <skos:inScheme rdf:resource="http://vocab.aodn.org.au/def/instrument/1" />
    <dcterms:created rdf:datatype="http://www.w3.org/2001/XMLSchema#dateTime">2014-05-22T00:00:00Z</dcterms:created>
    <skos:definition xml:lang="en">A device mounted on a ship that holds water samples under conditions of controlled temperature or controlled temperature and illumination.</skos:definition>
    <dc:source>(L051) SeaDataNet device categories</dc:source>
    <dc:publisher>British Oceanographic Data Centre (BODC)</dc:publisher>
  </rdf:Description>
  <rdf:Description rdf:about="http://vocab.nerc.ac.uk/collection/L05/current/LAB40">
    <rdf:type rdf:resource="http://www.w3.org/2004/02/skos/core#Concept" />
    <skos:prefLabel xml:lang="en">Volume measures</skos:prefLabel>
    <skos:topConceptOf rdf:resource="http://vocab.aodn.org.au/def/instrument/1" />
    <skos:inScheme rdf:resource="http://vocab.aodn.org.au/def/instrument/1" />
    <dcterms:created rdf:datatype="http://www.w3.org/2001/XMLSchema#dateTime">2013-07-18T00:00:00Z</dcterms:created>
    <skos:definition xml:lang="en">Pieces of apparatus that determine the volume of a liquid sample or dispense measured volumes of liquid. Includes devices covering a wide range of sophistication from measuring cylinders syringes and manual pipettes through to programmable electronic instruments.</skos:definition>
    <dc:source>(L051) SeaDataNet device categories</dc:source>
    <dc:publisher>British Oceanographic Data Centre (BODC)</dc:publisher>
  </rdf:Description>
  <rdf:Description rdf:about="http://vocab.nerc.ac.uk/collection/L05/current/FFES">
    <rdf:type rdf:resource="http://www.w3.org/2004/02/skos/core#Concept" />
    <skos:prefLabel xml:lang="en">Fish-finder echosounders</skos:prefLabel>
    <skos:topConceptOf rdf:resource="http://vocab.aodn.org.au/def/instrument/1" />
    <skos:inScheme rdf:resource="http://vocab.aodn.org.au/def/instrument/1" />
    <dcterms:created rdf:datatype="http://www.w3.org/2001/XMLSchema#dateTime">2013-10-09T00:00:00Z</dcterms:created>
    <skos:definition xml:lang="en">Instruments primarily designed to detect shoals of fish through transmission and reception of acoustic signals.  They are often optimised for this purpose through the use of multiple frequencies.</skos:definition>
    <dc:source>(L051) SeaDataNet device categories</dc:source>
    <dc:publisher>British Oceanographic Data Centre (BODC)</dc:publisher>
    <skos:narrower rdf:resource="http://vocab.nerc.ac.uk/collection/L22/current/TOOL0198" />
    <skos:narrower rdf:resource="http://vocab.nerc.ac.uk/collection/L22/current/TOOL0689" />
  </rdf:Description>
  <rdf:Description rdf:about="http://vocab.nerc.ac.uk/collection/L22/current/TOOL0689">
    <rdf:type rdf:resource="http://www.w3.org/2004/02/skos/core#Concept" />
    <skos:prefLabel xml:lang="en">Simrad ES60 echosounder</skos:prefLabel>
    <skos:inScheme rdf:resource="http://vocab.aodn.org.au/def/instrument/1" />
    <dcterms:created rdf:datatype="http://www.w3.org/2001/XMLSchema#dateTime">2013-10-09T00:00:00Z</dcterms:created>
    <skos:definition xml:lang="en">A third generation single-beam or split-beam multi-frequncy echosounder primarily designed for fish-finding but may also be used in fisheries research. More information may be found in http://www.simrad.com/www/01/NOKBG0397.nsf/AllWeb/1C1B8782314422F9C12570F300270EAC/$file/Simrad_ES60_Brochure_English.pdf?OpenElement.This instrument is now (April 2014) flagged as discontinues on the Simrad web site.</skos:definition>
    <dc:source>(L221) SeaVoX Device Catalogue</dc:source>
    <dc:publisher>British Oceanographic Data Centre (BODC)</dc:publisher>
    <skos:scopeNote xml:lang="en">manufacturer:Kongsberg Maritime AS</skos:scopeNote>
  </rdf:Description>
  <rdf:Description rdf:about="http://vocab.nerc.ac.uk/collection/L22/current/TOOL0198">
    <rdf:type rdf:resource="http://www.w3.org/2004/02/skos/core#Concept" />
    <skos:prefLabel xml:lang="en">Simrad EK-60 echosounder</skos:prefLabel>
    <skos:inScheme rdf:resource="http://vocab.aodn.org.au/def/instrument/1" />
    <dcterms:created rdf:datatype="http://www.w3.org/2001/XMLSchema#dateTime">2013-10-09T00:00:00Z</dcterms:created>
    <skos:definition xml:lang="en">A split-beam scientific echosounder primarily designed for fisheries research. It can operate seven frequencies simultaneously ranging from 18 to 710 kHz. Real time echo integration and target strength analysis in an unlimited number of layers is provided as well as storage of raw data for replay or analysis in one of several post-processing software packages such as Simrad's BI60.</skos:definition>
    <dc:source>(L221) SeaVoX Device Catalogue</dc:source>
    <dc:publisher>British Oceanographic Data Centre (BODC)</dc:publisher>
    <skos:scopeNote xml:lang="en">manufacturer:Kongsberg Maritime AS</skos:scopeNote>
  </rdf:Description>
  <rdf:Description rdf:about="http://vocab.nerc.ac.uk/collection/L05/current/122">
    <rdf:type rdf:resource="http://www.w3.org/2004/02/skos/core#Concept" />
    <skos:prefLabel xml:lang="en">radiometers</skos:prefLabel>
    <skos:narrower rdf:resource="http://vocab.aodn.org.au/def/instrument/entity/545" />
    <skos:topConceptOf rdf:resource="http://vocab.aodn.org.au/def/instrument/1" />
    <dcterms:created rdf:datatype="http://www.w3.org/2001/XMLSchema#dateTime">2013-03-28T00:00:00Z</dcterms:created>
    <skos:definition xml:lang="en">Instrument that measures the intensity of electromagnetic radiation in either the atmosphere or the water column</skos:definition>
    <dc:source>(L051) SeaDataNet device categories</dc:source>
    <dc:publisher>British Oceanographic Data Centre (BODC)</dc:publisher>
    <skos:inScheme rdf:resource="http://vocab.aodn.org.au/def/instrument/1" />
    <skos:narrower rdf:resource="http://vocab.nerc.ac.uk/collection/L22/current/TOOL0083" />
    <skos:narrower rdf:resource="http://vocab.nerc.ac.uk/collection/L22/current/TOOL0120" />
    <skos:narrower rdf:resource="http://vocab.nerc.ac.uk/collection/L22/current/TOOL0193" />
    <skos:narrower rdf:resource="http://vocab.nerc.ac.uk/collection/L22/current/TOOL0625" />
    <skos:narrower rdf:resource="http://vocab.nerc.ac.uk/collection/L22/current/TOOL0666" />
    <skos:narrower rdf:resource="http://vocab.nerc.ac.uk/collection/L22/current/TOOL0676" />
  </rdf:Description>
  <rdf:Description rdf:about="http://vocab.nerc.ac.uk/collection/L22/current/TOOL0120">
    <rdf:type rdf:resource="http://www.w3.org/2004/02/skos/core#Concept" />
    <skos:prefLabel xml:lang="en">LI-COR LI-192 PAR sensor</skos:prefLabel>
    <skos:inScheme rdf:resource="http://vocab.aodn.org.au/def/instrument/1" />
    <dcterms:created rdf:datatype="http://www.w3.org/2001/XMLSchema#dateTime">2013-10-15T00:00:00Z</dcterms:created>
    <skos:definition xml:lang="en">An underwater or atmospheric quantum sensor with cosine correction that can operate down to 560m. Fitted with a blue-enhanced silicon photovoltaic detector.</skos:definition>
    <dc:source>(L221) SeaVoX Device Catalogue</dc:source>
    <dc:publisher>British Oceanographic Data Centre (BODC)</dc:publisher>
    <skos:scopeNote xml:lang="en">manufacturer:LI-COR Incorporated</skos:scopeNote>
  </rdf:Description>
  <rdf:Description rdf:about="http://vocab.nerc.ac.uk/collection/L22/current/TOOL0666">
    <rdf:type rdf:resource="http://www.w3.org/2004/02/skos/core#Concept" />
    <skos:prefLabel xml:lang="en">Eppley Precision Spectral Pyranometer</skos:prefLabel>
    <skos:inScheme rdf:resource="http://vocab.aodn.org.au/def/instrument/1" />
    <dcterms:created rdf:datatype="http://www.w3.org/2001/XMLSchema#dateTime">2013-10-15T00:00:00Z</dcterms:created>
    <skos:definition xml:lang="en">A discontinued instrument that measured sun and sky irradiance in the range of wavelengths 0.285 to 2.8 microns, including most of the solar spectrum.  It had a "hemispheric receiver" intended to approximate the cosine response for oblique rays. More information may be found at http://www.yale.edu/ceo/Documentation/Eppley%20Precision%20Spectral%20Pyranometer.pdf.</skos:definition>
    <dc:source>(L221) SeaVoX Device Catalogue</dc:source>
    <dc:publisher>British Oceanographic Data Centre (BODC)</dc:publisher>
    <skos:scopeNote xml:lang="en">manufacturer:The Eppley Laboratory Inc.</skos:scopeNote>
  </rdf:Description>
  <rdf:Description rdf:about="http://vocab.nerc.ac.uk/collection/L22/current/TOOL0083">
    <rdf:type rdf:resource="http://www.w3.org/2004/02/skos/core#Concept" />
    <skos:prefLabel xml:lang="en">Eppley Precision Infrared Radiometer Pyrgyometer</skos:prefLabel>
    <skos:inScheme rdf:resource="http://vocab.aodn.org.au/def/instrument/1" />
    <dcterms:created rdf:datatype="http://www.w3.org/2001/XMLSchema#dateTime">2013-10-15T00:00:00Z</dcterms:created>
    <skos:definition xml:lang="en">The Eppley Precision Infrared Radiometer (PIR) pyrgyometer measures longwave (infrared) radiation. It is housed in a weatherproof titanium canister that has been painted with a very flat black paint that absorbs radiation. A small glass dome at the top of the instrument is covered with an 'interference coating' which allows only infrared radiation to come through. Light levels are detected as temperature changes creating voltages in fine wire coil detectors.</skos:definition>
    <dc:source>(L221) SeaVoX Device Catalogue</dc:source>
    <dc:publisher>British Oceanographic Data Centre (BODC)</dc:publisher>
    <skos:scopeNote xml:lang="en">manufacturer:The Eppley Laboratory Inc.</skos:scopeNote>
  </rdf:Description>
  <rdf:Description rdf:about="http://vocab.nerc.ac.uk/collection/L22/current/TOOL0676">
    <rdf:type rdf:resource="http://www.w3.org/2004/02/skos/core#Concept" />
    <skos:prefLabel xml:lang="en">WETLabs ECO-PAR</skos:prefLabel>
    <skos:inScheme rdf:resource="http://vocab.aodn.org.au/def/instrument/1" />
    <dcterms:created rdf:datatype="http://www.w3.org/2001/XMLSchema#dateTime">2014-04-01T00:00:00Z</dcterms:created>
    <skos:definition xml:lang="en">A cosine-collector underwater light meter in an acetal co-polymer housing sensitive to photosynthetically-active (400-700nm) radiation (PAR).  It is equipped with 'Bio-wiper' technology to prevent biofouling and so is capable of long-term deployments on buoys and moorings. For more information see http://www.wetlabs.com/eco-par.</skos:definition>
    <dc:source>(L221) SeaVoX Device Catalogue</dc:source>
    <dc:publisher>British Oceanographic Data Centre (BODC)</dc:publisher>
    <skos:scopeNote xml:lang="en">manufacture:WETLabs Inc.</skos:scopeNote>
  </rdf:Description>
  <rdf:Description rdf:about="http://vocab.nerc.ac.uk/collection/L22/current/TOOL0193">
    <rdf:type rdf:resource="http://www.w3.org/2004/02/skos/core#Concept" />
    <skos:prefLabel xml:lang="en">LI-COR LI-190 PAR sensor</skos:prefLabel>
    <skos:inScheme rdf:resource="http://vocab.aodn.org.au/def/instrument/1" />
    <dcterms:created rdf:datatype="http://www.w3.org/2001/XMLSchema#dateTime">2013-10-15T00:00:00Z</dcterms:created>
    <skos:definition xml:lang="en">A non-submersible cosine-corrected PAR sensor sensitive wavelengths from 400-700nm with sharp cut-off due to an interference filter. It may be used as a reference sensor for LI-192 and LI-193 Underwater Quantum Sensor.</skos:definition>
    <dc:source>(L221) SeaVoX Device Catalogue</dc:source>
    <dc:publisher>British Oceanographic Data Centre (BODC)</dc:publisher>
    <skos:scopeNote xml:lang="en">manufacturer:LI-COR Incorporated</skos:scopeNote>
  </rdf:Description>
  <rdf:Description rdf:about="http://vocab.aodn.org.au/def/instrument/entity/545">
    <rdf:type rdf:resource="http://www.w3.org/2004/02/skos/core#Concept" />
    <skos:prefLabel xml:lang="en">Eppley Ultraviolet Radiometer (UVB)</skos:prefLabel>
    <dcterms:created rdf:datatype="http://www.w3.org/2001/XMLSchema#dateTime">2013-10-15T00:00:00Z</dcterms:created>
    <skos:definition xml:lang="en" />
    <dc:source>Australian Ocean Data Network instrument register</dc:source>
    <dc:publisher>eMarine Information Infrastructure (eMII)</dc:publisher>
    <skos:scopeNote xml:lang="en">manufacturer:The Eppley Laboratory Inc.</skos:scopeNote>
    <dcterms:creator xml:lang="en">Sebastien Mancini</dcterms:creator>
    <skos:inScheme rdf:resource="http://vocab.aodn.org.au/def/instrument/1" />
  </rdf:Description>
  <rdf:Description rdf:about="http://vocab.nerc.ac.uk/collection/L22/current/TOOL0625">
    <rdf:type rdf:resource="http://www.w3.org/2004/02/skos/core#Concept" />
    <skos:prefLabel xml:lang="en">Satlantic OCR-504 multispectral radiometer</skos:prefLabel>
    <skos:inScheme rdf:resource="http://vocab.aodn.org.au/def/instrument/1" />
    <dcterms:created rdf:datatype="http://www.w3.org/2001/XMLSchema#dateTime">2013-09-09T00:00:00Z</dcterms:created>
    <skos:definition xml:lang="en">In 2010, Satlantic joined Sea-Bird Electronics and WET Labs Inc. to form Sea-Bird Scientific. Within Sea-Bird Scientific, Satlantic works closely with Sea-Bird and WET Labs to design integrated physical and biogeochemical sensors for the global scientific community. The OCR-500 Series Radiometers are fully digital optical sensors that combine precision optics and high performance microelectronics.  The radiometers may be operated as a stand-alone device or in a networked environment as part of a larger system.  These units are available in four (this model) or seven channel discrete wavelengths.     Features: Irradiance and Radiance sensors for in-water and in-air applications, Standard wavelengths from 400 - 865 nm, UV wavelengths available 305, 325, 340 &amp; 380 nm, Fully characterized cosine response, Custom low fluorescence filters,  Networking capability, Data logging and processing software included, Fast sampling rate (7 - 24 Hz optional), and Compatible with the Bioshutter anti-biofouling solution.</skos:definition>
    <dc:source>(L221) SeaVoX Device Catalogue</dc:source>
    <dc:publisher>British Oceanographic Data Centre (BODC)</dc:publisher>
    <skos:scopeNote xml:lang="en">manufacturer:Satlantic</skos:scopeNote>
  </rdf:Description>
  <rdf:Description rdf:about="http://vocab.nerc.ac.uk/collection/L05/current/123">
    <rdf:type rdf:resource="http://www.w3.org/2004/02/skos/core#Concept" />
    <skos:prefLabel xml:lang="en">optical backscatter sensors</skos:prefLabel>
    <skos:topConceptOf rdf:resource="http://vocab.aodn.org.au/def/instrument/1" />
    <skos:inScheme rdf:resource="http://vocab.aodn.org.au/def/instrument/1" />
    <dcterms:created rdf:datatype="http://www.w3.org/2001/XMLSchema#dateTime">2013-07-18T00:00:00Z</dcterms:created>
    <skos:definition xml:lang="en">Instrument that measures the amount of electromagnetic radiation emitted into the water column returned to the instrument.</skos:definition>
    <dc:source>(L051) SeaDataNet device categories</dc:source>
    <dc:publisher>British Oceanographic Data Centre (BODC)</dc:publisher>
    <skos:narrower rdf:resource="http://vocab.nerc.ac.uk/collection/L22/current/TOOL0215" />
    <skos:narrower rdf:resource="http://vocab.nerc.ac.uk/collection/L22/current/TOOL0673" />
    <skos:narrower rdf:resource="http://vocab.nerc.ac.uk/collection/L22/current/TOOL0674" />
    <skos:narrower rdf:resource="http://vocab.nerc.ac.uk/collection/L22/current/TOOL0675" />
    <skos:narrower rdf:resource="http://vocab.nerc.ac.uk/collection/L22/current/TOOL0879/" />
  </rdf:Description>
  <rdf:Description rdf:about="http://vocab.nerc.ac.uk/collection/L22/current/TOOL0675">
    <rdf:type rdf:resource="http://www.w3.org/2004/02/skos/core#Concept" />
    <skos:prefLabel xml:lang="en">WETLabs Water Quality Monitor</skos:prefLabel>
    <dcterms:created rdf:datatype="http://www.w3.org/2001/XMLSchema#dateTime">2014-04-01T00:00:00Z</dcterms:created>
    <skos:definition xml:lang="en">An instrument that incorporates WET Labs fluorometer-turbidity and Sea-Bird's CTD sensors, providing temperature, salinity, depth, dissolved oxygen, chlorophyll fluorescence, turbidity and backscattering data. It is designed for long-term deployment in coastal waters with protection against biofouling and fouling by sediment loads. More information is available at http://www.wetlabs.com/wqm.</skos:definition>
    <dc:source>(L221) SeaVoX Device Catalogue</dc:source>
    <dc:publisher>British Oceanographic Data Centre (BODC)</dc:publisher>
    <skos:inScheme rdf:resource="http://vocab.aodn.org.au/def/instrument/1" />
    <skos:scopeNote xml:lang="en">manufacture:WETLabs Inc.</skos:scopeNote>
  </rdf:Description>
  <rdf:Description rdf:about="http://vocab.nerc.ac.uk/collection/L22/current/TOOL0215">
    <rdf:type rdf:resource="http://www.w3.org/2004/02/skos/core#Concept" />
    <skos:prefLabel xml:lang="en">WETLabs ECO-FLNTU combined fluorometer and turbidity sensor</skos:prefLabel>
    <dcterms:created rdf:datatype="http://www.w3.org/2001/XMLSchema#dateTime">2013-12-16T00:00:00Z</dcterms:created>
    <skos:definition xml:lang="en">The ECO-FLNTU combines the ECO fluorometer with an optical scattering measurement at 700nm for simultaneous determination of turbidity. The fluorometer can typically measure phytoplankton concentrations in the range 0.01-50 ug/l, with a sensitivity of 0.01 ug/l. The turbidity sensor can measure within the range 0.01-25 NTU, with a sensitivity of 0.01 NTU. The instrument is stable over a temperature range of 0-20 degC and is rated to a depth of 600 m as standard, with the option of a 'deep' instrument rated to 6000m.</skos:definition>
    <dc:source>(L221) SeaVoX Device Catalogue</dc:source>
    <dc:publisher>British Oceanographic Data Centre (BODC)</dc:publisher>
    <skos:inScheme rdf:resource="http://vocab.aodn.org.au/def/instrument/1" />
    <skos:scopeNote xml:lang="en">manufacture:WETLabs Inc.</skos:scopeNote>
  </rdf:Description>
  <rdf:Description rdf:about="http://vocab.nerc.ac.uk/collection/L22/current/TOOL0674">
    <rdf:type rdf:resource="http://www.w3.org/2004/02/skos/core#Concept" />
    <skos:prefLabel xml:lang="en">WETLabs ECO Triplet</skos:prefLabel>
    <dcterms:created rdf:datatype="http://www.w3.org/2001/XMLSchema#dateTime">2013-09-10T00:00:00Z</dcterms:created>
    <skos:definition xml:lang="en">A three-optical-sensor instrument that may carry any combination of fluorometers or single-wavelength scattering meters. The fluorometers are single wavelength sensors that can be configured for chlorophyll-a, CDOM, phycocyanin, phycoerythrin, fluorescein or rhodamine. Scattering meters measure optical scattering at blue, green or red wavelengths. More information may be found at http://www.wetlabs.com/eco-triplet.</skos:definition>
    <dc:source>(L221) SeaVoX Device Catalogue</dc:source>
    <dc:publisher>British Oceanographic Data Centre (BODC)</dc:publisher>
    <skos:inScheme rdf:resource="http://vocab.aodn.org.au/def/instrument/1" />
    <skos:scopeNote xml:lang="en">manufacture:WETLabs Inc.</skos:scopeNote>
  </rdf:Description>
  <rdf:Description rdf:about="http://vocab.nerc.ac.uk/collection/L22/current/TOOL0673">
    <rdf:type rdf:resource="http://www.w3.org/2004/02/skos/core#Concept" />
    <skos:prefLabel xml:lang="en">WETLabs ECO Puck Triple-Measurement Meter</skos:prefLabel>
    <dcterms:created rdf:datatype="http://www.w3.org/2001/XMLSchema#dateTime">2013-09-11T00:00:00Z</dcterms:created>
    <skos:definition xml:lang="en">A miniature version of the Environmental Characterisation Optics (ECO) sensors built for OEM applications, with the design specifically targeted at AUVs, gliders and profiling floats. The triplet version carries a fluorometer plus two other sensors that may be additional fluorometers, single-wavelength scattering meters (BB) or a volume scattering function meter (VSF). The fluorometers are single wavelength sensors that can be configured for chlorophyll-a, CDOM, phycocyanin, phycoerythrin, fluorescein or rhodamine. BB measures optical scattering at 117 degrees at 470, 532 or 650 nm wavelengths. VSF measures optical scattering at 100, 125 and 150 degrees. More information may be found at http://www.wetlabs.com/eco-puck.</skos:definition>
    <dc:source>(L221) SeaVoX Device Catalogue</dc:source>
    <dc:publisher>British Oceanographic Data Centre (BODC)</dc:publisher>
    <skos:inScheme rdf:resource="http://vocab.aodn.org.au/def/instrument/1" />
    <skos:scopeNote xml:lang="en">manufacture:WETLabs Inc.</skos:scopeNote>
  </rdf:Description>
  <rdf:Description rdf:about="http://vocab.nerc.ac.uk/collection/L22/current/TOOL0879/">
    <rdf:type rdf:resource="http://www.w3.org/2004/02/skos/core#Concept" />
    <skos:prefLabel xml:lang="en">WETLabs ECO-NTU turbidity sensor</skos:prefLabel>
    <skos:altLabel xml:lang="en">WETLabs ECO-NTU turbidity</skos:altLabel>
    <skos:inScheme rdf:resource="http://vocab.aodn.org.au/def/instrument/1" />
    <dcterms:created rdf:datatype="http://www.w3.org/2001/XMLSchema#dateTime">2015-06-03T00:00:00Z</dcterms:created>
    <skos:definition xml:lang="en">The ECO-NTU uses optical scattering at 700m to measure turbidity over the range 0-125 NTU (nephelometric turbidity units), with a sensitivity of 0.02 NTU or a range of 0-1000 NTU at a sensitivity of 0.12 NTU. The instrument is stable over a temperature range of 0-30 degC.   It has an analog signal output and a depth ratting of 600 m (300 m if the optional bio-wiper is fitted).</skos:definition>
    <dc:publisher>British Oceanographic Data Centre (BODC)</dc:publisher>
  </rdf:Description>
  <rdf:Description rdf:about="http://vocab.nerc.ac.uk/collection/L05/current/121">
    <rdf:type rdf:resource="http://www.w3.org/2004/02/skos/core#Concept" />
    <skos:prefLabel xml:lang="en">satellite tracking system</skos:prefLabel>
    <skos:topConceptOf rdf:resource="http://vocab.aodn.org.au/def/instrument/1" />
    <skos:inScheme rdf:resource="http://vocab.aodn.org.au/def/instrument/1" />
    <dcterms:created rdf:datatype="http://www.w3.org/2001/XMLSchema#dateTime">2013-07-18T00:00:00Z</dcterms:created>
    <skos:definition xml:lang="en">A network of statellites that determines the position of a transponder by triangulation such as Argos.  Generally used to track surface buoys for the determination of Lagrangian currents.</skos:definition>
    <dc:source>(L051) SeaDataNet device categories</dc:source>
    <dc:publisher>British Oceanographic Data Centre (BODC)</dc:publisher>
  </rdf:Description>
  <rdf:Description rdf:about="http://vocab.nerc.ac.uk/collection/L05/current/90">
    <rdf:type rdf:resource="http://www.w3.org/2004/02/skos/core#Concept" />
    <skos:prefLabel xml:lang="en">manual biota samplers</skos:prefLabel>
    <skos:topConceptOf rdf:resource="http://vocab.aodn.org.au/def/instrument/1" />
    <skos:inScheme rdf:resource="http://vocab.aodn.org.au/def/instrument/1" />
    <dcterms:created rdf:datatype="http://www.w3.org/2001/XMLSchema#dateTime">2014-05-22T00:00:00Z</dcterms:created>
    <skos:definition xml:lang="en">A simple tool like a hammer saw or even just a hand for the collection of biota samples</skos:definition>
    <dc:source>(L051) SeaDataNet device categories</dc:source>
    <dc:publisher>British Oceanographic Data Centre (BODC)</dc:publisher>
  </rdf:Description>
  <rdf:Description rdf:about="http://vocab.nerc.ac.uk/collection/L05/current/91">
    <rdf:type rdf:resource="http://www.w3.org/2004/02/skos/core#Concept" />
    <skos:prefLabel xml:lang="en">observers</skos:prefLabel>
    <skos:topConceptOf rdf:resource="http://vocab.aodn.org.au/def/instrument/1" />
    <skos:inScheme rdf:resource="http://vocab.aodn.org.au/def/instrument/1" />
    <dcterms:created rdf:datatype="http://www.w3.org/2001/XMLSchema#dateTime">2014-05-22T00:00:00Z</dcterms:created>
    <skos:definition xml:lang="en">Humans who estimate a parameter through observation of a phenomenon such as bird counts and visual wave observations</skos:definition>
    <dc:source>(L051) SeaDataNet device categories</dc:source>
    <dc:publisher>British Oceanographic Data Centre (BODC)</dc:publisher>
  </rdf:Description>
  <rdf:Description rdf:about="http://vocab.nerc.ac.uk/collection/L05/current/124">
    <rdf:type rdf:resource="http://www.w3.org/2004/02/skos/core#Concept" />
    <skos:prefLabel xml:lang="en">transmissometers</skos:prefLabel>
    <skos:topConceptOf rdf:resource="http://vocab.aodn.org.au/def/instrument/1" />
    <skos:inScheme rdf:resource="http://vocab.aodn.org.au/def/instrument/1" />
    <dcterms:created rdf:datatype="http://www.w3.org/2001/XMLSchema#dateTime">2013-07-18T00:00:00Z</dcterms:created>
    <skos:definition xml:lang="en">Systems that measure the attenuation of electromagnetic radiation by the water column. Includes human observer plus Secchi Disk.</skos:definition>
    <dc:source>(L051) SeaDataNet device categories</dc:source>
    <dc:publisher>British Oceanographic Data Centre (BODC)</dc:publisher>
  </rdf:Description>
  <rdf:Description rdf:about="http://vocab.nerc.ac.uk/collection/L05/current/53">
    <rdf:type rdf:resource="http://www.w3.org/2004/02/skos/core#Concept" />
    <skos:prefLabel xml:lang="en">rock corers</skos:prefLabel>
    <skos:topConceptOf rdf:resource="http://vocab.aodn.org.au/def/instrument/1" />
    <skos:inScheme rdf:resource="http://vocab.aodn.org.au/def/instrument/1" />
    <dcterms:created rdf:datatype="http://www.w3.org/2001/XMLSchema#dateTime">2014-05-22T00:00:00Z</dcterms:created>
    <skos:definition xml:lang="en">A device that drills into rock extracting a cylindrical sample</skos:definition>
    <dc:source>(L051) SeaDataNet device categories</dc:source>
    <dc:publisher>British Oceanographic Data Centre (BODC)</dc:publisher>
  </rdf:Description>
  <rdf:Description rdf:about="http://vocab.nerc.ac.uk/collection/L05/current/LAB02">
    <rdf:type rdf:resource="http://www.w3.org/2004/02/skos/core#Concept" />
    <skos:prefLabel xml:lang="en">gas chromatographs</skos:prefLabel>
    <skos:topConceptOf rdf:resource="http://vocab.aodn.org.au/def/instrument/1" />
    <skos:inScheme rdf:resource="http://vocab.aodn.org.au/def/instrument/1" />
    <dcterms:created rdf:datatype="http://www.w3.org/2001/XMLSchema#dateTime">2014-05-22T00:00:00Z</dcterms:created>
    <skos:definition xml:lang="en">Instruments separating gases volatile substances or substances dissolved in a volatile solvent by transporting an inert gas through a column packed with a sorbent to a detector for assay.</skos:definition>
    <dc:source>(L051) SeaDataNet device categories</dc:source>
    <dc:publisher>British Oceanographic Data Centre (BODC)</dc:publisher>
  </rdf:Description>
  <rdf:Description rdf:about="http://vocab.nerc.ac.uk/collection/L05/current/LAB05">
    <rdf:type rdf:resource="http://www.w3.org/2004/02/skos/core#Concept" />
    <skos:prefLabel xml:lang="en">optical microscopes</skos:prefLabel>
    <skos:topConceptOf rdf:resource="http://vocab.aodn.org.au/def/instrument/1" />
    <skos:inScheme rdf:resource="http://vocab.aodn.org.au/def/instrument/1" />
    <dcterms:created rdf:datatype="http://www.w3.org/2001/XMLSchema#dateTime">2014-05-22T00:00:00Z</dcterms:created>
    <skos:definition xml:lang="en">Instruments that generate enlarged images of samples using the phenomena of reflection and absorption of visible light. Includes conventional and inverted instruments.</skos:definition>
    <dc:source>(L051) SeaDataNet device categories</dc:source>
    <dc:publisher>British Oceanographic Data Centre (BODC)</dc:publisher>
  </rdf:Description>
  <rdf:Description rdf:about="http://vocab.nerc.ac.uk/collection/L05/current/LAB15">
    <rdf:type rdf:resource="http://www.w3.org/2004/02/skos/core#Concept" />
    <skos:prefLabel xml:lang="en">inductively-coupled plasma mass spectrometers</skos:prefLabel>
    <skos:topConceptOf rdf:resource="http://vocab.aodn.org.au/def/instrument/1" />
    <skos:inScheme rdf:resource="http://vocab.aodn.org.au/def/instrument/1" />
    <dcterms:created rdf:datatype="http://www.w3.org/2001/XMLSchema#dateTime">2014-05-22T00:00:00Z</dcterms:created>
    <skos:definition xml:lang="en">Instruments that pass nebulised samples into an inductively-coupled gas plasma (8-10000 K) where they are atomised and ionised. Ions of specific mass-to-charge ratios are quantified in a quadrupole mass spectrometer.</skos:definition>
    <dc:source>(L051) SeaDataNet device categories</dc:source>
    <dc:publisher>British Oceanographic Data Centre (BODC)</dc:publisher>
  </rdf:Description>
  <rdf:Description rdf:about="http://vocab.nerc.ac.uk/collection/L05/current/54">
    <rdf:type rdf:resource="http://www.w3.org/2004/02/skos/core#Concept" />
    <skos:prefLabel xml:lang="en">rock dredges</skos:prefLabel>
    <skos:topConceptOf rdf:resource="http://vocab.aodn.org.au/def/instrument/1" />
    <skos:inScheme rdf:resource="http://vocab.aodn.org.au/def/instrument/1" />
    <dcterms:created rdf:datatype="http://www.w3.org/2001/XMLSchema#dateTime">2014-05-22T00:00:00Z</dcterms:created>
    <skos:definition xml:lang="en">A device dragged across the seabed designed to collect loose rock samples.</skos:definition>
    <dc:source>(L051) SeaDataNet device categories</dc:source>
    <dc:publisher>British Oceanographic Data Centre (BODC)</dc:publisher>
  </rdf:Description>
  <rdf:Description rdf:about="http://vocab.nerc.ac.uk/collection/L05/current/LAB16">
    <rdf:type rdf:resource="http://www.w3.org/2004/02/skos/core#Concept" />
    <skos:prefLabel xml:lang="en">mass spectrometers</skos:prefLabel>
    <skos:topConceptOf rdf:resource="http://vocab.aodn.org.au/def/instrument/1" />
    <skos:inScheme rdf:resource="http://vocab.aodn.org.au/def/instrument/1" />
    <dcterms:created rdf:datatype="http://www.w3.org/2001/XMLSchema#dateTime">2014-05-22T00:00:00Z</dcterms:created>
    <skos:definition xml:lang="en">Instruments used to measure the mass-to-charge ratio of ions most generally used to find the composition of a sample by generating a mass spectrum representing the masses of sample components.</skos:definition>
    <dc:source>(L051) SeaDataNet device categories</dc:source>
    <dc:publisher>British Oceanographic Data Centre (BODC)</dc:publisher>
  </rdf:Description>
  <rdf:Description rdf:about="http://vocab.nerc.ac.uk/collection/L05/current/LAB07">
    <rdf:type rdf:resource="http://www.w3.org/2004/02/skos/core#Concept" />
    <skos:prefLabel xml:lang="en">electron microscopes</skos:prefLabel>
    <skos:topConceptOf rdf:resource="http://vocab.aodn.org.au/def/instrument/1" />
    <skos:inScheme rdf:resource="http://vocab.aodn.org.au/def/instrument/1" />
    <dcterms:created rdf:datatype="http://www.w3.org/2001/XMLSchema#dateTime">2014-05-22T00:00:00Z</dcterms:created>
    <skos:definition xml:lang="en">Instruments that generate enlarged images of samples using the phenomena of reflection and absorption of electrons behaving as waves.</skos:definition>
    <dc:source>(L051) SeaDataNet device categories</dc:source>
    <dc:publisher>British Oceanographic Data Centre (BODC)</dc:publisher>
  </rdf:Description>
  <rdf:Description rdf:about="http://vocab.nerc.ac.uk/collection/L05/current/LAB17">
    <rdf:type rdf:resource="http://www.w3.org/2004/02/skos/core#Concept" />
    <skos:prefLabel xml:lang="en">accelerator mass spectrometers</skos:prefLabel>
    <skos:topConceptOf rdf:resource="http://vocab.aodn.org.au/def/instrument/1" />
    <skos:inScheme rdf:resource="http://vocab.aodn.org.au/def/instrument/1" />
    <dcterms:created rdf:datatype="http://www.w3.org/2001/XMLSchema#dateTime">2014-05-22T00:00:00Z</dcterms:created>
    <skos:definition xml:lang="en">Instruments measuring the mass-to-charge ratio of the products of sample molecule disassociation atom ionisation and ion acceleration in a particle accelerator.</skos:definition>
    <dc:source>(L051) SeaDataNet device categories</dc:source>
    <dc:publisher>British Oceanographic Data Centre (BODC)</dc:publisher>
  </rdf:Description>
  <rdf:Description rdf:about="http://vocab.nerc.ac.uk/collection/L05/current/LAB06">
    <rdf:type rdf:resource="http://www.w3.org/2004/02/skos/core#Concept" />
    <skos:prefLabel xml:lang="en">fluorescence microscopes</skos:prefLabel>
    <skos:topConceptOf rdf:resource="http://vocab.aodn.org.au/def/instrument/1" />
    <skos:inScheme rdf:resource="http://vocab.aodn.org.au/def/instrument/1" />
    <dcterms:created rdf:datatype="http://www.w3.org/2001/XMLSchema#dateTime">2014-05-22T00:00:00Z</dcterms:created>
    <skos:definition xml:lang="en">Instruments that generate enlarged images of samples using the phenomena of fluorescence and phosphorescence instead of or in addition to reflection and absorption of visible light. Includes conventional and inverted instruments.</skos:definition>
    <dc:source>(L051) SeaDataNet device categories</dc:source>
    <dc:publisher>British Oceanographic Data Centre (BODC)</dc:publisher>
  </rdf:Description>
  <rdf:Description rdf:about="http://vocab.nerc.ac.uk/collection/L05/current/LAB18">
    <rdf:type rdf:resource="http://www.w3.org/2004/02/skos/core#Concept" />
    <skos:prefLabel xml:lang="en">nuclear magnetic resonance spectrometers</skos:prefLabel>
    <skos:topConceptOf rdf:resource="http://vocab.aodn.org.au/def/instrument/1" />
    <skos:inScheme rdf:resource="http://vocab.aodn.org.au/def/instrument/1" />
    <dcterms:created rdf:datatype="http://www.w3.org/2001/XMLSchema#dateTime">2014-05-22T00:00:00Z</dcterms:created>
    <skos:definition xml:lang="en">Instruments that identify and quantify magnetically active chemical entities by subjecting a sample to orthogonal magnetic and electrical fields.</skos:definition>
    <dc:source>(L051) SeaDataNet device categories</dc:source>
    <dc:publisher>British Oceanographic Data Centre (BODC)</dc:publisher>
  </rdf:Description>
  <rdf:Description rdf:about="http://vocab.nerc.ac.uk/collection/L05/current/51">
    <rdf:type rdf:resource="http://www.w3.org/2004/02/skos/core#Concept" />
    <skos:prefLabel xml:lang="en">unconsolidated sediment corers</skos:prefLabel>
    <skos:topConceptOf rdf:resource="http://vocab.aodn.org.au/def/instrument/1" />
    <skos:inScheme rdf:resource="http://vocab.aodn.org.au/def/instrument/1" />
    <dcterms:created rdf:datatype="http://www.w3.org/2001/XMLSchema#dateTime">2014-05-22T00:00:00Z</dcterms:created>
    <skos:definition xml:lang="en">Devices designed to collect samples of unconsolidated sediment from between the surface and depths from a metre to 10s of metres with minimal disturbance of the sediment structure.</skos:definition>
    <dc:source>(L051) SeaDataNet device categories</dc:source>
    <dc:publisher>British Oceanographic Data Centre (BODC)</dc:publisher>
  </rdf:Description>
  <rdf:Description rdf:about="http://vocab.nerc.ac.uk/collection/L05/current/LAB09">
    <rdf:type rdf:resource="http://www.w3.org/2004/02/skos/core#Concept" />
    <skos:prefLabel xml:lang="en">ion microprobes</skos:prefLabel>
    <skos:topConceptOf rdf:resource="http://vocab.aodn.org.au/def/instrument/1" />
    <skos:inScheme rdf:resource="http://vocab.aodn.org.au/def/instrument/1" />
    <dcterms:created rdf:datatype="http://www.w3.org/2001/XMLSchema#dateTime">2014-05-22T00:00:00Z</dcterms:created>
    <skos:definition xml:lang="en">Instruments that isotopically analyse a small area of sample by bombarding it with ions to form a plasma that is analysed in a mass spectrometer.</skos:definition>
    <dc:source>(L051) SeaDataNet device categories</dc:source>
    <dc:publisher>British Oceanographic Data Centre (BODC)</dc:publisher>
  </rdf:Description>
  <rdf:Description rdf:about="http://vocab.nerc.ac.uk/collection/L05/current/LAB19">
    <rdf:type rdf:resource="http://www.w3.org/2004/02/skos/core#Concept" />
    <skos:prefLabel xml:lang="en">gas chromatograph mass spectrometers</skos:prefLabel>
    <skos:topConceptOf rdf:resource="http://vocab.aodn.org.au/def/instrument/1" />
    <skos:inScheme rdf:resource="http://vocab.aodn.org.au/def/instrument/1" />
    <dcterms:created rdf:datatype="http://www.w3.org/2001/XMLSchema#dateTime">2014-05-22T00:00:00Z</dcterms:created>
    <skos:definition xml:lang="en">Instruments separating gases volatile substances or substances dissolved in a volatile solvent by transporting an inert gas through a column packed with a sorbent to a detector for assay by a mass spectrometer.</skos:definition>
    <dc:source>(L051) SeaDataNet device categories</dc:source>
    <dc:publisher>British Oceanographic Data Centre (BODC)</dc:publisher>
  </rdf:Description>
  <rdf:Description rdf:about="http://vocab.nerc.ac.uk/collection/L05/current/50">
    <rdf:type rdf:resource="http://www.w3.org/2004/02/skos/core#Concept" />
    <skos:prefLabel xml:lang="en">sediment grabs</skos:prefLabel>
    <skos:topConceptOf rdf:resource="http://vocab.aodn.org.au/def/instrument/1" />
    <skos:inScheme rdf:resource="http://vocab.aodn.org.au/def/instrument/1" />
    <dcterms:created rdf:datatype="http://www.w3.org/2001/XMLSchema#dateTime">2014-05-22T00:00:00Z</dcterms:created>
    <skos:definition xml:lang="en">A device that collects a sample of surface sediment including manually deployed equipment like a shovel or bucket.</skos:definition>
    <dc:source>(L051) SeaDataNet device categories</dc:source>
    <dc:publisher>British Oceanographic Data Centre (BODC)</dc:publisher>
  </rdf:Description>
  <rdf:Description rdf:about="http://vocab.nerc.ac.uk/collection/L05/current/LAB08">
    <rdf:type rdf:resource="http://www.w3.org/2004/02/skos/core#Concept" />
    <skos:prefLabel xml:lang="en">electron microprobes</skos:prefLabel>
    <skos:topConceptOf rdf:resource="http://vocab.aodn.org.au/def/instrument/1" />
    <skos:inScheme rdf:resource="http://vocab.aodn.org.au/def/instrument/1" />
    <dcterms:created rdf:datatype="http://www.w3.org/2001/XMLSchema#dateTime">2014-05-22T00:00:00Z</dcterms:created>
    <skos:definition xml:lang="en">Instruments that chemically analyse a small area of a sample by bombarding it with electrons and spectroscopically assaying the resulting X-Ray emissions.</skos:definition>
    <dc:source>(L051) SeaDataNet device categories</dc:source>
    <dc:publisher>British Oceanographic Data Centre (BODC)</dc:publisher>
  </rdf:Description>
  <rdf:Description rdf:about="http://vocab.nerc.ac.uk/collection/L05/current/LAB10">
    <rdf:type rdf:resource="http://www.w3.org/2004/02/skos/core#Concept" />
    <skos:prefLabel xml:lang="en">atomic absorption spectrometers</skos:prefLabel>
    <skos:topConceptOf rdf:resource="http://vocab.aodn.org.au/def/instrument/1" />
    <skos:inScheme rdf:resource="http://vocab.aodn.org.au/def/instrument/1" />
    <dcterms:created rdf:datatype="http://www.w3.org/2001/XMLSchema#dateTime">2014-05-22T00:00:00Z</dcterms:created>
    <skos:definition xml:lang="en">Instruments that volatilise the sample illuminate the resultant vapour with light wavelengths matched to the analyte of interest and quantify the radiation absorbed which is proportional to concentration.</skos:definition>
    <dc:source>(L051) SeaDataNet device categories</dc:source>
    <dc:publisher>British Oceanographic Data Centre (BODC)</dc:publisher>
  </rdf:Description>
  <rdf:Description rdf:about="http://vocab.nerc.ac.uk/collection/L05/current/POS17">
    <rdf:type rdf:resource="http://www.w3.org/2004/02/skos/core#Concept" />
    <skos:prefLabel xml:lang="en">Argos doppler-localised transmitters</skos:prefLabel>
    <skos:topConceptOf rdf:resource="http://vocab.aodn.org.au/def/instrument/1" />
    <skos:inScheme rdf:resource="http://vocab.aodn.org.au/def/instrument/1" />
    <dcterms:created rdf:datatype="http://www.w3.org/2001/XMLSchema#dateTime">2013-07-18T00:00:00Z</dcterms:created>
    <skos:definition xml:lang="en">&lt;mode&gt;Doppler-derived Argos localisation&lt;/mode&gt;&lt;accuracy&gt;better than 250m (class 3) to worse than 1500m (class 0)&lt;/accuracy&gt;</skos:definition>
    <dc:source>(L051) SeaDataNet device categories</dc:source>
    <dc:publisher>British Oceanographic Data Centre (BODC)</dc:publisher>
    <skos:narrower rdf:resource="http://vocab.nerc.ac.uk/collection/L22/current/TOOL0446" />
    <dcterms:contributor>Natalia_Atkins</dcterms:contributor>
    <skos:narrower rdf:resource="http://vocab.nerc.ac.uk/collection/L22/current/TOOL0720" />
    <dcterms:modified rdf:datatype="http://www.w3.org/2001/XMLSchema#dateTime">2015-07-17T01:38:50Z</dcterms:modified>
    <skos:narrower rdf:resource="http://vocab.nerc.ac.uk/collection/L22/current/TOOL0719" />
  </rdf:Description>
  <rdf:Description rdf:about="http://vocab.nerc.ac.uk/collection/L22/current/TOOL0719">
    <owl:deprecated rdf:datatype="http://www.w3.org/2001/XMLSchema#boolean">true</owl:deprecated>
    <rdfs:label xml:lang="en">SMRU Ltd Satellite Relay Data Logger 9000x</rdfs:label>
    <rdf:type rdf:resource="http://www.w3.org/2004/02/skos/core#Concept" />
    <skos:prefLabel xml:lang="en">SMRU Ltd Satellite Relay Data Logger 9000x</skos:prefLabel>
    <skos:altLabel xml:lang="en">SMRU Ltd SRDL 9000x</skos:altLabel>
    <skos:inScheme rdf:resource="http://vocab.aodn.org.au/instrument/1" />
    <dcterms:created rdf:datatype="http://www.w3.org/2001/XMLSchema#dateTime">2015-07-08T00:00:00Z</dcterms:created>
    <skos:definition xml:lang="en">A depth and temperature sensor package combined with an RF unit and antenna suitable for transmission of data via the Argos satellite system. The unit contains an internal battery and a microprocessor that logs data and schedules the transfer of data. The package is designed for attachment to marine mammals and has an operational depth range of down to 2000 m. It is built and calibrated at Valeport Ltd, while SMRU Ltd, the commercial arm of the Sea Mammal Research Unit of the University of St Andrews, is responsible for its distribution, and for streaming and processing the data. More information is available at http://www.smru.st-and.ac.uk/Instrumentation/SRDL/.</skos:definition>
    <dc:source>(L221) SeaVoX Device Catalogue</dc:source>
    <dc:publisher>British Oceanographic Data Centre (BODC)</dc:publisher>
    <dcterms:modified rdf:datatype="http://www.w3.org/2001/XMLSchema#dateTime">2015-07-17T01:39:47Z</dcterms:modified>
    <dcterms:contributor>Natalia_Atkins</dcterms:contributor>
  </rdf:Description>
  <rdf:Description rdf:about="http://vocab.nerc.ac.uk/collection/L22/current/TOOL0446">
    <rdf:type rdf:resource="http://www.w3.org/2004/02/skos/core#Concept" />
    <skos:prefLabel xml:lang="en">SMRU CTD Satellite Relay Data Logger</skos:prefLabel>
    <skos:inScheme rdf:resource="http://vocab.aodn.org.au/def/instrument/1" />
    <dcterms:created rdf:datatype="http://www.w3.org/2001/XMLSchema#dateTime">2013-10-10T00:00:00Z</dcterms:created>
    <skos:definition xml:lang="en">This tag provides oceanographic quality Conductivity/Temperature/Depth casts. Oceanographic quality temperature &amp; salinity profiles (4 - 12 profiles per day), CTD data automatically submitted to the GTS in near real-time. Up to 50,000 full length Argos data transmissions and pressure-proof to 2000m.  Retains a continuous record of depth readings (4 sec sample rate), which can be retrieved by bluetooth link if the tag is recovered. Also records all individual temperature and salinity measurements (1 Hz) made during profiling. Longevity: up to one year. Size: 10.5 x 7 x 4 cm. Weight: 545 g.</skos:definition>
    <dc:source>(L221) SeaVoX Device Catalogue</dc:source>
    <dc:publisher>British Oceanographic Data Centre (BODC)</dc:publisher>
    <skos:scopeNote xml:lang="en">manufacturer:SMRU Instrumentation</skos:scopeNote>
  </rdf:Description>
  <rdf:Description rdf:about="http://vocab.nerc.ac.uk/collection/L22/current/TOOL0720">
    <rdf:type rdf:resource="http://www.w3.org/2004/02/skos/core#Concept" />
    <skos:prefLabel xml:lang="en">SMRU Ltd CTD/Fluorometer Satellite Relay Data Logger</skos:prefLabel>
    <skos:inScheme rdf:resource="http://vocab.aodn.org.au/def/instrument/1" />
    <dcterms:created rdf:datatype="http://www.w3.org/2001/XMLSchema#dateTime">2013-10-10T00:00:00Z</dcterms:created>
    <skos:definition xml:lang="en">A package comprising a Valeport CTD sensor head plus a customised Turner Cyclops-7 fluorometer combined with an RF unit and antenna suitable for transmission of data via the Argos satellite system. The unit contains an internal battery and a microprocessor that logs data and schedules the transfer of data. The package is designed for attachment to marine mammals and has an operational depth range of down to 2000 m. CTD accuracy is 0.005 C (temperature), 0.01 mS/cm (conductivity) and 2 dBar (pressure).  It is built and calibrated at Valeport Ltd, while SMRU Ltd, the commercial arm of the Sea Mammal Research Unit of the University of St Andrews, is responsible for its distribution, and for streaming and processing the data. More information is available at http://www.smru.st-and.ac.uk/Instrumentation/FluorometryTag/.</skos:definition>
    <dc:source>(L221) SeaVoX Device Catalogue</dc:source>
    <dc:publisher>British Oceanographic Data Centre (BODC)</dc:publisher>
    <skos:scopeNote xml:lang="en">manufacturer:SMRU Instrumentation</skos:scopeNote>
  </rdf:Description>
  <rdf:Description rdf:about="http://vocab.nerc.ac.uk/collection/L05/current/LAB11">
    <rdf:type rdf:resource="http://www.w3.org/2004/02/skos/core#Concept" />
    <skos:prefLabel xml:lang="en">high performance liquid chromatographs</skos:prefLabel>
    <skos:topConceptOf rdf:resource="http://vocab.aodn.org.au/def/instrument/1" />
    <skos:inScheme rdf:resource="http://vocab.aodn.org.au/def/instrument/1" />
    <dcterms:created rdf:datatype="http://www.w3.org/2001/XMLSchema#dateTime">2013-03-28T00:00:00Z</dcterms:created>
    <skos:definition xml:lang="en">Instruments that separate and analyse mixtures of substances by high pressure pumping the sample through a column packed with microspheres coated with the stationary phase.</skos:definition>
    <dc:source>(L051) SeaDataNet device categories</dc:source>
    <dc:publisher>British Oceanographic Data Centre (BODC)</dc:publisher>
  </rdf:Description>
  <rdf:Description rdf:about="http://vocab.nerc.ac.uk/collection/L05/current/130">
    <rdf:type rdf:resource="http://www.w3.org/2004/02/skos/core#Concept" />
    <skos:prefLabel xml:lang="en">CTD</skos:prefLabel>
    <skos:topConceptOf rdf:resource="http://vocab.aodn.org.au/def/instrument/1" />
    <skos:inScheme rdf:resource="http://vocab.aodn.org.au/def/instrument/1" />
    <dcterms:created rdf:datatype="http://www.w3.org/2001/XMLSchema#dateTime">2013-07-18T00:00:00Z</dcterms:created>
    <skos:definition xml:lang="en">A CTD (acronym for Conductivity - Temperature - Depth) is a package carrying conductivity, temperature and pressure sensors. The package can be mounted on different platform like for examples Argo float, glider, marine mammals and moorings. Definal on the type of platform used, the measurements of the different parameters are collected through the vertical column of water or at fixed water depth.</skos:definition>
    <dc:source>(L051) SeaDataNet device categories</dc:source>
    <dc:publisher>British Oceanographic Data Centre (BODC)</dc:publisher>
    <skos:narrower rdf:resource="http://vocab.nerc.ac.uk/collection/L22/current/TOOL0040" />
    <skos:narrower rdf:resource="http://vocab.nerc.ac.uk/collection/L22/current/TOOL0042" />
    <skos:narrower rdf:resource="http://vocab.nerc.ac.uk/collection/L22/current/TOOL0047" />
    <skos:narrower rdf:resource="http://vocab.nerc.ac.uk/collection/L22/current/TOOL0058" />
    <skos:narrower rdf:resource="http://vocab.nerc.ac.uk/collection/L22/current/TOOL0173" />
    <skos:narrower rdf:resource="http://vocab.nerc.ac.uk/collection/L22/current/TOOL0446" />
    <skos:narrower rdf:resource="http://vocab.nerc.ac.uk/collection/L22/current/TOOL0668" />
    <skos:narrower rdf:resource="http://vocab.nerc.ac.uk/collection/L22/current/TOOL0669" />
    <skos:narrower rdf:resource="http://vocab.nerc.ac.uk/collection/L22/current/TOOL0720" />
    <skos:narrower rdf:resource="http://vocab.nerc.ac.uk/collection/L22/current/TOOL0730" />
    <skos:narrower rdf:resource="http://vocab.nerc.ac.uk/collection/L22/current/TOOL0871/" />
    <dcterms:modified rdf:datatype="http://www.w3.org/2001/XMLSchema#dateTime">2015-06-10T02:07:18Z</dcterms:modified>
  </rdf:Description>
  <rdf:Description rdf:about="http://vocab.nerc.ac.uk/collection/L22/current/TOOL0042">
    <rdf:type rdf:resource="http://www.w3.org/2004/02/skos/core#Concept" />
    <skos:prefLabel xml:lang="en">Sea-Bird SBE 19 SEACAT CTD</skos:prefLabel>
    <skos:inScheme rdf:resource="http://vocab.aodn.org.au/def/instrument/1" />
    <dcterms:created rdf:datatype="http://www.w3.org/2001/XMLSchema#dateTime">2014-02-17T00:00:00Z</dcterms:created>
    <skos:definition xml:lang="en">A self-contained battery powered CTD with precision semiconductor strain gauge pressure sensor. Water was supplied to the conductivity sensor by a pump. Housing was plastic (up to 600m depth), aluminium (up to 6800m depth) or titanium (up to 10500m depth). Optional oxygen, pH, fluorescence, PAR, light transmission and turbidity sensors could be fitted. Primarily designed for profiling applications but may be used on a short (less than 2 weeks) duration mooring. Replaced by the SBE19plus model in 2001.</skos:definition>
    <dc:source>(L221) SeaVoX Device Catalogue</dc:source>
    <dc:publisher>British Oceanographic Data Centre (BODC)</dc:publisher>
    <skos:scopeNote xml:lang="en">manufacturer:Sea-Bird Electronics Inc.</skos:scopeNote>
  </rdf:Description>
  <rdf:Description rdf:about="http://vocab.nerc.ac.uk/collection/L22/current/TOOL0730">
    <rdf:type rdf:resource="http://www.w3.org/2004/02/skos/core#Concept" />
    <skos:prefLabel xml:lang="en">RBR XR-620 CTD Profiler</skos:prefLabel>
    <skos:inScheme rdf:resource="http://vocab.aodn.org.au/def/instrument/1" />
    <dcterms:created rdf:datatype="http://www.w3.org/2001/XMLSchema#dateTime">2014-07-14T00:00:00Z</dcterms:created>
    <skos:definition xml:lang="en">A small profiling data logger designed to monitor conductivity, temperature and depth. Conductivity (accuracy ± 0.003 mS/cm) is measured using a 3-coil closed loop feedback inductive cell for superior temperature compensation. The thermistor (Themometrics) used to record temperature (accuracy ± 0.002°C) is aged and hermetically sealed in the tip of a shock resistant solid glass rod. Pressure (accuracy 0.05% full scale) sensors use reliable semiconductor technology and 316 stainless steel housing developed for long-term stability in harsh environments. The XR-620 is a profiling version of the XR-420.</skos:definition>
    <dc:source>(L221) SeaVoX Device Catalogue</dc:source>
    <dc:publisher>British Oceanographic Data Centre (BODC)</dc:publisher>
  </rdf:Description>
  <rdf:Description rdf:about="http://vocab.nerc.ac.uk/collection/L22/current/TOOL0040">
    <rdf:type rdf:resource="http://www.w3.org/2004/02/skos/core#Concept" />
    <skos:prefLabel xml:lang="en">Sea-Bird SBE 25 Sealogger CTD</skos:prefLabel>
    <skos:inScheme rdf:resource="http://vocab.aodn.org.au/def/instrument/1" />
    <dcterms:created rdf:datatype="http://www.w3.org/2001/XMLSchema#dateTime">2014-02-07T00:00:00Z</dcterms:created>
    <skos:definition xml:lang="en">A compact self-contained CTD comprising a conductivity sensor plumbed into a pumped water supply and separate pressure and temperature sensor modules. The whole unit is mounted in a stainless steel cage with a battery pack, data logger and memory. A dissolved oxygen sensor may be plumbed into the pumped water supply and other sensor modules such as fluorometers and transmissometers may be mounted in the cage and interfaced to the data logger. The instrument may also be used with external power and data logging through an RS-232 interface.</skos:definition>
    <dc:source>(L221) SeaVoX Device Catalogue</dc:source>
    <dc:publisher>British Oceanographic Data Centre (BODC)</dc:publisher>
    <skos:scopeNote xml:lang="en">manufacturer:Sea-Bird Electronics Inc.</skos:scopeNote>
  </rdf:Description>
  <rdf:Description rdf:about="http://vocab.nerc.ac.uk/collection/L22/current/TOOL0871/">
    <rdf:type rdf:resource="http://www.w3.org/2004/02/skos/core#Concept" />
    <skos:prefLabel xml:lang="en">Sea-Bird SBE 19plus V2 SEACAT CTD</skos:prefLabel>
    <skos:altLabel xml:lang="en">SBE 19+ V2 SEACAT</skos:altLabel>
    <skos:inScheme rdf:resource="http://vocab.aodn.org.au/def/instrument/1" />
    <dcterms:created rdf:datatype="http://www.w3.org/2001/XMLSchema#dateTime">2015-06-03T00:00:00Z</dcterms:created>
    <skos:definition xml:lang="en">Self-contained self-powered CTD profiler. Measures conductivity, temperature and pressure (Digiquartz sensor) in both profiling (samples at 4 scans/sec) and moored (sample rates of once every 5 seconds to once every 9 hours) mode. Available in plastic or titanium housing with depth ranges of 600m and 7000m respectively. Miniature submersible pump provides water to the conductivity cell.  Compared to the previous 19plus, the V2 incorporates an electronics upgrade and additional features, with six differentially amplified A/D input channels, one RS-232 data input channel, and 64 MB FLASH memory.</skos:definition>
    <dc:source>(L221) SeaVoX Device Catalogue</dc:source>
    <dc:publisher>British Oceanographic Data Centre (BODC)</dc:publisher>
    <dcterms:modified rdf:datatype="http://www.w3.org/2001/XMLSchema#dateTime">2015-06-10T02:07:18Z</dcterms:modified>
  </rdf:Description>
  <rdf:Description rdf:about="http://vocab.nerc.ac.uk/collection/L22/current/TOOL0669">
    <rdf:type rdf:resource="http://www.w3.org/2004/02/skos/core#Concept" />
    <skos:prefLabel xml:lang="en">Sea-Bird SBE 41CP CTD</skos:prefLabel>
    <skos:inScheme rdf:resource="http://vocab.aodn.org.au/def/instrument/1" />
    <dcterms:created rdf:datatype="http://www.w3.org/2001/XMLSchema#dateTime">2014-04-02T00:00:00Z</dcterms:created>
    <skos:definition xml:lang="en">A self-contained unit comprising the MicroCAT temperature, conductivity and pressure sensors and a pump that is designed specifically for deployment on profiling floats, particularly Argo.  The unit is designed to provide stable salinity data accurate to 0.005 PSU for periods in excess of three years without any form of maintenance. Temperature is within 0.002 C (stability 0.0002 C/year) and pressure within 2 dbar (stability 0.8 dbar/year).  During float ascent samples are collected at 1 Hz and logged to internal storage to provide a continuous profile passed to the float controller at the surface.  More information is given in http://www.seabird.com/products/spec_sheets/41data.htm.</skos:definition>
    <dc:source>(L221) SeaVoX Device Catalogue</dc:source>
    <dc:publisher>British Oceanographic Data Centre (BODC)</dc:publisher>
    <skos:scopeNote xml:lang="en">manufacturer:Sea-Bird Electronics Inc.</skos:scopeNote>
  </rdf:Description>
  <rdf:Description rdf:about="http://vocab.nerc.ac.uk/collection/L22/current/TOOL0668">
    <rdf:type rdf:resource="http://www.w3.org/2004/02/skos/core#Concept" />
    <skos:prefLabel xml:lang="en">Sea-Bird SBE 41 CTD</skos:prefLabel>
    <skos:inScheme rdf:resource="http://vocab.aodn.org.au/def/instrument/1" />
    <dcterms:created rdf:datatype="http://www.w3.org/2001/XMLSchema#dateTime">2013-09-09T00:00:00Z</dcterms:created>
    <skos:definition xml:lang="en">A self-contained unit comprising the MicroCAT temperature, conductivity and pressure sensors and a pump that is designed specifically for deployment on profiling floats, particularly Argo.  The unit is designed to provide stable salinity data accurate to 0.005 PSU for periods in excess of three years without any form of maintenance. Temperature is within 0.002 C (stability 0.0002 C/year) and pressure within 2 dbar (stability 0.8 dbar/year).  During float ascent spot samples are taken and transmitted to the float controller.  More information is given in http://www.seabird.com/products/spec_sheets/41data.htm.</skos:definition>
    <dc:source>(L221) SeaVoX Device Catalogue</dc:source>
    <dc:publisher>British Oceanographic Data Centre (BODC)</dc:publisher>
    <skos:scopeNote xml:lang="en">manufacturer:Sea-Bird Electronics Inc.</skos:scopeNote>
  </rdf:Description>
  <rdf:Description rdf:about="http://vocab.nerc.ac.uk/collection/L22/current/TOOL0047">
    <rdf:type rdf:resource="http://www.w3.org/2004/02/skos/core#Concept" />
    <skos:prefLabel xml:lang="en">Sea-Bird SBE 19plus SEACAT CTD</skos:prefLabel>
    <skos:inScheme rdf:resource="http://vocab.aodn.org.au/def/instrument/1" />
    <dcterms:created rdf:datatype="http://www.w3.org/2001/XMLSchema#dateTime">2014-02-07T00:00:00Z</dcterms:created>
    <skos:definition xml:lang="en">Self contained self powered CTD profiler. Measures conductivity, temperature and pressure in both profiling (samples at 4 scans/sec) and moored (sample rates of once every 5 seconds to once every 9 hours) mode. Available in plastic or titanium housing with depth ranges of 600m and 7000m respectively. Minature submersible pump provides water to conductivity cell.</skos:definition>
    <dc:source>(L221) SeaVoX Device Catalogue</dc:source>
    <dc:publisher>British Oceanographic Data Centre (BODC)</dc:publisher>
    <skos:scopeNote xml:lang="en">manufacturer:Sea-Bird Electronics Inc.</skos:scopeNote>
  </rdf:Description>
  <rdf:Description rdf:about="http://vocab.nerc.ac.uk/collection/L22/current/TOOL0173">
    <rdf:type rdf:resource="http://www.w3.org/2004/02/skos/core#Concept" />
    <skos:prefLabel xml:lang="en">Falmouth Scientific Instruments NXIC CTD</skos:prefLabel>
    <skos:inScheme rdf:resource="http://vocab.aodn.org.au/def/instrument/1" />
    <dcterms:created rdf:datatype="http://www.w3.org/2001/XMLSchema#dateTime">2014-02-07T00:00:00Z</dcterms:created>
    <skos:definition xml:lang="en">A collection of sensors which are generally linked to a common data logger that samples at up to 15Hz. Parameters are measured to an accuracy of ±0.0002 S/m for conductivity, ±0.005°C for temperature and 0.08% for full scale pressure. Now marketed by Teledyne RD Instruments.</skos:definition>
    <dc:source>(L221) SeaVoX Device Catalogue</dc:source>
    <dc:publisher>British Oceanographic Data Centre (BODC)</dc:publisher>
    <skos:scopeNote xml:lang="en">manufacturer:Falmouth Scientific Inc.</skos:scopeNote>
  </rdf:Description>
  <rdf:Description rdf:about="http://vocab.nerc.ac.uk/collection/L22/current/TOOL0446">
    <rdf:type rdf:resource="http://www.w3.org/2004/02/skos/core#Concept" />
    <skos:prefLabel xml:lang="en">SMRU CTD Satellite Relay Data Logger</skos:prefLabel>
    <skos:inScheme rdf:resource="http://vocab.aodn.org.au/def/instrument/1" />
    <dcterms:created rdf:datatype="http://www.w3.org/2001/XMLSchema#dateTime">2013-10-10T00:00:00Z</dcterms:created>
    <skos:definition xml:lang="en">This tag provides oceanographic quality Conductivity/Temperature/Depth casts. Oceanographic quality temperature &amp; salinity profiles (4 - 12 profiles per day), CTD data automatically submitted to the GTS in near real-time. Up to 50,000 full length Argos data transmissions and pressure-proof to 2000m.  Retains a continuous record of depth readings (4 sec sample rate), which can be retrieved by bluetooth link if the tag is recovered. Also records all individual temperature and salinity measurements (1 Hz) made during profiling. Longevity: up to one year. Size: 10.5 x 7 x 4 cm. Weight: 545 g.</skos:definition>
    <dc:source>(L221) SeaVoX Device Catalogue</dc:source>
    <dc:publisher>British Oceanographic Data Centre (BODC)</dc:publisher>
    <skos:scopeNote xml:lang="en">manufacturer:SMRU Instrumentation</skos:scopeNote>
  </rdf:Description>
  <rdf:Description rdf:about="http://vocab.nerc.ac.uk/collection/L22/current/TOOL0058">
    <rdf:type rdf:resource="http://www.w3.org/2004/02/skos/core#Concept" />
    <skos:prefLabel xml:lang="en">Sea-Bird SBE 911plus CTD</skos:prefLabel>
    <skos:inScheme rdf:resource="http://vocab.aodn.org.au/def/instrument/1" />
    <dcterms:created rdf:datatype="http://www.w3.org/2001/XMLSchema#dateTime">2014-07-14T00:00:00Z</dcterms:created>
    <skos:definition xml:lang="en">High precision and accuracy CTD comprising an SBE 9plus underwater unit (SBE 3 temperature and SBE 4 conductivity sensors) and an SBE 11plus deck unit. Sensors may be connected to a pump-fed plastic tubing circuit (usually temperature, salinity and oxygen) or stand-alone. All instruments (8 channels available) on the package are logged by the SBE 11. The unit is the production off the shelf version of the SBE 911 (each 911 was custom built to individual specification).</skos:definition>
    <dc:source>(L221) SeaVoX Device Catalogue</dc:source>
    <dc:publisher>British Oceanographic Data Centre (BODC)</dc:publisher>
  </rdf:Description>
  <rdf:Description rdf:about="http://vocab.nerc.ac.uk/collection/L22/current/TOOL0720">
    <rdf:type rdf:resource="http://www.w3.org/2004/02/skos/core#Concept" />
    <skos:prefLabel xml:lang="en">SMRU Ltd CTD/Fluorometer Satellite Relay Data Logger</skos:prefLabel>
    <skos:inScheme rdf:resource="http://vocab.aodn.org.au/def/instrument/1" />
    <dcterms:created rdf:datatype="http://www.w3.org/2001/XMLSchema#dateTime">2013-10-10T00:00:00Z</dcterms:created>
    <skos:definition xml:lang="en">A package comprising a Valeport CTD sensor head plus a customised Turner Cyclops-7 fluorometer combined with an RF unit and antenna suitable for transmission of data via the Argos satellite system. The unit contains an internal battery and a microprocessor that logs data and schedules the transfer of data. The package is designed for attachment to marine mammals and has an operational depth range of down to 2000 m. CTD accuracy is 0.005 C (temperature), 0.01 mS/cm (conductivity) and 2 dBar (pressure).  It is built and calibrated at Valeport Ltd, while SMRU Ltd, the commercial arm of the Sea Mammal Research Unit of the University of St Andrews, is responsible for its distribution, and for streaming and processing the data. More information is available at http://www.smru.st-and.ac.uk/Instrumentation/FluorometryTag/.</skos:definition>
    <dc:source>(L221) SeaVoX Device Catalogue</dc:source>
    <dc:publisher>British Oceanographic Data Centre (BODC)</dc:publisher>
    <skos:scopeNote xml:lang="en">manufacturer:SMRU Instrumentation</skos:scopeNote>
  </rdf:Description>
  <rdf:Description rdf:about="http://vocab.nerc.ac.uk/collection/L05/current/135">
    <rdf:type rdf:resource="http://www.w3.org/2004/02/skos/core#Concept" />
    <skos:prefLabel xml:lang="en">thermistor chains</skos:prefLabel>
    <skos:topConceptOf rdf:resource="http://vocab.aodn.org.au/def/instrument/1" />
    <skos:inScheme rdf:resource="http://vocab.aodn.org.au/def/instrument/1" />
    <dcterms:created rdf:datatype="http://www.w3.org/2001/XMLSchema#dateTime">2013-03-28T00:00:00Z</dcterms:created>
    <skos:definition xml:lang="en">A group of rigidly-mounted temperature sensors sampled by a common data logger held at various depths in the water column.</skos:definition>
    <dc:source>(L051) SeaDataNet device categories</dc:source>
    <dc:publisher>British Oceanographic Data Centre (BODC)</dc:publisher>
  </rdf:Description>
  <rdf:Description rdf:about="http://vocab.nerc.ac.uk/collection/L05/current/311">
    <rdf:type rdf:resource="http://www.w3.org/2004/02/skos/core#Concept" />
    <skos:prefLabel xml:lang="en">cameras</skos:prefLabel>
    <skos:topConceptOf rdf:resource="http://vocab.aodn.org.au/def/instrument/1" />
    <skos:inScheme rdf:resource="http://vocab.aodn.org.au/def/instrument/1" />
    <dcterms:created rdf:datatype="http://www.w3.org/2001/XMLSchema#dateTime">2014-05-22T00:00:00Z</dcterms:created>
    <skos:definition xml:lang="en">All types of photographic equipment that may be deployed in aircraft or satellites including stills video film and digital systems.</skos:definition>
    <dc:source>(L051) SeaDataNet device categories</dc:source>
    <dc:publisher>British Oceanographic Data Centre (BODC)</dc:publisher>
  </rdf:Description>
  <rdf:Description rdf:about="http://vocab.nerc.ac.uk/collection/L05/current/312">
    <rdf:type rdf:resource="http://www.w3.org/2004/02/skos/core#Concept" />
    <skos:prefLabel xml:lang="en">bathymetric LiDARs</skos:prefLabel>
    <skos:topConceptOf rdf:resource="http://vocab.aodn.org.au/def/instrument/1" />
    <skos:inScheme rdf:resource="http://vocab.aodn.org.au/def/instrument/1" />
    <dcterms:created rdf:datatype="http://www.w3.org/2001/XMLSchema#dateTime">2014-05-22T00:00:00Z</dcterms:created>
    <skos:definition xml:lang="en">Instruments that measure the depth of a water body by determining the distances from the platform to the surface and the bed by timing reflected pulses of laser light.</skos:definition>
    <dc:source>(L051) SeaDataNet device categories</dc:source>
    <dc:publisher>British Oceanographic Data Centre (BODC)</dc:publisher>
  </rdf:Description>
  <rdf:Description rdf:about="http://vocab.nerc.ac.uk/collection/L05/current/310">
    <rdf:type rdf:resource="http://www.w3.org/2004/02/skos/core#Concept" />
    <skos:prefLabel xml:lang="en">laser altimeters</skos:prefLabel>
    <skos:topConceptOf rdf:resource="http://vocab.aodn.org.au/def/instrument/1" />
    <skos:inScheme rdf:resource="http://vocab.aodn.org.au/def/instrument/1" />
    <dcterms:created rdf:datatype="http://www.w3.org/2001/XMLSchema#dateTime">2014-05-22T00:00:00Z</dcterms:created>
    <skos:definition xml:lang="en">Instruments that determine the distance between the platform and the Earth's surface by timing reflected pulses of laser light.</skos:definition>
    <dc:source>(L051) SeaDataNet device categories</dc:source>
    <dc:publisher>British Oceanographic Data Centre (BODC)</dc:publisher>
  </rdf:Description>
  <rdf:Description rdf:about="http://vocab.nerc.ac.uk/collection/L05/current/132">
    <rdf:type rdf:resource="http://www.w3.org/2004/02/skos/core#Concept" />
    <skos:prefLabel xml:lang="en">bathythermographs</skos:prefLabel>
    <skos:narrower rdf:resource="http://vocab.aodn.org.au/def/instrument/entity/39" />
    <skos:topConceptOf rdf:resource="http://vocab.aodn.org.au/def/instrument/1" />
    <dcterms:created rdf:datatype="http://www.w3.org/2001/XMLSchema#dateTime">2013-03-28T00:00:00Z</dcterms:created>
    <skos:definition xml:lang="en">Instruments that measure vertical profiles of sea temperature by either lowering a pressure plus temperature senor package (MBT) or dropping a free falling disposable sensor (XBT).</skos:definition>
    <dc:source>(L051) SeaDataNet device categories</dc:source>
    <dc:publisher>British Oceanographic Data Centre (BODC)</dc:publisher>
    <skos:inScheme rdf:resource="http://vocab.aodn.org.au/def/instrument/1" />
    <skos:narrower rdf:resource="http://vocab.nerc.ac.uk/collection/L22/current/TOOL0263" />
    <skos:narrower rdf:resource="http://vocab.nerc.ac.uk/collection/L22/current/TOOL0435" />
  </rdf:Description>
  <rdf:Description rdf:about="http://vocab.nerc.ac.uk/collection/L22/current/TOOL0435">
    <rdf:type rdf:resource="http://www.w3.org/2004/02/skos/core#Concept" />
    <skos:prefLabel xml:lang="en">Lockheed Martin Sippican T-4 XBT probe</skos:prefLabel>
    <skos:inScheme rdf:resource="http://vocab.aodn.org.au/def/instrument/1" />
    <dcterms:created rdf:datatype="http://www.w3.org/2001/XMLSchema#dateTime">2013-03-28T00:00:00Z</dcterms:created>
    <skos:definition xml:lang="en">An expendable free-fall temperature probe that provides a profile of measured temperature against depth calculated from a fall-rate model. The T-4 XBT Probe can be used within a maximum depth of 460m, may be deployed at a ship speed of up to 30 knots and has a vertical resolution of 65cm.</skos:definition>
    <dc:source>(L221) SeaVoX Device Catalogue</dc:source>
    <dc:publisher>British Oceanographic Data Centre (BODC)</dc:publisher>
    <skos:scopeNote xml:lang="en">manufacturer: Lockheed Martin</skos:scopeNote>
  </rdf:Description>
  <rdf:Description rdf:about="http://vocab.nerc.ac.uk/collection/L22/current/TOOL0263">
    <rdf:type rdf:resource="http://www.w3.org/2004/02/skos/core#Concept" />
    <skos:prefLabel xml:lang="en">Lockheed Martin Sippican T-7 XBT probe</skos:prefLabel>
    <skos:inScheme rdf:resource="http://vocab.aodn.org.au/def/instrument/1" />
    <dcterms:created rdf:datatype="http://www.w3.org/2001/XMLSchema#dateTime">2013-03-28T00:00:00Z</dcterms:created>
    <skos:definition xml:lang="en">An expendable free-fall temperature probe that provides a profile of measured temperature against depth calculated from a fall-rate model. The T-7 XBT Probe can be used within a maximum depth of 760m, may be deployed at a ship speed of up to 15 knots and has a vertical resolution of 65cm.</skos:definition>
    <dc:source>(L221) SeaVoX Device Catalogue</dc:source>
    <dc:publisher>British Oceanographic Data Centre (BODC)</dc:publisher>
    <skos:scopeNote xml:lang="en">manufacturer: Lockheed Martin</skos:scopeNote>
  </rdf:Description>
  <rdf:Description rdf:about="http://vocab.aodn.org.au/def/instrument/entity/39">
    <rdf:type rdf:resource="http://www.w3.org/2004/02/skos/core#Concept" />
    <skos:prefLabel xml:lang="en">Lockheed Martin Sippican Deep Blue XBT probe</skos:prefLabel>
    <dcterms:created rdf:datatype="http://www.w3.org/2001/XMLSchema#dateTime">2013-03-28T00:00:00Z</dcterms:created>
    <dcterms:contributor>Natalia_Atkins</dcterms:contributor>
    <dc:source>Australian Ocean Data Network instrument register</dc:source>
    <dc:publisher>eMarine Information Infrastructure (eMII)</dc:publisher>
    <skos:scopeNote xml:lang="en">manufacturer: Lockheed Martin</skos:scopeNote>
    <dcterms:creator xml:lang="en">Sebastien Mancini</dcterms:creator>
    <skos:definition xml:lang="en">An expendable free-fall temperature probe that provides a profile of measured temperature against depth calculated from a fall-rate model. The Deep Blue XBT Probe (sometimes referred to as the T-7DB) can be used to a maximum depth of 460m, may be deployed at a ship speed of up to 20 knots and has a vertical resolution of 65cm.</skos:definition>
    <dcterms:modified rdf:datatype="http://www.w3.org/2001/XMLSchema#dateTime">2015-06-30T05:43:15Z</dcterms:modified>
    <skos:inScheme rdf:resource="http://vocab.aodn.org.au/def/instrument/1" />
  </rdf:Description>
  <rdf:Description rdf:about="http://vocab.nerc.ac.uk/collection/L05/current/133">
    <rdf:type rdf:resource="http://www.w3.org/2004/02/skos/core#Concept" />
    <skos:prefLabel xml:lang="en">thermosalinographs</skos:prefLabel>
    <skos:topConceptOf rdf:resource="http://vocab.aodn.org.au/def/instrument/1" />
    <skos:inScheme rdf:resource="http://vocab.aodn.org.au/def/instrument/1" />
    <dcterms:created rdf:datatype="http://www.w3.org/2001/XMLSchema#dateTime">2013-03-28T00:00:00Z</dcterms:created>
    <skos:definition xml:lang="en">Temperature and conductivity sensors mounted on a sea-surface platform continuously measuring a surface water supply.</skos:definition>
    <dc:source>(L051) SeaDataNet device categories</dc:source>
    <dc:publisher>British Oceanographic Data Centre (BODC)</dc:publisher>
    <skos:narrower rdf:resource="http://vocab.nerc.ac.uk/collection/L22/current/TOOL0190" />
    <skos:narrower rdf:resource="http://vocab.nerc.ac.uk/collection/L22/current/TOOL0667" />
  </rdf:Description>
  <rdf:Description rdf:about="http://vocab.nerc.ac.uk/collection/L22/current/TOOL0667">
    <rdf:type rdf:resource="http://www.w3.org/2004/02/skos/core#Concept" />
    <skos:prefLabel xml:lang="en">Sea-Bird SBE 21 Thermosalinograph</skos:prefLabel>
    <skos:inScheme rdf:resource="http://vocab.aodn.org.au/def/instrument/1" />
    <dcterms:created rdf:datatype="http://www.w3.org/2001/XMLSchema#dateTime">2013-10-08T00:00:00Z</dcterms:created>
    <skos:definition xml:lang="en">A platinum-electrode conductivity sensor and a thermistor mounted in a corrosion-resistant plastic and titanium housing designed to be continuously plumbed into a vessel's pumped seawater supply. The instrument may be interfaced to a remote SBE 38 temperature sensor mounted either on the hull or in the seawater inlet. Data are both stored in internal memory and output to a serial port for external logging.  Conductivity is measured in the range 0-7 S/m with an accuracy of 0.001 S/m and a resolution  of 0.0001 S/m. Housing temperature is measured in the range -5-35C with an accuracy of 0.01 C and a resolution  of 0.001 C. Remote temperature is measured in the range -5-35C  with an accuracy of 0.001 C and a resolution  of 0.0003 C. More information at http://www.seabird.com/products/spec_sheets/21data.htm.</skos:definition>
    <dc:source>(L221) SeaVoX Device Catalogue</dc:source>
    <dc:publisher>British Oceanographic Data Centre (BODC)</dc:publisher>
    <skos:scopeNote xml:lang="en">manufacturer:Sea-Bird Electronics Inc.</skos:scopeNote>
  </rdf:Description>
  <rdf:Description rdf:about="http://vocab.nerc.ac.uk/collection/L22/current/TOOL0190">
    <rdf:type rdf:resource="http://www.w3.org/2004/02/skos/core#Concept" />
    <skos:prefLabel xml:lang="en">Sea-Bird SBE 45 MicroTSG thermosalinograph</skos:prefLabel>
    <skos:inScheme rdf:resource="http://vocab.aodn.org.au/def/instrument/1" />
    <dcterms:created rdf:datatype="http://www.w3.org/2001/XMLSchema#dateTime">2013-10-08T00:00:00Z</dcterms:created>
    <skos:definition xml:lang="en">A small externally powered, high-accuracy instrument, designed for shipboard determination of sea surface (pumped-water) conductivity and temperature. It is constructed of plastic and titanium to ensure long life with minimum maintenance. It may optionally be interfaced to an external SBE 38 hull temperature sensor.</skos:definition>
    <dc:source>(L221) SeaVoX Device Catalogue</dc:source>
    <dc:publisher>British Oceanographic Data Centre (BODC)</dc:publisher>
    <skos:scopeNote xml:lang="en">manufacturer:Sea-Bird Electronics Inc.</skos:scopeNote>
  </rdf:Description>
  <rdf:Description rdf:about="http://vocab.nerc.ac.uk/collection/L05/current/134">
    <rdf:type rdf:resource="http://www.w3.org/2004/02/skos/core#Concept" />
    <skos:prefLabel xml:lang="en">water temperature sensor</skos:prefLabel>
    <skos:narrower rdf:resource="http://vocab.aodn.org.au/def/instrument/entity/39" />
    <skos:narrower rdf:resource="http://vocab.aodn.org.au/def/instrument/entity/553" />
    <dcterms:created rdf:datatype="http://www.w3.org/2001/XMLSchema#dateTime">2013-03-28T00:00:00Z</dcterms:created>
    <skos:definition xml:lang="en">An instrument that measures the temperature of the water with which it is in contact</skos:definition>
    <dc:source>(L051) SeaDataNet device categories</dc:source>
    <dc:publisher>British Oceanographic Data Centre (BODC)</dc:publisher>
    <skos:topConceptOf rdf:resource="http://vocab.aodn.org.au/def/instrument/1" />
    <skos:narrower rdf:resource="http://vocab.nerc.ac.uk/collection/L22/current/TOOL0017" />
    <skos:narrower rdf:resource="http://vocab.nerc.ac.uk/collection/L22/current/TOOL0018" />
    <skos:narrower rdf:resource="http://vocab.nerc.ac.uk/collection/L22/current/TOOL0019" />
    <skos:narrower rdf:resource="http://vocab.nerc.ac.uk/collection/L22/current/TOOL0020" />
    <skos:narrower rdf:resource="http://vocab.nerc.ac.uk/collection/L22/current/TOOL0023" />
    <skos:narrower rdf:resource="http://vocab.nerc.ac.uk/collection/L22/current/TOOL0040" />
    <skos:narrower rdf:resource="http://vocab.nerc.ac.uk/collection/L22/current/TOOL0042" />
    <skos:narrower rdf:resource="http://vocab.nerc.ac.uk/collection/L22/current/TOOL0047" />
    <skos:narrower rdf:resource="http://vocab.nerc.ac.uk/collection/L22/current/TOOL0053" />
    <skos:narrower rdf:resource="http://vocab.nerc.ac.uk/collection/L22/current/TOOL0054" />
    <skos:narrower rdf:resource="http://vocab.nerc.ac.uk/collection/L22/current/TOOL0058" />
    <skos:narrower rdf:resource="http://vocab.nerc.ac.uk/collection/L22/current/TOOL0100" />
    <skos:narrower rdf:resource="http://vocab.nerc.ac.uk/collection/L22/current/TOOL0105" />
    <skos:narrower rdf:resource="http://vocab.nerc.ac.uk/collection/L22/current/TOOL0173" />
    <skos:narrower rdf:resource="http://vocab.nerc.ac.uk/collection/L22/current/TOOL0181" />
    <skos:narrower rdf:resource="http://vocab.nerc.ac.uk/collection/L22/current/TOOL0190" />
    <skos:narrower rdf:resource="http://vocab.nerc.ac.uk/collection/L22/current/TOOL0191" />
    <skos:narrower rdf:resource="http://vocab.nerc.ac.uk/collection/L22/current/TOOL0266" />
    <skos:narrower rdf:resource="http://vocab.nerc.ac.uk/collection/L22/current/TOOL0267" />
    <skos:narrower rdf:resource="http://vocab.nerc.ac.uk/collection/L22/current/TOOL0416" />
    <skos:narrower rdf:resource="http://vocab.nerc.ac.uk/collection/L22/current/TOOL0446" />
    <skos:narrower rdf:resource="http://vocab.nerc.ac.uk/collection/L22/current/TOOL0490" />
    <skos:narrower rdf:resource="http://vocab.nerc.ac.uk/collection/L22/current/TOOL0640" />
    <skos:narrower rdf:resource="http://vocab.nerc.ac.uk/collection/L22/current/TOOL0665" />
    <skos:narrower rdf:resource="http://vocab.nerc.ac.uk/collection/L22/current/TOOL0667" />
    <skos:narrower rdf:resource="http://vocab.nerc.ac.uk/collection/L22/current/TOOL0668" />
    <skos:narrower rdf:resource="http://vocab.nerc.ac.uk/collection/L22/current/TOOL0669" />
    <skos:narrower rdf:resource="http://vocab.nerc.ac.uk/collection/L22/current/TOOL0670" />
    <skos:narrower rdf:resource="http://vocab.nerc.ac.uk/collection/L22/current/TOOL0675" />
    <skos:narrower rdf:resource="http://vocab.nerc.ac.uk/collection/L22/current/TOOL0684" />
    <skos:narrower rdf:resource="http://vocab.nerc.ac.uk/collection/L22/current/TOOL0685" />
    <skos:narrower rdf:resource="http://vocab.nerc.ac.uk/collection/L22/current/TOOL0687" />
    <skos:narrower rdf:resource="http://vocab.nerc.ac.uk/collection/L22/current/TOOL0688" />
    <skos:narrower rdf:resource="http://vocab.nerc.ac.uk/collection/L22/current/TOOL0696" />
    <skos:narrower rdf:resource="http://vocab.nerc.ac.uk/collection/L22/current/TOOL0706" />
    <skos:narrower rdf:resource="http://vocab.nerc.ac.uk/collection/L22/current/TOOL0707" />
    <skos:narrower rdf:resource="http://vocab.nerc.ac.uk/collection/L22/current/TOOL0712" />
    <skos:narrower rdf:resource="http://vocab.nerc.ac.uk/collection/L22/current/TOOL0809" />
    <skos:narrower rdf:resource="http://vocab.nerc.ac.uk/collection/L22/current/TOOL0720" />
    <skos:narrower rdf:resource="http://vocab.nerc.ac.uk/collection/L22/current/TOOL0728" />
    <skos:narrower rdf:resource="http://vocab.nerc.ac.uk/collection/L22/current/TOOL0729" />
    <skos:narrower rdf:resource="http://vocab.nerc.ac.uk/collection/L22/current/TOOL0731" />
    <skos:narrower rdf:resource="http://vocab.nerc.ac.uk/collection/L22/current/TOOL0888/" />
    <dcterms:contributor>Natalia_Atkins</dcterms:contributor>
    <skos:narrower rdf:resource="http://vocab.nerc.ac.uk/collection/L22/current/TOOL0870/" />
    <skos:narrower rdf:resource="http://vocab.nerc.ac.uk/collection/L22/current/TOOL0871/" />
    <skos:narrower rdf:resource="http://vocab.nerc.ac.uk/collection/L22/current/TOOL0869/" />
    <skos:narrower rdf:resource="http://vocab.nerc.ac.uk/collection/L22/current/TOOL0872/" />
    <skos:inScheme rdf:resource="http://vocab.aodn.org.au/def/instrument/1" />
    <dcterms:modified rdf:datatype="http://www.w3.org/2001/XMLSchema#dateTime">2015-07-17T01:39:47Z</dcterms:modified>
    <skos:narrower rdf:resource="http://vocab.nerc.ac.uk/collection/L22/current/TOOL0898/" />
    <skos:narrower rdf:resource="http://vocab.nerc.ac.uk/collection/L22/current/TOOL0873/" />
    <skos:narrower rdf:resource="http://vocab.nerc.ac.uk/collection/L22/current/TOOL0719" />
  </rdf:Description>
  <rdf:Description rdf:about="http://vocab.nerc.ac.uk/collection/L22/current/TOOL0042">
    <rdf:type rdf:resource="http://www.w3.org/2004/02/skos/core#Concept" />
    <skos:prefLabel xml:lang="en">Sea-Bird SBE 19 SEACAT CTD</skos:prefLabel>
    <skos:inScheme rdf:resource="http://vocab.aodn.org.au/def/instrument/1" />
    <dcterms:created rdf:datatype="http://www.w3.org/2001/XMLSchema#dateTime">2014-02-17T00:00:00Z</dcterms:created>
    <skos:definition xml:lang="en">A self-contained battery powered CTD with precision semiconductor strain gauge pressure sensor. Water was supplied to the conductivity sensor by a pump. Housing was plastic (up to 600m depth), aluminium (up to 6800m depth) or titanium (up to 10500m depth). Optional oxygen, pH, fluorescence, PAR, light transmission and turbidity sensors could be fitted. Primarily designed for profiling applications but may be used on a short (less than 2 weeks) duration mooring. Replaced by the SBE19plus model in 2001.</skos:definition>
    <dc:source>(L221) SeaVoX Device Catalogue</dc:source>
    <dc:publisher>British Oceanographic Data Centre (BODC)</dc:publisher>
    <skos:scopeNote xml:lang="en">manufacturer:Sea-Bird Electronics Inc.</skos:scopeNote>
  </rdf:Description>
  <rdf:Description rdf:about="http://vocab.nerc.ac.uk/collection/L22/current/TOOL0665">
    <rdf:type rdf:resource="http://www.w3.org/2004/02/skos/core#Concept" />
    <skos:prefLabel xml:lang="en">Vemco Minilog12 temperature-pressure recorder</skos:prefLabel>
    <skos:inScheme rdf:resource="http://vocab.aodn.org.au/def/instrument/1" />
    <dcterms:created rdf:datatype="http://www.w3.org/2001/XMLSchema#dateTime">2014-08-06T00:00:00Z</dcterms:created>
    <skos:definition xml:lang="en">A miniature data logger that records temperature and depth at a user programmed time interval. 12-bit version gives a resolution of 0.015 degC and an accuracy of +/-0.1 degC. It is housed in a waterproof cylinder and the temperature sensor is mounted on a protruding stainless steel probe.</skos:definition>
    <dc:source>(L221) SeaVoX Device Catalogue</dc:source>
    <dc:publisher>British Oceanographic Data Centre (BODC)</dc:publisher>
  </rdf:Description>
  <rdf:Description rdf:about="http://vocab.nerc.ac.uk/collection/L22/current/TOOL0040">
    <rdf:type rdf:resource="http://www.w3.org/2004/02/skos/core#Concept" />
    <skos:prefLabel xml:lang="en">Sea-Bird SBE 25 Sealogger CTD</skos:prefLabel>
    <skos:inScheme rdf:resource="http://vocab.aodn.org.au/def/instrument/1" />
    <dcterms:created rdf:datatype="http://www.w3.org/2001/XMLSchema#dateTime">2014-02-07T00:00:00Z</dcterms:created>
    <skos:definition xml:lang="en">A compact self-contained CTD comprising a conductivity sensor plumbed into a pumped water supply and separate pressure and temperature sensor modules. The whole unit is mounted in a stainless steel cage with a battery pack, data logger and memory. A dissolved oxygen sensor may be plumbed into the pumped water supply and other sensor modules such as fluorometers and transmissometers may be mounted in the cage and interfaced to the data logger. The instrument may also be used with external power and data logging through an RS-232 interface.</skos:definition>
    <dc:source>(L221) SeaVoX Device Catalogue</dc:source>
    <dc:publisher>British Oceanographic Data Centre (BODC)</dc:publisher>
    <skos:scopeNote xml:lang="en">manufacturer:Sea-Bird Electronics Inc.</skos:scopeNote>
  </rdf:Description>
  <rdf:Description rdf:about="http://vocab.nerc.ac.uk/collection/L22/current/TOOL0667">
    <rdf:type rdf:resource="http://www.w3.org/2004/02/skos/core#Concept" />
    <skos:prefLabel xml:lang="en">Sea-Bird SBE 21 Thermosalinograph</skos:prefLabel>
    <skos:inScheme rdf:resource="http://vocab.aodn.org.au/def/instrument/1" />
    <dcterms:created rdf:datatype="http://www.w3.org/2001/XMLSchema#dateTime">2013-10-08T00:00:00Z</dcterms:created>
    <skos:definition xml:lang="en">A platinum-electrode conductivity sensor and a thermistor mounted in a corrosion-resistant plastic and titanium housing designed to be continuously plumbed into a vessel's pumped seawater supply. The instrument may be interfaced to a remote SBE 38 temperature sensor mounted either on the hull or in the seawater inlet. Data are both stored in internal memory and output to a serial port for external logging.  Conductivity is measured in the range 0-7 S/m with an accuracy of 0.001 S/m and a resolution  of 0.0001 S/m. Housing temperature is measured in the range -5-35C with an accuracy of 0.01 C and a resolution  of 0.001 C. Remote temperature is measured in the range -5-35C  with an accuracy of 0.001 C and a resolution  of 0.0003 C. More information at http://www.seabird.com/products/spec_sheets/21data.htm.</skos:definition>
    <dc:source>(L221) SeaVoX Device Catalogue</dc:source>
    <dc:publisher>British Oceanographic Data Centre (BODC)</dc:publisher>
    <skos:scopeNote xml:lang="en">manufacturer:Sea-Bird Electronics Inc.</skos:scopeNote>
  </rdf:Description>
  <rdf:Description rdf:about="http://vocab.nerc.ac.uk/collection/L22/current/TOOL0669">
    <rdf:type rdf:resource="http://www.w3.org/2004/02/skos/core#Concept" />
    <skos:prefLabel xml:lang="en">Sea-Bird SBE 41CP CTD</skos:prefLabel>
    <skos:inScheme rdf:resource="http://vocab.aodn.org.au/def/instrument/1" />
    <dcterms:created rdf:datatype="http://www.w3.org/2001/XMLSchema#dateTime">2014-04-02T00:00:00Z</dcterms:created>
    <skos:definition xml:lang="en">A self-contained unit comprising the MicroCAT temperature, conductivity and pressure sensors and a pump that is designed specifically for deployment on profiling floats, particularly Argo.  The unit is designed to provide stable salinity data accurate to 0.005 PSU for periods in excess of three years without any form of maintenance. Temperature is within 0.002 C (stability 0.0002 C/year) and pressure within 2 dbar (stability 0.8 dbar/year).  During float ascent samples are collected at 1 Hz and logged to internal storage to provide a continuous profile passed to the float controller at the surface.  More information is given in http://www.seabird.com/products/spec_sheets/41data.htm.</skos:definition>
    <dc:source>(L221) SeaVoX Device Catalogue</dc:source>
    <dc:publisher>British Oceanographic Data Centre (BODC)</dc:publisher>
    <skos:scopeNote xml:lang="en">manufacturer:Sea-Bird Electronics Inc.</skos:scopeNote>
  </rdf:Description>
  <rdf:Description rdf:about="http://vocab.nerc.ac.uk/collection/L22/current/TOOL0729">
    <rdf:type rdf:resource="http://www.w3.org/2004/02/skos/core#Concept" />
    <skos:prefLabel xml:lang="en">RBR TWR-2050 Submersible Tide and Wave Recorder</skos:prefLabel>
    <skos:inScheme rdf:resource="http://vocab.aodn.org.au/def/instrument/1" />
    <dcterms:created rdf:datatype="http://www.w3.org/2001/XMLSchema#dateTime">2014-07-14T00:00:00Z</dcterms:created>
    <skos:definition xml:lang="en">The TWR-2050P is a small, self-contained, submersible temperature, wave and depth recorder (sensors and data logger). It can be deployed for a period of up to three years and can collect more than 1,200,000 sets of samples. Data can be retained in memory for 20 years (even without batteries). Available in two casings, plastic and titanium, with depth ratings of 740m and 6600m respectively. The temperature channel of the TWR-2050 is calibrated to an accuracy of ± 0.002°C (ITS-90) over the range -5 to +35°C.  Typical drift has been measured to be 0.002°C per year. The thermistor may be external (&lt;3sec time constant) or internal (&lt;20sec time constant). A fast thermistor probe (0.095sec) is also available. The depth channel is calibrated to an accuracy of 0.05%fs  Ranges from 10m to 6,600m are available. Temperature and depth only sensors (TDR) and surface-mounted sensors (HT) are also available.</skos:definition>
    <dc:source>(L221) SeaVoX Device Catalogue</dc:source>
    <dc:publisher>British Oceanographic Data Centre (BODC)</dc:publisher>
  </rdf:Description>
  <rdf:Description rdf:about="http://vocab.nerc.ac.uk/collection/L22/current/TOOL0047">
    <rdf:type rdf:resource="http://www.w3.org/2004/02/skos/core#Concept" />
    <skos:prefLabel xml:lang="en">Sea-Bird SBE 19plus SEACAT CTD</skos:prefLabel>
    <skos:inScheme rdf:resource="http://vocab.aodn.org.au/def/instrument/1" />
    <dcterms:created rdf:datatype="http://www.w3.org/2001/XMLSchema#dateTime">2014-02-07T00:00:00Z</dcterms:created>
    <skos:definition xml:lang="en">Self contained self powered CTD profiler. Measures conductivity, temperature and pressure in both profiling (samples at 4 scans/sec) and moored (sample rates of once every 5 seconds to once every 9 hours) mode. Available in plastic or titanium housing with depth ranges of 600m and 7000m respectively. Minature submersible pump provides water to conductivity cell.</skos:definition>
    <dc:source>(L221) SeaVoX Device Catalogue</dc:source>
    <dc:publisher>British Oceanographic Data Centre (BODC)</dc:publisher>
    <skos:scopeNote xml:lang="en">manufacturer:Sea-Bird Electronics Inc.</skos:scopeNote>
  </rdf:Description>
  <rdf:Description rdf:about="http://vocab.nerc.ac.uk/collection/L22/current/TOOL0668">
    <rdf:type rdf:resource="http://www.w3.org/2004/02/skos/core#Concept" />
    <skos:prefLabel xml:lang="en">Sea-Bird SBE 41 CTD</skos:prefLabel>
    <skos:inScheme rdf:resource="http://vocab.aodn.org.au/def/instrument/1" />
    <dcterms:created rdf:datatype="http://www.w3.org/2001/XMLSchema#dateTime">2013-09-09T00:00:00Z</dcterms:created>
    <skos:definition xml:lang="en">A self-contained unit comprising the MicroCAT temperature, conductivity and pressure sensors and a pump that is designed specifically for deployment on profiling floats, particularly Argo.  The unit is designed to provide stable salinity data accurate to 0.005 PSU for periods in excess of three years without any form of maintenance. Temperature is within 0.002 C (stability 0.0002 C/year) and pressure within 2 dbar (stability 0.8 dbar/year).  During float ascent spot samples are taken and transmitted to the float controller.  More information is given in http://www.seabird.com/products/spec_sheets/41data.htm.</skos:definition>
    <dc:source>(L221) SeaVoX Device Catalogue</dc:source>
    <dc:publisher>British Oceanographic Data Centre (BODC)</dc:publisher>
    <skos:scopeNote xml:lang="en">manufacturer:Sea-Bird Electronics Inc.</skos:scopeNote>
  </rdf:Description>
  <rdf:Description rdf:about="http://vocab.nerc.ac.uk/collection/L22/current/TOOL0728">
    <rdf:type rdf:resource="http://www.w3.org/2004/02/skos/core#Concept" />
    <skos:prefLabel xml:lang="en">RBR TR-1060P Temperature Logger</skos:prefLabel>
    <skos:inScheme rdf:resource="http://vocab.aodn.org.au/def/instrument/1" />
    <dcterms:created rdf:datatype="http://www.w3.org/2001/XMLSchema#dateTime">2014-07-14T00:00:00Z</dcterms:created>
    <skos:definition xml:lang="en">The TR-1060P is a small, self-contained, submersible temperature logger calibrated to +/-0.002 degC, with a typical calibration drift of less than 0.002 degC per year. It is a 25mm diameter version of the TR-1050, but has the same or better performance with a 24 bit a/d. It can be deployed for a period of up to three years and can collect more than 2,400,000 samples. Data are retained in memory for 20 years (even without batteries).  It has a depth rating of 1200 m, download speed ~115000 samples per minute, clock accuracy +/- 32 seconds per year, 8 Mb flash memory, and 240mm x 25 mm casing. Measures temperature from -5 to 35 degC, but can be calibrated to a wider range on request. Accuracy is +/-0.002 degC, resolution better than 0.00005 degC.</skos:definition>
    <dc:source>(L221) SeaVoX Device Catalogue</dc:source>
    <dc:publisher>British Oceanographic Data Centre (BODC)</dc:publisher>
  </rdf:Description>
  <rdf:Description rdf:about="http://vocab.nerc.ac.uk/collection/L22/current/TOOL0869/">
    <rdf:type rdf:resource="http://www.w3.org/2004/02/skos/core#Concept" />
    <skos:prefLabel xml:lang="en">Sea-Bird SBE 37-SMP-ODO MicroCAT C-T-ODO</skos:prefLabel>
    <skos:altLabel xml:lang="en">SBE 37-SMP-ODO MicroCAT</skos:altLabel>
    <skos:inScheme rdf:resource="http://vocab.aodn.org.au/def/instrument/1" />
    <dcterms:created rdf:datatype="http://www.w3.org/2001/XMLSchema#dateTime">2015-06-03T00:00:00Z</dcterms:created>
    <skos:definition xml:lang="en">The SBE 37 MicroCAT is a high accuracy conductivity and temperature recorder with an optional pressure sensor and an Optical Dissolved Oxygen (ODO) sensor designed for deployment on moorings. It is available with either a plastic (rated to 350m) or titanium (rated to 6000m) housing and has an internal pump to improve conductivity and oxygen response. Bio-fouling protection is provided by expendable anti-foulant devices, pump flow path and pumping regimen.</skos:definition>
    <dc:source>(L221) SeaVoX Device Catalogue</dc:source>
    <dc:publisher>British Oceanographic Data Centre (BODC)</dc:publisher>
    <dcterms:modified rdf:datatype="http://www.w3.org/2001/XMLSchema#dateTime">2015-06-10T02:11:20Z</dcterms:modified>
  </rdf:Description>
  <rdf:Description rdf:about="http://vocab.aodn.org.au/def/instrument/entity/553">
    <rdf:type rdf:resource="http://www.w3.org/2004/02/skos/core#Concept" />
    <skos:prefLabel xml:lang="en">Everest Interscience 4000.4ZL Temperature Sensor</skos:prefLabel>
    <dcterms:created rdf:datatype="http://www.w3.org/2001/XMLSchema#dateTime">2013-10-15T00:00:00Z</dcterms:created>
    <skos:definition xml:lang="en">Model 4000.4ZL is an analog, low-temperature, fixed-mounted, infrared temperature sensor. It measures temperatures from -40ºC to 100ºC or -40ºF to 212ºF with resolution of 0.1 ºC or ºF and an accuracy of ±0.5ºC or 1.0ºF.
These instruments are housed in stainless steel cases and are sealed.  This makes them extremely stable in a variety of environments and applications. 
The standard output of the Model 4000.4ZL is Analog Millivolt (10.0 mV/ºC).  Other optional outputs include 4-20 mA and 0-5 Volt.  The standard optics choice is 4º or 15º field of view (FOV).</skos:definition>
    <dc:source>Australian Ocean Data Network instrument register</dc:source>
    <dc:publisher>eMarine Information Infrastructure (eMII)</dc:publisher>
    <skos:scopeNote xml:lang="en">manufacturer:Everest Interscience</skos:scopeNote>
    <dcterms:creator xml:lang="en">Sebastien Mancini</dcterms:creator>
    <skos:inScheme rdf:resource="http://vocab.aodn.org.au/def/instrument/1" />
  </rdf:Description>
  <rdf:Description rdf:about="http://vocab.nerc.ac.uk/collection/L22/current/TOOL0100">
    <rdf:type rdf:resource="http://www.w3.org/2004/02/skos/core#Concept" />
    <skos:prefLabel xml:lang="en">Sea-Bird SBE 16Plus SEACAT C-T Recorder</skos:prefLabel>
    <dcterms:created rdf:datatype="http://www.w3.org/2001/XMLSchema#dateTime">2014-02-07T00:00:00Z</dcterms:created>
    <skos:definition xml:lang="en">The SBE 16plus is a high accuracy conductivity and temperature recorder (pressure optional) with RS232 or RS485 interfaces. It is designed for moorings and other long-duration, fixed-site deployments. The SBE 16plus has 6 amplified A/D input channels and conditioned power of 500 ma is avaliable for auxiliary sensors, dissolved oxygen, turbidity, fluorescence, PAR etc. Further information may be found on the BODC document server at URL: http://www.bodc.ac.uk/data/documents/nodb/153217/ (RS485) or http://www.bodc.ac.uk/data/documents/nodb/158981/ (RS232).</skos:definition>
    <dc:source>(L221) SeaVoX Device Catalogue</dc:source>
    <dc:publisher>British Oceanographic Data Centre (BODC)</dc:publisher>
    <skos:inScheme rdf:resource="http://vocab.aodn.org.au/def/instrument/1" />
    <skos:scopeNote xml:lang="en">manufacturer:Sea-Bird Electronics Inc.</skos:scopeNote>
  </rdf:Description>
  <rdf:Description rdf:about="http://vocab.nerc.ac.uk/collection/L22/current/TOOL0870/">
    <owl:deprecated rdf:datatype="http://www.w3.org/2001/XMLSchema#boolean">true</owl:deprecated>
    <rdfs:label xml:lang="en">Sea-Bird SBE 16Plus V2 SEACAT C-T Recorder</rdfs:label>
    <rdf:type rdf:resource="http://www.w3.org/2004/02/skos/core#Concept" />
    <skos:prefLabel xml:lang="en">Sea-Bird SBE 16Plus V2 SEACAT C-T Recorder</skos:prefLabel>
    <skos:altLabel xml:lang="en">SBE 16+ V2 SEACAT</skos:altLabel>
    <skos:inScheme rdf:resource="http://vocab.aodn.org.au/def/instrument/1" />
    <dcterms:created rdf:datatype="http://www.w3.org/2001/XMLSchema#dateTime">2015-06-03T00:00:00Z</dcterms:created>
    <skos:definition xml:lang="en">The SBE 16plus V2 is a high accuracy conductivity and temperature recorder (pressure optional) with RS232 or RS485 interfaces. It is designed for moorings and other long-duration, fixed-site deployments. It has 6 amplified A/D input channels and conditioned power of 500 ma is available for auxiliary sensors, dissolved oxygen, turbidity, fluorescence, PAR etc. Compared to the previous 16plus, the V2 incorporates an electronics upgrade and additional features, with six differentially amplified A/D input channels, one RS-232 data input channel, and 64 MB FLASH memory. Data can be output in XML as well as ASCII and HEX formats. Firmware upgrades can be downloaded through the communications port, without opening the instrument.</skos:definition>
    <dc:source>(L221) SeaVoX Device Catalogue</dc:source>
    <dc:publisher>British Oceanographic Data Centre (BODC)</dc:publisher>
    <dcterms:modified rdf:datatype="http://www.w3.org/2001/XMLSchema#dateTime">2015-06-10T01:18:45Z</dcterms:modified>
  </rdf:Description>
  <rdf:Description rdf:about="http://vocab.nerc.ac.uk/collection/L22/current/TOOL0190">
    <rdf:type rdf:resource="http://www.w3.org/2004/02/skos/core#Concept" />
    <skos:prefLabel xml:lang="en">Sea-Bird SBE 45 MicroTSG thermosalinograph</skos:prefLabel>
    <skos:inScheme rdf:resource="http://vocab.aodn.org.au/def/instrument/1" />
    <dcterms:created rdf:datatype="http://www.w3.org/2001/XMLSchema#dateTime">2013-10-08T00:00:00Z</dcterms:created>
    <skos:definition xml:lang="en">A small externally powered, high-accuracy instrument, designed for shipboard determination of sea surface (pumped-water) conductivity and temperature. It is constructed of plastic and titanium to ensure long life with minimum maintenance. It may optionally be interfaced to an external SBE 38 hull temperature sensor.</skos:definition>
    <dc:source>(L221) SeaVoX Device Catalogue</dc:source>
    <dc:publisher>British Oceanographic Data Centre (BODC)</dc:publisher>
    <skos:scopeNote xml:lang="en">manufacturer:Sea-Bird Electronics Inc.</skos:scopeNote>
  </rdf:Description>
  <rdf:Description rdf:about="http://vocab.nerc.ac.uk/collection/L22/current/TOOL0191">
    <rdf:type rdf:resource="http://www.w3.org/2004/02/skos/core#Concept" />
    <skos:prefLabel xml:lang="en">Sea-Bird SBE 38 thermometer</skos:prefLabel>
    <skos:inScheme rdf:resource="http://vocab.aodn.org.au/def/instrument/1" />
    <dcterms:created rdf:datatype="http://www.w3.org/2001/XMLSchema#dateTime">2013-10-08T00:00:00Z</dcterms:created>
    <skos:definition xml:lang="en">An oceanographic thermometer with a measurement range of -5 to +35C; absolute accuracy better than 0.001C and resolution of approximately 0.00025C. The sensor is an ultra-stable aged thermistor with a drift rate of less than 0.002C per year. The reference resistor is a hermetically sealed VISHAY. It may be fitted in a 10,500m titanium pressure housing.</skos:definition>
    <dc:source>(L221) SeaVoX Device Catalogue</dc:source>
    <dc:publisher>British Oceanographic Data Centre (BODC)</dc:publisher>
    <skos:scopeNote xml:lang="en">manufacturer:Sea-Bird Electronics Inc.</skos:scopeNote>
  </rdf:Description>
  <rdf:Description rdf:about="http://vocab.nerc.ac.uk/collection/L22/current/TOOL0105">
    <rdf:type rdf:resource="http://www.w3.org/2004/02/skos/core#Concept" />
    <skos:prefLabel xml:lang="en">Vemco Minilog12 temperature recorder</skos:prefLabel>
    <skos:inScheme rdf:resource="http://vocab.aodn.org.au/def/instrument/1" />
    <dcterms:created rdf:datatype="http://www.w3.org/2001/XMLSchema#dateTime">2014-08-06T00:00:00Z</dcterms:created>
    <skos:definition xml:lang="en">A miniature data logger that records temperature at a user programmed time interval. 12-bit version gives a resolution of 0.015C and an accuracy of +-0.1C. It is housed in a waterproof cylinder and the temperature sensor is mounted on a protruding stainless steel probe. Further information may be found on the BODC document server at URL: http://www.bodc.ac.uk/data/documents/nodb/108661/</skos:definition>
    <dc:source>(L221) SeaVoX Device Catalogue</dc:source>
    <dc:publisher>British Oceanographic Data Centre (BODC)</dc:publisher>
  </rdf:Description>
  <rdf:Description rdf:about="http://vocab.nerc.ac.uk/collection/L22/current/TOOL0720">
    <rdf:type rdf:resource="http://www.w3.org/2004/02/skos/core#Concept" />
    <skos:prefLabel xml:lang="en">SMRU Ltd CTD/Fluorometer Satellite Relay Data Logger</skos:prefLabel>
    <skos:inScheme rdf:resource="http://vocab.aodn.org.au/def/instrument/1" />
    <dcterms:created rdf:datatype="http://www.w3.org/2001/XMLSchema#dateTime">2013-10-10T00:00:00Z</dcterms:created>
    <skos:definition xml:lang="en">A package comprising a Valeport CTD sensor head plus a customised Turner Cyclops-7 fluorometer combined with an RF unit and antenna suitable for transmission of data via the Argos satellite system. The unit contains an internal battery and a microprocessor that logs data and schedules the transfer of data. The package is designed for attachment to marine mammals and has an operational depth range of down to 2000 m. CTD accuracy is 0.005 C (temperature), 0.01 mS/cm (conductivity) and 2 dBar (pressure).  It is built and calibrated at Valeport Ltd, while SMRU Ltd, the commercial arm of the Sea Mammal Research Unit of the University of St Andrews, is responsible for its distribution, and for streaming and processing the data. More information is available at http://www.smru.st-and.ac.uk/Instrumentation/FluorometryTag/.</skos:definition>
    <dc:source>(L221) SeaVoX Device Catalogue</dc:source>
    <dc:publisher>British Oceanographic Data Centre (BODC)</dc:publisher>
    <skos:scopeNote xml:lang="en">manufacturer:SMRU Instrumentation</skos:scopeNote>
  </rdf:Description>
  <rdf:Description rdf:about="http://vocab.nerc.ac.uk/collection/L22/current/TOOL0173">
    <rdf:type rdf:resource="http://www.w3.org/2004/02/skos/core#Concept" />
    <skos:prefLabel xml:lang="en">Falmouth Scientific Instruments NXIC CTD</skos:prefLabel>
    <skos:inScheme rdf:resource="http://vocab.aodn.org.au/def/instrument/1" />
    <dcterms:created rdf:datatype="http://www.w3.org/2001/XMLSchema#dateTime">2014-02-07T00:00:00Z</dcterms:created>
    <skos:definition xml:lang="en">A collection of sensors which are generally linked to a common data logger that samples at up to 15Hz. Parameters are measured to an accuracy of ±0.0002 S/m for conductivity, ±0.005°C for temperature and 0.08% for full scale pressure. Now marketed by Teledyne RD Instruments.</skos:definition>
    <dc:source>(L221) SeaVoX Device Catalogue</dc:source>
    <dc:publisher>British Oceanographic Data Centre (BODC)</dc:publisher>
    <skos:scopeNote xml:lang="en">manufacturer:Falmouth Scientific Inc.</skos:scopeNote>
  </rdf:Description>
  <rdf:Description rdf:about="http://vocab.nerc.ac.uk/collection/L22/current/TOOL0898/">
    <rdf:type rdf:resource="http://www.w3.org/2004/02/skos/core#Concept" />
    <skos:prefLabel xml:lang="en">Nortek acoustic wave and current profiler</skos:prefLabel>
    <skos:altLabel xml:lang="en">Nortek AWAC</skos:altLabel>
    <skos:inScheme rdf:resource="http://vocab.aodn.org.au/def/instrument/1" />
    <dcterms:created rdf:datatype="http://www.w3.org/2001/XMLSchema#dateTime">2015-06-03T00:00:00Z</dcterms:created>
    <skos:definition xml:lang="en">A family of instruments that simultaneously measure current profiles and wave height and direction designed for coastal monitoring.  It is available in three transmit frequencies: 1 MHz (range 30 m, cell size 0.25-4 m); 600 kHz (range 50 m, cell size 0.5-8 m), 400 kHz (range 100 m, cell size 1-8 m) and has  four beams, one vertical and the other three 120 degrees apart slanted at 25 degrees. Maximum number of cells is 128. Current speeds up to 10 m/s may be measured at an accuracy of 1% of measured value ±0.5cm/s. Temperature (embedded thermistor with 0.1C accuracy and 0.01C resolution), compass (magnetometer with 2 degrees accuracy and 0.1 degree resolution providing tilt less than 15 degrees), tilt (liquid level) and pressure (piezo resistive with accuracy of 0.5% (optional 0.1%) full scale - usually 100m - and resolution of 0.005% full scale) sensors are provided as standard.</skos:definition>
    <dc:publisher>British Oceanographic Data Centre (BODC)</dc:publisher>
    <dcterms:modified rdf:datatype="http://www.w3.org/2001/XMLSchema#dateTime">2015-06-30T06:19:13Z</dcterms:modified>
    <dcterms:contributor>Natalia_Atkins</dcterms:contributor>
  </rdf:Description>
  <rdf:Description rdf:about="http://vocab.nerc.ac.uk/collection/L22/current/TOOL0490">
    <rdf:type rdf:resource="http://www.w3.org/2004/02/skos/core#Concept" />
    <skos:prefLabel xml:lang="en">Star-Oddi DST Pitch and Roll Recorder</skos:prefLabel>
    <skos:inScheme rdf:resource="http://vocab.aodn.org.au/def/instrument/1" />
    <dcterms:created rdf:datatype="http://www.w3.org/2001/XMLSchema#dateTime">2014-02-06T00:00:00Z</dcterms:created>
    <skos:definition xml:lang="en">A miniature underwater data logger which measures temperature, pressure and pitch and roll (tilt angle) relative to the earth gravity. It has a range of depth ratings from 30 m to 3000 m and a temperature range of -1 degC to 40 degC with an accuracy of +/- 0.1 degC and a resolution of 0.032 degC. The tilt range is 160 deg (+/- 80 deg) with an accuracy of +/- 5deg and a resolution of 0.3 deg.</skos:definition>
    <dc:source>(L221) SeaVoX Device Catalogue</dc:source>
    <dc:publisher>British Oceanographic Data Centre (BODC)</dc:publisher>
    <skos:scopeNote xml:lang="en">manufacturer:Star-Oddi</skos:scopeNote>
  </rdf:Description>
  <rdf:Description rdf:about="http://vocab.nerc.ac.uk/collection/L22/current/TOOL0871/">
    <rdf:type rdf:resource="http://www.w3.org/2004/02/skos/core#Concept" />
    <skos:prefLabel xml:lang="en">Sea-Bird SBE 19plus V2 SEACAT CTD</skos:prefLabel>
    <skos:altLabel xml:lang="en">SBE 19+ V2 SEACAT</skos:altLabel>
    <skos:inScheme rdf:resource="http://vocab.aodn.org.au/def/instrument/1" />
    <dcterms:created rdf:datatype="http://www.w3.org/2001/XMLSchema#dateTime">2015-06-03T00:00:00Z</dcterms:created>
    <skos:definition xml:lang="en">Self-contained self-powered CTD profiler. Measures conductivity, temperature and pressure (Digiquartz sensor) in both profiling (samples at 4 scans/sec) and moored (sample rates of once every 5 seconds to once every 9 hours) mode. Available in plastic or titanium housing with depth ranges of 600m and 7000m respectively. Miniature submersible pump provides water to the conductivity cell.  Compared to the previous 19plus, the V2 incorporates an electronics upgrade and additional features, with six differentially amplified A/D input channels, one RS-232 data input channel, and 64 MB FLASH memory.</skos:definition>
    <dc:source>(L221) SeaVoX Device Catalogue</dc:source>
    <dc:publisher>British Oceanographic Data Centre (BODC)</dc:publisher>
    <dcterms:modified rdf:datatype="http://www.w3.org/2001/XMLSchema#dateTime">2015-06-10T02:07:18Z</dcterms:modified>
  </rdf:Description>
  <rdf:Description rdf:about="http://vocab.nerc.ac.uk/collection/L22/current/TOOL0809">
    <owl:deprecated rdf:datatype="http://www.w3.org/2001/XMLSchema#boolean">true</owl:deprecated>
    <rdfs:label xml:lang="en">RBR TGR-2050 submersible tide gauge</rdfs:label>
    <rdf:type rdf:resource="http://www.w3.org/2004/02/skos/core#Concept" />
    <skos:prefLabel xml:lang="en">RBR TGR-2050 submersible tide gauge</skos:prefLabel>
    <skos:altLabel xml:lang="en">RBR TGR-2050 TG</skos:altLabel>
    <skos:inScheme rdf:resource="http://vocab.aodn.org.au/def/instrument/1" />
    <dcterms:created rdf:datatype="http://www.w3.org/2001/XMLSchema#dateTime">2013-03-28T00:00:00Z</dcterms:created>
    <skos:definition xml:lang="en">A small (265mm x 38mm OD) self-contained, submersible temperature and pressure logger designed to monitor tide levels without interference from wave action by averaging pressure data sampled at 4 Hz. This operating mode differentiates it from the similar TDR-2050. Temperature channel is calibrated to ±0.002C. Depth channel is calibrated to an accuracy of ±0.05% full scale.</skos:definition>
    <dc:source>(L221) SeaVoX Device Catalogue</dc:source>
    <dc:publisher>British Oceanographic Data Centre (BODC)</dc:publisher>
    <dcterms:modified rdf:datatype="http://www.w3.org/2001/XMLSchema#dateTime">2015-07-07T04:49:53Z</dcterms:modified>
    <dcterms:contributor>Natalia_Atkins</dcterms:contributor>
  </rdf:Description>
  <rdf:Description rdf:about="http://vocab.nerc.ac.uk/collection/L22/current/TOOL0416">
    <rdf:type rdf:resource="http://www.w3.org/2004/02/skos/core#Concept" />
    <skos:prefLabel xml:lang="en">Sea-Bird SBE 3plus (SBE 3P) temperature sensor</skos:prefLabel>
    <skos:inScheme rdf:resource="http://vocab.aodn.org.au/def/instrument/1" />
    <dcterms:created rdf:datatype="http://www.w3.org/2001/XMLSchema#dateTime">2014-07-21T00:00:00Z</dcterms:created>
    <skos:definition xml:lang="en">Water temperature sensor designed for use on the SBE 9plus CTD system. The sensor operates over the range -5 to +35 °C, a resolution of 0.0003 °C at 24 Hz and an initial accuracy of ± 0.001 °C. The typical sampling rate is 24 Hz, and the sensor has a depth rating of 6800 meters (aluminum housing) or 10500 meters (titanium housing).</skos:definition>
    <dc:source>(L221) SeaVoX Device Catalogue</dc:source>
    <dc:publisher>British Oceanographic Data Centre (BODC)</dc:publisher>
  </rdf:Description>
  <rdf:Description rdf:about="http://vocab.nerc.ac.uk/collection/L22/current/TOOL0181">
    <rdf:type rdf:resource="http://www.w3.org/2004/02/skos/core#Concept" />
    <skos:prefLabel xml:lang="en">Vemco Minilog8 temperature recorder</skos:prefLabel>
    <skos:inScheme rdf:resource="http://vocab.aodn.org.au/def/instrument/1" />
    <dcterms:created rdf:datatype="http://www.w3.org/2001/XMLSchema#dateTime">2014-08-06T00:00:00Z</dcterms:created>
    <skos:definition xml:lang="en">A miniature data logger that records temperature at a user programmed time interval. 8-bit version gives a resolution of 0.1C and an accuracy of between +-0.2C to +-0.3C depending on range specified. It is housed in a waterproof cylinder and the temperature sensor is mounted on a protruding stainless steel probe.</skos:definition>
    <dc:source>(L221) SeaVoX Device Catalogue</dc:source>
    <dc:publisher>British Oceanographic Data Centre (BODC)</dc:publisher>
  </rdf:Description>
  <rdf:Description rdf:about="http://vocab.nerc.ac.uk/collection/L22/current/TOOL0712">
    <rdf:type rdf:resource="http://www.w3.org/2004/02/skos/core#Concept" />
    <skos:prefLabel xml:lang="en">Aanderaa temperature sensor 4050</skos:prefLabel>
    <skos:inScheme rdf:resource="http://vocab.aodn.org.au/def/instrument/1" />
    <dcterms:created rdf:datatype="http://www.w3.org/2001/XMLSchema#dateTime">2013-10-15T00:00:00Z</dcterms:created>
    <skos:definition xml:lang="en">A compact fully integrated sensor for measuring the water temperature. The sensor is designed to be mounted on Aanderaa recording instruments (e.g. RCM 9/11 doppler current meter) and data loggers. The sensor can also be used as stand alone, and is easily integrated in other measurement systems with third party data loggers. Resolution is 0.001 C and accuracy is 0.03 C. Further development of the 4050 has been suspended in favour of the replacement 4060 model. More information may be found in http://www.aanderaa.com/productsdetail.php?Temperature-Sensor-12.</skos:definition>
    <dc:source>(L221) SeaVoX Device Catalogue</dc:source>
    <dc:publisher>British Oceanographic Data Centre (BODC)</dc:publisher>
    <skos:scopeNote xml:lang="en">manufacturer:Aanderaa Data Instruments</skos:scopeNote>
  </rdf:Description>
  <rdf:Description rdf:about="http://vocab.aodn.org.au/def/instrument/entity/39">
    <rdf:type rdf:resource="http://www.w3.org/2004/02/skos/core#Concept" />
    <skos:prefLabel xml:lang="en">Lockheed Martin Sippican Deep Blue XBT probe</skos:prefLabel>
    <dcterms:created rdf:datatype="http://www.w3.org/2001/XMLSchema#dateTime">2013-03-28T00:00:00Z</dcterms:created>
    <dcterms:contributor>Natalia_Atkins</dcterms:contributor>
    <dc:source>Australian Ocean Data Network instrument register</dc:source>
    <dc:publisher>eMarine Information Infrastructure (eMII)</dc:publisher>
    <skos:scopeNote xml:lang="en">manufacturer: Lockheed Martin</skos:scopeNote>
    <dcterms:creator xml:lang="en">Sebastien Mancini</dcterms:creator>
    <skos:definition xml:lang="en">An expendable free-fall temperature probe that provides a profile of measured temperature against depth calculated from a fall-rate model. The Deep Blue XBT Probe (sometimes referred to as the T-7DB) can be used to a maximum depth of 460m, may be deployed at a ship speed of up to 20 knots and has a vertical resolution of 65cm.</skos:definition>
    <dcterms:modified rdf:datatype="http://www.w3.org/2001/XMLSchema#dateTime">2015-06-30T05:43:15Z</dcterms:modified>
    <skos:inScheme rdf:resource="http://vocab.aodn.org.au/def/instrument/1" />
  </rdf:Description>
  <rdf:Description rdf:about="http://vocab.nerc.ac.uk/collection/L22/current/TOOL0888/">
    <rdf:type rdf:resource="http://www.w3.org/2004/02/skos/core#Concept" />
    <skos:prefLabel xml:lang="en">Nortek Aquadopp Doppler current profiler</skos:prefLabel>
    <skos:altLabel xml:lang="en">Aquadopp profiler</skos:altLabel>
    <skos:inScheme rdf:resource="http://vocab.aodn.org.au/def/instrument/1" />
    <dcterms:created rdf:datatype="http://www.w3.org/2001/XMLSchema#dateTime">2015-06-03T00:00:00Z</dcterms:created>
    <skos:definition xml:lang="en">A family of self-contained Doppler current profilers designed for deployment on the seabed, moorings, buoys or fixed structures.  A range of transducers - 400 kHz (60-90m range: 2-8m cell size), 600 kHz (30-40m range: 1-4m cell size), Z-cell 600 kHz, 1 MHz (12-20m range: 0.3-4m cell size), Z-cell 1MHz, 2 MHz (4-10m range:0.1-2m cell size) and side-looking.  Each transducer has 3 beams and the instrument has a maximum of 128 cells. Current speeds up to 10 m/s may be measured at an accuracy of 1% of measured value ±0.5cm/s. The standard depth rating is 300 m with 3000 m or 600m versions available. Temperature (embedded thermistor with 0.1C accuracy and 0.01C resolution), compass (magnetometer with 2 degrees accuracy and 0.1 degree resolution providing tilt less than 20 degrees), tilt (liquid level with 0.2 degree accuracy and 0.1 degree resolution) and pressure (piezo resistive with accuracy of 0.5% full scale - usually 100m - and resolution of 0.005% full scale) sensors are provided as standard.</skos:definition>
    <dc:publisher>British Oceanographic Data Centre (BODC)</dc:publisher>
    <dcterms:modified rdf:datatype="http://www.w3.org/2001/XMLSchema#dateTime">2015-07-01T02:07:35Z</dcterms:modified>
    <dcterms:contributor>Natalia_Atkins</dcterms:contributor>
  </rdf:Description>
  <rdf:Description rdf:about="http://vocab.nerc.ac.uk/collection/L22/current/TOOL0707">
    <rdf:type rdf:resource="http://www.w3.org/2004/02/skos/core#Concept" />
    <skos:prefLabel xml:lang="en">Analog Devices AD590 Temperature Transducer</skos:prefLabel>
    <skos:inScheme rdf:resource="http://vocab.aodn.org.au/def/instrument/1" />
    <dcterms:created rdf:datatype="http://www.w3.org/2001/XMLSchema#dateTime">2013-10-15T00:00:00Z</dcterms:created>
    <skos:definition xml:lang="en">This is a 2-terminal integrated circuit temperature transducer that produces an output current proportional to absolute temperature (one microAmp per Kelvin). It is calibrated by laser trimming of the resistors on the chip to produce an output of 298.2 microAmps at 298.2K. It is supplied in a range of standard electronic component packages for inclusion on circuit boards. It can operate from -55-150C, is linear to 0.3C over full range and has an accuracy of 0.5C. Further details may be found at http://www.analog.com/en/mems-sensors/digital-temperature-sensors/ad590/products/product.html.</skos:definition>
    <dc:source>(L221) SeaVoX Device Catalogue</dc:source>
    <dc:publisher>British Oceanographic Data Centre (BODC)</dc:publisher>
    <skos:scopeNote xml:lang="en">manufacturer:Analog Devices</skos:scopeNote>
  </rdf:Description>
  <rdf:Description rdf:about="http://vocab.nerc.ac.uk/collection/L22/current/TOOL0640">
    <rdf:type rdf:resource="http://www.w3.org/2004/02/skos/core#Concept" />
    <skos:prefLabel xml:lang="en">Sea-Bird SBE 3F temperature sensor</skos:prefLabel>
    <skos:inScheme rdf:resource="http://vocab.aodn.org.au/def/instrument/1" />
    <dcterms:created rdf:datatype="http://www.w3.org/2001/XMLSchema#dateTime">2013-10-31T00:00:00Z</dcterms:created>
    <skos:definition xml:lang="en">Water temperature sensor primarily designed for use on the SBE 25 and 25plus Sealogger CTD systems but can be used as a component in custom oceanographic profiling systems or high-accuracy temperature-monitoring applications. The sensor operates over the range -5 to +35 degC and has an initial accuracy of +/-0.001 degC. The sensor has a depth rating of 6800 m (aluminum housing) or 10500 m (titanium housing). The SBE 3F is an enhanced version of the SBE 3 temperature sensor.</skos:definition>
    <dc:source>(L221) SeaVoX Device Catalogue</dc:source>
    <dc:publisher>British Oceanographic Data Centre (BODC)</dc:publisher>
    <skos:scopeNote xml:lang="en">manufacturer:Sea-Bird Electronics Inc.</skos:scopeNote>
  </rdf:Description>
  <rdf:Description rdf:about="http://vocab.nerc.ac.uk/collection/L22/current/TOOL0023">
    <rdf:type rdf:resource="http://www.w3.org/2004/02/skos/core#Concept" />
    <skos:prefLabel xml:lang="en">Sea-Bird SBE 16 SEACAT C-T Recorder</skos:prefLabel>
    <dcterms:created rdf:datatype="http://www.w3.org/2001/XMLSchema#dateTime">2014-02-17T00:00:00Z</dcterms:created>
    <skos:definition xml:lang="en">The SBE 16 SEACAT is a conductivity and temperature recorder with an optional pressure sensor designed for depolyment on moorings. Further information may be found on the BODC document server at URL http://www.bodc.ac.uk/data/documents/nodb/117180/. Replaced by the SBE 16plus range in 2001.</skos:definition>
    <dc:source>(L221) SeaVoX Device Catalogue</dc:source>
    <dc:publisher>British Oceanographic Data Centre (BODC)</dc:publisher>
    <skos:inScheme rdf:resource="http://vocab.aodn.org.au/def/instrument/1" />
    <skos:scopeNote xml:lang="en">manufacturer:Sea-Bird Electronics Inc.</skos:scopeNote>
  </rdf:Description>
  <rdf:Description rdf:about="http://vocab.nerc.ac.uk/collection/L22/current/TOOL0706">
    <rdf:type rdf:resource="http://www.w3.org/2004/02/skos/core#Concept" />
    <skos:prefLabel xml:lang="en">Vemco Minilog II T 16-bit Temperature Logger</skos:prefLabel>
    <skos:inScheme rdf:resource="http://vocab.aodn.org.au/def/instrument/1" />
    <dcterms:created rdf:datatype="http://www.w3.org/2001/XMLSchema#dateTime">2014-06-16T00:00:00Z</dcterms:created>
    <skos:definition xml:lang="en">The VEMCO Minilog II T is a fully submersible, 10-year temperature data logger measures and stores temperature at specified sampling intervals. The Minilog- II-T data logger is manufactured to withstand both fresh and saltwater environments.</skos:definition>
    <dc:source>(L221) SeaVoX Device Catalogue</dc:source>
    <dc:publisher>British Oceanographic Data Centre (BODC)</dc:publisher>
  </rdf:Description>
  <rdf:Description rdf:about="http://vocab.nerc.ac.uk/collection/L22/current/TOOL0020">
    <rdf:type rdf:resource="http://www.w3.org/2004/02/skos/core#Concept" />
    <skos:prefLabel xml:lang="en">Sea-Bird SBE 37-SIP MicroCAT C-T Sensor</skos:prefLabel>
    <dcterms:created rdf:datatype="http://www.w3.org/2001/XMLSchema#dateTime">2014-02-26T00:00:00Z</dcterms:created>
    <skos:definition xml:lang="en">The SBE 37 MicroCAT is a high accuracy conductivity and temperature recorder with an optional pressure sensor designed for depolyment on moorings. The SIP model has a serial interface with an internal pump to improve conductivity response and protection against fouling.</skos:definition>
    <dc:source>(L221) SeaVoX Device Catalogue</dc:source>
    <dc:publisher>British Oceanographic Data Centre (BODC)</dc:publisher>
    <skos:inScheme rdf:resource="http://vocab.aodn.org.au/def/instrument/1" />
    <skos:scopeNote xml:lang="en">manufacturer:Sea-Bird Electronics Inc.</skos:scopeNote>
  </rdf:Description>
  <rdf:Description rdf:about="http://vocab.nerc.ac.uk/collection/L22/current/TOOL0687">
    <rdf:type rdf:resource="http://www.w3.org/2004/02/skos/core#Concept" />
    <skos:prefLabel xml:lang="en">Sea-Bird SBE 56 temperature recorder</skos:prefLabel>
    <skos:inScheme rdf:resource="http://vocab.aodn.org.au/def/instrument/1" />
    <dcterms:created rdf:datatype="http://www.w3.org/2001/XMLSchema#dateTime">2014-06-05T00:00:00Z</dcterms:created>
    <skos:definition xml:lang="en">This is a small (30cm by 2.54cm diameter) high-accuracy battery-powered temperature and time logger capable of sampling intervals from 0.5 seconds to 9 hours. Battery life with a sampling rate of 15 seconds is almost two years and the memory can store over 15 million samples. Temperature is measured by a pressure-protected (1500m depth) thermistor. Initial accuracy is 0.002C and drift is typically less than 0.002C per year. More information may be found at http://www.seabird.com/products/spec_sheets/39imdata.htm.</skos:definition>
    <dc:source>(L221) SeaVoX Device Catalogue</dc:source>
    <dc:publisher>British Oceanographic Data Centre (BODC)</dc:publisher>
  </rdf:Description>
  <rdf:Description rdf:about="http://vocab.nerc.ac.uk/collection/L22/current/TOOL0688">
    <rdf:type rdf:resource="http://www.w3.org/2004/02/skos/core#Concept" />
    <skos:prefLabel xml:lang="en">Sea-Bird SBE 39-IM temperature recorder</skos:prefLabel>
    <skos:inScheme rdf:resource="http://vocab.aodn.org.au/def/instrument/1" />
    <dcterms:created rdf:datatype="http://www.w3.org/2001/XMLSchema#dateTime">2014-06-05T00:00:00Z</dcterms:created>
    <skos:definition xml:lang="en">A high-accuracy temperature recorder (pressure optional) with internal battery and a built-in inductive modem intended for moorings with either real-time telemetry or a surface data logger.  Data are also stored in internal non-volatile memory as insurance against data loss.  Calibration coefficients stored in EEPROM allow the SBE 39 to transmit data in engineering units. The SBE 39 thermistor has a long history of exceptional initial accuracy (0.002C) and stability (typical drift is 0.0002C per month).  The standard plastic housing is for depths down to 600m, but an optional titanium housing can withstand depths of 10500m.  For more information see http://www.seabird.com/products/spec_sheets/39imdata.htm.</skos:definition>
    <dc:source>(L221) SeaVoX Device Catalogue</dc:source>
    <dc:publisher>British Oceanographic Data Centre (BODC)</dc:publisher>
  </rdf:Description>
  <rdf:Description rdf:about="http://vocab.nerc.ac.uk/collection/L22/current/TOOL0685">
    <rdf:type rdf:resource="http://www.w3.org/2004/02/skos/core#Concept" />
    <skos:prefLabel xml:lang="en">Aquatech AQUAlogger 520PT mini temperature and pressure logger</skos:prefLabel>
    <skos:inScheme rdf:resource="http://vocab.aodn.org.au/def/instrument/1" />
    <dcterms:created rdf:datatype="http://www.w3.org/2001/XMLSchema#dateTime">2014-06-04T00:00:00Z</dcterms:created>
    <skos:definition xml:lang="en">A miniature (200mm long, 32mm diameter) self-contained data logger incorporating a thermistor temperature sensor (resolution better that 0.007C, accuracy 0.05C) and a pressure sensor in a housing designed to operate at depths down to 1000m.  The type of pressure sensor fitted depends upon the maximum operating depth required with resolution and accuracy a function of the full-scale reading. The logger may be programmed to provide a wide variety of sampling regimes, including burst recording. More information may be found in http://www.aquatecgroup.com/images/manual_guides/bg%20-%20520.pdf.</skos:definition>
    <dc:source>(L221) SeaVoX Device Catalogue</dc:source>
    <dc:publisher>British Oceanographic Data Centre (BODC)</dc:publisher>
  </rdf:Description>
  <rdf:Description rdf:about="http://vocab.nerc.ac.uk/collection/L22/current/TOOL0684">
    <rdf:type rdf:resource="http://www.w3.org/2004/02/skos/core#Concept" />
    <skos:prefLabel xml:lang="en">Aquatech AQUAlogger 520T mini temperature logger</skos:prefLabel>
    <skos:inScheme rdf:resource="http://vocab.aodn.org.au/def/instrument/1" />
    <dcterms:created rdf:datatype="http://www.w3.org/2001/XMLSchema#dateTime">2014-06-04T00:00:00Z</dcterms:created>
    <skos:definition xml:lang="en">A miniature (200mm long, 32mm diameter) self-contained data logger incorporating a thermistor temperature sensor (resolution better that 0.007C, accuracy 0.05C) in a housing designed to operate at depths down to 1000m.  The logger may be programmed to provide a wide variety of sampling regimes, including burst recording. More information may be found in http://www.aquatecgroup.com/images/manual_guides/bg%20-%20520.pdf.</skos:definition>
    <dc:source>(L221) SeaVoX Device Catalogue</dc:source>
    <dc:publisher>British Oceanographic Data Centre (BODC)</dc:publisher>
  </rdf:Description>
  <rdf:Description rdf:about="http://vocab.nerc.ac.uk/collection/L22/current/TOOL0266">
    <rdf:type rdf:resource="http://www.w3.org/2004/02/skos/core#Concept" />
    <skos:prefLabel xml:lang="en">Sea-Bird SBE 39 temperature recorder</skos:prefLabel>
    <skos:inScheme rdf:resource="http://vocab.aodn.org.au/def/instrument/1" />
    <dcterms:created rdf:datatype="http://www.w3.org/2001/XMLSchema#dateTime">2014-02-06T00:00:00Z</dcterms:created>
    <skos:definition xml:lang="en">A high-accuracy temperature recorder (pressure optional) with internal battery and non-volatile memory for deployment at depths up to 10500 meters. It is intended for moorings or other long-term, fixed-site applications, as well as shorter-term deployments on nets, towed vehicles or ROVs. Calibration coefficients stored in EEPROM allow the SBE 39 to transmit data in engineering units. The SBE 39 thermistor has a long history of exceptional accuracy and stability (typical drift is less than 0.002C per year). The SBE 39 communicates directly with a computer via a standard RA-232 interface. For more information see http://www.bodc.ac.uk/data/documents/nodb/108627/</skos:definition>
    <dc:source>(L221) SeaVoX Device Catalogue</dc:source>
    <dc:publisher>British Oceanographic Data Centre (BODC)</dc:publisher>
    <skos:scopeNote xml:lang="en">manufacturer:Sea-Bird Electronics Inc.</skos:scopeNote>
  </rdf:Description>
  <rdf:Description rdf:about="http://vocab.nerc.ac.uk/collection/L22/current/TOOL0267">
    <rdf:type rdf:resource="http://www.w3.org/2004/02/skos/core#Concept" />
    <skos:prefLabel xml:lang="en">Star-Oddi Starmon mini temperature recorder</skos:prefLabel>
    <skos:inScheme rdf:resource="http://vocab.aodn.org.au/def/instrument/1" />
    <dcterms:created rdf:datatype="http://www.w3.org/2001/XMLSchema#dateTime">2014-02-06T00:00:00Z</dcterms:created>
    <skos:definition xml:lang="en">An underwater temperature recorder in either a plastic (400m) or titanium (11000m) casing.  Temperature average resolution is 0.013C and accuracy is +-0.05C over a range -2C to 40C: clock accuray better than 1 minute per month. Temperature equilibration: 63% 18 seconds (plastic case) or 6 seconds (titanium case); 100% 3 minutes (plastic case) or 1 minute (titanium case).</skos:definition>
    <dc:source>(L221) SeaVoX Device Catalogue</dc:source>
    <dc:publisher>British Oceanographic Data Centre (BODC)</dc:publisher>
    <skos:scopeNote xml:lang="en">manufacturer:Star-Oddi</skos:scopeNote>
  </rdf:Description>
  <rdf:Description rdf:about="http://vocab.nerc.ac.uk/collection/L22/current/TOOL0872/">
    <rdf:type rdf:resource="http://www.w3.org/2004/02/skos/core#Concept" />
    <skos:prefLabel xml:lang="en">Teledyne RDI Workhorse Navigator 1200kHz Doppler Velocity Log</skos:prefLabel>
    <skos:altLabel xml:lang="en">RDI Workhorse Navigator 1200kHz DVL</skos:altLabel>
    <skos:inScheme rdf:resource="http://vocab.aodn.org.au/def/instrument/1" />
    <dcterms:created rdf:datatype="http://www.w3.org/2001/XMLSchema#dateTime">2015-06-03T00:00:00Z</dcterms:created>
    <skos:definition xml:lang="en">A Doppler velocity log (DVL) measuring bottom track and water track velocities, altitude, heading, tilt, temperature and echo intensity. 1200kHz Broadband signal processing gives high data resolution and a four-beam solution gives an independent error velocity measurement as an indicator of data quality. It has a bottom track range of 30m and velocity accuracy for both bottom and water track modes is 0.2% of the velocity, ±0.1cm/s. The instrument operates effectively over a temperature range of -5°C to 45°C and with a tilt of up to ±15 deg.</skos:definition>
    <dc:publisher>British Oceanographic Data Centre (BODC)</dc:publisher>
    <dcterms:modified rdf:datatype="http://www.w3.org/2001/XMLSchema#dateTime">2015-06-30T03:42:14Z</dcterms:modified>
    <dcterms:contributor>Natalia_Atkins</dcterms:contributor>
  </rdf:Description>
  <rdf:Description rdf:about="http://vocab.nerc.ac.uk/collection/L22/current/TOOL0446">
    <rdf:type rdf:resource="http://www.w3.org/2004/02/skos/core#Concept" />
    <skos:prefLabel xml:lang="en">SMRU CTD Satellite Relay Data Logger</skos:prefLabel>
    <skos:inScheme rdf:resource="http://vocab.aodn.org.au/def/instrument/1" />
    <dcterms:created rdf:datatype="http://www.w3.org/2001/XMLSchema#dateTime">2013-10-10T00:00:00Z</dcterms:created>
    <skos:definition xml:lang="en">This tag provides oceanographic quality Conductivity/Temperature/Depth casts. Oceanographic quality temperature &amp; salinity profiles (4 - 12 profiles per day), CTD data automatically submitted to the GTS in near real-time. Up to 50,000 full length Argos data transmissions and pressure-proof to 2000m.  Retains a continuous record of depth readings (4 sec sample rate), which can be retrieved by bluetooth link if the tag is recovered. Also records all individual temperature and salinity measurements (1 Hz) made during profiling. Longevity: up to one year. Size: 10.5 x 7 x 4 cm. Weight: 545 g.</skos:definition>
    <dc:source>(L221) SeaVoX Device Catalogue</dc:source>
    <dc:publisher>British Oceanographic Data Centre (BODC)</dc:publisher>
    <skos:scopeNote xml:lang="en">manufacturer:SMRU Instrumentation</skos:scopeNote>
  </rdf:Description>
  <rdf:Description rdf:about="http://vocab.nerc.ac.uk/collection/L22/current/TOOL0696">
    <rdf:type rdf:resource="http://www.w3.org/2004/02/skos/core#Concept" />
    <skos:prefLabel xml:lang="en">Sea-Bird SBE 26plus SEAGAUGE Wave and Tide Recorder</skos:prefLabel>
    <skos:inScheme rdf:resource="http://vocab.aodn.org.au/def/instrument/1" />
    <dcterms:created rdf:datatype="http://www.w3.org/2001/XMLSchema#dateTime">2013-09-25T00:00:00Z</dcterms:created>
    <skos:definition xml:lang="en">The SBE 26 SEAGAUGE is a water level recorder with a Digiquartz pressure sensor, accurate clock, precision thermometer and optional conductivity sensor in a casing able to operate down to 600m. Pressure data are integrated to give sea level or are burst recorded at rates up to 4 Hz to measure characterise waves. The instrument offers improved temperature sensor accuracy (0.01C with 0.001C resolution or optionally 0.001C with 0.0001C resolution), data storage and operational functionality over the SBE-26. More information at http://www.seabird.com/products/spec_sheets/26plusdata.htm.</skos:definition>
    <dc:source>(L221) SeaVoX Device Catalogue</dc:source>
    <dc:publisher>British Oceanographic Data Centre (BODC)</dc:publisher>
    <skos:scopeNote xml:lang="en">manufacturer:Sea-Bird Electronics Inc.</skos:scopeNote>
  </rdf:Description>
  <rdf:Description rdf:about="http://vocab.nerc.ac.uk/collection/L22/current/TOOL0731">
    <rdf:type rdf:resource="http://www.w3.org/2004/02/skos/core#Concept" />
    <skos:prefLabel xml:lang="en">ReefNet Sensus Ultra</skos:prefLabel>
    <skos:inScheme rdf:resource="http://vocab.aodn.org.au/def/instrument/1" />
    <dcterms:created rdf:datatype="http://www.w3.org/2001/XMLSchema#dateTime">2014-07-14T00:00:00Z</dcterms:created>
    <skos:definition xml:lang="en">The ReefNet Sensus Ultra is a compact temperature and depth logging sensor designed for use as a dive computer. Depths between 0 and 500 feet are measured with precision better than 0.5 inches of water, and accuracy of +/-12 inches. Temperature is measured between -20 degC and + 40 degC, with precision of 0.01 degC, and accuracy of +/-0.8 degC. Sampling interval is configurable from 1 second to over 18 hours, with storage capacity of one year at 60 second sampling resolution.</skos:definition>
    <dc:source>(L221) SeaVoX Device Catalogue</dc:source>
    <dc:publisher>British Oceanographic Data Centre (BODC)</dc:publisher>
  </rdf:Description>
  <rdf:Description rdf:about="http://vocab.nerc.ac.uk/collection/L22/current/TOOL0675">
    <rdf:type rdf:resource="http://www.w3.org/2004/02/skos/core#Concept" />
    <skos:prefLabel xml:lang="en">WETLabs Water Quality Monitor</skos:prefLabel>
    <dcterms:created rdf:datatype="http://www.w3.org/2001/XMLSchema#dateTime">2014-04-01T00:00:00Z</dcterms:created>
    <skos:definition xml:lang="en">An instrument that incorporates WET Labs fluorometer-turbidity and Sea-Bird's CTD sensors, providing temperature, salinity, depth, dissolved oxygen, chlorophyll fluorescence, turbidity and backscattering data. It is designed for long-term deployment in coastal waters with protection against biofouling and fouling by sediment loads. More information is available at http://www.wetlabs.com/wqm.</skos:definition>
    <dc:source>(L221) SeaVoX Device Catalogue</dc:source>
    <dc:publisher>British Oceanographic Data Centre (BODC)</dc:publisher>
    <skos:inScheme rdf:resource="http://vocab.aodn.org.au/def/instrument/1" />
    <skos:scopeNote xml:lang="en">manufacture:WETLabs Inc.</skos:scopeNote>
  </rdf:Description>
  <rdf:Description rdf:about="http://vocab.nerc.ac.uk/collection/L22/current/TOOL0019">
    <rdf:type rdf:resource="http://www.w3.org/2004/02/skos/core#Concept" />
    <skos:prefLabel xml:lang="en">Sea-Bird SBE 37-IMP MicroCAT C-T Sensor</skos:prefLabel>
    <dcterms:created rdf:datatype="http://www.w3.org/2001/XMLSchema#dateTime">2014-02-17T00:00:00Z</dcterms:created>
    <skos:definition xml:lang="en">The SBE 37 MicroCAT is a high accuracy conductivity and temperature recorder with an optional pressure sensor designed for depolyment on moorings. The IMP model has an inductive modem for real-time data transmission plus internal flash memory data storage with an internal pump to improve conductivity response and protection against fouling.</skos:definition>
    <dc:source>(L221) SeaVoX Device Catalogue</dc:source>
    <dc:publisher>British Oceanographic Data Centre (BODC)</dc:publisher>
    <skos:inScheme rdf:resource="http://vocab.aodn.org.au/def/instrument/1" />
    <skos:scopeNote xml:lang="en">manufacturer:Sea-Bird Electronics Inc.</skos:scopeNote>
  </rdf:Description>
  <rdf:Description rdf:about="http://vocab.nerc.ac.uk/collection/L22/current/TOOL0670">
    <rdf:type rdf:resource="http://www.w3.org/2004/02/skos/core#Concept" />
    <skos:prefLabel xml:lang="en">Sea-Bird SBE 48 Hull Temperature Sensor</skos:prefLabel>
    <skos:inScheme rdf:resource="http://vocab.aodn.org.au/def/instrument/1" />
    <dcterms:created rdf:datatype="http://www.w3.org/2001/XMLSchema#dateTime">2013-10-15T00:00:00Z</dcterms:created>
    <skos:definition xml:lang="en">A high-accuracy temperature recorder with non-volatile memory and RS-232 port, designed for shipboard determination of sea surface temperature. It is magnetically fixed just below the water line with the temperature sensor in contact with the inside of the ship's hull. The thermistor is the same as the SBE 39 which has an accuracy of 0.002C, stability of 0.0002 C/month and resolution of 0.0001 C .  A real-time clock accurate within 1 minute/year is included for self-contained operation. More information is given in http://www.seabird.com/pdf_documents/manuals/48_004.pdf.</skos:definition>
    <dc:source>(L221) SeaVoX Device Catalogue</dc:source>
    <dc:publisher>British Oceanographic Data Centre (BODC)</dc:publisher>
    <skos:scopeNote xml:lang="en">manufacturer:Sea-Bird Electronics Inc.</skos:scopeNote>
  </rdf:Description>
  <rdf:Description rdf:about="http://vocab.nerc.ac.uk/collection/L22/current/TOOL0017">
    <rdf:type rdf:resource="http://www.w3.org/2004/02/skos/core#Concept" />
    <skos:prefLabel xml:lang="en">Sea-Bird SBE 37-SM MicroCAT C-T Sensor</skos:prefLabel>
    <dcterms:created rdf:datatype="http://www.w3.org/2001/XMLSchema#dateTime">2014-02-06T00:00:00Z</dcterms:created>
    <skos:definition xml:lang="en">The SBE 37 MicroCAT is a high accuracy conductivity and temperature recorder with an optional pressure sensor designed for depolyment on moorings. The SM model has a serial interface plus internal flash memory data storage. Further information may be found on the BODC document server at URL http://www.bodc.ac.uk/data/documents/nodb/108613/.</skos:definition>
    <dc:source>(L221) SeaVoX Device Catalogue</dc:source>
    <dc:publisher>British Oceanographic Data Centre (BODC)</dc:publisher>
    <skos:inScheme rdf:resource="http://vocab.aodn.org.au/def/instrument/1" />
    <skos:scopeNote xml:lang="en">manufacturer:Sea-Bird Electronics Inc.</skos:scopeNote>
  </rdf:Description>
  <rdf:Description rdf:about="http://vocab.nerc.ac.uk/collection/L22/current/TOOL0018">
    <rdf:type rdf:resource="http://www.w3.org/2004/02/skos/core#Concept" />
    <skos:prefLabel xml:lang="en">Sea-Bird SBE 37-SMP MicroCAT C-T Sensor</skos:prefLabel>
    <dcterms:created rdf:datatype="http://www.w3.org/2001/XMLSchema#dateTime">2014-02-06T00:00:00Z</dcterms:created>
    <skos:definition xml:lang="en">The SBE 37 MicroCAT is a high accuracy conductivity and temperature recorder with an optional pressure sensor designed for depolyment on moorings. The SMP model has a serial interface plus internal flash memory data storage with an internal pump to improve conductivity response and protection against fouling.</skos:definition>
    <dc:source>(L221) SeaVoX Device Catalogue</dc:source>
    <dc:publisher>British Oceanographic Data Centre (BODC)</dc:publisher>
    <skos:inScheme rdf:resource="http://vocab.aodn.org.au/def/instrument/1" />
    <skos:scopeNote xml:lang="en">manufacturer:Sea-Bird Electronics Inc.</skos:scopeNote>
  </rdf:Description>
  <rdf:Description rdf:about="http://vocab.nerc.ac.uk/collection/L22/current/TOOL0058">
    <rdf:type rdf:resource="http://www.w3.org/2004/02/skos/core#Concept" />
    <skos:prefLabel xml:lang="en">Sea-Bird SBE 911plus CTD</skos:prefLabel>
    <skos:inScheme rdf:resource="http://vocab.aodn.org.au/def/instrument/1" />
    <dcterms:created rdf:datatype="http://www.w3.org/2001/XMLSchema#dateTime">2014-07-14T00:00:00Z</dcterms:created>
    <skos:definition xml:lang="en">High precision and accuracy CTD comprising an SBE 9plus underwater unit (SBE 3 temperature and SBE 4 conductivity sensors) and an SBE 11plus deck unit. Sensors may be connected to a pump-fed plastic tubing circuit (usually temperature, salinity and oxygen) or stand-alone. All instruments (8 channels available) on the package are logged by the SBE 11. The unit is the production off the shelf version of the SBE 911 (each 911 was custom built to individual specification).</skos:definition>
    <dc:source>(L221) SeaVoX Device Catalogue</dc:source>
    <dc:publisher>British Oceanographic Data Centre (BODC)</dc:publisher>
  </rdf:Description>
  <rdf:Description rdf:about="http://vocab.nerc.ac.uk/collection/L22/current/TOOL0054">
    <rdf:type rdf:resource="http://www.w3.org/2004/02/skos/core#Concept" />
    <skos:prefLabel xml:lang="en">RBR TDR-2050 underwater temperature logger</skos:prefLabel>
    <skos:inScheme rdf:resource="http://vocab.aodn.org.au/def/instrument/1" />
    <dcterms:created rdf:datatype="http://www.w3.org/2001/XMLSchema#dateTime">2014-02-06T00:00:00Z</dcterms:created>
    <skos:definition xml:lang="en">The TDR-2050 is a small (235mm x 38mm OD), self-contained, submersible temperature and depth recorder (sensors and data logger). It can be deployed for a period of up to three years and can collect more than 1,200,000 sets of samples. Data can be retained in memory for 20 years (even without batteries). Available in two casings, plastic and titanium, with depth ratings of 740m and 6600m respectively. The temperature channel of the TDR-2050 is calibrated to an accuracy of ± 0.002°C (ITS-90) over the range -5 to +35°C.  Typical drift has been measured to be 0.002°C per year. The thermistor may be external (&lt;3sec time constant) or internal (&lt;20sec time constant). A fast thermistor probe (0.095sec) is also available. The depth channel is calibrated to an accuracy of 0.05%fs  Ranges from 10m to 6,600m are available.</skos:definition>
    <dc:source>(L221) SeaVoX Device Catalogue</dc:source>
    <dc:publisher>British Oceanographic Data Centre (BODC)</dc:publisher>
    <skos:scopeNote xml:lang="en">manufacturer:RBR Ltd.</skos:scopeNote>
  </rdf:Description>
  <rdf:Description rdf:about="http://vocab.nerc.ac.uk/collection/L22/current/TOOL0053">
    <rdf:type rdf:resource="http://www.w3.org/2004/02/skos/core#Concept" />
    <skos:prefLabel xml:lang="en">RBR XR-420 CTD Marine</skos:prefLabel>
    <dcterms:created rdf:datatype="http://www.w3.org/2001/XMLSchema#dateTime">2014-02-17T00:00:00Z</dcterms:created>
    <skos:definition xml:lang="en">A small autonomous data logger designed to monitor conductivity, temperature and depth. Conductivity (accuracy ± 0.003 mS/cm) is measured using a 3-coil closed loop feedback inductive cell for superior temperature compensation. The thermistor (Themometrics) used to record temperature (accuracy ± 0.002°C) is aged and hermetically sealed in the tip of a shock resistant solid glass rod. Pressure (accuracy 0.05% full scale) sensors use reliable semiconductor technology and 316 stainless steel housing developed for long-term stability in harsh environments.</skos:definition>
    <dc:source>(L221) SeaVoX Device Catalogue</dc:source>
    <dc:publisher>British Oceanographic Data Centre (BODC)</dc:publisher>
    <skos:inScheme rdf:resource="http://vocab.aodn.org.au/def/instrument/1" />
    <skos:scopeNote xml:lang="en">manufacturer: RBR</skos:scopeNote>
  </rdf:Description>
  <rdf:Description rdf:about="http://vocab.nerc.ac.uk/collection/L22/current/TOOL0873/">
    <rdf:type rdf:resource="http://www.w3.org/2004/02/skos/core#Concept" />
    <skos:prefLabel xml:lang="en">SMRU GPS Satellite Relay Data Logger (Argos)</skos:prefLabel>
    <skos:altLabel xml:lang="en">SMRU GPS SRDL</skos:altLabel>
    <skos:inScheme rdf:resource="http://vocab.aodn.org.au/def/instrument/1" />
    <dcterms:created rdf:datatype="http://www.w3.org/2001/XMLSchema#dateTime">2015-06-03T00:00:00Z</dcterms:created>
    <skos:definition xml:lang="en">A package comprising a wet/dry, pressure and temperature sensors with a GPS receiver for high accuracy position data and antenna suitable for transmission of data via the Argos satellite system. The unit contains an internal battery and a microprocessor that logs data and schedules the transfer of data.  GPS locations are acquired in less than a second so position may be transferred to the satellite on every surfacing. The package is designed for attachment to marine mammals and has an operational depth range of down to 2000 m. More information is available at http://www.smru.st-and.ac.uk/Instrumentation/GPSArgosTag/.</skos:definition>
    <dc:publisher>British Oceanographic Data Centre (BODC)</dc:publisher>
    <dcterms:modified rdf:datatype="http://www.w3.org/2001/XMLSchema#dateTime">2015-07-01T01:19:54Z</dcterms:modified>
    <dcterms:contributor>Natalia_Atkins</dcterms:contributor>
  </rdf:Description>
  <rdf:Description rdf:about="http://vocab.nerc.ac.uk/collection/L05/current/65">
    <rdf:type rdf:resource="http://www.w3.org/2004/02/skos/core#Concept" />
    <skos:prefLabel xml:lang="en">gill nets</skos:prefLabel>
    <skos:topConceptOf rdf:resource="http://vocab.aodn.org.au/def/instrument/1" />
    <skos:inScheme rdf:resource="http://vocab.aodn.org.au/def/instrument/1" />
    <dcterms:created rdf:datatype="http://www.w3.org/2001/XMLSchema#dateTime">2014-05-22T00:00:00Z</dcterms:created>
    <skos:definition xml:lang="en">Nets drifting in the sea or standing on the sea floor in which fish become entangled usually through their gill covers.</skos:definition>
    <dc:source>(L051) SeaDataNet device categories</dc:source>
    <dc:publisher>British Oceanographic Data Centre (BODC)</dc:publisher>
  </rdf:Description>
  <rdf:Description rdf:about="http://vocab.nerc.ac.uk/collection/L05/current/64">
    <rdf:type rdf:resource="http://www.w3.org/2004/02/skos/core#Concept" />
    <skos:prefLabel xml:lang="en">active fishing gear</skos:prefLabel>
    <skos:topConceptOf rdf:resource="http://vocab.aodn.org.au/def/instrument/1" />
    <skos:inScheme rdf:resource="http://vocab.aodn.org.au/def/instrument/1" />
    <dcterms:created rdf:datatype="http://www.w3.org/2001/XMLSchema#dateTime">2014-05-22T00:00:00Z</dcterms:created>
    <skos:definition xml:lang="en">Apparatus where capture is based on chasing the target species (e.g. a trawl).</skos:definition>
    <dc:source>(L051) SeaDataNet device categories</dc:source>
    <dc:publisher>British Oceanographic Data Centre (BODC)</dc:publisher>
  </rdf:Description>
  <rdf:Description rdf:about="http://vocab.nerc.ac.uk/collection/L05/current/63">
    <rdf:type rdf:resource="http://www.w3.org/2004/02/skos/core#Concept" />
    <skos:prefLabel xml:lang="en">passive fishing gear</skos:prefLabel>
    <skos:topConceptOf rdf:resource="http://vocab.aodn.org.au/def/instrument/1" />
    <skos:inScheme rdf:resource="http://vocab.aodn.org.au/def/instrument/1" />
    <dcterms:created rdf:datatype="http://www.w3.org/2001/XMLSchema#dateTime">2014-05-22T00:00:00Z</dcterms:created>
    <skos:definition xml:lang="en">Apparatus where capture is based on the movement of the target species towards the gear (e.g. creels and fish traps).</skos:definition>
    <dc:source>(L051) SeaDataNet device categories</dc:source>
    <dc:publisher>British Oceanographic Data Centre (BODC)</dc:publisher>
  </rdf:Description>
  <rdf:Description rdf:about="http://vocab.nerc.ac.uk/collection/L05/current/LAB25">
    <rdf:type rdf:resource="http://www.w3.org/2004/02/skos/core#Concept" />
    <skos:prefLabel xml:lang="en">X-ray fluorescence analysers</skos:prefLabel>
    <skos:topConceptOf rdf:resource="http://vocab.aodn.org.au/def/instrument/1" />
    <skos:inScheme rdf:resource="http://vocab.aodn.org.au/def/instrument/1" />
    <dcterms:created rdf:datatype="http://www.w3.org/2001/XMLSchema#dateTime">2014-05-22T00:00:00Z</dcterms:created>
    <skos:definition xml:lang="en">Instruments that identify and quantify the elemental constituents of a sample from the spectrum of electromagnetic radiation emitted by the atoms in the sample when excited by X-ray radiation.</skos:definition>
    <dc:source>(L051) SeaDataNet device categories</dc:source>
    <dc:publisher>British Oceanographic Data Centre (BODC)</dc:publisher>
  </rdf:Description>
  <rdf:Description rdf:about="http://vocab.nerc.ac.uk/collection/L05/current/62">
    <rdf:type rdf:resource="http://www.w3.org/2004/02/skos/core#Concept" />
    <skos:prefLabel xml:lang="en">beam trawls</skos:prefLabel>
    <skos:topConceptOf rdf:resource="http://vocab.aodn.org.au/def/instrument/1" />
    <skos:inScheme rdf:resource="http://vocab.aodn.org.au/def/instrument/1" />
    <dcterms:created rdf:datatype="http://www.w3.org/2001/XMLSchema#dateTime">2014-05-22T00:00:00Z</dcterms:created>
    <skos:definition xml:lang="en">Nets towed over the sea floor having the horizontal net opening provided by a wooden or metal beam that disrupts the surface of the bed.</skos:definition>
    <dc:source>(L051) SeaDataNet device categories</dc:source>
    <dc:publisher>British Oceanographic Data Centre (BODC)</dc:publisher>
  </rdf:Description>
  <rdf:Description rdf:about="http://vocab.nerc.ac.uk/collection/L05/current/61">
    <rdf:type rdf:resource="http://www.w3.org/2004/02/skos/core#Concept" />
    <skos:prefLabel xml:lang="en">demersal trawl nets</skos:prefLabel>
    <skos:topConceptOf rdf:resource="http://vocab.aodn.org.au/def/instrument/1" />
    <skos:inScheme rdf:resource="http://vocab.aodn.org.au/def/instrument/1" />
    <dcterms:created rdf:datatype="http://www.w3.org/2001/XMLSchema#dateTime">2014-05-22T00:00:00Z</dcterms:created>
    <skos:definition xml:lang="en">Nets towed over the sea floor designed to sample species living on or near the bottom.</skos:definition>
    <dc:source>(L051) SeaDataNet device categories</dc:source>
    <dc:publisher>British Oceanographic Data Centre (BODC)</dc:publisher>
  </rdf:Description>
  <rdf:Description rdf:about="http://vocab.nerc.ac.uk/collection/L05/current/60">
    <rdf:type rdf:resource="http://www.w3.org/2004/02/skos/core#Concept" />
    <skos:prefLabel xml:lang="en">sediment dredges</skos:prefLabel>
    <skos:topConceptOf rdf:resource="http://vocab.aodn.org.au/def/instrument/1" />
    <skos:inScheme rdf:resource="http://vocab.aodn.org.au/def/instrument/1" />
    <dcterms:created rdf:datatype="http://www.w3.org/2001/XMLSchema#dateTime">2014-05-22T00:00:00Z</dcterms:created>
    <skos:definition xml:lang="en">Bucket-like containers hauled over the sea bed collecting integrated samples of surface sediment along a segment of ship track.</skos:definition>
    <dc:source>(L051) SeaDataNet device categories</dc:source>
    <dc:publisher>British Oceanographic Data Centre (BODC)</dc:publisher>
  </rdf:Description>
  <rdf:Description rdf:about="http://vocab.nerc.ac.uk/collection/L05/current/LAB22">
    <rdf:type rdf:resource="http://www.w3.org/2004/02/skos/core#Concept" />
    <skos:prefLabel xml:lang="en">gamma-ray spectrometers</skos:prefLabel>
    <skos:topConceptOf rdf:resource="http://vocab.aodn.org.au/def/instrument/1" />
    <skos:inScheme rdf:resource="http://vocab.aodn.org.au/def/instrument/1" />
    <dcterms:created rdf:datatype="http://www.w3.org/2001/XMLSchema#dateTime">2014-05-22T00:00:00Z</dcterms:created>
    <skos:definition xml:lang="en">Instruments measuring the relative levels of electromagnetic radiation of different wavelengths in the gamma-ray waveband.</skos:definition>
    <dc:source>(L051) SeaDataNet device categories</dc:source>
    <dc:publisher>British Oceanographic Data Centre (BODC)</dc:publisher>
  </rdf:Description>
  <rdf:Description rdf:about="http://vocab.nerc.ac.uk/collection/L05/current/69">
    <rdf:type rdf:resource="http://www.w3.org/2004/02/skos/core#Concept" />
    <skos:prefLabel xml:lang="en">neuston net</skos:prefLabel>
    <skos:topConceptOf rdf:resource="http://vocab.aodn.org.au/def/instrument/1" />
    <skos:inScheme rdf:resource="http://vocab.aodn.org.au/def/instrument/1" />
    <dcterms:created rdf:datatype="http://www.w3.org/2001/XMLSchema#dateTime">2014-05-22T00:00:00Z</dcterms:created>
    <skos:definition xml:lang="en">A fine-meshed net designed to collect samples living within a few centimetres of the sea surface. Samples microzooplankton mesozooplankton and nekton.</skos:definition>
    <dc:source>(L051) SeaDataNet device categories</dc:source>
    <dc:publisher>British Oceanographic Data Centre (BODC)</dc:publisher>
  </rdf:Description>
  <rdf:Description rdf:about="http://vocab.nerc.ac.uk/collection/L05/current/68">
    <rdf:type rdf:resource="http://www.w3.org/2004/02/skos/core#Concept" />
    <skos:prefLabel xml:lang="en">multinet</skos:prefLabel>
    <skos:topConceptOf rdf:resource="http://vocab.aodn.org.au/def/instrument/1" />
    <skos:inScheme rdf:resource="http://vocab.aodn.org.au/def/instrument/1" />
    <dcterms:created rdf:datatype="http://www.w3.org/2001/XMLSchema#dateTime">2014-05-22T00:00:00Z</dcterms:created>
    <skos:definition xml:lang="en">A system comprising several nets that can be opened and closed sequentially to collect a series of samples during a tow or haul. Samples microzooplankton mesozooplankton and nekton.</skos:definition>
    <dc:source>(L051) SeaDataNet device categories</dc:source>
    <dc:publisher>British Oceanographic Data Centre (BODC)</dc:publisher>
  </rdf:Description>
  <rdf:Description rdf:about="http://vocab.nerc.ac.uk/collection/L05/current/LAB20">
    <rdf:type rdf:resource="http://www.w3.org/2004/02/skos/core#Concept" />
    <skos:prefLabel xml:lang="en">spectrophotometers</skos:prefLabel>
    <skos:topConceptOf rdf:resource="http://vocab.aodn.org.au/def/instrument/1" />
    <skos:inScheme rdf:resource="http://vocab.aodn.org.au/def/instrument/1" />
    <dcterms:created rdf:datatype="http://www.w3.org/2001/XMLSchema#dateTime">2014-05-22T00:00:00Z</dcterms:created>
    <skos:definition xml:lang="en">Instruments measuring the relative absorption of electromagnetic radiation of different wavelengths in the near infra-red visible and ultraviolet wavebands by samples.</skos:definition>
    <dc:source>(L051) SeaDataNet device categories</dc:source>
    <dc:publisher>British Oceanographic Data Centre (BODC)</dc:publisher>
  </rdf:Description>
  <rdf:Description rdf:about="http://vocab.nerc.ac.uk/collection/L05/current/LAB21">
    <rdf:type rdf:resource="http://www.w3.org/2004/02/skos/core#Concept" />
    <skos:prefLabel xml:lang="en">liquid scintillation counters</skos:prefLabel>
    <skos:topConceptOf rdf:resource="http://vocab.aodn.org.au/def/instrument/1" />
    <skos:inScheme rdf:resource="http://vocab.aodn.org.au/def/instrument/1" />
    <dcterms:created rdf:datatype="http://www.w3.org/2001/XMLSchema#dateTime">2014-05-22T00:00:00Z</dcterms:created>
    <skos:definition xml:lang="en">Instruments assaying beta radiation by quantitative detection of visible light produced by the passage of rays or particles through a suitable scintillant incorporated into the sample.</skos:definition>
    <dc:source>(L051) SeaDataNet device categories</dc:source>
    <dc:publisher>British Oceanographic Data Centre (BODC)</dc:publisher>
  </rdf:Description>
  <rdf:Description rdf:about="http://vocab.nerc.ac.uk/collection/L05/current/WPS">
    <rdf:type rdf:resource="http://www.w3.org/2004/02/skos/core#Concept" />
    <skos:prefLabel xml:lang="en">water pressure sensors</skos:prefLabel>
    <skos:altLabel xml:lang="en" />
    <skos:inScheme rdf:resource="http://vocab.aodn.org.au/def/instrument/1" />
    <dcterms:created rdf:datatype="http://www.w3.org/2001/XMLSchema#dateTime">2015-06-03T00:00:00Z</dcterms:created>
    <skos:definition xml:lang="en">Sensors measuring hydrostatic pressure that are capable of withstanding the physical demands made by in-situ measurements in water bodies. Depending upon the mode of deployment they may measure sea level, waves, mooring performance or the depth of a profiling instrument.</skos:definition>
    <dc:publisher>British Oceanographic Data Centre (BODC)</dc:publisher>
    <skos:narrower rdf:resource="http://vocab.nerc.ac.uk/collection/L22/current/TOOL0873/" />
  </rdf:Description>
  <rdf:Description rdf:about="http://vocab.nerc.ac.uk/collection/L22/current/TOOL0873/">
    <rdf:type rdf:resource="http://www.w3.org/2004/02/skos/core#Concept" />
    <skos:prefLabel xml:lang="en">SMRU GPS Satellite Relay Data Logger (Argos)</skos:prefLabel>
    <skos:altLabel xml:lang="en">SMRU GPS SRDL</skos:altLabel>
    <skos:inScheme rdf:resource="http://vocab.aodn.org.au/def/instrument/1" />
    <dcterms:created rdf:datatype="http://www.w3.org/2001/XMLSchema#dateTime">2015-06-03T00:00:00Z</dcterms:created>
    <skos:definition xml:lang="en">A package comprising a wet/dry, pressure and temperature sensors with a GPS receiver for high accuracy position data and antenna suitable for transmission of data via the Argos satellite system. The unit contains an internal battery and a microprocessor that logs data and schedules the transfer of data.  GPS locations are acquired in less than a second so position may be transferred to the satellite on every surfacing. The package is designed for attachment to marine mammals and has an operational depth range of down to 2000 m. More information is available at http://www.smru.st-and.ac.uk/Instrumentation/GPSArgosTag/.</skos:definition>
    <dc:publisher>British Oceanographic Data Centre (BODC)</dc:publisher>
    <dcterms:modified rdf:datatype="http://www.w3.org/2001/XMLSchema#dateTime">2015-07-01T01:19:54Z</dcterms:modified>
    <dcterms:contributor>Natalia_Atkins</dcterms:contributor>
  </rdf:Description>
  <rdf:Description rdf:about="http://vocab.nerc.ac.uk/collection/L05/current/101">
    <rdf:type rdf:resource="http://www.w3.org/2004/02/skos/core#Concept" />
    <skos:prefLabel xml:lang="en">anemometers</skos:prefLabel>
    <skos:topConceptOf rdf:resource="http://vocab.aodn.org.au/def/instrument/1" />
    <skos:inScheme rdf:resource="http://vocab.aodn.org.au/def/instrument/1" />
    <dcterms:created rdf:datatype="http://www.w3.org/2001/XMLSchema#dateTime">2013-03-28T00:00:00Z</dcterms:created>
    <skos:definition xml:lang="en">Instrument that measures wind speed and direction at a single elevation</skos:definition>
    <dc:source>(L051) SeaDataNet device categories</dc:source>
    <dc:publisher>British Oceanographic Data Centre (BODC)</dc:publisher>
    <dcterms:contributor>Natalia_Atkins</dcterms:contributor>
    <skos:narrower rdf:resource="http://vocab.nerc.ac.uk/collection/L22/current/TOOL0126" />
    <skos:narrower rdf:resource="http://vocab.nerc.ac.uk/collection/L22/current/TOOL0127" />
    <skos:narrower rdf:resource="http://vocab.nerc.ac.uk/collection/L22/current/TOOL0195" />
    <skos:narrower rdf:resource="http://vocab.nerc.ac.uk/collection/L22/current/TOOL0260" />
    <skos:narrower rdf:resource="http://vocab.nerc.ac.uk/collection/L22/current/TOOL0704" />
    <skos:narrower rdf:resource="http://vocab.nerc.ac.uk/collection/L22/current/TOOL0877/" />
    <dcterms:modified rdf:datatype="http://www.w3.org/2001/XMLSchema#dateTime">2015-06-30T03:57:19Z</dcterms:modified>
  </rdf:Description>
  <rdf:Description rdf:about="http://vocab.nerc.ac.uk/collection/L22/current/TOOL0195">
    <rdf:type rdf:resource="http://www.w3.org/2004/02/skos/core#Concept" />
    <skos:prefLabel xml:lang="en">Young MA05106 Wind Monitor anemometer</skos:prefLabel>
    <skos:inScheme rdf:resource="http://vocab.aodn.org.au/def/instrument/1" />
    <dcterms:created rdf:datatype="http://www.w3.org/2001/XMLSchema#dateTime">2013-10-11T00:00:00Z</dcterms:created>
    <skos:definition xml:lang="en">A lightweight anemometer with a helicoid propellor speed sensor attached to a vane. The instrument is designed to withstand the marine environment.</skos:definition>
    <dc:source>(L221) SeaVoX Device Catalogue</dc:source>
    <dc:publisher>British Oceanographic Data Centre (BODC)</dc:publisher>
    <skos:scopeNote xml:lang="en">manufacturer:R.M. Young Company</skos:scopeNote>
  </rdf:Description>
  <rdf:Description rdf:about="http://vocab.nerc.ac.uk/collection/L22/current/TOOL0877/">
    <rdf:type rdf:resource="http://www.w3.org/2004/02/skos/core#Concept" />
    <skos:prefLabel xml:lang="en">Vaisala WAA15A cup anemometer</skos:prefLabel>
    <skos:altLabel xml:lang="en">Vaisala WAA15A anemometer</skos:altLabel>
    <skos:inScheme rdf:resource="http://vocab.aodn.org.au/def/instrument/1" />
    <dcterms:created rdf:datatype="http://www.w3.org/2001/XMLSchema#dateTime">2015-06-03T00:00:00Z</dcterms:created>
    <skos:definition xml:lang="en">Three lightweight, conical cups mounted on the cup wheel providing linearity with windspeeds up to 75m/s. Rotation speed is measured by a disk attached to the shaft cutting an infrared light beam 14 times per revolution producing pulses counted by a phototransistor. The output rate is directly proportional to wind speed. It was replaced by the WAA151 model which introduced a number of improvements such as plug-and-play design, an improved mechanical shaft attachment and addition of electrical lightning protection. Both models have the same output, mounting and wiring scheme and so are totally interchangeable.</skos:definition>
    <dc:publisher>British Oceanographic Data Centre (BODC)</dc:publisher>
  </rdf:Description>
  <rdf:Description rdf:about="http://vocab.nerc.ac.uk/collection/L22/current/TOOL0260">
    <rdf:type rdf:resource="http://www.w3.org/2004/02/skos/core#Concept" />
    <skos:prefLabel xml:lang="en">Young MA05103 Wind Monitor anemometer</skos:prefLabel>
    <skos:inScheme rdf:resource="http://vocab.aodn.org.au/def/instrument/1" />
    <dcterms:created rdf:datatype="http://www.w3.org/2001/XMLSchema#dateTime">2013-10-11T00:00:00Z</dcterms:created>
    <skos:definition xml:lang="en">An anemometer with a four blade helicoid propeller and lightweight direction vane. Vane angle is sensed by a precision potentiometer. The instrument body is UV stabilized plastic with stainless steel and anodized aluminum fittings. The instrument mounts on standard 1 inch pipe. Windspeed accuracy is +-0.3m/s and wind direction accuracy is 3 degrees.</skos:definition>
    <dc:source>(L221) SeaVoX Device Catalogue</dc:source>
    <dc:publisher>British Oceanographic Data Centre (BODC)</dc:publisher>
    <skos:scopeNote xml:lang="en">manufacturer:R.M. Young Company</skos:scopeNote>
  </rdf:Description>
  <rdf:Description rdf:about="http://vocab.nerc.ac.uk/collection/L22/current/TOOL0127">
    <rdf:type rdf:resource="http://www.w3.org/2004/02/skos/core#Concept" />
    <skos:prefLabel xml:lang="en">Vaisala WAV151 wind vane</skos:prefLabel>
    <skos:inScheme rdf:resource="http://vocab.aodn.org.au/def/instrument/1" />
    <dcterms:created rdf:datatype="http://www.w3.org/2001/XMLSchema#dateTime">2013-10-11T00:00:00Z</dcterms:created>
    <skos:definition xml:lang="en">A counter-balanced, low-threshold, optoelectic wind-vane. Infrared LEDs and phototransistors are mounted on six orbits on each side of a 6-bit GRAY-coded disc. Turning the vane causes the disc to change the code received by the phototransistors.</skos:definition>
    <dc:source>(L221) SeaVoX Device Catalogue</dc:source>
    <dc:publisher>British Oceanographic Data Centre (BODC)</dc:publisher>
    <skos:scopeNote xml:lang="en">manufacturer:Vaisala</skos:scopeNote>
  </rdf:Description>
  <rdf:Description rdf:about="http://vocab.nerc.ac.uk/collection/L22/current/TOOL0126">
    <rdf:type rdf:resource="http://www.w3.org/2004/02/skos/core#Concept" />
    <skos:prefLabel xml:lang="en">Vaisala WAA151 cup anemometer</skos:prefLabel>
    <skos:inScheme rdf:resource="http://vocab.aodn.org.au/def/instrument/1" />
    <dcterms:created rdf:datatype="http://www.w3.org/2001/XMLSchema#dateTime">2013-10-11T00:00:00Z</dcterms:created>
    <skos:definition xml:lang="en">Three lightweight, conical cups mounted on the cup wheel providing linearity with windspeeds up to 75m/s. Rotation speed is measured by a disk attached to the shaft cutting an infrared light beam 14 times per revolution producing pulses counted by a phototransistor. The output rate is directly proportional to wind speed.</skos:definition>
    <dc:source>(L221) SeaVoX Device Catalogue</dc:source>
    <dc:publisher>British Oceanographic Data Centre (BODC)</dc:publisher>
    <skos:scopeNote xml:lang="en">manufacturer:Vaisala</skos:scopeNote>
  </rdf:Description>
  <rdf:Description rdf:about="http://vocab.nerc.ac.uk/collection/L22/current/TOOL0704">
    <rdf:type rdf:resource="http://www.w3.org/2004/02/skos/core#Concept" />
    <skos:prefLabel xml:lang="en">Gill Instruments WindObserver II Anemometer</skos:prefLabel>
    <skos:inScheme rdf:resource="http://vocab.aodn.org.au/def/instrument/1" />
    <dcterms:created rdf:datatype="http://www.w3.org/2001/XMLSchema#dateTime">2013-10-11T00:00:00Z</dcterms:created>
    <skos:definition xml:lang="en">The WindObserver II is a solid state ultrasonic anemometer, with a stainless steel housing suitable for marine and offshore applications. It measures wind speed and direction over ranges of 0-65 m/s and 0-359 degrees respectively.</skos:definition>
    <dc:source>(L221) SeaVoX Device Catalogue</dc:source>
    <dc:publisher>British Oceanographic Data Centre (BODC)</dc:publisher>
    <skos:scopeNote xml:lang="en">manufacturer:Gill Instruments</skos:scopeNote>
  </rdf:Description>
  <rdf:Description rdf:about="http://vocab.nerc.ac.uk/collection/L05/current/30">
    <rdf:type rdf:resource="http://www.w3.org/2004/02/skos/core#Concept" />
    <skos:prefLabel xml:lang="en">discrete water samplers</skos:prefLabel>
    <skos:topConceptOf rdf:resource="http://vocab.aodn.org.au/def/instrument/1" />
    <skos:inScheme rdf:resource="http://vocab.aodn.org.au/def/instrument/1" />
    <dcterms:created rdf:datatype="http://www.w3.org/2001/XMLSchema#dateTime">2013-03-28T00:00:00Z</dcterms:created>
    <skos:definition xml:lang="en">A device that collects an in-situ discrete water sample from any depth and returns it to the surface without contamination by the waters through which it passes such as a water bottle</skos:definition>
    <dc:source>(L051) SeaDataNet device categories</dc:source>
    <dc:publisher>British Oceanographic Data Centre (BODC)</dc:publisher>
  </rdf:Description>
  <rdf:Description rdf:about="http://vocab.nerc.ac.uk/collection/L05/current/103">
    <rdf:type rdf:resource="http://www.w3.org/2004/02/skos/core#Concept" />
    <skos:prefLabel xml:lang="en">radiosondes</skos:prefLabel>
    <skos:topConceptOf rdf:resource="http://vocab.aodn.org.au/def/instrument/1" />
    <skos:inScheme rdf:resource="http://vocab.aodn.org.au/def/instrument/1" />
    <dcterms:created rdf:datatype="http://www.w3.org/2001/XMLSchema#dateTime">2014-05-22T00:00:00Z</dcterms:created>
    <skos:definition xml:lang="en">A balloon-borne package equipped with a radio transmitter and meteorological sensors typically measuring temperature pressure and humidity.</skos:definition>
    <dc:source>(L051) SeaDataNet device categories</dc:source>
    <dc:publisher>British Oceanographic Data Centre (BODC)</dc:publisher>
  </rdf:Description>
  <rdf:Description rdf:about="http://vocab.nerc.ac.uk/collection/L05/current/369">
    <rdf:type rdf:resource="http://www.w3.org/2004/02/skos/core#Concept" />
    <skos:prefLabel xml:lang="en">hydrophones</skos:prefLabel>
    <skos:topConceptOf rdf:resource="http://vocab.aodn.org.au/def/instrument/1" />
    <skos:inScheme rdf:resource="http://vocab.aodn.org.au/def/instrument/1" />
    <dcterms:created rdf:datatype="http://www.w3.org/2001/XMLSchema#dateTime">2013-03-28T00:00:00Z</dcterms:created>
    <skos:definition xml:lang="en">Devices containing transducers that convert underwater sound waves into electrical signals.</skos:definition>
    <dc:source>(L051) SeaDataNet device categories</dc:source>
    <dc:publisher>British Oceanographic Data Centre (BODC)</dc:publisher>
    <skos:narrower rdf:resource="http://vocab.nerc.ac.uk/collection/L22/current/TOOL0663" />
  </rdf:Description>
  <rdf:Description rdf:about="http://vocab.nerc.ac.uk/collection/L22/current/TOOL0663">
    <rdf:type rdf:resource="http://www.w3.org/2004/02/skos/core#Concept" />
    <skos:prefLabel xml:lang="en">CMST-DSTO underwater sound recorder</skos:prefLabel>
    <skos:inScheme rdf:resource="http://vocab.aodn.org.au/def/instrument/1" />
    <dcterms:created rdf:datatype="http://www.w3.org/2001/XMLSchema#dateTime">2014-02-11T00:00:00Z</dcterms:created>
    <skos:definition xml:lang="en">Instrument that contains a hydrophone plus a data logger in a deep-water housing designed for long-term monitoring of underwater noise. It can be deployed for periods of up to two years. Sampling frequency and schedule (including burst recording) may be programmed. More information at http://cmst.curtin.edu.au/products/usr.cfm.</skos:definition>
    <dc:source>(L221) SeaVoX Device Catalogue</dc:source>
    <dc:publisher>British Oceanographic Data Centre (BODC)</dc:publisher>
    <skos:scopeNote xml:lang="en">manufacturer:CMST</skos:scopeNote>
  </rdf:Description>
  <rdf:Description rdf:about="http://vocab.nerc.ac.uk/collection/L05/current/31">
    <rdf:type rdf:resource="http://www.w3.org/2004/02/skos/core#Concept" />
    <skos:prefLabel xml:lang="en">continuous water samplers</skos:prefLabel>
    <skos:topConceptOf rdf:resource="http://vocab.aodn.org.au/def/instrument/1" />
    <skos:inScheme rdf:resource="http://vocab.aodn.org.au/def/instrument/1" />
    <dcterms:created rdf:datatype="http://www.w3.org/2001/XMLSchema#dateTime">2013-03-28T00:00:00Z</dcterms:created>
    <skos:definition xml:lang="en">A device that continuously supplies a flow of water either to an analytical instrument over a sensor or from which samples may be drawn</skos:definition>
    <dc:source>(L051) SeaDataNet device categories</dc:source>
    <dc:publisher>British Oceanographic Data Centre (BODC)</dc:publisher>
  </rdf:Description>
  <rdf:Description rdf:about="http://vocab.nerc.ac.uk/collection/L05/current/102">
    <rdf:type rdf:resource="http://www.w3.org/2004/02/skos/core#Concept" />
    <skos:prefLabel xml:lang="en">meteorological packages</skos:prefLabel>
    <skos:topConceptOf rdf:resource="http://vocab.aodn.org.au/def/instrument/1" />
    <skos:inScheme rdf:resource="http://vocab.aodn.org.au/def/instrument/1" />
    <dcterms:created rdf:datatype="http://www.w3.org/2001/XMLSchema#dateTime">2013-03-28T00:00:00Z</dcterms:created>
    <skos:definition xml:lang="en">Instrument that makes routine meteorological measurements on the atmosphere typically air pressure temperature and humidity</skos:definition>
    <dc:source>(L051) SeaDataNet device categories</dc:source>
    <dc:publisher>British Oceanographic Data Centre (BODC)</dc:publisher>
    <skos:narrower rdf:resource="http://vocab.nerc.ac.uk/collection/L22/current/TOOL0780" />
    <skos:narrower rdf:resource="http://vocab.nerc.ac.uk/collection/L22/current/TOOL0779" />
    <skos:narrower rdf:resource="http://vocab.nerc.ac.uk/collection/L22/current/TOOL0808" />
    <skos:narrower rdf:resource="http://vocab.nerc.ac.uk/collection/L22/current/TOOL0081" />
    <skos:narrower rdf:resource="http://vocab.nerc.ac.uk/collection/L22/current/TOOL0617" />
    <skos:narrower rdf:resource="http://vocab.nerc.ac.uk/collection/L22/current/TOOL0672" />
    <skos:narrower rdf:resource="http://vocab.nerc.ac.uk/collection/L22/current/TOOL0677" />
    <skos:narrower rdf:resource="http://vocab.nerc.ac.uk/collection/L22/current/TOOL0680" />
    <skos:narrower rdf:resource="http://vocab.nerc.ac.uk/collection/L22/current/TOOL0682" />
    <skos:narrower rdf:resource="http://vocab.nerc.ac.uk/collection/L22/current/TOOL0683" />
    <skos:narrower rdf:resource="http://vocab.nerc.ac.uk/collection/L22/current/TOOL0726" />
    <skos:narrower rdf:resource="http://vocab.nerc.ac.uk/collection/L22/current/TOOL0727" />
    <skos:narrower rdf:resource="http://vocab.nerc.ac.uk/collection/L22/current/TOOL0741" />
  </rdf:Description>
  <rdf:Description rdf:about="http://vocab.nerc.ac.uk/collection/L22/current/TOOL0741">
    <rdf:type rdf:resource="http://www.w3.org/2004/02/skos/core#Concept" />
    <skos:prefLabel xml:lang="en">Vaisala PTU300 Pressure, Humidity and Temperature Transmitter</skos:prefLabel>
    <skos:inScheme rdf:resource="http://vocab.aodn.org.au/def/instrument/1" />
    <dcterms:created rdf:datatype="http://www.w3.org/2001/XMLSchema#dateTime">2013-10-11T00:00:00Z</dcterms:created>
    <skos:definition xml:lang="en">The Vaisala PTU300 is a series of air pressure, humidity and temperature transmitters comprising a base station and sensors that may be attached directly or on a remote probe suited to the application. The probes are designed for installation in various environments: PTU301 for laboratories, PTU303 for general use and PTU307 for outdoor and meteorological applications (warmed probe). All incorporate the Vaisala BAROCAP pressure sensor, a thermistor and the Vaisala HUMICAP humidity sensor giving pressure accurate to 0.1-0.3 hPa (depends upon sensor class), temperature accurate to 0.2C and humidity accurate to 1%. The base station includes a graphical display giving continuous digital readout and keypad for operation control. Depending upon the options selected data may be logged internally (up 4 years) or transmitted via wired LAN, wireless LAN, USB, RS232 or RS485. More information is available at http://www.vaisala.com/Vaisala%20Documents/Brochures%20and%20Datasheets/CEN-TIA-G-PTU300-Combined-Brochure-B210954EN-E-LOW-v6.pdf.</skos:definition>
    <dc:source>(L221) SeaVoX Device Catalogue</dc:source>
    <dc:publisher>British Oceanographic Data Centre (BODC)</dc:publisher>
    <skos:scopeNote xml:lang="en">manufacturer:Vaisala</skos:scopeNote>
  </rdf:Description>
  <rdf:Description rdf:about="http://vocab.nerc.ac.uk/collection/L22/current/TOOL0780">
    <rdf:type rdf:resource="http://www.w3.org/2004/02/skos/core#Concept" />
    <skos:prefLabel xml:lang="en">Vaisala PA 11 digital barometer</skos:prefLabel>
    <skos:inScheme rdf:resource="http://vocab.aodn.org.au/def/instrument/1" />
    <dcterms:created rdf:datatype="http://www.w3.org/2001/XMLSchema#dateTime">2013-10-11T00:00:00Z</dcterms:created>
    <skos:definition xml:lang="en">An aviation quality digital barometer providing accurate and reliable pressure measurement over the range of 800 to 1050 mb.It had a unique construction consisting of three independently operating sensors controlled by a microprocessor. Triple redundancy ensured excellent long-term stability and measurement accuracy. Short term accuracy was determined by WMO as about 0.2 hPa and long-term accuracy (over approximately a year) was determined as approximately 0.35 hPa or 0.45 hPa if subjected to temperature variations in excess of 20C.</skos:definition>
    <dc:source>(L221) SeaVoX Device Catalogue</dc:source>
    <dc:publisher>British Oceanographic Data Centre (BODC)</dc:publisher>
    <skos:scopeNote xml:lang="en">manufacturer:Vaisala</skos:scopeNote>
  </rdf:Description>
  <rdf:Description rdf:about="http://vocab.nerc.ac.uk/collection/L22/current/TOOL0617">
    <rdf:type rdf:resource="http://www.w3.org/2004/02/skos/core#Concept" />
    <skos:prefLabel xml:lang="en">Rotronic Instruments MP1xxA humidity and temperature probe series</skos:prefLabel>
    <skos:inScheme rdf:resource="http://vocab.aodn.org.au/def/instrument/1" />
    <dcterms:created rdf:datatype="http://www.w3.org/2001/XMLSchema#dateTime">2014-02-07T00:00:00Z</dcterms:created>
    <skos:definition xml:lang="en">An analogue, linear response atmospheric humidity and temperature probe. The instrument operates within 0-100 percent relative humidity (0 to 1 volts), with an accuracy of +/-1 percent. The temperature range varies between -40 to 60 degC (-0.4 to 0.6 volts) definal on the specific model and has an accuracy of +/-0.3 degC.</skos:definition>
    <dc:source>(L221) SeaVoX Device Catalogue</dc:source>
    <dc:publisher>British Oceanographic Data Centre (BODC)</dc:publisher>
    <skos:scopeNote xml:lang="en">manufacturer:Rotronic Instrument Corp.</skos:scopeNote>
  </rdf:Description>
  <rdf:Description rdf:about="http://vocab.nerc.ac.uk/collection/L22/current/TOOL0808">
    <rdf:type rdf:resource="http://www.w3.org/2004/02/skos/core#Concept" />
    <skos:prefLabel xml:lang="en">Rosemount ST2401 temperature probe</skos:prefLabel>
    <skos:inScheme rdf:resource="http://vocab.aodn.org.au/def/instrument/1" />
    <dcterms:created rdf:datatype="http://www.w3.org/2001/XMLSchema#dateTime">2013-10-11T00:00:00Z</dcterms:created>
    <skos:definition xml:lang="en">A platinum resistor thermometer with a serial interface primarily used for air temperature measurements in meteorological packages but also used as a shipboard hull thermometer.</skos:definition>
    <dc:source>(L221) SeaVoX Device Catalogue</dc:source>
    <dc:publisher>British Oceanographic Data Centre (BODC)</dc:publisher>
    <skos:scopeNote xml:lang="en">manufacturer:Emerson Electric Co.</skos:scopeNote>
  </rdf:Description>
  <rdf:Description rdf:about="http://vocab.nerc.ac.uk/collection/L22/current/TOOL0677">
    <rdf:type rdf:resource="http://www.w3.org/2004/02/skos/core#Concept" />
    <skos:prefLabel xml:lang="en">Vaisala HMT330 temperature and humidity transmitter</skos:prefLabel>
    <skos:inScheme rdf:resource="http://vocab.aodn.org.au/def/instrument/1" />
    <dcterms:created rdf:datatype="http://www.w3.org/2001/XMLSchema#dateTime">2013-10-14T00:00:00Z</dcterms:created>
    <skos:definition xml:lang="en">The Vaisala HMT330 is a series of humidity and temperature transmitters comprising a base station and sensors that may be attached directly or on a remote probe suited to the application. The probes are designed for installation in various environments: HMT331 for wall mounting, HMT333 for duct mounting and tight spaces, HMT334 for high pressures up to 100 bar and vacuum conditions, HMT335 for high temperature, HMT337 for high humidity and meteorological applications and HMT338 for pressurized pipelines up to 40 bar. All incorporate a thermistor and the Vaisala HUMICAP humidity sensor giving temperature accurate to 0.2C and humidity accurate to 1%. The base station includes a graphical display giving continuous digital readout and keypad for operation control. Definal upon the options selected data may be logged internally (up 4 years) or transmitted via wired LAN, wireless LAN, USB, RS232 or RS485. More information is available at http://www.vaisala.com/en/products/humidity/Pages/HMT330.aspx.</skos:definition>
    <dc:source>(L221) SeaVoX Device Catalogue</dc:source>
    <dc:publisher>British Oceanographic Data Centre (BODC)</dc:publisher>
    <skos:scopeNote xml:lang="en">manufacturer:Vaisala</skos:scopeNote>
  </rdf:Description>
  <rdf:Description rdf:about="http://vocab.nerc.ac.uk/collection/L22/current/TOOL0727">
    <rdf:type rdf:resource="http://www.w3.org/2004/02/skos/core#Concept" />
    <skos:prefLabel xml:lang="en">Pico Technologies PT-104 Platinum Resistance Data Logger</skos:prefLabel>
    <skos:inScheme rdf:resource="http://vocab.aodn.org.au/def/instrument/1" />
    <dcterms:created rdf:datatype="http://www.w3.org/2001/XMLSchema#dateTime">2013-10-15T00:00:00Z</dcterms:created>
    <skos:definition xml:lang="en">The Pico Technologies Pt104 is a four-channel temperature measuring data logger. It measures temperatures in the range -200 to 800 degC, with accuracy of 0.015degC plus 0.01% of reading, and resolution of 0.001 degC.</skos:definition>
    <dc:source>(L221) SeaVoX Device Catalogue</dc:source>
    <dc:publisher>British Oceanographic Data Centre (BODC)</dc:publisher>
    <skos:scopeNote xml:lang="en">manufacturer:Pico Technology</skos:scopeNote>
  </rdf:Description>
  <rdf:Description rdf:about="http://vocab.nerc.ac.uk/collection/L22/current/TOOL0081">
    <rdf:type rdf:resource="http://www.w3.org/2004/02/skos/core#Concept" />
    <skos:prefLabel xml:lang="en">Vaisala HMP temperature and humidity sensor</skos:prefLabel>
    <skos:inScheme rdf:resource="http://vocab.aodn.org.au/def/instrument/1" />
    <dcterms:created rdf:datatype="http://www.w3.org/2001/XMLSchema#dateTime">2013-10-11T00:00:00Z</dcterms:created>
    <skos:definition xml:lang="en">A family of sensors and instruments (sensors plus integral displays or loggers) for the measurement of air temperature and relative humidity. All are based on a probe containing a patent (HUMICAP) capacitive thin film polymer humidity sensor and a Pt100 platinum resistance thermometer. The probes are available with a wide range of packaging, cabling and interface options all of which have designations of the form HMPnn such as HMP45 and HMP75. Vaisala sensors are incorporated into weather stations and marketed by Campbell Scientific.</skos:definition>
    <dc:source>(L221) SeaVoX Device Catalogue</dc:source>
    <dc:publisher>British Oceanographic Data Centre (BODC)</dc:publisher>
    <skos:scopeNote xml:lang="en">manufacturer:Vaisala</skos:scopeNote>
  </rdf:Description>
  <rdf:Description rdf:about="http://vocab.nerc.ac.uk/collection/L22/current/TOOL0726">
    <rdf:type rdf:resource="http://www.w3.org/2004/02/skos/core#Concept" />
    <skos:prefLabel xml:lang="en">OSi OWI-430 DSP-WIVIS Present Weather and Visibility Sensor</skos:prefLabel>
    <skos:inScheme rdf:resource="http://vocab.aodn.org.au/def/instrument/1" />
    <dcterms:created rdf:datatype="http://www.w3.org/2001/XMLSchema#dateTime">2013-10-14T00:00:00Z</dcterms:created>
    <skos:definition xml:lang="en">The Osi OWI-430 WIVIS is an optical weather and visibility sensor that measures visibility, rain, snow, drizzle, freezing and mixed precipitation conditions. It measures rain in dynamic range 0.1 to 3000 mm/hr; snow in dynamic range 0.01 to 300 mm/hr; visibility in dynamic range 0.001 to 10 km. It is designed to operate in temperatures from -40 to 50 degC, and humidity from 0 to 100 percent.</skos:definition>
    <dc:source>(L221) SeaVoX Device Catalogue</dc:source>
    <dc:publisher>British Oceanographic Data Centre (BODC)</dc:publisher>
    <skos:scopeNote xml:lang="en">manufacturer:Optical Scientific Inc.</skos:scopeNote>
  </rdf:Description>
  <rdf:Description rdf:about="http://vocab.nerc.ac.uk/collection/L22/current/TOOL0683">
    <rdf:type rdf:resource="http://www.w3.org/2004/02/skos/core#Concept" />
    <skos:prefLabel xml:lang="en">Vaisala WXT520 weather transmitter</skos:prefLabel>
    <skos:inScheme rdf:resource="http://vocab.aodn.org.au/def/instrument/1" />
    <dcterms:created rdf:datatype="http://www.w3.org/2001/XMLSchema#dateTime">2014-06-05T00:00:00Z</dcterms:created>
    <skos:definition xml:lang="en">This is a a self-contained weather station measuring wind speed and direction, precipitation , air temperature, humidity and barometric pressure. The station has the following sensors: Vaisala WINDCAP ultrasonic wind sensor measuring average, maximum and minimum windspeed  accurate to the 3% at 10 m/s and average, maximum and minimum wind direction to an accuracy of 3 degrees. Default averaging interval is 60 minutes. Vaisala RAINCAP sensor-2 - a piezoelectrical sensor that measures rainfall amount and intensity (rate) to an accuracy of 5% by counting raindrop impacts. Capacitive silicon BAROCAP air pressure sensor giving an accuracy of 0.5 hPa at 0-30C  or 1 hPa at -52-60C. Capacitive ceramic THERMOCAP air temperature sensor giving an accuracy of 0.3C at 20C. Capacitive thin film polymer HUMICAP 180 humidity sensor giving an accuracy of 3% below 90% humidity or 5% above 90% humidity. The precipitation and wind sensors may be optionally heated to keep them free from snow and ice. Output is via USB connection. This is an upgrade of the WXT510 weather transmitter that may be applied to existing units during service by Vaisala. More information may be found at http://www.vaisala.com/en/products/multiweathersensors/Pages/WXT520.aspx.</skos:definition>
    <dc:source>(L221) SeaVoX Device Catalogue</dc:source>
    <dc:publisher>British Oceanographic Data Centre (BODC)</dc:publisher>
  </rdf:Description>
  <rdf:Description rdf:about="http://vocab.nerc.ac.uk/collection/L22/current/TOOL0682">
    <rdf:type rdf:resource="http://www.w3.org/2004/02/skos/core#Concept" />
    <skos:prefLabel xml:lang="en">Vaisala WXT510 weather transmitter</skos:prefLabel>
    <skos:inScheme rdf:resource="http://vocab.aodn.org.au/def/instrument/1" />
    <dcterms:created rdf:datatype="http://www.w3.org/2001/XMLSchema#dateTime">2014-06-05T00:00:00Z</dcterms:created>
    <skos:definition xml:lang="en">This is a a self-contained weather station measuring wind speed and direction, precipitation , air temperature, humidity and barometric pressure. The station has the following sensors: Vaisala WINDCAP ultrasonic wind sensor measuring average, maximum and minimum windspeed  accurate to the greater of 0.3 m/s or 3% (0-35 m/s range) or 5% (36-60 m/s) range and average, maximum and minimum wind direction to an accuracy of 3 degrees. Default averaging interval is 60 minutes. Vaisala RAINCAP sensor-2 - a piezoelectrical sensor that measures rainfall amount and intensity (rate) to an accuracy of 5% by counting raindrop impacts. Capacitive silicon BAROCAP air pressure sensor. Capacitive ceramic THERMOCAP air temperature sensor. Capacitive thin film polymer HUMICAP 180 humidity sensor. The precipitation and wind sensors may be optionally heated to keep them free from snow and ice. Output is via an RS232 connection. More information may be found at http://www.vaisala.com/Vaisala%20Documents/User%20Guides%20and%20Quick%20Ref%20Guides/WXT510_User_Guide_in_English.pdf.</skos:definition>
    <dc:source>(L221) SeaVoX Device Catalogue</dc:source>
    <dc:publisher>British Oceanographic Data Centre (BODC)</dc:publisher>
  </rdf:Description>
  <rdf:Description rdf:about="http://vocab.nerc.ac.uk/collection/L22/current/TOOL0672">
    <rdf:type rdf:resource="http://www.w3.org/2004/02/skos/core#Concept" />
    <skos:prefLabel xml:lang="en">Vaisala PTB220 Digital Barometer</skos:prefLabel>
    <skos:inScheme rdf:resource="http://vocab.aodn.org.au/def/instrument/1" />
    <dcterms:created rdf:datatype="http://www.w3.org/2001/XMLSchema#dateTime">2013-10-11T00:00:00Z</dcterms:created>
    <skos:definition xml:lang="en">Fully compensated digital barometer using a silicon capacitive absolute pressure sensor designed to cover a wide range of environmental pressure and temperature. The pressure and temperature adjustment in the PTB220 consists of seven temperature levels over the operating temperature range of the barometer and of six to eleven pressure levels over the operating pressure range of the barometer at each temperature level. The instrument can operate over a pressure range of 50 to 1100 hPa and a temperature range of -40 to 60 degC with an accuracy better than 0.1%. More information may be found at http://www.vaisala.com/Vaisala%20Documents/User%20Guides%20and%20Quick%20Ref%20Guides/PTB220_User_Guide_in_English.pdf.</skos:definition>
    <dc:source>(L221) SeaVoX Device Catalogue</dc:source>
    <dc:publisher>British Oceanographic Data Centre (BODC)</dc:publisher>
    <skos:scopeNote xml:lang="en">manufacturer:Vaisala</skos:scopeNote>
  </rdf:Description>
  <rdf:Description rdf:about="http://vocab.nerc.ac.uk/collection/L22/current/TOOL0779">
    <rdf:type rdf:resource="http://www.w3.org/2004/02/skos/core#Concept" />
    <skos:prefLabel xml:lang="en">Vaisala DPA21 digital barometer</skos:prefLabel>
    <skos:inScheme rdf:resource="http://vocab.aodn.org.au/def/instrument/1" />
    <dcterms:created rdf:datatype="http://www.w3.org/2001/XMLSchema#dateTime">2013-10-11T00:00:00Z</dcterms:created>
    <skos:definition xml:lang="en" />
    <dc:source>(L221) SeaVoX Device Catalogue</dc:source>
    <dc:publisher>British Oceanographic Data Centre (BODC)</dc:publisher>
    <skos:scopeNote xml:lang="en">manufacturer:Vaisala</skos:scopeNote>
    <skos:definition xml:lang="en">A digital aneroid barometer with serial communication in use since the late 1980s.</skos:definition>
    <dcterms:modified rdf:datatype="http://www.w3.org/2001/XMLSchema#dateTime">2015-06-02T03:00:09Z</dcterms:modified>
  </rdf:Description>
  <rdf:Description rdf:about="http://vocab.nerc.ac.uk/collection/L22/current/TOOL0680">
    <rdf:type rdf:resource="http://www.w3.org/2004/02/skos/core#Concept" />
    <skos:prefLabel xml:lang="en">GE Druck RPT 350 Resonant Pressure Transducer</skos:prefLabel>
    <skos:inScheme rdf:resource="http://vocab.aodn.org.au/def/instrument/1" />
    <dcterms:created rdf:datatype="http://www.w3.org/2001/XMLSchema#dateTime">2013-10-15T00:00:00Z</dcterms:created>
    <skos:definition xml:lang="en">The GE Druck RPT350 Resonant Pressure Transducer, uses silicon technology to give high accuracy and stability with low manufacturing costs. It ranges from 35 to 3500 mbar abs.</skos:definition>
    <dc:source>(L221) SeaVoX Device Catalogue</dc:source>
    <dc:publisher>British Oceanographic Data Centre (BODC)</dc:publisher>
    <skos:scopeNote xml:lang="en">manufacturer:General Electric Company</skos:scopeNote>
  </rdf:Description>
  <rdf:Description rdf:about="http://vocab.nerc.ac.uk/collection/L05/current/33">
    <rdf:type rdf:resource="http://www.w3.org/2004/02/skos/core#Concept" />
    <skos:prefLabel xml:lang="en">sediment traps</skos:prefLabel>
    <skos:topConceptOf rdf:resource="http://vocab.aodn.org.au/def/instrument/1" />
    <skos:inScheme rdf:resource="http://vocab.aodn.org.au/def/instrument/1" />
    <dcterms:created rdf:datatype="http://www.w3.org/2001/XMLSchema#dateTime">2013-03-28T00:00:00Z</dcterms:created>
    <skos:definition xml:lang="en">A collector of particulates as they sink through the water column</skos:definition>
    <dc:source>(L051) SeaDataNet device categories</dc:source>
    <dc:publisher>British Oceanographic Data Centre (BODC)</dc:publisher>
    <skos:narrower rdf:resource="http://vocab.nerc.ac.uk/collection/L22/current/TOOL0786" />
    <skos:narrower rdf:resource="http://vocab.nerc.ac.uk/collection/L22/current/TOOL0785" />
  </rdf:Description>
  <rdf:Description rdf:about="http://vocab.nerc.ac.uk/collection/L22/current/TOOL0786">
    <rdf:type rdf:resource="http://www.w3.org/2004/02/skos/core#Concept" />
    <skos:prefLabel xml:lang="en">McLane PARFLUX Mark78HW-13 Sediment Traps</skos:prefLabel>
    <skos:altLabel xml:lang="en">PARFLUX Mark78HW-13</skos:altLabel>
    <skos:inScheme rdf:resource="http://vocab.aodn.org.au/def/instrument/1" />
    <dcterms:created rdf:datatype="http://www.w3.org/2001/XMLSchema#dateTime">2013-03-28T00:00:00Z</dcterms:created>
    <skos:definition xml:lang="en">A sediment trap designed for mid-water mooring deployment (maximum depth 6500m) with a conical collector passing settled particles into one of a set of bottles mounted in a carousel. The bottles are changed after a user-selected period of time.  An optional wet sample particle divider may be fitted to divide wet specimens into 5-10 equal parts. Compass/tilt and pressure sensors may also be fitted. This model carries 13 wide bottles (250 or 500 ml) and is 1.64m tall and 0.91m diameter.</skos:definition>
    <dc:source>(L221) SeaVoX Device Catalogue</dc:source>
    <dc:publisher>British Oceanographic Data Centre (BODC)</dc:publisher>
  </rdf:Description>
  <rdf:Description rdf:about="http://vocab.nerc.ac.uk/collection/L22/current/TOOL0785">
    <rdf:type rdf:resource="http://www.w3.org/2004/02/skos/core#Concept" />
    <skos:prefLabel xml:lang="en">McLane PARFLUX Mark78H-21 Sediment Traps</skos:prefLabel>
    <skos:altLabel xml:lang="en">PARFLUX Mark78H-21</skos:altLabel>
    <skos:inScheme rdf:resource="http://vocab.aodn.org.au/def/instrument/1" />
    <dcterms:created rdf:datatype="http://www.w3.org/2001/XMLSchema#dateTime">2013-03-28T00:00:00Z</dcterms:created>
    <skos:definition xml:lang="en">A sediment trap designed for mid-water mooring deployment (maximum depth 6500m) with a conical collector passing settled particles into one of a set of bottles mounted in a carousel. The bottles are changed after a user-selected period of time.  An optional wet sample particle divider may be fitted to divide wet specimens into 5-10 equal parts. Compass/tilt and pressure sensors may also be fitted.  This model carries 21 bottles (250 or 500 ml) and is 1.64m tall and 0.91m diameter.</skos:definition>
    <dc:source>(L221) SeaVoX Device Catalogue</dc:source>
    <dc:publisher>British Oceanographic Data Centre (BODC)</dc:publisher>
  </rdf:Description>
  <rdf:Description rdf:about="http://vocab.aodn.org.au/def/instrument/entity/365">
    <rdf:type rdf:resource="http://www.w3.org/2004/02/skos/core#Concept" />
    <skos:prefLabel xml:lang="en">Conductivity-Temperature sensors</skos:prefLabel>
    <dcterms:created rdf:datatype="http://www.w3.org/2001/XMLSchema#dateTime">2013-07-18T00:00:00Z</dcterms:created>
    <skos:definition xml:lang="en">Instrument that simultaneously measures electrical conductivity and temperature in the water column. To reduce costs, the instrument may not include a pressure sensor, because the deployment depth is know (approximately).</skos:definition>
    <dc:source>Australian Ocean Data Network instrument register</dc:source>
    <dc:publisher>eMarine Information Infrastructure (eMII)</dc:publisher>
    <dcterms:creator xml:lang="en">Sebastien Mancini</dcterms:creator>
    <skos:narrower rdf:resource="http://vocab.nerc.ac.uk/collection/L22/current/TOOL0017" />
    <skos:narrower rdf:resource="http://vocab.nerc.ac.uk/collection/L22/current/TOOL0018" />
    <skos:narrower rdf:resource="http://vocab.nerc.ac.uk/collection/L22/current/TOOL0019" />
    <skos:narrower rdf:resource="http://vocab.nerc.ac.uk/collection/L22/current/TOOL0020" />
    <skos:narrower rdf:resource="http://vocab.nerc.ac.uk/collection/L22/current/TOOL0023" />
    <skos:narrower rdf:resource="http://vocab.nerc.ac.uk/collection/L22/current/TOOL0053" />
    <skos:narrower rdf:resource="http://vocab.nerc.ac.uk/collection/L22/current/TOOL0100" />
    <skos:topConceptOf rdf:resource="http://vocab.aodn.org.au/def/instrument/1" />
    <skos:inScheme rdf:resource="http://vocab.aodn.org.au/def/instrument/1" />
  </rdf:Description>
  <rdf:Description rdf:about="http://vocab.nerc.ac.uk/collection/L22/current/TOOL0100">
    <rdf:type rdf:resource="http://www.w3.org/2004/02/skos/core#Concept" />
    <skos:prefLabel xml:lang="en">Sea-Bird SBE 16Plus SEACAT C-T Recorder</skos:prefLabel>
    <dcterms:created rdf:datatype="http://www.w3.org/2001/XMLSchema#dateTime">2014-02-07T00:00:00Z</dcterms:created>
    <skos:definition xml:lang="en">The SBE 16plus is a high accuracy conductivity and temperature recorder (pressure optional) with RS232 or RS485 interfaces. It is designed for moorings and other long-duration, fixed-site deployments. The SBE 16plus has 6 amplified A/D input channels and conditioned power of 500 ma is avaliable for auxiliary sensors, dissolved oxygen, turbidity, fluorescence, PAR etc. Further information may be found on the BODC document server at URL: http://www.bodc.ac.uk/data/documents/nodb/153217/ (RS485) or http://www.bodc.ac.uk/data/documents/nodb/158981/ (RS232).</skos:definition>
    <dc:source>(L221) SeaVoX Device Catalogue</dc:source>
    <dc:publisher>British Oceanographic Data Centre (BODC)</dc:publisher>
    <skos:inScheme rdf:resource="http://vocab.aodn.org.au/def/instrument/1" />
    <skos:scopeNote xml:lang="en">manufacturer:Sea-Bird Electronics Inc.</skos:scopeNote>
  </rdf:Description>
  <rdf:Description rdf:about="http://vocab.nerc.ac.uk/collection/L22/current/TOOL0023">
    <rdf:type rdf:resource="http://www.w3.org/2004/02/skos/core#Concept" />
    <skos:prefLabel xml:lang="en">Sea-Bird SBE 16 SEACAT C-T Recorder</skos:prefLabel>
    <dcterms:created rdf:datatype="http://www.w3.org/2001/XMLSchema#dateTime">2014-02-17T00:00:00Z</dcterms:created>
    <skos:definition xml:lang="en">The SBE 16 SEACAT is a conductivity and temperature recorder with an optional pressure sensor designed for depolyment on moorings. Further information may be found on the BODC document server at URL http://www.bodc.ac.uk/data/documents/nodb/117180/. Replaced by the SBE 16plus range in 2001.</skos:definition>
    <dc:source>(L221) SeaVoX Device Catalogue</dc:source>
    <dc:publisher>British Oceanographic Data Centre (BODC)</dc:publisher>
    <skos:inScheme rdf:resource="http://vocab.aodn.org.au/def/instrument/1" />
    <skos:scopeNote xml:lang="en">manufacturer:Sea-Bird Electronics Inc.</skos:scopeNote>
  </rdf:Description>
  <rdf:Description rdf:about="http://vocab.nerc.ac.uk/collection/L22/current/TOOL0020">
    <rdf:type rdf:resource="http://www.w3.org/2004/02/skos/core#Concept" />
    <skos:prefLabel xml:lang="en">Sea-Bird SBE 37-SIP MicroCAT C-T Sensor</skos:prefLabel>
    <dcterms:created rdf:datatype="http://www.w3.org/2001/XMLSchema#dateTime">2014-02-26T00:00:00Z</dcterms:created>
    <skos:definition xml:lang="en">The SBE 37 MicroCAT is a high accuracy conductivity and temperature recorder with an optional pressure sensor designed for depolyment on moorings. The SIP model has a serial interface with an internal pump to improve conductivity response and protection against fouling.</skos:definition>
    <dc:source>(L221) SeaVoX Device Catalogue</dc:source>
    <dc:publisher>British Oceanographic Data Centre (BODC)</dc:publisher>
    <skos:inScheme rdf:resource="http://vocab.aodn.org.au/def/instrument/1" />
    <skos:scopeNote xml:lang="en">manufacturer:Sea-Bird Electronics Inc.</skos:scopeNote>
  </rdf:Description>
  <rdf:Description rdf:about="http://vocab.nerc.ac.uk/collection/L22/current/TOOL0019">
    <rdf:type rdf:resource="http://www.w3.org/2004/02/skos/core#Concept" />
    <skos:prefLabel xml:lang="en">Sea-Bird SBE 37-IMP MicroCAT C-T Sensor</skos:prefLabel>
    <dcterms:created rdf:datatype="http://www.w3.org/2001/XMLSchema#dateTime">2014-02-17T00:00:00Z</dcterms:created>
    <skos:definition xml:lang="en">The SBE 37 MicroCAT is a high accuracy conductivity and temperature recorder with an optional pressure sensor designed for depolyment on moorings. The IMP model has an inductive modem for real-time data transmission plus internal flash memory data storage with an internal pump to improve conductivity response and protection against fouling.</skos:definition>
    <dc:source>(L221) SeaVoX Device Catalogue</dc:source>
    <dc:publisher>British Oceanographic Data Centre (BODC)</dc:publisher>
    <skos:inScheme rdf:resource="http://vocab.aodn.org.au/def/instrument/1" />
    <skos:scopeNote xml:lang="en">manufacturer:Sea-Bird Electronics Inc.</skos:scopeNote>
  </rdf:Description>
  <rdf:Description rdf:about="http://vocab.nerc.ac.uk/collection/L22/current/TOOL0053">
    <rdf:type rdf:resource="http://www.w3.org/2004/02/skos/core#Concept" />
    <skos:prefLabel xml:lang="en">RBR XR-420 CTD Marine</skos:prefLabel>
    <dcterms:created rdf:datatype="http://www.w3.org/2001/XMLSchema#dateTime">2014-02-17T00:00:00Z</dcterms:created>
    <skos:definition xml:lang="en">A small autonomous data logger designed to monitor conductivity, temperature and depth. Conductivity (accuracy ± 0.003 mS/cm) is measured using a 3-coil closed loop feedback inductive cell for superior temperature compensation. The thermistor (Themometrics) used to record temperature (accuracy ± 0.002°C) is aged and hermetically sealed in the tip of a shock resistant solid glass rod. Pressure (accuracy 0.05% full scale) sensors use reliable semiconductor technology and 316 stainless steel housing developed for long-term stability in harsh environments.</skos:definition>
    <dc:source>(L221) SeaVoX Device Catalogue</dc:source>
    <dc:publisher>British Oceanographic Data Centre (BODC)</dc:publisher>
    <skos:inScheme rdf:resource="http://vocab.aodn.org.au/def/instrument/1" />
    <skos:scopeNote xml:lang="en">manufacturer: RBR</skos:scopeNote>
  </rdf:Description>
  <rdf:Description rdf:about="http://vocab.nerc.ac.uk/collection/L22/current/TOOL0017">
    <rdf:type rdf:resource="http://www.w3.org/2004/02/skos/core#Concept" />
    <skos:prefLabel xml:lang="en">Sea-Bird SBE 37-SM MicroCAT C-T Sensor</skos:prefLabel>
    <dcterms:created rdf:datatype="http://www.w3.org/2001/XMLSchema#dateTime">2014-02-06T00:00:00Z</dcterms:created>
    <skos:definition xml:lang="en">The SBE 37 MicroCAT is a high accuracy conductivity and temperature recorder with an optional pressure sensor designed for depolyment on moorings. The SM model has a serial interface plus internal flash memory data storage. Further information may be found on the BODC document server at URL http://www.bodc.ac.uk/data/documents/nodb/108613/.</skos:definition>
    <dc:source>(L221) SeaVoX Device Catalogue</dc:source>
    <dc:publisher>British Oceanographic Data Centre (BODC)</dc:publisher>
    <skos:inScheme rdf:resource="http://vocab.aodn.org.au/def/instrument/1" />
    <skos:scopeNote xml:lang="en">manufacturer:Sea-Bird Electronics Inc.</skos:scopeNote>
  </rdf:Description>
  <rdf:Description rdf:about="http://vocab.nerc.ac.uk/collection/L22/current/TOOL0018">
    <rdf:type rdf:resource="http://www.w3.org/2004/02/skos/core#Concept" />
    <skos:prefLabel xml:lang="en">Sea-Bird SBE 37-SMP MicroCAT C-T Sensor</skos:prefLabel>
    <dcterms:created rdf:datatype="http://www.w3.org/2001/XMLSchema#dateTime">2014-02-06T00:00:00Z</dcterms:created>
    <skos:definition xml:lang="en">The SBE 37 MicroCAT is a high accuracy conductivity and temperature recorder with an optional pressure sensor designed for depolyment on moorings. The SMP model has a serial interface plus internal flash memory data storage with an internal pump to improve conductivity response and protection against fouling.</skos:definition>
    <dc:source>(L221) SeaVoX Device Catalogue</dc:source>
    <dc:publisher>British Oceanographic Data Centre (BODC)</dc:publisher>
    <skos:inScheme rdf:resource="http://vocab.aodn.org.au/def/instrument/1" />
    <skos:scopeNote xml:lang="en">manufacturer:Sea-Bird Electronics Inc.</skos:scopeNote>
  </rdf:Description>
  <rdf:Description rdf:about="http://vocab.aodn.org.au/def/instrument/entity/363">
    <rdf:type rdf:resource="http://www.w3.org/2004/02/skos/core#Concept" />
    <skos:prefLabel xml:lang="en">CTD Rosette</skos:prefLabel>
    <dcterms:created rdf:datatype="http://www.w3.org/2001/XMLSchema#dateTime">2013-07-18T00:00:00Z</dcterms:created>
    <skos:definition xml:lang="en">A package lowered and raised vertically from a surface platform usually a ship. A CTD measures Conductivity, Temperature and Depth. Despite the name, all CTDs actually measure pressure. The CTD is attached to a frame fitted with a number of large water-collecting bottles called Niskins, the instrument together with the bottles is called the CTD rosette. The Niskin bottles are designed so that they have lids at both ends. They are sent down open, and triggered to close electronically at the depth that water needs to be collected. Additional optional sensors include ADCP, fluorometers, transmissometers and radiometers.</skos:definition>
    <dc:source>Australian Ocean Data Network instrument register</dc:source>
    <dc:publisher>eMarine Information Infrastructure (eMII)</dc:publisher>
    <dcterms:creator xml:lang="en">Sebastien Mancini</dcterms:creator>
    <skos:topConceptOf rdf:resource="http://vocab.aodn.org.au/def/instrument/1" />
    <skos:inScheme rdf:resource="http://vocab.aodn.org.au/def/instrument/1" />
  </rdf:Description>
  <rdf:Description rdf:about="http://vocab.nerc.ac.uk/collection/L05/current/157">
    <rdf:type rdf:resource="http://www.w3.org/2004/02/skos/core#Concept" />
    <skos:prefLabel xml:lang="en">multi-beam echosounders</skos:prefLabel>
    <skos:topConceptOf rdf:resource="http://vocab.aodn.org.au/def/instrument/1" />
    <skos:inScheme rdf:resource="http://vocab.aodn.org.au/def/instrument/1" />
    <dcterms:created rdf:datatype="http://www.w3.org/2001/XMLSchema#dateTime">2014-05-22T00:00:00Z</dcterms:created>
    <skos:definition xml:lang="en">Instruments that measure water depth along several tracks parallel to the platform track by timing pulses of sound reflected on the seafloor</skos:definition>
    <dc:source>(L051) SeaDataNet device categories</dc:source>
    <dc:publisher>British Oceanographic Data Centre (BODC)</dc:publisher>
  </rdf:Description>
  <rdf:Description rdf:about="http://vocab.aodn.org.au/def/instrument/entity/361">
    <rdf:type rdf:resource="http://www.w3.org/2004/02/skos/core#Concept" />
    <skos:prefLabel xml:lang="en">water biogeochemical sensor</skos:prefLabel>
    <dcterms:created rdf:datatype="http://www.w3.org/2001/XMLSchema#dateTime">2013-07-18T00:00:00Z</dcterms:created>
    <skos:definition xml:lang="en">A package of sensors that measure physical, chemical and biological properties in the water column. These typically include temperature, conductivity, pressure, dissolved oxygen, fluorescence and turbidity.</skos:definition>
    <dc:source>Australian Ocean Data Network instrument register</dc:source>
    <dc:publisher>eMarine Information Infrastructure (eMII)</dc:publisher>
    <dcterms:creator xml:lang="en">Sebastien Mancini</dcterms:creator>
    <skos:narrower rdf:resource="http://vocab.nerc.ac.uk/collection/L22/current/TOOL0215" />
    <skos:narrower rdf:resource="http://vocab.nerc.ac.uk/collection/L22/current/TOOL0673" />
    <skos:narrower rdf:resource="http://vocab.nerc.ac.uk/collection/L22/current/TOOL0674" />
    <skos:narrower rdf:resource="http://vocab.nerc.ac.uk/collection/L22/current/TOOL0675" />
    <skos:topConceptOf rdf:resource="http://vocab.aodn.org.au/def/instrument/1" />
    <skos:inScheme rdf:resource="http://vocab.aodn.org.au/def/instrument/1" />
  </rdf:Description>
  <rdf:Description rdf:about="http://vocab.nerc.ac.uk/collection/L22/current/TOOL0675">
    <rdf:type rdf:resource="http://www.w3.org/2004/02/skos/core#Concept" />
    <skos:prefLabel xml:lang="en">WETLabs Water Quality Monitor</skos:prefLabel>
    <dcterms:created rdf:datatype="http://www.w3.org/2001/XMLSchema#dateTime">2014-04-01T00:00:00Z</dcterms:created>
    <skos:definition xml:lang="en">An instrument that incorporates WET Labs fluorometer-turbidity and Sea-Bird's CTD sensors, providing temperature, salinity, depth, dissolved oxygen, chlorophyll fluorescence, turbidity and backscattering data. It is designed for long-term deployment in coastal waters with protection against biofouling and fouling by sediment loads. More information is available at http://www.wetlabs.com/wqm.</skos:definition>
    <dc:source>(L221) SeaVoX Device Catalogue</dc:source>
    <dc:publisher>British Oceanographic Data Centre (BODC)</dc:publisher>
    <skos:inScheme rdf:resource="http://vocab.aodn.org.au/def/instrument/1" />
    <skos:scopeNote xml:lang="en">manufacture:WETLabs Inc.</skos:scopeNote>
  </rdf:Description>
  <rdf:Description rdf:about="http://vocab.nerc.ac.uk/collection/L22/current/TOOL0215">
    <rdf:type rdf:resource="http://www.w3.org/2004/02/skos/core#Concept" />
    <skos:prefLabel xml:lang="en">WETLabs ECO-FLNTU combined fluorometer and turbidity sensor</skos:prefLabel>
    <dcterms:created rdf:datatype="http://www.w3.org/2001/XMLSchema#dateTime">2013-12-16T00:00:00Z</dcterms:created>
    <skos:definition xml:lang="en">The ECO-FLNTU combines the ECO fluorometer with an optical scattering measurement at 700nm for simultaneous determination of turbidity. The fluorometer can typically measure phytoplankton concentrations in the range 0.01-50 ug/l, with a sensitivity of 0.01 ug/l. The turbidity sensor can measure within the range 0.01-25 NTU, with a sensitivity of 0.01 NTU. The instrument is stable over a temperature range of 0-20 degC and is rated to a depth of 600 m as standard, with the option of a 'deep' instrument rated to 6000m.</skos:definition>
    <dc:source>(L221) SeaVoX Device Catalogue</dc:source>
    <dc:publisher>British Oceanographic Data Centre (BODC)</dc:publisher>
    <skos:inScheme rdf:resource="http://vocab.aodn.org.au/def/instrument/1" />
    <skos:scopeNote xml:lang="en">manufacture:WETLabs Inc.</skos:scopeNote>
  </rdf:Description>
  <rdf:Description rdf:about="http://vocab.nerc.ac.uk/collection/L22/current/TOOL0674">
    <rdf:type rdf:resource="http://www.w3.org/2004/02/skos/core#Concept" />
    <skos:prefLabel xml:lang="en">WETLabs ECO Triplet</skos:prefLabel>
    <dcterms:created rdf:datatype="http://www.w3.org/2001/XMLSchema#dateTime">2013-09-10T00:00:00Z</dcterms:created>
    <skos:definition xml:lang="en">A three-optical-sensor instrument that may carry any combination of fluorometers or single-wavelength scattering meters. The fluorometers are single wavelength sensors that can be configured for chlorophyll-a, CDOM, phycocyanin, phycoerythrin, fluorescein or rhodamine. Scattering meters measure optical scattering at blue, green or red wavelengths. More information may be found at http://www.wetlabs.com/eco-triplet.</skos:definition>
    <dc:source>(L221) SeaVoX Device Catalogue</dc:source>
    <dc:publisher>British Oceanographic Data Centre (BODC)</dc:publisher>
    <skos:inScheme rdf:resource="http://vocab.aodn.org.au/def/instrument/1" />
    <skos:scopeNote xml:lang="en">manufacture:WETLabs Inc.</skos:scopeNote>
  </rdf:Description>
  <rdf:Description rdf:about="http://vocab.nerc.ac.uk/collection/L22/current/TOOL0673">
    <rdf:type rdf:resource="http://www.w3.org/2004/02/skos/core#Concept" />
    <skos:prefLabel xml:lang="en">WETLabs ECO Puck Triple-Measurement Meter</skos:prefLabel>
    <dcterms:created rdf:datatype="http://www.w3.org/2001/XMLSchema#dateTime">2013-09-11T00:00:00Z</dcterms:created>
    <skos:definition xml:lang="en">A miniature version of the Environmental Characterisation Optics (ECO) sensors built for OEM applications, with the design specifically targeted at AUVs, gliders and profiling floats. The triplet version carries a fluorometer plus two other sensors that may be additional fluorometers, single-wavelength scattering meters (BB) or a volume scattering function meter (VSF). The fluorometers are single wavelength sensors that can be configured for chlorophyll-a, CDOM, phycocyanin, phycoerythrin, fluorescein or rhodamine. BB measures optical scattering at 117 degrees at 470, 532 or 650 nm wavelengths. VSF measures optical scattering at 100, 125 and 150 degrees. More information may be found at http://www.wetlabs.com/eco-puck.</skos:definition>
    <dc:source>(L221) SeaVoX Device Catalogue</dc:source>
    <dc:publisher>British Oceanographic Data Centre (BODC)</dc:publisher>
    <skos:inScheme rdf:resource="http://vocab.aodn.org.au/def/instrument/1" />
    <skos:scopeNote xml:lang="en">manufacture:WETLabs Inc.</skos:scopeNote>
  </rdf:Description>
  <rdf:Description rdf:about="http://vocab.nerc.ac.uk/collection/L05/current/151">
    <rdf:type rdf:resource="http://www.w3.org/2004/02/skos/core#Concept" />
    <skos:prefLabel xml:lang="en">benthic incubation chambers</skos:prefLabel>
    <skos:topConceptOf rdf:resource="http://vocab.aodn.org.au/def/instrument/1" />
    <skos:inScheme rdf:resource="http://vocab.aodn.org.au/def/instrument/1" />
    <dcterms:created rdf:datatype="http://www.w3.org/2001/XMLSchema#dateTime">2014-05-22T00:00:00Z</dcterms:created>
    <skos:definition xml:lang="en">A device that isolates a portion of seabed plus overlying water from its surroundings. Either returns the entire system to the surface or incorporates sampling devices and/or in-situ sensors.</skos:definition>
    <dc:source>(L051) SeaDataNet device categories</dc:source>
    <dc:publisher>British Oceanographic Data Centre (BODC)</dc:publisher>
  </rdf:Description>
  <rdf:Description rdf:about="http://vocab.nerc.ac.uk/collection/L05/current/350">
    <rdf:type rdf:resource="http://www.w3.org/2004/02/skos/core#Concept" />
    <skos:prefLabel xml:lang="en">salinity sensor</skos:prefLabel>
    <skos:topConceptOf rdf:resource="http://vocab.aodn.org.au/def/instrument/1" />
    <skos:inScheme rdf:resource="http://vocab.aodn.org.au/def/instrument/1" />
    <dcterms:created rdf:datatype="http://www.w3.org/2001/XMLSchema#dateTime">2013-10-10T00:00:00Z</dcterms:created>
    <skos:definition xml:lang="en">Instrument that simultaneously measures electrical conductivity and temperature in the water column to provide temperature and salinity data</skos:definition>
    <dc:source>(L051) SeaDataNet device categories</dc:source>
    <dc:publisher>British Oceanographic Data Centre (BODC)</dc:publisher>
    <skos:narrower rdf:resource="http://vocab.nerc.ac.uk/collection/L22/current/TOOL0017" />
    <skos:narrower rdf:resource="http://vocab.nerc.ac.uk/collection/L22/current/TOOL0018" />
    <skos:narrower rdf:resource="http://vocab.nerc.ac.uk/collection/L22/current/TOOL0019" />
    <skos:narrower rdf:resource="http://vocab.nerc.ac.uk/collection/L22/current/TOOL0020" />
    <skos:narrower rdf:resource="http://vocab.nerc.ac.uk/collection/L22/current/TOOL0023" />
    <skos:narrower rdf:resource="http://vocab.nerc.ac.uk/collection/L22/current/TOOL0040" />
    <skos:narrower rdf:resource="http://vocab.nerc.ac.uk/collection/L22/current/TOOL0042" />
    <skos:narrower rdf:resource="http://vocab.nerc.ac.uk/collection/L22/current/TOOL0047" />
    <skos:narrower rdf:resource="http://vocab.nerc.ac.uk/collection/L22/current/TOOL0053" />
    <skos:narrower rdf:resource="http://vocab.nerc.ac.uk/collection/L22/current/TOOL0058" />
    <skos:narrower rdf:resource="http://vocab.nerc.ac.uk/collection/L22/current/TOOL0100" />
    <skos:narrower rdf:resource="http://vocab.nerc.ac.uk/collection/L22/current/TOOL0173" />
    <skos:narrower rdf:resource="http://vocab.nerc.ac.uk/collection/L22/current/TOOL0190" />
    <skos:narrower rdf:resource="http://vocab.nerc.ac.uk/collection/L22/current/TOOL0446" />
    <skos:narrower rdf:resource="http://vocab.nerc.ac.uk/collection/L22/current/TOOL0667" />
    <skos:narrower rdf:resource="http://vocab.nerc.ac.uk/collection/L22/current/TOOL0668" />
    <skos:narrower rdf:resource="http://vocab.nerc.ac.uk/collection/L22/current/TOOL0669" />
    <skos:narrower rdf:resource="http://vocab.nerc.ac.uk/collection/L22/current/TOOL0675" />
    <skos:narrower rdf:resource="http://vocab.nerc.ac.uk/collection/L22/current/TOOL0720" />
    <skos:narrower rdf:resource="http://vocab.nerc.ac.uk/collection/L22/current/TOOL0022" />
    <skos:narrower rdf:resource="http://vocab.nerc.ac.uk/collection/L22/current/TOOL0870/" />
    <skos:narrower rdf:resource="http://vocab.nerc.ac.uk/collection/L22/current/TOOL0871/" />
    <skos:narrower rdf:resource="http://vocab.nerc.ac.uk/collection/L22/current/TOOL0869/" />
    <dcterms:modified rdf:datatype="http://www.w3.org/2001/XMLSchema#dateTime">2015-06-10T02:09:08Z</dcterms:modified>
  </rdf:Description>
  <rdf:Description rdf:about="http://vocab.nerc.ac.uk/collection/L22/current/TOOL0042">
    <rdf:type rdf:resource="http://www.w3.org/2004/02/skos/core#Concept" />
    <skos:prefLabel xml:lang="en">Sea-Bird SBE 19 SEACAT CTD</skos:prefLabel>
    <skos:inScheme rdf:resource="http://vocab.aodn.org.au/def/instrument/1" />
    <dcterms:created rdf:datatype="http://www.w3.org/2001/XMLSchema#dateTime">2014-02-17T00:00:00Z</dcterms:created>
    <skos:definition xml:lang="en">A self-contained battery powered CTD with precision semiconductor strain gauge pressure sensor. Water was supplied to the conductivity sensor by a pump. Housing was plastic (up to 600m depth), aluminium (up to 6800m depth) or titanium (up to 10500m depth). Optional oxygen, pH, fluorescence, PAR, light transmission and turbidity sensors could be fitted. Primarily designed for profiling applications but may be used on a short (less than 2 weeks) duration mooring. Replaced by the SBE19plus model in 2001.</skos:definition>
    <dc:source>(L221) SeaVoX Device Catalogue</dc:source>
    <dc:publisher>British Oceanographic Data Centre (BODC)</dc:publisher>
    <skos:scopeNote xml:lang="en">manufacturer:Sea-Bird Electronics Inc.</skos:scopeNote>
  </rdf:Description>
  <rdf:Description rdf:about="http://vocab.nerc.ac.uk/collection/L22/current/TOOL0022">
    <rdf:type rdf:resource="http://www.w3.org/2004/02/skos/core#Concept" />
    <skos:prefLabel xml:lang="en">Sea-Bird SBE 37-IM MicroCAT C-T Sensor</skos:prefLabel>
    <skos:altLabel xml:lang="en">SBE 37-IM MicroCAT</skos:altLabel>
    <skos:inScheme rdf:resource="http://vocab.aodn.org.au/def/instrument/1" />
    <dcterms:created rdf:datatype="http://www.w3.org/2001/XMLSchema#dateTime">2013-03-28T00:00:00Z</dcterms:created>
    <skos:definition xml:lang="en">The SBE 37 MicroCAT is a high accuracy conductivity and temperature recorder with an optional pressure sensor designed for depolyment on moorings. The IM model has an inductive modem for real-time data transmission plus internal flash memory data storage. Further information may be found on the BODC document server at URL http://www.bodc.ac.uk/data/documents/nodb/113079/.</skos:definition>
    <dc:source>(L221) SeaVoX Device Catalogue</dc:source>
    <dc:publisher>British Oceanographic Data Centre (BODC)</dc:publisher>
  </rdf:Description>
  <rdf:Description rdf:about="http://vocab.nerc.ac.uk/collection/L22/current/TOOL0667">
    <rdf:type rdf:resource="http://www.w3.org/2004/02/skos/core#Concept" />
    <skos:prefLabel xml:lang="en">Sea-Bird SBE 21 Thermosalinograph</skos:prefLabel>
    <skos:inScheme rdf:resource="http://vocab.aodn.org.au/def/instrument/1" />
    <dcterms:created rdf:datatype="http://www.w3.org/2001/XMLSchema#dateTime">2013-10-08T00:00:00Z</dcterms:created>
    <skos:definition xml:lang="en">A platinum-electrode conductivity sensor and a thermistor mounted in a corrosion-resistant plastic and titanium housing designed to be continuously plumbed into a vessel's pumped seawater supply. The instrument may be interfaced to a remote SBE 38 temperature sensor mounted either on the hull or in the seawater inlet. Data are both stored in internal memory and output to a serial port for external logging.  Conductivity is measured in the range 0-7 S/m with an accuracy of 0.001 S/m and a resolution  of 0.0001 S/m. Housing temperature is measured in the range -5-35C with an accuracy of 0.01 C and a resolution  of 0.001 C. Remote temperature is measured in the range -5-35C  with an accuracy of 0.001 C and a resolution  of 0.0003 C. More information at http://www.seabird.com/products/spec_sheets/21data.htm.</skos:definition>
    <dc:source>(L221) SeaVoX Device Catalogue</dc:source>
    <dc:publisher>British Oceanographic Data Centre (BODC)</dc:publisher>
    <skos:scopeNote xml:lang="en">manufacturer:Sea-Bird Electronics Inc.</skos:scopeNote>
  </rdf:Description>
  <rdf:Description rdf:about="http://vocab.nerc.ac.uk/collection/L22/current/TOOL0040">
    <rdf:type rdf:resource="http://www.w3.org/2004/02/skos/core#Concept" />
    <skos:prefLabel xml:lang="en">Sea-Bird SBE 25 Sealogger CTD</skos:prefLabel>
    <skos:inScheme rdf:resource="http://vocab.aodn.org.au/def/instrument/1" />
    <dcterms:created rdf:datatype="http://www.w3.org/2001/XMLSchema#dateTime">2014-02-07T00:00:00Z</dcterms:created>
    <skos:definition xml:lang="en">A compact self-contained CTD comprising a conductivity sensor plumbed into a pumped water supply and separate pressure and temperature sensor modules. The whole unit is mounted in a stainless steel cage with a battery pack, data logger and memory. A dissolved oxygen sensor may be plumbed into the pumped water supply and other sensor modules such as fluorometers and transmissometers may be mounted in the cage and interfaced to the data logger. The instrument may also be used with external power and data logging through an RS-232 interface.</skos:definition>
    <dc:source>(L221) SeaVoX Device Catalogue</dc:source>
    <dc:publisher>British Oceanographic Data Centre (BODC)</dc:publisher>
    <skos:scopeNote xml:lang="en">manufacturer:Sea-Bird Electronics Inc.</skos:scopeNote>
  </rdf:Description>
  <rdf:Description rdf:about="http://vocab.nerc.ac.uk/collection/L22/current/TOOL0023">
    <rdf:type rdf:resource="http://www.w3.org/2004/02/skos/core#Concept" />
    <skos:prefLabel xml:lang="en">Sea-Bird SBE 16 SEACAT C-T Recorder</skos:prefLabel>
    <dcterms:created rdf:datatype="http://www.w3.org/2001/XMLSchema#dateTime">2014-02-17T00:00:00Z</dcterms:created>
    <skos:definition xml:lang="en">The SBE 16 SEACAT is a conductivity and temperature recorder with an optional pressure sensor designed for depolyment on moorings. Further information may be found on the BODC document server at URL http://www.bodc.ac.uk/data/documents/nodb/117180/. Replaced by the SBE 16plus range in 2001.</skos:definition>
    <dc:source>(L221) SeaVoX Device Catalogue</dc:source>
    <dc:publisher>British Oceanographic Data Centre (BODC)</dc:publisher>
    <skos:inScheme rdf:resource="http://vocab.aodn.org.au/def/instrument/1" />
    <skos:scopeNote xml:lang="en">manufacturer:Sea-Bird Electronics Inc.</skos:scopeNote>
  </rdf:Description>
  <rdf:Description rdf:about="http://vocab.nerc.ac.uk/collection/L22/current/TOOL0669">
    <rdf:type rdf:resource="http://www.w3.org/2004/02/skos/core#Concept" />
    <skos:prefLabel xml:lang="en">Sea-Bird SBE 41CP CTD</skos:prefLabel>
    <skos:inScheme rdf:resource="http://vocab.aodn.org.au/def/instrument/1" />
    <dcterms:created rdf:datatype="http://www.w3.org/2001/XMLSchema#dateTime">2014-04-02T00:00:00Z</dcterms:created>
    <skos:definition xml:lang="en">A self-contained unit comprising the MicroCAT temperature, conductivity and pressure sensors and a pump that is designed specifically for deployment on profiling floats, particularly Argo.  The unit is designed to provide stable salinity data accurate to 0.005 PSU for periods in excess of three years without any form of maintenance. Temperature is within 0.002 C (stability 0.0002 C/year) and pressure within 2 dbar (stability 0.8 dbar/year).  During float ascent samples are collected at 1 Hz and logged to internal storage to provide a continuous profile passed to the float controller at the surface.  More information is given in http://www.seabird.com/products/spec_sheets/41data.htm.</skos:definition>
    <dc:source>(L221) SeaVoX Device Catalogue</dc:source>
    <dc:publisher>British Oceanographic Data Centre (BODC)</dc:publisher>
    <skos:scopeNote xml:lang="en">manufacturer:Sea-Bird Electronics Inc.</skos:scopeNote>
  </rdf:Description>
  <rdf:Description rdf:about="http://vocab.nerc.ac.uk/collection/L22/current/TOOL0020">
    <rdf:type rdf:resource="http://www.w3.org/2004/02/skos/core#Concept" />
    <skos:prefLabel xml:lang="en">Sea-Bird SBE 37-SIP MicroCAT C-T Sensor</skos:prefLabel>
    <dcterms:created rdf:datatype="http://www.w3.org/2001/XMLSchema#dateTime">2014-02-26T00:00:00Z</dcterms:created>
    <skos:definition xml:lang="en">The SBE 37 MicroCAT is a high accuracy conductivity and temperature recorder with an optional pressure sensor designed for depolyment on moorings. The SIP model has a serial interface with an internal pump to improve conductivity response and protection against fouling.</skos:definition>
    <dc:source>(L221) SeaVoX Device Catalogue</dc:source>
    <dc:publisher>British Oceanographic Data Centre (BODC)</dc:publisher>
    <skos:inScheme rdf:resource="http://vocab.aodn.org.au/def/instrument/1" />
    <skos:scopeNote xml:lang="en">manufacturer:Sea-Bird Electronics Inc.</skos:scopeNote>
  </rdf:Description>
  <rdf:Description rdf:about="http://vocab.nerc.ac.uk/collection/L22/current/TOOL0668">
    <rdf:type rdf:resource="http://www.w3.org/2004/02/skos/core#Concept" />
    <skos:prefLabel xml:lang="en">Sea-Bird SBE 41 CTD</skos:prefLabel>
    <skos:inScheme rdf:resource="http://vocab.aodn.org.au/def/instrument/1" />
    <dcterms:created rdf:datatype="http://www.w3.org/2001/XMLSchema#dateTime">2013-09-09T00:00:00Z</dcterms:created>
    <skos:definition xml:lang="en">A self-contained unit comprising the MicroCAT temperature, conductivity and pressure sensors and a pump that is designed specifically for deployment on profiling floats, particularly Argo.  The unit is designed to provide stable salinity data accurate to 0.005 PSU for periods in excess of three years without any form of maintenance. Temperature is within 0.002 C (stability 0.0002 C/year) and pressure within 2 dbar (stability 0.8 dbar/year).  During float ascent spot samples are taken and transmitted to the float controller.  More information is given in http://www.seabird.com/products/spec_sheets/41data.htm.</skos:definition>
    <dc:source>(L221) SeaVoX Device Catalogue</dc:source>
    <dc:publisher>British Oceanographic Data Centre (BODC)</dc:publisher>
    <skos:scopeNote xml:lang="en">manufacturer:Sea-Bird Electronics Inc.</skos:scopeNote>
  </rdf:Description>
  <rdf:Description rdf:about="http://vocab.nerc.ac.uk/collection/L22/current/TOOL0047">
    <rdf:type rdf:resource="http://www.w3.org/2004/02/skos/core#Concept" />
    <skos:prefLabel xml:lang="en">Sea-Bird SBE 19plus SEACAT CTD</skos:prefLabel>
    <skos:inScheme rdf:resource="http://vocab.aodn.org.au/def/instrument/1" />
    <dcterms:created rdf:datatype="http://www.w3.org/2001/XMLSchema#dateTime">2014-02-07T00:00:00Z</dcterms:created>
    <skos:definition xml:lang="en">Self contained self powered CTD profiler. Measures conductivity, temperature and pressure in both profiling (samples at 4 scans/sec) and moored (sample rates of once every 5 seconds to once every 9 hours) mode. Available in plastic or titanium housing with depth ranges of 600m and 7000m respectively. Minature submersible pump provides water to conductivity cell.</skos:definition>
    <dc:source>(L221) SeaVoX Device Catalogue</dc:source>
    <dc:publisher>British Oceanographic Data Centre (BODC)</dc:publisher>
    <skos:scopeNote xml:lang="en">manufacturer:Sea-Bird Electronics Inc.</skos:scopeNote>
  </rdf:Description>
  <rdf:Description rdf:about="http://vocab.nerc.ac.uk/collection/L22/current/TOOL0173">
    <rdf:type rdf:resource="http://www.w3.org/2004/02/skos/core#Concept" />
    <skos:prefLabel xml:lang="en">Falmouth Scientific Instruments NXIC CTD</skos:prefLabel>
    <skos:inScheme rdf:resource="http://vocab.aodn.org.au/def/instrument/1" />
    <dcterms:created rdf:datatype="http://www.w3.org/2001/XMLSchema#dateTime">2014-02-07T00:00:00Z</dcterms:created>
    <skos:definition xml:lang="en">A collection of sensors which are generally linked to a common data logger that samples at up to 15Hz. Parameters are measured to an accuracy of ±0.0002 S/m for conductivity, ±0.005°C for temperature and 0.08% for full scale pressure. Now marketed by Teledyne RD Instruments.</skos:definition>
    <dc:source>(L221) SeaVoX Device Catalogue</dc:source>
    <dc:publisher>British Oceanographic Data Centre (BODC)</dc:publisher>
    <skos:scopeNote xml:lang="en">manufacturer:Falmouth Scientific Inc.</skos:scopeNote>
  </rdf:Description>
  <rdf:Description rdf:about="http://vocab.nerc.ac.uk/collection/L22/current/TOOL0869/">
    <rdf:type rdf:resource="http://www.w3.org/2004/02/skos/core#Concept" />
    <skos:prefLabel xml:lang="en">Sea-Bird SBE 37-SMP-ODO MicroCAT C-T-ODO</skos:prefLabel>
    <skos:altLabel xml:lang="en">SBE 37-SMP-ODO MicroCAT</skos:altLabel>
    <skos:inScheme rdf:resource="http://vocab.aodn.org.au/def/instrument/1" />
    <dcterms:created rdf:datatype="http://www.w3.org/2001/XMLSchema#dateTime">2015-06-03T00:00:00Z</dcterms:created>
    <skos:definition xml:lang="en">The SBE 37 MicroCAT is a high accuracy conductivity and temperature recorder with an optional pressure sensor and an Optical Dissolved Oxygen (ODO) sensor designed for deployment on moorings. It is available with either a plastic (rated to 350m) or titanium (rated to 6000m) housing and has an internal pump to improve conductivity and oxygen response. Bio-fouling protection is provided by expendable anti-foulant devices, pump flow path and pumping regimen.</skos:definition>
    <dc:source>(L221) SeaVoX Device Catalogue</dc:source>
    <dc:publisher>British Oceanographic Data Centre (BODC)</dc:publisher>
    <dcterms:modified rdf:datatype="http://www.w3.org/2001/XMLSchema#dateTime">2015-06-10T02:11:20Z</dcterms:modified>
  </rdf:Description>
  <rdf:Description rdf:about="http://vocab.nerc.ac.uk/collection/L22/current/TOOL0675">
    <rdf:type rdf:resource="http://www.w3.org/2004/02/skos/core#Concept" />
    <skos:prefLabel xml:lang="en">WETLabs Water Quality Monitor</skos:prefLabel>
    <dcterms:created rdf:datatype="http://www.w3.org/2001/XMLSchema#dateTime">2014-04-01T00:00:00Z</dcterms:created>
    <skos:definition xml:lang="en">An instrument that incorporates WET Labs fluorometer-turbidity and Sea-Bird's CTD sensors, providing temperature, salinity, depth, dissolved oxygen, chlorophyll fluorescence, turbidity and backscattering data. It is designed for long-term deployment in coastal waters with protection against biofouling and fouling by sediment loads. More information is available at http://www.wetlabs.com/wqm.</skos:definition>
    <dc:source>(L221) SeaVoX Device Catalogue</dc:source>
    <dc:publisher>British Oceanographic Data Centre (BODC)</dc:publisher>
    <skos:inScheme rdf:resource="http://vocab.aodn.org.au/def/instrument/1" />
    <skos:scopeNote xml:lang="en">manufacture:WETLabs Inc.</skos:scopeNote>
  </rdf:Description>
  <rdf:Description rdf:about="http://vocab.nerc.ac.uk/collection/L22/current/TOOL0019">
    <rdf:type rdf:resource="http://www.w3.org/2004/02/skos/core#Concept" />
    <skos:prefLabel xml:lang="en">Sea-Bird SBE 37-IMP MicroCAT C-T Sensor</skos:prefLabel>
    <dcterms:created rdf:datatype="http://www.w3.org/2001/XMLSchema#dateTime">2014-02-17T00:00:00Z</dcterms:created>
    <skos:definition xml:lang="en">The SBE 37 MicroCAT is a high accuracy conductivity and temperature recorder with an optional pressure sensor designed for depolyment on moorings. The IMP model has an inductive modem for real-time data transmission plus internal flash memory data storage with an internal pump to improve conductivity response and protection against fouling.</skos:definition>
    <dc:source>(L221) SeaVoX Device Catalogue</dc:source>
    <dc:publisher>British Oceanographic Data Centre (BODC)</dc:publisher>
    <skos:inScheme rdf:resource="http://vocab.aodn.org.au/def/instrument/1" />
    <skos:scopeNote xml:lang="en">manufacturer:Sea-Bird Electronics Inc.</skos:scopeNote>
  </rdf:Description>
  <rdf:Description rdf:about="http://vocab.nerc.ac.uk/collection/L22/current/TOOL0017">
    <rdf:type rdf:resource="http://www.w3.org/2004/02/skos/core#Concept" />
    <skos:prefLabel xml:lang="en">Sea-Bird SBE 37-SM MicroCAT C-T Sensor</skos:prefLabel>
    <dcterms:created rdf:datatype="http://www.w3.org/2001/XMLSchema#dateTime">2014-02-06T00:00:00Z</dcterms:created>
    <skos:definition xml:lang="en">The SBE 37 MicroCAT is a high accuracy conductivity and temperature recorder with an optional pressure sensor designed for depolyment on moorings. The SM model has a serial interface plus internal flash memory data storage. Further information may be found on the BODC document server at URL http://www.bodc.ac.uk/data/documents/nodb/108613/.</skos:definition>
    <dc:source>(L221) SeaVoX Device Catalogue</dc:source>
    <dc:publisher>British Oceanographic Data Centre (BODC)</dc:publisher>
    <skos:inScheme rdf:resource="http://vocab.aodn.org.au/def/instrument/1" />
    <skos:scopeNote xml:lang="en">manufacturer:Sea-Bird Electronics Inc.</skos:scopeNote>
  </rdf:Description>
  <rdf:Description rdf:about="http://vocab.nerc.ac.uk/collection/L22/current/TOOL0018">
    <rdf:type rdf:resource="http://www.w3.org/2004/02/skos/core#Concept" />
    <skos:prefLabel xml:lang="en">Sea-Bird SBE 37-SMP MicroCAT C-T Sensor</skos:prefLabel>
    <dcterms:created rdf:datatype="http://www.w3.org/2001/XMLSchema#dateTime">2014-02-06T00:00:00Z</dcterms:created>
    <skos:definition xml:lang="en">The SBE 37 MicroCAT is a high accuracy conductivity and temperature recorder with an optional pressure sensor designed for depolyment on moorings. The SMP model has a serial interface plus internal flash memory data storage with an internal pump to improve conductivity response and protection against fouling.</skos:definition>
    <dc:source>(L221) SeaVoX Device Catalogue</dc:source>
    <dc:publisher>British Oceanographic Data Centre (BODC)</dc:publisher>
    <skos:inScheme rdf:resource="http://vocab.aodn.org.au/def/instrument/1" />
    <skos:scopeNote xml:lang="en">manufacturer:Sea-Bird Electronics Inc.</skos:scopeNote>
  </rdf:Description>
  <rdf:Description rdf:about="http://vocab.nerc.ac.uk/collection/L22/current/TOOL0100">
    <rdf:type rdf:resource="http://www.w3.org/2004/02/skos/core#Concept" />
    <skos:prefLabel xml:lang="en">Sea-Bird SBE 16Plus SEACAT C-T Recorder</skos:prefLabel>
    <dcterms:created rdf:datatype="http://www.w3.org/2001/XMLSchema#dateTime">2014-02-07T00:00:00Z</dcterms:created>
    <skos:definition xml:lang="en">The SBE 16plus is a high accuracy conductivity and temperature recorder (pressure optional) with RS232 or RS485 interfaces. It is designed for moorings and other long-duration, fixed-site deployments. The SBE 16plus has 6 amplified A/D input channels and conditioned power of 500 ma is avaliable for auxiliary sensors, dissolved oxygen, turbidity, fluorescence, PAR etc. Further information may be found on the BODC document server at URL: http://www.bodc.ac.uk/data/documents/nodb/153217/ (RS485) or http://www.bodc.ac.uk/data/documents/nodb/158981/ (RS232).</skos:definition>
    <dc:source>(L221) SeaVoX Device Catalogue</dc:source>
    <dc:publisher>British Oceanographic Data Centre (BODC)</dc:publisher>
    <skos:inScheme rdf:resource="http://vocab.aodn.org.au/def/instrument/1" />
    <skos:scopeNote xml:lang="en">manufacturer:Sea-Bird Electronics Inc.</skos:scopeNote>
  </rdf:Description>
  <rdf:Description rdf:about="http://vocab.nerc.ac.uk/collection/L22/current/TOOL0871/">
    <rdf:type rdf:resource="http://www.w3.org/2004/02/skos/core#Concept" />
    <skos:prefLabel xml:lang="en">Sea-Bird SBE 19plus V2 SEACAT CTD</skos:prefLabel>
    <skos:altLabel xml:lang="en">SBE 19+ V2 SEACAT</skos:altLabel>
    <skos:inScheme rdf:resource="http://vocab.aodn.org.au/def/instrument/1" />
    <dcterms:created rdf:datatype="http://www.w3.org/2001/XMLSchema#dateTime">2015-06-03T00:00:00Z</dcterms:created>
    <skos:definition xml:lang="en">Self-contained self-powered CTD profiler. Measures conductivity, temperature and pressure (Digiquartz sensor) in both profiling (samples at 4 scans/sec) and moored (sample rates of once every 5 seconds to once every 9 hours) mode. Available in plastic or titanium housing with depth ranges of 600m and 7000m respectively. Miniature submersible pump provides water to the conductivity cell.  Compared to the previous 19plus, the V2 incorporates an electronics upgrade and additional features, with six differentially amplified A/D input channels, one RS-232 data input channel, and 64 MB FLASH memory.</skos:definition>
    <dc:source>(L221) SeaVoX Device Catalogue</dc:source>
    <dc:publisher>British Oceanographic Data Centre (BODC)</dc:publisher>
    <dcterms:modified rdf:datatype="http://www.w3.org/2001/XMLSchema#dateTime">2015-06-10T02:07:18Z</dcterms:modified>
  </rdf:Description>
  <rdf:Description rdf:about="http://vocab.nerc.ac.uk/collection/L22/current/TOOL0870/">
    <owl:deprecated rdf:datatype="http://www.w3.org/2001/XMLSchema#boolean">true</owl:deprecated>
    <rdfs:label xml:lang="en">Sea-Bird SBE 16Plus V2 SEACAT C-T Recorder</rdfs:label>
    <rdf:type rdf:resource="http://www.w3.org/2004/02/skos/core#Concept" />
    <skos:prefLabel xml:lang="en">Sea-Bird SBE 16Plus V2 SEACAT C-T Recorder</skos:prefLabel>
    <skos:altLabel xml:lang="en">SBE 16+ V2 SEACAT</skos:altLabel>
    <skos:inScheme rdf:resource="http://vocab.aodn.org.au/def/instrument/1" />
    <dcterms:created rdf:datatype="http://www.w3.org/2001/XMLSchema#dateTime">2015-06-03T00:00:00Z</dcterms:created>
    <skos:definition xml:lang="en">The SBE 16plus V2 is a high accuracy conductivity and temperature recorder (pressure optional) with RS232 or RS485 interfaces. It is designed for moorings and other long-duration, fixed-site deployments. It has 6 amplified A/D input channels and conditioned power of 500 ma is available for auxiliary sensors, dissolved oxygen, turbidity, fluorescence, PAR etc. Compared to the previous 16plus, the V2 incorporates an electronics upgrade and additional features, with six differentially amplified A/D input channels, one RS-232 data input channel, and 64 MB FLASH memory. Data can be output in XML as well as ASCII and HEX formats. Firmware upgrades can be downloaded through the communications port, without opening the instrument.</skos:definition>
    <dc:source>(L221) SeaVoX Device Catalogue</dc:source>
    <dc:publisher>British Oceanographic Data Centre (BODC)</dc:publisher>
    <dcterms:modified rdf:datatype="http://www.w3.org/2001/XMLSchema#dateTime">2015-06-10T01:18:45Z</dcterms:modified>
  </rdf:Description>
  <rdf:Description rdf:about="http://vocab.nerc.ac.uk/collection/L22/current/TOOL0446">
    <rdf:type rdf:resource="http://www.w3.org/2004/02/skos/core#Concept" />
    <skos:prefLabel xml:lang="en">SMRU CTD Satellite Relay Data Logger</skos:prefLabel>
    <skos:inScheme rdf:resource="http://vocab.aodn.org.au/def/instrument/1" />
    <dcterms:created rdf:datatype="http://www.w3.org/2001/XMLSchema#dateTime">2013-10-10T00:00:00Z</dcterms:created>
    <skos:definition xml:lang="en">This tag provides oceanographic quality Conductivity/Temperature/Depth casts. Oceanographic quality temperature &amp; salinity profiles (4 - 12 profiles per day), CTD data automatically submitted to the GTS in near real-time. Up to 50,000 full length Argos data transmissions and pressure-proof to 2000m.  Retains a continuous record of depth readings (4 sec sample rate), which can be retrieved by bluetooth link if the tag is recovered. Also records all individual temperature and salinity measurements (1 Hz) made during profiling. Longevity: up to one year. Size: 10.5 x 7 x 4 cm. Weight: 545 g.</skos:definition>
    <dc:source>(L221) SeaVoX Device Catalogue</dc:source>
    <dc:publisher>British Oceanographic Data Centre (BODC)</dc:publisher>
    <skos:scopeNote xml:lang="en">manufacturer:SMRU Instrumentation</skos:scopeNote>
  </rdf:Description>
  <rdf:Description rdf:about="http://vocab.nerc.ac.uk/collection/L22/current/TOOL0190">
    <rdf:type rdf:resource="http://www.w3.org/2004/02/skos/core#Concept" />
    <skos:prefLabel xml:lang="en">Sea-Bird SBE 45 MicroTSG thermosalinograph</skos:prefLabel>
    <skos:inScheme rdf:resource="http://vocab.aodn.org.au/def/instrument/1" />
    <dcterms:created rdf:datatype="http://www.w3.org/2001/XMLSchema#dateTime">2013-10-08T00:00:00Z</dcterms:created>
    <skos:definition xml:lang="en">A small externally powered, high-accuracy instrument, designed for shipboard determination of sea surface (pumped-water) conductivity and temperature. It is constructed of plastic and titanium to ensure long life with minimum maintenance. It may optionally be interfaced to an external SBE 38 hull temperature sensor.</skos:definition>
    <dc:source>(L221) SeaVoX Device Catalogue</dc:source>
    <dc:publisher>British Oceanographic Data Centre (BODC)</dc:publisher>
    <skos:scopeNote xml:lang="en">manufacturer:Sea-Bird Electronics Inc.</skos:scopeNote>
  </rdf:Description>
  <rdf:Description rdf:about="http://vocab.nerc.ac.uk/collection/L22/current/TOOL0058">
    <rdf:type rdf:resource="http://www.w3.org/2004/02/skos/core#Concept" />
    <skos:prefLabel xml:lang="en">Sea-Bird SBE 911plus CTD</skos:prefLabel>
    <skos:inScheme rdf:resource="http://vocab.aodn.org.au/def/instrument/1" />
    <dcterms:created rdf:datatype="http://www.w3.org/2001/XMLSchema#dateTime">2014-07-14T00:00:00Z</dcterms:created>
    <skos:definition xml:lang="en">High precision and accuracy CTD comprising an SBE 9plus underwater unit (SBE 3 temperature and SBE 4 conductivity sensors) and an SBE 11plus deck unit. Sensors may be connected to a pump-fed plastic tubing circuit (usually temperature, salinity and oxygen) or stand-alone. All instruments (8 channels available) on the package are logged by the SBE 11. The unit is the production off the shelf version of the SBE 911 (each 911 was custom built to individual specification).</skos:definition>
    <dc:source>(L221) SeaVoX Device Catalogue</dc:source>
    <dc:publisher>British Oceanographic Data Centre (BODC)</dc:publisher>
  </rdf:Description>
  <rdf:Description rdf:about="http://vocab.nerc.ac.uk/collection/L22/current/TOOL0053">
    <rdf:type rdf:resource="http://www.w3.org/2004/02/skos/core#Concept" />
    <skos:prefLabel xml:lang="en">RBR XR-420 CTD Marine</skos:prefLabel>
    <dcterms:created rdf:datatype="http://www.w3.org/2001/XMLSchema#dateTime">2014-02-17T00:00:00Z</dcterms:created>
    <skos:definition xml:lang="en">A small autonomous data logger designed to monitor conductivity, temperature and depth. Conductivity (accuracy ± 0.003 mS/cm) is measured using a 3-coil closed loop feedback inductive cell for superior temperature compensation. The thermistor (Themometrics) used to record temperature (accuracy ± 0.002°C) is aged and hermetically sealed in the tip of a shock resistant solid glass rod. Pressure (accuracy 0.05% full scale) sensors use reliable semiconductor technology and 316 stainless steel housing developed for long-term stability in harsh environments.</skos:definition>
    <dc:source>(L221) SeaVoX Device Catalogue</dc:source>
    <dc:publisher>British Oceanographic Data Centre (BODC)</dc:publisher>
    <skos:inScheme rdf:resource="http://vocab.aodn.org.au/def/instrument/1" />
    <skos:scopeNote xml:lang="en">manufacturer: RBR</skos:scopeNote>
  </rdf:Description>
  <rdf:Description rdf:about="http://vocab.nerc.ac.uk/collection/L22/current/TOOL0720">
    <rdf:type rdf:resource="http://www.w3.org/2004/02/skos/core#Concept" />
    <skos:prefLabel xml:lang="en">SMRU Ltd CTD/Fluorometer Satellite Relay Data Logger</skos:prefLabel>
    <skos:inScheme rdf:resource="http://vocab.aodn.org.au/def/instrument/1" />
    <dcterms:created rdf:datatype="http://www.w3.org/2001/XMLSchema#dateTime">2013-10-10T00:00:00Z</dcterms:created>
    <skos:definition xml:lang="en">A package comprising a Valeport CTD sensor head plus a customised Turner Cyclops-7 fluorometer combined with an RF unit and antenna suitable for transmission of data via the Argos satellite system. The unit contains an internal battery and a microprocessor that logs data and schedules the transfer of data. The package is designed for attachment to marine mammals and has an operational depth range of down to 2000 m. CTD accuracy is 0.005 C (temperature), 0.01 mS/cm (conductivity) and 2 dBar (pressure).  It is built and calibrated at Valeport Ltd, while SMRU Ltd, the commercial arm of the Sea Mammal Research Unit of the University of St Andrews, is responsible for its distribution, and for streaming and processing the data. More information is available at http://www.smru.st-and.ac.uk/Instrumentation/FluorometryTag/.</skos:definition>
    <dc:source>(L221) SeaVoX Device Catalogue</dc:source>
    <dc:publisher>British Oceanographic Data Centre (BODC)</dc:publisher>
    <skos:scopeNote xml:lang="en">manufacturer:SMRU Instrumentation</skos:scopeNote>
  </rdf:Description>
  <rdf:Description rdf:about="http://vocab.nerc.ac.uk/collection/L05/current/304">
    <rdf:type rdf:resource="http://www.w3.org/2004/02/skos/core#Concept" />
    <skos:prefLabel xml:lang="en">ocean colour radiometers</skos:prefLabel>
    <skos:topConceptOf rdf:resource="http://vocab.aodn.org.au/def/instrument/1" />
    <skos:inScheme rdf:resource="http://vocab.aodn.org.au/def/instrument/1" />
    <dcterms:created rdf:datatype="http://www.w3.org/2001/XMLSchema#dateTime">2013-09-24T00:00:00Z</dcterms:created>
    <skos:definition xml:lang="en">Sensors that measure the intensity and nature of electromagnetic radiation in a manner optimised for the determination of ocean chlorophyll concentration.</skos:definition>
    <dc:source>(L051) SeaDataNet device categories</dc:source>
    <dc:publisher>British Oceanographic Data Centre (BODC)</dc:publisher>
  </rdf:Description>
  <rdf:Description rdf:about="http://vocab.nerc.ac.uk/collection/L05/current/305">
    <rdf:type rdf:resource="http://www.w3.org/2004/02/skos/core#Concept" />
    <skos:prefLabel xml:lang="en">scatterometers</skos:prefLabel>
    <skos:topConceptOf rdf:resource="http://vocab.aodn.org.au/def/instrument/1" />
    <skos:inScheme rdf:resource="http://vocab.aodn.org.au/def/instrument/1" />
    <dcterms:created rdf:datatype="http://www.w3.org/2001/XMLSchema#dateTime">2014-05-22T00:00:00Z</dcterms:created>
    <skos:definition xml:lang="en">Sensors that measure the reflection or scattering effect produced while scanning the surface of the earth. Primarily used to measure near surface winds over the oceans.</skos:definition>
    <dc:source>(L051) SeaDataNet device categories</dc:source>
    <dc:publisher>British Oceanographic Data Centre (BODC)</dc:publisher>
  </rdf:Description>
  <rdf:Description rdf:about="http://vocab.nerc.ac.uk/collection/L05/current/351">
    <rdf:type rdf:resource="http://www.w3.org/2004/02/skos/core#Concept" />
    <skos:prefLabel xml:lang="en">dissolved gas sensors</skos:prefLabel>
    <skos:topConceptOf rdf:resource="http://vocab.aodn.org.au/def/instrument/1" />
    <skos:inScheme rdf:resource="http://vocab.aodn.org.au/def/instrument/1" />
    <dcterms:created rdf:datatype="http://www.w3.org/2001/XMLSchema#dateTime">2013-03-28T00:00:00Z</dcterms:created>
    <skos:definition xml:lang="en">Instrument that measures the concentration of gases generally oxygen dissolved in the water column</skos:definition>
    <dc:source>(L051) SeaDataNet device categories</dc:source>
    <dc:publisher>British Oceanographic Data Centre (BODC)</dc:publisher>
    <skos:narrower rdf:resource="http://vocab.nerc.ac.uk/collection/L22/current/TOOL0805" />
    <skos:narrower rdf:resource="http://vocab.nerc.ac.uk/collection/L22/current/TOOL0036" />
    <skos:narrower rdf:resource="http://vocab.nerc.ac.uk/collection/L22/current/TOOL0037" />
    <skos:narrower rdf:resource="http://vocab.nerc.ac.uk/collection/L22/current/TOOL0369" />
    <skos:narrower rdf:resource="http://vocab.nerc.ac.uk/collection/L22/current/TOOL0675" />
    <skos:narrower rdf:resource="http://vocab.nerc.ac.uk/collection/L22/current/TOOL0679" />
    <skos:narrower rdf:resource="http://vocab.nerc.ac.uk/collection/L22/current/TOOL0724" />
    <skos:narrower rdf:resource="http://vocab.nerc.ac.uk/collection/L22/current/TOOL0739" />
    <skos:narrower rdf:resource="http://vocab.nerc.ac.uk/collection/L22/current/TOOL0869/" />
    <dcterms:contributor>Natalia_Atkins</dcterms:contributor>
    <dcterms:modified rdf:datatype="http://www.w3.org/2001/XMLSchema#dateTime">2015-07-08T04:08:18Z</dcterms:modified>
    <skos:narrower rdf:resource="http://vocab.nerc.ac.uk/collection/L22/current/TOOL0878/" />
  </rdf:Description>
  <rdf:Description rdf:about="http://vocab.nerc.ac.uk/collection/L22/current/TOOL0805">
    <rdf:type rdf:resource="http://www.w3.org/2004/02/skos/core#Concept" />
    <skos:prefLabel xml:lang="en">Aanderaa optode</skos:prefLabel>
    <skos:inScheme rdf:resource="http://vocab.aodn.org.au/def/instrument/1" />
    <dcterms:created rdf:datatype="http://www.w3.org/2001/XMLSchema#dateTime">2013-09-09T00:00:00Z</dcterms:created>
    <skos:definition xml:lang="en">A generic label for a range of dissolved oxygen sensors produced by Aanderaa covering various mounting options. Each has a specific model number but in this case it is not known. All make measurements based on the ability of selected substances to act as dynamic fluorescence quenchers. The fluorescent indicator is a special platinum porphyrin complex embedded in a gas permeable foil that is exposed to the surrounding water. A black optical isolation coating protects the complex from sunlight and fluorescent particles in the water. This sensing foil is attached to a window providing optical access for the measuring system from inside a watertight titanium housing.The foil is excited by modulated blue light, and the phase of a returned red light is measured. By linearizing and temperature compensating, with an incorporated temperature sensor, the absolute O2 concentration can be determined.</skos:definition>
    <dc:source>(L221) SeaVoX Device Catalogue</dc:source>
    <dc:publisher>British Oceanographic Data Centre (BODC)</dc:publisher>
    <skos:scopeNote xml:lang="en">manufacturer:Aanderaa Data Instruments</skos:scopeNote>
  </rdf:Description>
  <rdf:Description rdf:about="http://vocab.nerc.ac.uk/collection/L22/current/TOOL0679">
    <rdf:type rdf:resource="http://www.w3.org/2004/02/skos/core#Concept" />
    <skos:prefLabel xml:lang="en">Pro Oceanus GTD-Pro dissolved gas sensor</skos:prefLabel>
    <skos:inScheme rdf:resource="http://vocab.aodn.org.au/def/instrument/1" />
    <dcterms:created rdf:datatype="http://www.w3.org/2001/XMLSchema#dateTime">2014-06-04T00:00:00Z</dcterms:created>
    <skos:definition xml:lang="en">In-situ dissolved gas sensor measuring the sum of the partial pressures of all dissolved gases, i.e. gas tension.</skos:definition>
    <dc:source>(L221) SeaVoX Device Catalogue</dc:source>
    <dc:publisher>British Oceanographic Data Centre (BODC)</dc:publisher>
  </rdf:Description>
  <rdf:Description rdf:about="http://vocab.nerc.ac.uk/collection/L22/current/TOOL0869/">
    <rdf:type rdf:resource="http://www.w3.org/2004/02/skos/core#Concept" />
    <skos:prefLabel xml:lang="en">Sea-Bird SBE 37-SMP-ODO MicroCAT C-T-ODO</skos:prefLabel>
    <skos:altLabel xml:lang="en">SBE 37-SMP-ODO MicroCAT</skos:altLabel>
    <skos:inScheme rdf:resource="http://vocab.aodn.org.au/def/instrument/1" />
    <dcterms:created rdf:datatype="http://www.w3.org/2001/XMLSchema#dateTime">2015-06-03T00:00:00Z</dcterms:created>
    <skos:definition xml:lang="en">The SBE 37 MicroCAT is a high accuracy conductivity and temperature recorder with an optional pressure sensor and an Optical Dissolved Oxygen (ODO) sensor designed for deployment on moorings. It is available with either a plastic (rated to 350m) or titanium (rated to 6000m) housing and has an internal pump to improve conductivity and oxygen response. Bio-fouling protection is provided by expendable anti-foulant devices, pump flow path and pumping regimen.</skos:definition>
    <dc:source>(L221) SeaVoX Device Catalogue</dc:source>
    <dc:publisher>British Oceanographic Data Centre (BODC)</dc:publisher>
    <dcterms:modified rdf:datatype="http://www.w3.org/2001/XMLSchema#dateTime">2015-06-10T02:11:20Z</dcterms:modified>
  </rdf:Description>
  <rdf:Description rdf:about="http://vocab.nerc.ac.uk/collection/L22/current/TOOL0675">
    <rdf:type rdf:resource="http://www.w3.org/2004/02/skos/core#Concept" />
    <skos:prefLabel xml:lang="en">WETLabs Water Quality Monitor</skos:prefLabel>
    <dcterms:created rdf:datatype="http://www.w3.org/2001/XMLSchema#dateTime">2014-04-01T00:00:00Z</dcterms:created>
    <skos:definition xml:lang="en">An instrument that incorporates WET Labs fluorometer-turbidity and Sea-Bird's CTD sensors, providing temperature, salinity, depth, dissolved oxygen, chlorophyll fluorescence, turbidity and backscattering data. It is designed for long-term deployment in coastal waters with protection against biofouling and fouling by sediment loads. More information is available at http://www.wetlabs.com/wqm.</skos:definition>
    <dc:source>(L221) SeaVoX Device Catalogue</dc:source>
    <dc:publisher>British Oceanographic Data Centre (BODC)</dc:publisher>
    <skos:inScheme rdf:resource="http://vocab.aodn.org.au/def/instrument/1" />
    <skos:scopeNote xml:lang="en">manufacture:WETLabs Inc.</skos:scopeNote>
  </rdf:Description>
  <rdf:Description rdf:about="http://vocab.nerc.ac.uk/collection/L22/current/TOOL0036">
    <rdf:type rdf:resource="http://www.w3.org/2004/02/skos/core#Concept" />
    <skos:prefLabel xml:lang="en">Sea-Bird SBE 43 Dissolved Oxygen sensor</skos:prefLabel>
    <skos:inScheme rdf:resource="http://vocab.aodn.org.au/def/instrument/1" />
    <dcterms:created rdf:datatype="http://www.w3.org/2001/XMLSchema#dateTime">2013-09-09T00:00:00Z</dcterms:created>
    <skos:definition xml:lang="en">High performance through-flow Clark polarographic membrane sensor designed to be plumbed in to a Sea-Bird underwater unit pumped water supply on a profiling CTD package. Designed specifically to give rapid temperature response and minimal pressure hysteresis. Signal output is voltage based to interface to a CTD deck unit.</skos:definition>
    <dc:source>(L221) SeaVoX Device Catalogue</dc:source>
    <dc:publisher>British Oceanographic Data Centre (BODC)</dc:publisher>
    <skos:scopeNote xml:lang="en">manufacturer:Sea-Bird Electronics Inc.</skos:scopeNote>
  </rdf:Description>
  <rdf:Description rdf:about="http://vocab.nerc.ac.uk/collection/L22/current/TOOL0369">
    <rdf:type rdf:resource="http://www.w3.org/2004/02/skos/core#Concept" />
    <skos:prefLabel xml:lang="en">Aanderaa Oxygen Optode 3975</skos:prefLabel>
    <skos:inScheme rdf:resource="http://vocab.aodn.org.au/def/instrument/1" />
    <dcterms:created rdf:datatype="http://www.w3.org/2001/XMLSchema#dateTime">2014-02-06T00:00:00Z</dcterms:created>
    <skos:definition xml:lang="en">A dissolved oxygen sensor which provides analogue output to third party data loggers. Measurement is based on the ability of selected substances to act as dynamic fluorescence quenchers. The fluorescent indicator is a special platinum porphyrin complex embedded in a gas permeable foil that is exposed to the surrounding water. A black optical isolation coating protects the complex from sunlight and fluorescent particles in the water. This sensing foil is attached to a window providing optical access for the measuring system from inside a watertight titanium housing.The foil is excited by modulated blue light, and the phase of a returned red light is measured. By linearizing and temperature compensating, with an incorporated temperature sensor, the absolute O2 concentration can be determined.</skos:definition>
    <dc:source>(L221) SeaVoX Device Catalogue</dc:source>
    <dc:publisher>British Oceanographic Data Centre (BODC)</dc:publisher>
    <skos:scopeNote xml:lang="en">manufacturer:Aanderaa Data Instruments</skos:scopeNote>
  </rdf:Description>
  <rdf:Description rdf:about="http://vocab.nerc.ac.uk/collection/L22/current/TOOL0037">
    <rdf:type rdf:resource="http://www.w3.org/2004/02/skos/core#Concept" />
    <skos:prefLabel xml:lang="en">Sea-Bird SBE 43F Dissolved Oxygen Sensor</skos:prefLabel>
    <skos:inScheme rdf:resource="http://vocab.aodn.org.au/def/instrument/1" />
    <dcterms:created rdf:datatype="http://www.w3.org/2001/XMLSchema#dateTime">2014-02-26T00:00:00Z</dcterms:created>
    <skos:definition xml:lang="en">High performance through-flow Clark polarographic membrane sensor designed to be interfaced to an SBE 52-MP profiling moored CTD or integrated into OEM moorings. Designed specifically to give rapid temperature response and minimal pressure hysteresis. Signal output is frequency based.</skos:definition>
    <dc:source>(L221) SeaVoX Device Catalogue</dc:source>
    <dc:publisher>British Oceanographic Data Centre (BODC)</dc:publisher>
    <skos:scopeNote xml:lang="en">manufacturer:Sea-Bird Electronics Inc.</skos:scopeNote>
  </rdf:Description>
  <rdf:Description rdf:about="http://vocab.nerc.ac.uk/collection/L22/current/TOOL0739">
    <owl:deprecated rdf:datatype="http://www.w3.org/2001/XMLSchema#boolean">true</owl:deprecated>
    <rdfs:label xml:lang="en">Sea-Bird SBE 63 dissolved oxygen sensor</rdfs:label>
    <rdf:type rdf:resource="http://www.w3.org/2004/02/skos/core#Concept" />
    <skos:prefLabel xml:lang="en">Sea-Bird SBE 63 dissolved oxygen sensor</skos:prefLabel>
    <skos:altLabel xml:lang="en">Sea-Bird SBE 63 DO</skos:altLabel>
    <skos:inScheme rdf:resource="http://vocab.aodn.org.au/def/instrument/1" />
    <dcterms:created rdf:datatype="http://www.w3.org/2001/XMLSchema#dateTime">2013-03-28T00:00:00Z</dcterms:created>
    <skos:definition xml:lang="en">An optode dissolved oxygen sensor mounted in plastic (600m operating depth) or titanium (7000m operating depth) housing that interfaces through an RS-232 connection to SeaCAT  or MicroCAT CTDs or Navis Argo float. Accuracy is the greater of 3 micromole/kg or 2%. More information is available at http://www.seabird.com/products/spec_sheets/63data.htm.</skos:definition>
    <dc:source>(L221) SeaVoX Device Catalogue</dc:source>
    <dc:publisher>British Oceanographic Data Centre (BODC)</dc:publisher>
  </rdf:Description>
  <rdf:Description rdf:about="http://vocab.nerc.ac.uk/collection/L22/current/TOOL0724">
    <rdf:type rdf:resource="http://www.w3.org/2004/02/skos/core#Concept" />
    <skos:prefLabel xml:lang="en">General Oceanics model 8050 pCO2 measuring system</skos:prefLabel>
    <skos:inScheme rdf:resource="http://vocab.aodn.org.au/def/instrument/1" />
    <dcterms:created rdf:datatype="http://www.w3.org/2001/XMLSchema#dateTime">2013-10-08T00:00:00Z</dcterms:created>
    <skos:definition xml:lang="en">The General Oceanics model 8050 pCO2 Measuring System is an autonomous analytical system for measuring carbon dioxide in surface water. It includes a headspace equilibrator, an infrared CO2 analyser, and computer-controlled and -monitored pumps. It measures: pressure (flow) in range 0 to 10 dbar, with accuracy of 0.2 percent and resolution of 0.03 percent; temperature in range -3 to 50 degC, with accuracy of 0.003 percent and resolution of 0.0005 degC; conductivity in range 0 to 64 mS/cm, with accuracy of 0.003 mS/cm and resolution of 0.001 mS/cm; Oxygen in range 0 to 25ppm (250 percent saturation), with accuracy of 0.1ppm (1 percent saturation) and 0.01ppm (0.1 percent saturation); pH in range 0 to 0.14 pH, with accuracy of 0.01 pH and resolution of 0.001 pH; Redox in range -1000 to 1000 mV, with accuracy of 1 mV and resolution of 0.1 mV.</skos:definition>
    <dc:source>(L221) SeaVoX Device Catalogue</dc:source>
    <dc:publisher>British Oceanographic Data Centre (BODC)</dc:publisher>
    <skos:scopeNote xml:lang="en">manufacturer:General Oceanics</skos:scopeNote>
  </rdf:Description>
  <rdf:Description rdf:about="http://vocab.nerc.ac.uk/collection/L22/current/TOOL0878/">
    <owl:deprecated rdf:datatype="http://www.w3.org/2001/XMLSchema#boolean">true</owl:deprecated>
    <rdfs:label xml:lang="en">Battele Seaology pCO2 monitoring system</rdfs:label>
    <rdf:type rdf:resource="http://www.w3.org/2004/02/skos/core#Concept" />
    <skos:prefLabel xml:lang="en">Battele Seaology pCO2 monitoring system</skos:prefLabel>
    <skos:altLabel xml:lang="en">Battele pCO2</skos:altLabel>
    <skos:inScheme rdf:resource="http://vocab.aodn.org.au/def/instrument/1" />
    <dcterms:created rdf:datatype="http://www.w3.org/2001/XMLSchema#dateTime">2015-06-03T00:00:00Z</dcterms:created>
    <skos:definition xml:lang="en">An autonomous air and water pCO2 monitoring device comprising an equilibrator to extract diffused gases from seawater, an air block that collects an air sample whilst excluding seawater and a non-dispersive infrared (NDIR) carbon dioxide detector. These are designed to be mounted in a surface buoy (moored or drifting) with a power source (battery and solar), a stock of calibration standard gas, a control system, satellite communications including GPS and data storage. It has a measurement range of 100 to 600 ppm and precision of about 1 ppm.More information at http://battelle.org/our-work/national-security/maritime-technologies/sensors/battelle-seaology/battelle-pco2-monitoring-system#sthash.qWbxMCsQ.dpuf.</skos:definition>
    <dc:publisher>British Oceanographic Data Centre (BODC)</dc:publisher>
    <dcterms:modified rdf:datatype="http://www.w3.org/2001/XMLSchema#dateTime">2015-07-08T04:08:18Z</dcterms:modified>
    <dcterms:contributor>Natalia_Atkins</dcterms:contributor>
  </rdf:Description>
  <rdf:Description rdf:about="http://vocab.nerc.ac.uk/collection/L05/current/306">
    <rdf:type rdf:resource="http://www.w3.org/2004/02/skos/core#Concept" />
    <skos:prefLabel xml:lang="en">synthetic aperture radars</skos:prefLabel>
    <skos:topConceptOf rdf:resource="http://vocab.aodn.org.au/def/instrument/1" />
    <skos:inScheme rdf:resource="http://vocab.aodn.org.au/def/instrument/1" />
    <dcterms:created rdf:datatype="http://www.w3.org/2001/XMLSchema#dateTime">2014-05-22T00:00:00Z</dcterms:created>
    <skos:definition xml:lang="en">Instruments that generate maps of radar reflectivity through the synthesis of multiple pulses from a moving platform.</skos:definition>
    <dc:source>(L051) SeaDataNet device categories</dc:source>
    <dc:publisher>British Oceanographic Data Centre (BODC)</dc:publisher>
  </rdf:Description>
  <rdf:Description rdf:about="http://vocab.nerc.ac.uk/collection/L05/current/353">
    <rdf:type rdf:resource="http://www.w3.org/2004/02/skos/core#Concept" />
    <skos:prefLabel xml:lang="en">active fluorometers</skos:prefLabel>
    <skos:topConceptOf rdf:resource="http://vocab.aodn.org.au/def/instrument/1" />
    <skos:inScheme rdf:resource="http://vocab.aodn.org.au/def/instrument/1" />
    <dcterms:created rdf:datatype="http://www.w3.org/2001/XMLSchema#dateTime">2013-03-28T00:00:00Z</dcterms:created>
    <skos:definition xml:lang="en">Fluorometers that measure photosynthetic parameters by taking measurements whilst manipulating the phytoplankton with controlled high-intensity illumination such as pump and probe and FRRF</skos:definition>
    <dc:source>(L051) SeaDataNet device categories</dc:source>
    <dc:publisher>British Oceanographic Data Centre (BODC)</dc:publisher>
  </rdf:Description>
  <rdf:Description rdf:about="http://vocab.nerc.ac.uk/collection/L05/current/308">
    <rdf:type rdf:resource="http://www.w3.org/2004/02/skos/core#Concept" />
    <skos:prefLabel xml:lang="en">atmospheric radiometers</skos:prefLabel>
    <skos:topConceptOf rdf:resource="http://vocab.aodn.org.au/def/instrument/1" />
    <skos:inScheme rdf:resource="http://vocab.aodn.org.au/def/instrument/1" />
    <dcterms:created rdf:datatype="http://www.w3.org/2001/XMLSchema#dateTime">2014-07-11T00:00:00Z</dcterms:created>
    <skos:definition xml:lang="en">Sensors that measure the intensity an nature of electromagnetic radiation in a manner optimised for the quantification of atmospheric phenomena.</skos:definition>
    <dc:source>(L051) SeaDataNet device categories</dc:source>
    <dc:publisher>British Oceanographic Data Centre (BODC)</dc:publisher>
    <skos:narrower rdf:resource="http://vocab.nerc.ac.uk/collection/L22/current/TOOL0702" />
    <skos:narrower rdf:resource="http://vocab.nerc.ac.uk/collection/L22/current/TOOL0703" />
    <skos:narrower rdf:resource="http://vocab.nerc.ac.uk/collection/L22/current/TOOL0722" />
    <skos:narrower rdf:resource="http://vocab.nerc.ac.uk/collection/L22/current/TOOL0723" />
  </rdf:Description>
  <rdf:Description rdf:about="http://vocab.nerc.ac.uk/collection/L22/current/TOOL0723">
    <rdf:type rdf:resource="http://www.w3.org/2004/02/skos/core#Concept" />
    <skos:prefLabel xml:lang="en">Middleton Solar SK01-DP2 Pyranometer</skos:prefLabel>
    <skos:inScheme rdf:resource="http://vocab.aodn.org.au/def/instrument/1" />
    <dcterms:created rdf:datatype="http://www.w3.org/2001/XMLSchema#dateTime">2013-10-15T00:00:00Z</dcterms:created>
    <skos:definition xml:lang="en">The Middleton SK01-DP2 PAR Sensor (or Quantum Sensor) is for measuring electromagnetic radiation  at Photosynthetically Active wavelengths. It uses a silicon photodiode detector, shielded by a cosine-corrected diffuser and an interference reflector, to measure PAR on a horizontal surface. The detector is boosted by a low noise amplifier that is drift stabilised. The SK01-DP2 features: viewing angle 2*pi steradians; spectral range of 400-700nm; irradiance of 0-3000 umol/s/m2; sensitivity of 0.5 mV/umol/s/m2; response time (to 95 percent) of 30 ms; operating temperature of -35 to 60 degreesC; non-linearity of less than 1 percent; spectral response of +/- 5 percent.</skos:definition>
    <dc:source>(L221) SeaVoX Device Catalogue</dc:source>
    <dc:publisher>British Oceanographic Data Centre (BODC)</dc:publisher>
    <skos:scopeNote xml:lang="en">manufacturer:Middleton Solar</skos:scopeNote>
  </rdf:Description>
  <rdf:Description rdf:about="http://vocab.nerc.ac.uk/collection/L22/current/TOOL0722">
    <rdf:type rdf:resource="http://www.w3.org/2004/02/skos/core#Concept" />
    <skos:prefLabel xml:lang="en">Middleton Solar EQ08 Pyranometer</skos:prefLabel>
    <skos:inScheme rdf:resource="http://vocab.aodn.org.au/def/instrument/1" />
    <dcterms:created rdf:datatype="http://www.w3.org/2001/XMLSchema#dateTime">2013-10-15T00:00:00Z</dcterms:created>
    <skos:definition xml:lang="en">The Middleton EQ08 Solar Pyranometer is designed for the measurement of global solar irradiance on a plane surface. It has a response time (to 95%) of less than 11 seconds; zero offset at 200 W/m2 of less than 3 W/m2 and at 5K/h of less than 2W/m2; non-linearity of less than 0.5 percent; directional response with respect to 1000 W/m2 of less than 15 W/m2, Spectral selectivity (0.35 to 1.5 um) of less than 3 percent; temperature response (for 50K interval) of less than 2 percent; and tilt response (0-90 degrees) of less than 0.35 percent.</skos:definition>
    <dc:source>(L221) SeaVoX Device Catalogue</dc:source>
    <dc:publisher>British Oceanographic Data Centre (BODC)</dc:publisher>
    <skos:scopeNote xml:lang="en">manufacturer:Middleton Solar</skos:scopeNote>
  </rdf:Description>
  <rdf:Description rdf:about="http://vocab.nerc.ac.uk/collection/L22/current/TOOL0703">
    <rdf:type rdf:resource="http://www.w3.org/2004/02/skos/core#Concept" />
    <skos:prefLabel xml:lang="en">Kipp and Zonen CNR1 Net Radiometer</skos:prefLabel>
    <skos:inScheme rdf:resource="http://vocab.aodn.org.au/def/instrument/1" />
    <dcterms:created rdf:datatype="http://www.w3.org/2001/XMLSchema#dateTime">2014-07-11T00:00:00Z</dcterms:created>
    <skos:definition xml:lang="en">The CNR4 is a net radiometer that measures the energy balance between incoming and shortwave IR radiation versus surface reflected shortwave and outgoing longwave IR radiation. The instrument comprises an upward-facing pyranometer/pyrgeometer pair, and a downward facing pair. There is an internal RTD, and a heater to prevent condensation.</skos:definition>
    <dc:source>(L221) SeaVoX Device Catalogue</dc:source>
    <dc:publisher>British Oceanographic Data Centre (BODC)</dc:publisher>
  </rdf:Description>
  <rdf:Description rdf:about="http://vocab.nerc.ac.uk/collection/L22/current/TOOL0702">
    <rdf:type rdf:resource="http://www.w3.org/2004/02/skos/core#Concept" />
    <skos:prefLabel xml:lang="en">Kipp and Zonen CNR4 Net Radiometer</skos:prefLabel>
    <skos:inScheme rdf:resource="http://vocab.aodn.org.au/def/instrument/1" />
    <dcterms:created rdf:datatype="http://www.w3.org/2001/XMLSchema#dateTime">2014-07-11T00:00:00Z</dcterms:created>
    <skos:definition xml:lang="en">The CNR4 is a net radiometer that measures the energy balance between incoming and shortwave IR radiation versus surface reflected shortwave and outgoing longwave IR radiation. The instrument comprises an upward-facing pyranometer/pyrgeometer pair, and a downward facing pair. There is an internal thermisor, an internal Pt-100 RTD, and a solar shield. There is an optional ventilation unit with heater to minimise condensation.</skos:definition>
    <dc:source>(L221) SeaVoX Device Catalogue</dc:source>
    <dc:publisher>British Oceanographic Data Centre (BODC)</dc:publisher>
  </rdf:Description>
  <rdf:Description rdf:about="http://vocab.nerc.ac.uk/collection/L05/current/356">
    <rdf:type rdf:resource="http://www.w3.org/2004/02/skos/core#Concept" />
    <skos:prefLabel xml:lang="en">redox potential sensors</skos:prefLabel>
    <skos:topConceptOf rdf:resource="http://vocab.aodn.org.au/def/instrument/1" />
    <skos:inScheme rdf:resource="http://vocab.aodn.org.au/def/instrument/1" />
    <dcterms:created rdf:datatype="http://www.w3.org/2001/XMLSchema#dateTime">2013-07-18T00:00:00Z</dcterms:created>
    <skos:definition xml:lang="en">Instruments that measure the tendency of the water column to either gain or lose electrons when it is subject to change by introduction of a new species</skos:definition>
    <dc:source>(L051) SeaDataNet device categories</dc:source>
    <dc:publisher>British Oceanographic Data Centre (BODC)</dc:publisher>
  </rdf:Description>
  <rdf:Description rdf:about="http://vocab.nerc.ac.uk/collection/L05/current/355">
    <rdf:type rdf:resource="http://www.w3.org/2004/02/skos/core#Concept" />
    <skos:prefLabel xml:lang="en">pH sensors</skos:prefLabel>
    <skos:topConceptOf rdf:resource="http://vocab.aodn.org.au/def/instrument/1" />
    <skos:inScheme rdf:resource="http://vocab.aodn.org.au/def/instrument/1" />
    <dcterms:created rdf:datatype="http://www.w3.org/2001/XMLSchema#dateTime">2013-07-18T00:00:00Z</dcterms:created>
    <skos:definition xml:lang="en">Instruments that measure the hydrogen ion concentration in the water column</skos:definition>
    <dc:source>(L051) SeaDataNet device categories</dc:source>
    <dc:publisher>British Oceanographic Data Centre (BODC)</dc:publisher>
  </rdf:Description>
  <rdf:Description rdf:about="http://vocab.nerc.ac.uk/collection/L05/current/POS03">
    <rdf:type rdf:resource="http://www.w3.org/2004/02/skos/core#Concept" />
    <skos:prefLabel xml:lang="en">NAVSTAR Global Positioning System receivers</skos:prefLabel>
    <skos:altLabel xml:lang="en">GPS</skos:altLabel>
    <skos:inScheme rdf:resource="http://vocab.aodn.org.au/def/instrument/1" />
    <dcterms:created rdf:datatype="http://www.w3.org/2001/XMLSchema#dateTime">2015-06-03T00:00:00Z</dcterms:created>
    <skos:definition xml:lang="en">Accuracy better than 100m, Global navigation based on a network of satellites deployed and maintained by the USA.</skos:definition>
    <dc:publisher>British Oceanographic Data Centre (BODC)</dc:publisher>
    <skos:narrower rdf:resource="http://vocab.nerc.ac.uk/collection/L22/current/TOOL0873/" />
    <dcterms:modified rdf:datatype="http://www.w3.org/2001/XMLSchema#dateTime">2015-07-08T04:07:04Z</dcterms:modified>
    <dcterms:contributor>Natalia_Atkins</dcterms:contributor>
    <skos:narrower rdf:resource="http://vocab.nerc.ac.uk/collection/L22/current/TOOL0878/" />
  </rdf:Description>
  <rdf:Description rdf:about="http://vocab.nerc.ac.uk/collection/L22/current/TOOL0878/">
    <owl:deprecated rdf:datatype="http://www.w3.org/2001/XMLSchema#boolean">true</owl:deprecated>
    <rdfs:label xml:lang="en">Battele Seaology pCO2 monitoring system</rdfs:label>
    <rdf:type rdf:resource="http://www.w3.org/2004/02/skos/core#Concept" />
    <skos:prefLabel xml:lang="en">Battele Seaology pCO2 monitoring system</skos:prefLabel>
    <skos:altLabel xml:lang="en">Battele pCO2</skos:altLabel>
    <skos:inScheme rdf:resource="http://vocab.aodn.org.au/def/instrument/1" />
    <dcterms:created rdf:datatype="http://www.w3.org/2001/XMLSchema#dateTime">2015-06-03T00:00:00Z</dcterms:created>
    <skos:definition xml:lang="en">An autonomous air and water pCO2 monitoring device comprising an equilibrator to extract diffused gases from seawater, an air block that collects an air sample whilst excluding seawater and a non-dispersive infrared (NDIR) carbon dioxide detector. These are designed to be mounted in a surface buoy (moored or drifting) with a power source (battery and solar), a stock of calibration standard gas, a control system, satellite communications including GPS and data storage. It has a measurement range of 100 to 600 ppm and precision of about 1 ppm.More information at http://battelle.org/our-work/national-security/maritime-technologies/sensors/battelle-seaology/battelle-pco2-monitoring-system#sthash.qWbxMCsQ.dpuf.</skos:definition>
    <dc:publisher>British Oceanographic Data Centre (BODC)</dc:publisher>
    <dcterms:modified rdf:datatype="http://www.w3.org/2001/XMLSchema#dateTime">2015-07-08T04:08:18Z</dcterms:modified>
    <dcterms:contributor>Natalia_Atkins</dcterms:contributor>
  </rdf:Description>
  <rdf:Description rdf:about="http://vocab.nerc.ac.uk/collection/L22/current/TOOL0873/">
    <rdf:type rdf:resource="http://www.w3.org/2004/02/skos/core#Concept" />
    <skos:prefLabel xml:lang="en">SMRU GPS Satellite Relay Data Logger (Argos)</skos:prefLabel>
    <skos:altLabel xml:lang="en">SMRU GPS SRDL</skos:altLabel>
    <skos:inScheme rdf:resource="http://vocab.aodn.org.au/def/instrument/1" />
    <dcterms:created rdf:datatype="http://www.w3.org/2001/XMLSchema#dateTime">2015-06-03T00:00:00Z</dcterms:created>
    <skos:definition xml:lang="en">A package comprising a wet/dry, pressure and temperature sensors with a GPS receiver for high accuracy position data and antenna suitable for transmission of data via the Argos satellite system. The unit contains an internal battery and a microprocessor that logs data and schedules the transfer of data.  GPS locations are acquired in less than a second so position may be transferred to the satellite on every surfacing. The package is designed for attachment to marine mammals and has an operational depth range of down to 2000 m. More information is available at http://www.smru.st-and.ac.uk/Instrumentation/GPSArgosTag/.</skos:definition>
    <dc:publisher>British Oceanographic Data Centre (BODC)</dc:publisher>
    <dcterms:modified rdf:datatype="http://www.w3.org/2001/XMLSchema#dateTime">2015-07-01T01:19:54Z</dcterms:modified>
    <dcterms:contributor>Natalia_Atkins</dcterms:contributor>
  </rdf:Description>
  <rdf:Description rdf:about="http://vocab.nerc.ac.uk/collection/L05/current/301">
    <rdf:type rdf:resource="http://www.w3.org/2004/02/skos/core#Concept" />
    <skos:prefLabel xml:lang="en">satellite positioning systems</skos:prefLabel>
    <skos:topConceptOf rdf:resource="http://vocab.aodn.org.au/def/instrument/1" />
    <skos:inScheme rdf:resource="http://vocab.aodn.org.au/def/instrument/1" />
    <dcterms:created rdf:datatype="http://www.w3.org/2001/XMLSchema#dateTime">2013-07-18T00:00:00Z</dcterms:created>
    <skos:definition xml:lang="en">A network of statellites that generate signals that allow a receiver to determine its position such as GPS.</skos:definition>
    <dc:source>(L051) SeaDataNet device categories</dc:source>
    <dc:publisher>British Oceanographic Data Centre (BODC)</dc:publisher>
  </rdf:Description>
  <rdf:Description rdf:about="http://vocab.nerc.ac.uk/collection/L05/current/303">
    <rdf:type rdf:resource="http://www.w3.org/2004/02/skos/core#Concept" />
    <skos:prefLabel xml:lang="en">surface current radars</skos:prefLabel>
    <skos:topConceptOf rdf:resource="http://vocab.aodn.org.au/def/instrument/1" />
    <skos:inScheme rdf:resource="http://vocab.aodn.org.au/def/instrument/1" />
    <dcterms:created rdf:datatype="http://www.w3.org/2001/XMLSchema#dateTime">2013-03-28T00:00:00Z</dcterms:created>
    <skos:definition xml:lang="en">Instruments that measure the speed and direction of sea surface travel by timing reflected radio waves</skos:definition>
    <dc:source>(L051) SeaDataNet device categories</dc:source>
    <dc:publisher>British Oceanographic Data Centre (BODC)</dc:publisher>
  </rdf:Description>
  <rdf:Description rdf:about="http://vocab.nerc.ac.uk/collection/L05/current/383">
    <rdf:type rdf:resource="http://www.w3.org/2004/02/skos/core#Concept" />
    <skos:prefLabel xml:lang="en">metal analysers</skos:prefLabel>
    <skos:topConceptOf rdf:resource="http://vocab.aodn.org.au/def/instrument/1" />
    <skos:inScheme rdf:resource="http://vocab.aodn.org.au/def/instrument/1" />
    <dcterms:created rdf:datatype="http://www.w3.org/2001/XMLSchema#dateTime">2013-03-28T00:00:00Z</dcterms:created>
    <skos:definition xml:lang="en">In-situ instruments that can determine the total dissolved or particulate concentration of one or more metallic elements (including trace metalloids like arsenic) in a water body.</skos:definition>
    <dc:source>(L051) SeaDataNet device categories</dc:source>
    <dc:publisher>British Oceanographic Data Centre (BODC)</dc:publisher>
  </rdf:Description>
  <rdf:Description rdf:about="http://vocab.nerc.ac.uk/collection/L05/current/382">
    <rdf:type rdf:resource="http://www.w3.org/2004/02/skos/core#Concept" />
    <skos:prefLabel xml:lang="en">atmospheric gas analysers</skos:prefLabel>
    <skos:topConceptOf rdf:resource="http://vocab.aodn.org.au/def/instrument/1" />
    <skos:inScheme rdf:resource="http://vocab.aodn.org.au/def/instrument/1" />
    <dcterms:created rdf:datatype="http://www.w3.org/2001/XMLSchema#dateTime">2013-10-08T00:00:00Z</dcterms:created>
    <skos:definition xml:lang="en">In-situ instruments that can determine the proportion of one or more gaseous components of the atmosphere.</skos:definition>
    <dc:source>(L051) SeaDataNet device categories</dc:source>
    <dc:publisher>British Oceanographic Data Centre (BODC)</dc:publisher>
    <skos:narrower rdf:resource="http://vocab.nerc.ac.uk/collection/L22/current/TOOL0705" />
    <skos:narrower rdf:resource="http://vocab.nerc.ac.uk/collection/L22/current/TOOL0724" />
    <dcterms:contributor>Natalia_Atkins</dcterms:contributor>
    <dcterms:modified rdf:datatype="http://www.w3.org/2001/XMLSchema#dateTime">2015-07-08T04:07:58Z</dcterms:modified>
    <skos:narrower rdf:resource="http://vocab.nerc.ac.uk/collection/L22/current/TOOL0878/" />
  </rdf:Description>
  <rdf:Description rdf:about="http://vocab.nerc.ac.uk/collection/L22/current/TOOL0705">
    <rdf:type rdf:resource="http://www.w3.org/2004/02/skos/core#Concept" />
    <skos:prefLabel xml:lang="en">LI-COR LI-7000 CO2/H20 Gas Analyser</skos:prefLabel>
    <skos:inScheme rdf:resource="http://vocab.aodn.org.au/def/instrument/1" />
    <dcterms:created rdf:datatype="http://www.w3.org/2001/XMLSchema#dateTime">2013-10-08T00:00:00Z</dcterms:created>
    <skos:definition xml:lang="en">The LI-7000 is a differential, single source, non-dispersive, infrared gas analyser. Two solid state detectors, one each for CO2 and H2O, filter at 4.255 microns and 2.595 microns respectively. CO2 is measured in the range 0-3000ppm, with accuracy of 1 percent nominally. H2O is measured in the range 0-60 mmol per mol, with accuracy of one 1 percent.</skos:definition>
    <dc:source>(L221) SeaVoX Device Catalogue</dc:source>
    <dc:publisher>British Oceanographic Data Centre (BODC)</dc:publisher>
    <skos:scopeNote xml:lang="en">manufacturer:LI-COR Incorporated</skos:scopeNote>
  </rdf:Description>
  <rdf:Description rdf:about="http://vocab.nerc.ac.uk/collection/L22/current/TOOL0724">
    <rdf:type rdf:resource="http://www.w3.org/2004/02/skos/core#Concept" />
    <skos:prefLabel xml:lang="en">General Oceanics model 8050 pCO2 measuring system</skos:prefLabel>
    <skos:inScheme rdf:resource="http://vocab.aodn.org.au/def/instrument/1" />
    <dcterms:created rdf:datatype="http://www.w3.org/2001/XMLSchema#dateTime">2013-10-08T00:00:00Z</dcterms:created>
    <skos:definition xml:lang="en">The General Oceanics model 8050 pCO2 Measuring System is an autonomous analytical system for measuring carbon dioxide in surface water. It includes a headspace equilibrator, an infrared CO2 analyser, and computer-controlled and -monitored pumps. It measures: pressure (flow) in range 0 to 10 dbar, with accuracy of 0.2 percent and resolution of 0.03 percent; temperature in range -3 to 50 degC, with accuracy of 0.003 percent and resolution of 0.0005 degC; conductivity in range 0 to 64 mS/cm, with accuracy of 0.003 mS/cm and resolution of 0.001 mS/cm; Oxygen in range 0 to 25ppm (250 percent saturation), with accuracy of 0.1ppm (1 percent saturation) and 0.01ppm (0.1 percent saturation); pH in range 0 to 0.14 pH, with accuracy of 0.01 pH and resolution of 0.001 pH; Redox in range -1000 to 1000 mV, with accuracy of 1 mV and resolution of 0.1 mV.</skos:definition>
    <dc:source>(L221) SeaVoX Device Catalogue</dc:source>
    <dc:publisher>British Oceanographic Data Centre (BODC)</dc:publisher>
    <skos:scopeNote xml:lang="en">manufacturer:General Oceanics</skos:scopeNote>
  </rdf:Description>
  <rdf:Description rdf:about="http://vocab.nerc.ac.uk/collection/L22/current/TOOL0878/">
    <owl:deprecated rdf:datatype="http://www.w3.org/2001/XMLSchema#boolean">true</owl:deprecated>
    <rdfs:label xml:lang="en">Battele Seaology pCO2 monitoring system</rdfs:label>
    <rdf:type rdf:resource="http://www.w3.org/2004/02/skos/core#Concept" />
    <skos:prefLabel xml:lang="en">Battele Seaology pCO2 monitoring system</skos:prefLabel>
    <skos:altLabel xml:lang="en">Battele pCO2</skos:altLabel>
    <skos:inScheme rdf:resource="http://vocab.aodn.org.au/def/instrument/1" />
    <dcterms:created rdf:datatype="http://www.w3.org/2001/XMLSchema#dateTime">2015-06-03T00:00:00Z</dcterms:created>
    <skos:definition xml:lang="en">An autonomous air and water pCO2 monitoring device comprising an equilibrator to extract diffused gases from seawater, an air block that collects an air sample whilst excluding seawater and a non-dispersive infrared (NDIR) carbon dioxide detector. These are designed to be mounted in a surface buoy (moored or drifting) with a power source (battery and solar), a stock of calibration standard gas, a control system, satellite communications including GPS and data storage. It has a measurement range of 100 to 600 ppm and precision of about 1 ppm.More information at http://battelle.org/our-work/national-security/maritime-technologies/sensors/battelle-seaology/battelle-pco2-monitoring-system#sthash.qWbxMCsQ.dpuf.</skos:definition>
    <dc:publisher>British Oceanographic Data Centre (BODC)</dc:publisher>
    <dcterms:modified rdf:datatype="http://www.w3.org/2001/XMLSchema#dateTime">2015-07-08T04:08:18Z</dcterms:modified>
    <dcterms:contributor>Natalia_Atkins</dcterms:contributor>
  </rdf:Description>
  <rdf:Description rdf:about="http://vocab.nerc.ac.uk/collection/L05/current/381">
    <rdf:type rdf:resource="http://www.w3.org/2004/02/skos/core#Concept" />
    <skos:prefLabel xml:lang="en">precipitation gauges</skos:prefLabel>
    <skos:topConceptOf rdf:resource="http://vocab.aodn.org.au/def/instrument/1" />
    <skos:inScheme rdf:resource="http://vocab.aodn.org.au/def/instrument/1" />
    <dcterms:created rdf:datatype="http://www.w3.org/2001/XMLSchema#dateTime">2013-03-28T00:00:00Z</dcterms:created>
    <skos:definition xml:lang="en">Instruments that measure either the rate of fall or integrated amount of rain snow sleet hail or graupel.</skos:definition>
    <dc:source>(L051) SeaDataNet device categories</dc:source>
    <dc:publisher>British Oceanographic Data Centre (BODC)</dc:publisher>
    <skos:narrower rdf:resource="http://vocab.nerc.ac.uk/collection/L22/current/TOOL0671" />
    <skos:narrower rdf:resource="http://vocab.nerc.ac.uk/collection/L22/current/TOOL0725" />
  </rdf:Description>
  <rdf:Description rdf:about="http://vocab.nerc.ac.uk/collection/L22/current/TOOL0725">
    <rdf:type rdf:resource="http://www.w3.org/2004/02/skos/core#Concept" />
    <skos:prefLabel xml:lang="en">OSi ORG-815-DR Optical Rain Gauge</skos:prefLabel>
    <skos:inScheme rdf:resource="http://vocab.aodn.org.au/def/instrument/1" />
    <dcterms:created rdf:datatype="http://www.w3.org/2001/XMLSchema#dateTime">2013-10-14T00:00:00Z</dcterms:created>
    <skos:definition xml:lang="en">The OSi ORG-815-DR is an optical scintillation rain gauge that measures rain rate in the range 0.1 to 500 mm/hr; rain accumulation in the range 0.001 to 999.999 mm with accuracy of 5% accumulation and resolution of 0.001 mm. It features RS-232 serial input/output, and operates in temperatures from -40 to 50 degrees C.</skos:definition>
    <dc:source>(L221) SeaVoX Device Catalogue</dc:source>
    <dc:publisher>British Oceanographic Data Centre (BODC)</dc:publisher>
    <skos:scopeNote xml:lang="en">manufacturer:Optical Scientific Inc.</skos:scopeNote>
  </rdf:Description>
  <rdf:Description rdf:about="http://vocab.nerc.ac.uk/collection/L22/current/TOOL0671">
    <rdf:type rdf:resource="http://www.w3.org/2004/02/skos/core#Concept" />
    <skos:prefLabel xml:lang="en">Young 50202 Precipitation Gauge</skos:prefLabel>
    <skos:inScheme rdf:resource="http://vocab.aodn.org.au/def/instrument/1" />
    <dcterms:created rdf:datatype="http://www.w3.org/2001/XMLSchema#dateTime">2013-10-14T00:00:00Z</dcterms:created>
    <skos:definition xml:lang="en">An instrument that accurately measures rain or snow precipitation without moving parts, making it ideal for use on moving platforms such as buoys and ships. Insulated housings and thermostatically controlled heaters permit operation at temperatures below freezing. Precipitation measurement is made with a capacitive transducer and electronic circuit that produce a voltage output. Total precipitation can be tracked by a data logger or recorder. It has an accuracy and threshold of 1mm. More information may be found at http://www.youngusa.com/products/3/17.html.</skos:definition>
    <dc:source>(L221) SeaVoX Device Catalogue</dc:source>
    <dc:publisher>British Oceanographic Data Centre (BODC)</dc:publisher>
    <skos:scopeNote xml:lang="en">manufacturer:R.M. Young Company</skos:scopeNote>
  </rdf:Description>
  <rdf:Description rdf:about="http://vocab.nerc.ac.uk/collection/L05/current/14">
    <rdf:type rdf:resource="http://www.w3.org/2004/02/skos/core#Concept" />
    <skos:prefLabel xml:lang="en">precipitation samplers</skos:prefLabel>
    <skos:topConceptOf rdf:resource="http://vocab.aodn.org.au/def/instrument/1" />
    <skos:inScheme rdf:resource="http://vocab.aodn.org.au/def/instrument/1" />
    <dcterms:created rdf:datatype="http://www.w3.org/2001/XMLSchema#dateTime">2013-03-28T00:00:00Z</dcterms:created>
    <skos:definition xml:lang="en">A device that collects a sample of precipitation (rain hail or snow) as it falls</skos:definition>
    <dc:source>(L051) SeaDataNet device categories</dc:source>
    <dc:publisher>British Oceanographic Data Centre (BODC)</dc:publisher>
  </rdf:Description>
  <rdf:Description rdf:about="http://vocab.nerc.ac.uk/collection/L05/current/388">
    <rdf:type rdf:resource="http://www.w3.org/2004/02/skos/core#Concept" />
    <skos:prefLabel xml:lang="en">flow meters</skos:prefLabel>
    <skos:topConceptOf rdf:resource="http://vocab.aodn.org.au/def/instrument/1" />
    <skos:inScheme rdf:resource="http://vocab.aodn.org.au/def/instrument/1" />
    <dcterms:created rdf:datatype="http://www.w3.org/2001/XMLSchema#dateTime">2013-03-28T00:00:00Z</dcterms:created>
    <skos:definition xml:lang="en">Sensors that quantify the rate at which fluids (e.g. water or air) pass through sensor packages instruments or sampling devices.</skos:definition>
    <dc:source>(L051) SeaDataNet device categories</dc:source>
    <dc:publisher>British Oceanographic Data Centre (BODC)</dc:publisher>
  </rdf:Description>
  <rdf:Description rdf:about="http://vocab.nerc.ac.uk/collection/L05/current/385">
    <rdf:type rdf:resource="http://www.w3.org/2004/02/skos/core#Concept" />
    <skos:prefLabel xml:lang="en">platform altitude sensors</skos:prefLabel>
    <skos:topConceptOf rdf:resource="http://vocab.aodn.org.au/def/instrument/1" />
    <skos:inScheme rdf:resource="http://vocab.aodn.org.au/def/instrument/1" />
    <dcterms:created rdf:datatype="http://www.w3.org/2001/XMLSchema#dateTime">2014-02-06T00:00:00Z</dcterms:created>
    <skos:definition xml:lang="en">Instruments that measure platform orientation or rates of platform motion or acceleration in any direction or along any axis. Excludes inertial navigation systems that are designed to determine platform location with respect to an external co-ordinate reference system.</skos:definition>
    <dc:source>(L051) SeaDataNet device categories</dc:source>
    <dc:publisher>British Oceanographic Data Centre (BODC)</dc:publisher>
    <skos:narrower rdf:resource="http://vocab.nerc.ac.uk/collection/L22/current/TOOL0490" />
    <skos:narrower rdf:resource="http://vocab.nerc.ac.uk/collection/L22/current/TOOL0721" />
    <skos:narrower rdf:resource="http://vocab.nerc.ac.uk/collection/L22/current/TOOL0872/" />
    <dcterms:modified rdf:datatype="http://www.w3.org/2001/XMLSchema#dateTime">2015-06-30T03:42:14Z</dcterms:modified>
    <dcterms:contributor>Natalia_Atkins</dcterms:contributor>
  </rdf:Description>
  <rdf:Description rdf:about="http://vocab.nerc.ac.uk/collection/L22/current/TOOL0872/">
    <rdf:type rdf:resource="http://www.w3.org/2004/02/skos/core#Concept" />
    <skos:prefLabel xml:lang="en">Teledyne RDI Workhorse Navigator 1200kHz Doppler Velocity Log</skos:prefLabel>
    <skos:altLabel xml:lang="en">RDI Workhorse Navigator 1200kHz DVL</skos:altLabel>
    <skos:inScheme rdf:resource="http://vocab.aodn.org.au/def/instrument/1" />
    <dcterms:created rdf:datatype="http://www.w3.org/2001/XMLSchema#dateTime">2015-06-03T00:00:00Z</dcterms:created>
    <skos:definition xml:lang="en">A Doppler velocity log (DVL) measuring bottom track and water track velocities, altitude, heading, tilt, temperature and echo intensity. 1200kHz Broadband signal processing gives high data resolution and a four-beam solution gives an independent error velocity measurement as an indicator of data quality. It has a bottom track range of 30m and velocity accuracy for both bottom and water track modes is 0.2% of the velocity, ±0.1cm/s. The instrument operates effectively over a temperature range of -5°C to 45°C and with a tilt of up to ±15 deg.</skos:definition>
    <dc:publisher>British Oceanographic Data Centre (BODC)</dc:publisher>
    <dcterms:modified rdf:datatype="http://www.w3.org/2001/XMLSchema#dateTime">2015-06-30T03:42:14Z</dcterms:modified>
    <dcterms:contributor>Natalia_Atkins</dcterms:contributor>
  </rdf:Description>
  <rdf:Description rdf:about="http://vocab.nerc.ac.uk/collection/L22/current/TOOL0490">
    <rdf:type rdf:resource="http://www.w3.org/2004/02/skos/core#Concept" />
    <skos:prefLabel xml:lang="en">Star-Oddi DST Pitch and Roll Recorder</skos:prefLabel>
    <skos:inScheme rdf:resource="http://vocab.aodn.org.au/def/instrument/1" />
    <dcterms:created rdf:datatype="http://www.w3.org/2001/XMLSchema#dateTime">2014-02-06T00:00:00Z</dcterms:created>
    <skos:definition xml:lang="en">A miniature underwater data logger which measures temperature, pressure and pitch and roll (tilt angle) relative to the earth gravity. It has a range of depth ratings from 30 m to 3000 m and a temperature range of -1 degC to 40 degC with an accuracy of +/- 0.1 degC and a resolution of 0.032 degC. The tilt range is 160 deg (+/- 80 deg) with an accuracy of +/- 5deg and a resolution of 0.3 deg.</skos:definition>
    <dc:source>(L221) SeaVoX Device Catalogue</dc:source>
    <dc:publisher>British Oceanographic Data Centre (BODC)</dc:publisher>
    <skos:scopeNote xml:lang="en">manufacturer:Star-Oddi</skos:scopeNote>
  </rdf:Description>
  <rdf:Description rdf:about="http://vocab.nerc.ac.uk/collection/L22/current/TOOL0721">
    <rdf:type rdf:resource="http://www.w3.org/2004/02/skos/core#Concept" />
    <skos:prefLabel xml:lang="en">Microstrain 3DM-GX1 Gyro Enhanced Orientation Sensor</skos:prefLabel>
    <skos:inScheme rdf:resource="http://vocab.aodn.org.au/def/instrument/1" />
    <dcterms:created rdf:datatype="http://www.w3.org/2001/XMLSchema#dateTime">2014-07-11T00:00:00Z</dcterms:created>
    <skos:definition xml:lang="en">The MicroStrain 3DM-GX3 is a triaxial accelerometer designed to measure 360 degrees of angular motion on three orthogonal axes. The 3DM-GX1 has now been retired in favour of later MicroStrain products. The 3DM-GX1 featured on-board processing/filtering of accelerometer, gyro and magnetometer channels, with standard RS-232 and RS-485 outputs, and optional analog output. It offers 16 bit A/D resolution, accuracy of +/-0.5 degrees for static test conditions or +/-2 degrees for dynamic test conditions, 100 Hz digital output rate for Euler, Matrix and Quaternion, and operates in temperatures of -40 to 70 degrees C with enclosure (or +85 degrees C without enclosure).</skos:definition>
    <dc:source>(L221) SeaVoX Device Catalogue</dc:source>
    <dc:publisher>British Oceanographic Data Centre (BODC)</dc:publisher>
  </rdf:Description>
  <rdf:Description rdf:about="http://vocab.nerc.ac.uk/collection/L05/current/384">
    <rdf:type rdf:resource="http://www.w3.org/2004/02/skos/core#Concept" />
    <skos:prefLabel xml:lang="en">ADVs and turbulence probes</skos:prefLabel>
    <skos:topConceptOf rdf:resource="http://vocab.aodn.org.au/def/instrument/1" />
    <skos:inScheme rdf:resource="http://vocab.aodn.org.au/def/instrument/1" />
    <dcterms:created rdf:datatype="http://www.w3.org/2001/XMLSchema#dateTime">2014-05-22T00:00:00Z</dcterms:created>
    <skos:definition xml:lang="en">ADV is the acronym for acoustic doppler velocimeter. The group includes all in-situ instruments that make high frequency measurements of three-dimensional current velocity in order to determine the extent of turbulence within a water body.</skos:definition>
    <dc:source>(L051) SeaDataNet device categories</dc:source>
    <dc:publisher>British Oceanographic Data Centre (BODC)</dc:publisher>
  </rdf:Description>
  <rdf:Description rdf:about="http://vocab.nerc.ac.uk/collection/L05/current/23">
    <rdf:type rdf:resource="http://www.w3.org/2004/02/skos/core#Concept" />
    <skos:prefLabel xml:lang="en">pelagic trawl nets</skos:prefLabel>
    <skos:topConceptOf rdf:resource="http://vocab.aodn.org.au/def/instrument/1" />
    <skos:inScheme rdf:resource="http://vocab.aodn.org.au/def/instrument/1" />
    <dcterms:created rdf:datatype="http://www.w3.org/2001/XMLSchema#dateTime">2014-05-22T00:00:00Z</dcterms:created>
    <skos:definition xml:lang="en">A net towed through the water column designed to sample free-swimming nekton or fish.</skos:definition>
    <dc:source>(L051) SeaDataNet device categories</dc:source>
    <dc:publisher>British Oceanographic Data Centre (BODC)</dc:publisher>
  </rdf:Description>
  <rdf:Description rdf:about="http://vocab.nerc.ac.uk/collection/L05/current/24">
    <rdf:type rdf:resource="http://www.w3.org/2004/02/skos/core#Concept" />
    <skos:prefLabel xml:lang="en">benthos samplers</skos:prefLabel>
    <skos:topConceptOf rdf:resource="http://vocab.aodn.org.au/def/instrument/1" />
    <skos:inScheme rdf:resource="http://vocab.aodn.org.au/def/instrument/1" />
    <dcterms:created rdf:datatype="http://www.w3.org/2001/XMLSchema#dateTime">2014-05-22T00:00:00Z</dcterms:created>
    <skos:definition xml:lang="en">A net or sledge dragged across the seabed designed to sample benthic fauna.</skos:definition>
    <dc:source>(L051) SeaDataNet device categories</dc:source>
    <dc:publisher>British Oceanographic Data Centre (BODC)</dc:publisher>
  </rdf:Description>
  <rdf:Description rdf:about="http://vocab.nerc.ac.uk/collection/L05/current/21">
    <rdf:type rdf:resource="http://www.w3.org/2004/02/skos/core#Concept" />
    <skos:prefLabel xml:lang="en">plankton recorders</skos:prefLabel>
    <skos:topConceptOf rdf:resource="http://vocab.aodn.org.au/def/instrument/1" />
    <skos:inScheme rdf:resource="http://vocab.aodn.org.au/def/instrument/1" />
    <dcterms:created rdf:datatype="http://www.w3.org/2001/XMLSchema#dateTime">2013-03-28T00:00:00Z</dcterms:created>
    <skos:definition xml:lang="en">A device that continuously samples a flow of water separating and fixing plankton for subsequent identification and counting</skos:definition>
    <dc:source>(L051) SeaDataNet device categories</dc:source>
    <dc:publisher>British Oceanographic Data Centre (BODC)</dc:publisher>
    <skos:narrower rdf:resource="http://vocab.nerc.ac.uk/collection/L22/current/NETT0026" />
  </rdf:Description>
  <rdf:Description rdf:about="http://vocab.nerc.ac.uk/collection/L22/current/NETT0026">
    <rdf:type rdf:resource="http://www.w3.org/2004/02/skos/core#Concept" />
    <skos:prefLabel xml:lang="en">Continuous Plankton Recorder - Hardy (1926, 1936); Glover (1962)</skos:prefLabel>
    <skos:inScheme rdf:resource="http://vocab.aodn.org.au/def/instrument/1" />
    <dcterms:created rdf:datatype="http://www.w3.org/2001/XMLSchema#dateTime">2014-02-26T00:00:00Z</dcterms:created>
    <skos:definition xml:lang="en">Construction is a 1.27 cm on side square mouth opening (originally 10.1 cm diameter) high-speed (12 to 17 knots) towed body collecting plankton on gauze (22.9 cm wide and 23.6 meshes per cm) rolls. The body is 50 cm wide x 50 cm tall x 100 cm long.  A propellor drives the rollers winding up the gauze.  The system is normally towed at 10 m depth at speeds up to 20 ktnos [Wiebe and Benfield 2003 Plate 19 A, B].</skos:definition>
    <dc:source>(L221) SeaVoX Device Catalogue</dc:source>
    <dc:publisher>British Oceanographic Data Centre (BODC)</dc:publisher>
  </rdf:Description>
  <rdf:Description rdf:about="http://vocab.nerc.ac.uk/collection/L05/current/22">
    <rdf:type rdf:resource="http://www.w3.org/2004/02/skos/core#Concept" />
    <skos:prefLabel xml:lang="en">plankton nets</skos:prefLabel>
    <skos:topConceptOf rdf:resource="http://vocab.aodn.org.au/def/instrument/1" />
    <skos:inScheme rdf:resource="http://vocab.aodn.org.au/def/instrument/1" />
    <dcterms:created rdf:datatype="http://www.w3.org/2001/XMLSchema#dateTime">2013-07-18T00:00:00Z</dcterms:created>
    <skos:definition xml:lang="en">A fine-meshed net designed for sampling microzooplankton mesozooplankton or nekton.</skos:definition>
    <dc:source>(L051) SeaDataNet device categories</dc:source>
    <dc:publisher>British Oceanographic Data Centre (BODC)</dc:publisher>
    <skos:narrower rdf:resource="http://vocab.nerc.ac.uk/collection/L22/current/NETT0044" />
  </rdf:Description>
  <rdf:Description rdf:about="http://vocab.nerc.ac.uk/collection/L22/current/NETT0044">
    <rdf:type rdf:resource="http://www.w3.org/2004/02/skos/core#Concept" />
    <skos:prefLabel xml:lang="en">Free-fall plankton net - Heron (1982)</skos:prefLabel>
    <skos:inScheme rdf:resource="http://vocab.aodn.org.au/def/instrument/1" />
    <dcterms:created rdf:datatype="http://www.w3.org/2001/XMLSchema#dateTime">2014-02-03T00:00:00Z</dcterms:created>
    <skos:definition xml:lang="en">A modified WP2 cylinder-cone closing net (mesh not specified) which is allowed to free-fall and then is strangled shut and retrieved.  [Wiebe and Benfield 2003 Plate 10C]</skos:definition>
    <dc:source>(L221) SeaVoX Device Catalogue</dc:source>
    <dc:publisher>British Oceanographic Data Centre (BODC)</dc:publisher>
  </rdf:Description>
  <rdf:Description rdf:about="http://vocab.nerc.ac.uk/collection/L05/current/377">
    <rdf:type rdf:resource="http://www.w3.org/2004/02/skos/core#Concept" />
    <skos:prefLabel xml:lang="en">water level markers</skos:prefLabel>
    <skos:topConceptOf rdf:resource="http://vocab.aodn.org.au/def/instrument/1" />
    <skos:inScheme rdf:resource="http://vocab.aodn.org.au/def/instrument/1" />
    <dcterms:created rdf:datatype="http://www.w3.org/2001/XMLSchema#dateTime">2014-05-22T00:00:00Z</dcterms:created>
    <skos:definition xml:lang="en">Fixed physical markers that allow changes in the position of the boundary between a water body and the atmosphere by visible comparison against marked graduations in units of measurement of dimension length.</skos:definition>
    <dc:source>(L051) SeaDataNet device categories</dc:source>
    <dc:publisher>British Oceanographic Data Centre (BODC)</dc:publisher>
  </rdf:Description>
  <rdf:Description rdf:about="http://vocab.nerc.ac.uk/collection/L05/current/379">
    <rdf:type rdf:resource="http://www.w3.org/2004/02/skos/core#Concept" />
    <skos:prefLabel xml:lang="en">altimeter</skos:prefLabel>
    <skos:topConceptOf rdf:resource="http://vocab.aodn.org.au/def/instrument/1" />
    <skos:inScheme rdf:resource="http://vocab.aodn.org.au/def/instrument/1" />
    <dcterms:created rdf:datatype="http://www.w3.org/2001/XMLSchema#dateTime">2013-07-18T00:00:00Z</dcterms:created>
    <skos:definition xml:lang="en">An instrument used to measure the altitude of an object above a fixed level</skos:definition>
    <dc:source>(L051) SeaDataNet device categories</dc:source>
    <dc:publisher>British Oceanographic Data Centre (BODC)</dc:publisher>
    <skos:narrower rdf:resource="http://vocab.nerc.ac.uk/collection/L22/current/TOOL0872/" />
    <dcterms:modified rdf:datatype="http://www.w3.org/2001/XMLSchema#dateTime">2015-06-30T03:39:42Z</dcterms:modified>
    <dcterms:contributor>Natalia_Atkins</dcterms:contributor>
  </rdf:Description>
  <rdf:Description rdf:about="http://vocab.nerc.ac.uk/collection/L22/current/TOOL0872/">
    <rdf:type rdf:resource="http://www.w3.org/2004/02/skos/core#Concept" />
    <skos:prefLabel xml:lang="en">Teledyne RDI Workhorse Navigator 1200kHz Doppler Velocity Log</skos:prefLabel>
    <skos:altLabel xml:lang="en">RDI Workhorse Navigator 1200kHz DVL</skos:altLabel>
    <skos:inScheme rdf:resource="http://vocab.aodn.org.au/def/instrument/1" />
    <dcterms:created rdf:datatype="http://www.w3.org/2001/XMLSchema#dateTime">2015-06-03T00:00:00Z</dcterms:created>
    <skos:definition xml:lang="en">A Doppler velocity log (DVL) measuring bottom track and water track velocities, altitude, heading, tilt, temperature and echo intensity. 1200kHz Broadband signal processing gives high data resolution and a four-beam solution gives an independent error velocity measurement as an indicator of data quality. It has a bottom track range of 30m and velocity accuracy for both bottom and water track modes is 0.2% of the velocity, ±0.1cm/s. The instrument operates effectively over a temperature range of -5°C to 45°C and with a tilt of up to ±15 deg.</skos:definition>
    <dc:publisher>British Oceanographic Data Centre (BODC)</dc:publisher>
    <dcterms:modified rdf:datatype="http://www.w3.org/2001/XMLSchema#dateTime">2015-06-30T03:42:14Z</dcterms:modified>
    <dcterms:contributor>Natalia_Atkins</dcterms:contributor>
  </rdf:Description>
  <rdf:Description rdf:about="http://vocab.nerc.ac.uk/collection/L05/current/186">
    <rdf:type rdf:resource="http://www.w3.org/2004/02/skos/core#Concept" />
    <skos:prefLabel xml:lang="en">radar altimeters</skos:prefLabel>
    <skos:topConceptOf rdf:resource="http://vocab.aodn.org.au/def/instrument/1" />
    <skos:inScheme rdf:resource="http://vocab.aodn.org.au/def/instrument/1" />
    <dcterms:created rdf:datatype="http://www.w3.org/2001/XMLSchema#dateTime">2013-07-18T00:00:00Z</dcterms:created>
    <skos:definition xml:lang="en">Instruments that determine the distance between the platform and the Earth's surface by timing reflected electromagnetic radiation usually microwaves.</skos:definition>
    <dc:source>(L051) SeaDataNet device categories</dc:source>
    <dc:publisher>British Oceanographic Data Centre (BODC)</dc:publisher>
  </rdf:Description>
  <rdf:Description rdf:about="http://vocab.nerc.ac.uk/collection/L05/current/185">
    <rdf:type rdf:resource="http://www.w3.org/2004/02/skos/core#Concept" />
    <skos:prefLabel xml:lang="en">sound velocity sensors</skos:prefLabel>
    <skos:topConceptOf rdf:resource="http://vocab.aodn.org.au/def/instrument/1" />
    <skos:inScheme rdf:resource="http://vocab.aodn.org.au/def/instrument/1" />
    <dcterms:created rdf:datatype="http://www.w3.org/2001/XMLSchema#dateTime">2013-03-28T00:00:00Z</dcterms:created>
    <skos:definition xml:lang="en">Instrument that measures the velocity of sound in seawater</skos:definition>
    <dc:source>(L051) SeaDataNet device categories</dc:source>
    <dc:publisher>British Oceanographic Data Centre (BODC)</dc:publisher>
  </rdf:Description>
  <rdf:Description rdf:about="http://vocab.nerc.ac.uk/collection/L05/current/183">
    <rdf:type rdf:resource="http://www.w3.org/2004/02/skos/core#Concept" />
    <skos:prefLabel xml:lang="en">acoustic backscatter sensors</skos:prefLabel>
    <skos:topConceptOf rdf:resource="http://vocab.aodn.org.au/def/instrument/1" />
    <skos:inScheme rdf:resource="http://vocab.aodn.org.au/def/instrument/1" />
    <dcterms:created rdf:datatype="http://www.w3.org/2001/XMLSchema#dateTime">2013-03-28T00:00:00Z</dcterms:created>
    <skos:definition xml:lang="en">Instrument that measures the amount of sound energy transmitted into the water column returned to the instrument.</skos:definition>
    <dc:source>(L051) SeaDataNet device categories</dc:source>
    <dc:publisher>British Oceanographic Data Centre (BODC)</dc:publisher>
  </rdf:Description>
  <rdf:Description rdf:about="http://vocab.nerc.ac.uk/collection/L05/current/181">
    <rdf:type rdf:resource="http://www.w3.org/2004/02/skos/core#Concept" />
    <skos:prefLabel xml:lang="en">nutrient analysers</skos:prefLabel>
    <skos:topConceptOf rdf:resource="http://vocab.aodn.org.au/def/instrument/1" />
    <skos:inScheme rdf:resource="http://vocab.aodn.org.au/def/instrument/1" />
    <dcterms:created rdf:datatype="http://www.w3.org/2001/XMLSchema#dateTime">2013-07-18T00:00:00Z</dcterms:created>
    <skos:definition xml:lang="en">Instrument that makes in-situ measurements of one or more of nitrate nitrite ammonium urea phosphate or silicate dissolved in the water column</skos:definition>
    <dc:source>(L051) SeaDataNet device categories</dc:source>
    <dc:publisher>British Oceanographic Data Centre (BODC)</dc:publisher>
    <skos:narrower rdf:resource="http://vocab.nerc.ac.uk/collection/L22/current/TOOL0528" />
  </rdf:Description>
  <rdf:Description rdf:about="http://vocab.nerc.ac.uk/collection/L22/current/TOOL0528">
    <rdf:type rdf:resource="http://www.w3.org/2004/02/skos/core#Concept" />
    <skos:prefLabel xml:lang="en">Satlantic ISUS V3 Nitrate Sensor</skos:prefLabel>
    <skos:inScheme rdf:resource="http://vocab.aodn.org.au/def/instrument/1" />
    <dcterms:created rdf:datatype="http://www.w3.org/2001/XMLSchema#dateTime">2014-02-07T00:00:00Z</dcterms:created>
    <skos:definition xml:lang="en">An active optical instrument with an internal UV light source and spectrometer used to measure in-situ dissolved nitrate. It is a chemical-free method that allows real-time and continuous nitrate concentration measurements in a variety of environments. It uses a Deuterium lamp as a light source and has a 1cm path length and 200-400 nm wavelength range. It has a depth rating of 1000 m and a detection range of  0.5 to 2000 uM *(0.007 to 28 mg/l-N)  and accuracy of +/- 0.2 uM (0.028 mg/l) or ± 10% of reading, whichever is greater. The V3 has USB data transfer ability and window based software.</skos:definition>
    <dc:source>(L221) SeaVoX Device Catalogue</dc:source>
    <dc:publisher>British Oceanographic Data Centre (BODC)</dc:publisher>
    <skos:scopeNote xml:lang="en">manufacturer:Satlantic</skos:scopeNote>
  </rdf:Description>
  <rdf:Description rdf:about="http://vocab.nerc.ac.uk/collection/L05/current/180">
    <rdf:type rdf:resource="http://www.w3.org/2004/02/skos/core#Concept" />
    <skos:prefLabel xml:lang="en">underwater cameras</skos:prefLabel>
    <skos:topConceptOf rdf:resource="http://vocab.aodn.org.au/def/instrument/1" />
    <skos:inScheme rdf:resource="http://vocab.aodn.org.au/def/instrument/1" />
    <dcterms:created rdf:datatype="http://www.w3.org/2001/XMLSchema#dateTime">2013-03-28T00:00:00Z</dcterms:created>
    <skos:definition xml:lang="en">All types of photographic equipment that may be deployed underwater including stills video film and digital systems</skos:definition>
    <dc:source>(L051) SeaDataNet device categories</dc:source>
    <dc:publisher>British Oceanographic Data Centre (BODC)</dc:publisher>
  </rdf:Description>
  <rdf:Description rdf:about="http://vocab.nerc.ac.uk/collection/L22/current/TOOL0720">
    <skos:broader rdf:resource="http://vocab.nerc.ac.uk/collection/L05/current/350" />
  </rdf:Description>
  <rdf:Description rdf:about="http://vocab.nerc.ac.uk/collection/L22/current/TOOL0898/">
    <skos:broader rdf:resource="http://vocab.nerc.ac.uk/collection/L05/current/110" />
    <skos:broader rdf:resource="http://vocab.nerc.ac.uk/collection/L05/current/115" />
  </rdf:Description>
  <rdf:Description rdf:about="http://vocab.nerc.ac.uk/collection/L22/current/TOOL0733">
    <skos:broader rdf:resource="http://vocab.nerc.ac.uk/collection/L05/current/110" />
  </rdf:Description>
  <rdf:Description rdf:about="http://vocab.nerc.ac.uk/collection/L22/current/TOOL0666">
    <skos:broader rdf:resource="http://vocab.nerc.ac.uk/collection/L05/current/122" />
  </rdf:Description>
  <rdf:Description rdf:about="http://vocab.nerc.ac.uk/collection/L22/current/TOOL0731">
    <skos:broader rdf:resource="http://vocab.nerc.ac.uk/collection/L05/current/111" />
  </rdf:Description>
  <rdf:Description rdf:about="http://vocab.nerc.ac.uk/collection/L22/current/TOOL0729">
    <skos:broader rdf:resource="http://vocab.nerc.ac.uk/collection/L05/current/134" />
  </rdf:Description>
  <rdf:Description rdf:about="http://vocab.nerc.ac.uk/collection/L22/current/TOOL0173">
    <skos:broader rdf:resource="http://vocab.nerc.ac.uk/collection/L05/current/130" />
  </rdf:Description>
  <rdf:Description rdf:about="http://vocab.nerc.ac.uk/collection/L22/current/TOOL0728">
    <skos:broader rdf:resource="http://vocab.nerc.ac.uk/collection/L05/current/134" />
  </rdf:Description>
  <rdf:Description rdf:about="http://vocab.nerc.ac.uk/collection/L22/current/TOOL0169">
    <skos:broader rdf:resource="http://vocab.nerc.ac.uk/collection/L05/current/111" />
  </rdf:Description>
  <rdf:Description rdf:about="http://vocab.nerc.ac.uk/collection/L22/current/TOOL0019">
    <skos:broader rdf:resource="http://vocab.aodn.org.au/def/instrument/entity/365" />
  </rdf:Description>
  <rdf:Description rdf:about="http://vocab.nerc.ac.uk/collection/L22/current/TOOL0668">
    <skos:broader rdf:resource="http://vocab.nerc.ac.uk/collection/L05/current/350" />
  </rdf:Description>
  <rdf:Description rdf:about="http://vocab.nerc.ac.uk/collection/L22/current/TOOL0435">
    <skos:broader rdf:resource="http://vocab.nerc.ac.uk/collection/L05/current/132" />
  </rdf:Description>
  <rdf:Description rdf:about="http://vocab.nerc.ac.uk/collection/L22/current/TOOL0173">
    <skos:broader rdf:resource="http://vocab.nerc.ac.uk/collection/L05/current/134" />
  </rdf:Description>
  <rdf:Description rdf:about="http://vocab.nerc.ac.uk/collection/L22/current/TOOL0696">
    <skos:broader rdf:resource="http://vocab.nerc.ac.uk/collection/L05/current/111" />
    <skos:broader rdf:resource="http://vocab.nerc.ac.uk/collection/L05/current/110" />
  </rdf:Description>
  <rdf:Description rdf:about="http://vocab.nerc.ac.uk/collection/L22/current/TOOL0871/">
    <skos:broader rdf:resource="http://vocab.nerc.ac.uk/collection/L05/current/350" />
  </rdf:Description>
  <rdf:Description rdf:about="http://vocab.nerc.ac.uk/collection/L22/current/TOOL0081">
    <skos:broader rdf:resource="http://vocab.nerc.ac.uk/collection/L05/current/102" />
  </rdf:Description>
  <rdf:Description rdf:about="http://vocab.nerc.ac.uk/collection/L22/current/TOOL0018">
    <skos:broader rdf:resource="http://vocab.nerc.ac.uk/collection/L05/current/350" />
  </rdf:Description>
  <rdf:Description rdf:about="http://vocab.nerc.ac.uk/collection/L22/current/TOOL0805">
    <skos:broader rdf:resource="http://vocab.nerc.ac.uk/collection/L05/current/351" />
  </rdf:Description>
  <rdf:Description rdf:about="http://vocab.nerc.ac.uk/collection/L22/current/TOOL0295">
    <skos:broader rdf:resource="http://vocab.nerc.ac.uk/collection/L05/current/115" />
  </rdf:Description>
  <rdf:Description rdf:about="http://vocab.nerc.ac.uk/collection/L22/current/TOOL0872/">
    <skos:broader rdf:resource="http://vocab.nerc.ac.uk/collection/L05/current/134" />
  </rdf:Description>
  <rdf:Description rdf:about="http://vocab.nerc.ac.uk/collection/L22/current/TOOL0266">
    <skos:broader rdf:resource="http://vocab.nerc.ac.uk/collection/L05/current/134" />
  </rdf:Description>
  <rdf:Description rdf:about="http://vocab.nerc.ac.uk/collection/L22/current/TOOL0675">
    <skos:broader rdf:resource="http://vocab.aodn.org.au/def/instrument/entity/361" />
  </rdf:Description>
  <rdf:Description rdf:about="http://vocab.nerc.ac.uk/collection/L22/current/TOOL0869/">
    <skos:broader rdf:resource="http://vocab.nerc.ac.uk/collection/L05/current/134" />
  </rdf:Description>
  <rdf:Description rdf:about="http://vocab.nerc.ac.uk/collection/L22/current/TOOL0268">
    <skos:broader rdf:resource="http://vocab.nerc.ac.uk/collection/L05/current/110" />
  </rdf:Description>
  <rdf:Description rdf:about="http://vocab.nerc.ac.uk/collection/L22/current/TOOL0731">
    <skos:broader rdf:resource="http://vocab.nerc.ac.uk/collection/L05/current/134" />
  </rdf:Description>
  <rdf:Description rdf:about="http://vocab.nerc.ac.uk/collection/L22/current/TOOL0673">
    <skos:broader rdf:resource="http://vocab.aodn.org.au/def/instrument/entity/361" />
  </rdf:Description>
  <rdf:Description rdf:about="http://vocab.nerc.ac.uk/collection/L22/current/TOOL0020">
    <skos:broader rdf:resource="http://vocab.nerc.ac.uk/collection/L05/current/350" />
  </rdf:Description>
  <rdf:Description rdf:about="http://vocab.nerc.ac.uk/collection/L22/current/TOOL0042">
    <skos:broader rdf:resource="http://vocab.nerc.ac.uk/collection/L05/current/134" />
  </rdf:Description>
  <rdf:Description rdf:about="http://vocab.nerc.ac.uk/collection/L22/current/TOOL0674">
    <skos:broader rdf:resource="http://vocab.aodn.org.au/def/instrument/entity/361" />
  </rdf:Description>
  <rdf:Description rdf:about="http://vocab.nerc.ac.uk/collection/L22/current/TOOL0721">
    <skos:broader rdf:resource="http://vocab.nerc.ac.uk/collection/L05/current/385" />
  </rdf:Description>
  <rdf:Description rdf:about="http://vocab.nerc.ac.uk/collection/L22/current/TOOL0040">
    <skos:broader rdf:resource="http://vocab.nerc.ac.uk/collection/L05/current/350" />
  </rdf:Description>
  <rdf:Description rdf:about="http://vocab.nerc.ac.uk/collection/L22/current/TOOL0696">
    <skos:broader rdf:resource="http://vocab.nerc.ac.uk/collection/L05/current/134" />
  </rdf:Description>
  <rdf:Description rdf:about="http://vocab.nerc.ac.uk/collection/L22/current/TOOL0871/">
    <skos:broader rdf:resource="http://vocab.nerc.ac.uk/collection/L05/current/130" />
  </rdf:Description>
  <rdf:Description rdf:about="http://vocab.aodn.org.au/def/instrument/entity/553">
    <skos:broader rdf:resource="http://vocab.nerc.ac.uk/collection/L05/current/134" />
  </rdf:Description>
  <rdf:Description rdf:about="http://vocab.nerc.ac.uk/collection/L22/current/TOOL0741">
    <skos:broader rdf:resource="http://vocab.nerc.ac.uk/collection/L05/current/102" />
  </rdf:Description>
  <rdf:Description rdf:about="http://vocab.nerc.ac.uk/collection/L22/current/TOOL0869/">
    <skos:broader rdf:resource="http://vocab.nerc.ac.uk/collection/L05/current/351" />
    <skos:broader rdf:resource="http://vocab.nerc.ac.uk/collection/L05/current/350" />
  </rdf:Description>
  <rdf:Description rdf:about="http://vocab.nerc.ac.uk/collection/L22/current/TOOL0871/">
    <skos:broader rdf:resource="http://vocab.nerc.ac.uk/collection/L05/current/134" />
  </rdf:Description>
  <rdf:Description rdf:about="http://vocab.nerc.ac.uk/collection/L22/current/TOOL0042">
    <skos:broader rdf:resource="http://vocab.nerc.ac.uk/collection/L05/current/350" />
  </rdf:Description>
  <rdf:Description rdf:about="http://vocab.nerc.ac.uk/collection/L22/current/TOOL0879/">
    <skos:broader rdf:resource="http://vocab.nerc.ac.uk/collection/L05/current/123" />
  </rdf:Description>
  <rdf:Description rdf:about="http://vocab.nerc.ac.uk/collection/L22/current/TOOL0685">
    <skos:broader rdf:resource="http://vocab.nerc.ac.uk/collection/L05/current/134" />
  </rdf:Description>
  <rdf:Description rdf:about="http://vocab.nerc.ac.uk/collection/L22/current/TOOL0663">
    <skos:broader rdf:resource="http://vocab.nerc.ac.uk/collection/L05/current/369" />
  </rdf:Description>
  <rdf:Description rdf:about="http://vocab.nerc.ac.uk/collection/L22/current/TOOL0528">
    <skos:broader rdf:resource="http://vocab.nerc.ac.uk/collection/L05/current/181" />
  </rdf:Description>
  <rdf:Description rdf:about="http://vocab.nerc.ac.uk/collection/L22/current/TOOL0732">
    <skos:broader rdf:resource="http://vocab.nerc.ac.uk/collection/L05/current/115" />
  </rdf:Description>
  <rdf:Description rdf:about="http://vocab.nerc.ac.uk/collection/L22/current/TOOL0675">
    <skos:broader rdf:resource="http://vocab.nerc.ac.uk/collection/L05/current/111" />
  </rdf:Description>
  <rdf:Description rdf:about="http://vocab.nerc.ac.uk/collection/L22/current/TOOL0017">
    <skos:broader rdf:resource="http://vocab.nerc.ac.uk/collection/L05/current/350" />
  </rdf:Description>
  <rdf:Description rdf:about="http://vocab.nerc.ac.uk/collection/L22/current/TOOL0675">
    <skos:broader rdf:resource="http://vocab.nerc.ac.uk/collection/L05/current/113" />
  </rdf:Description>
  <rdf:Description rdf:about="http://vocab.nerc.ac.uk/collection/L22/current/TOOL0669">
    <skos:broader rdf:resource="http://vocab.nerc.ac.uk/collection/L05/current/350" />
  </rdf:Description>
  <rdf:Description rdf:about="http://vocab.nerc.ac.uk/collection/L22/current/TOOL0727">
    <skos:broader rdf:resource="http://vocab.nerc.ac.uk/collection/L05/current/102" />
  </rdf:Description>
  <rdf:Description rdf:about="http://vocab.nerc.ac.uk/collection/L22/current/TOOL0042">
    <skos:broader rdf:resource="http://vocab.nerc.ac.uk/collection/L05/current/130" />
  </rdf:Description>
  <rdf:Description rdf:about="http://vocab.nerc.ac.uk/collection/L22/current/TOOL0726">
    <skos:broader rdf:resource="http://vocab.nerc.ac.uk/collection/L05/current/102" />
  </rdf:Description>
  <rdf:Description rdf:about="http://vocab.nerc.ac.uk/collection/L22/current/TOOL0877/">
    <skos:broader rdf:resource="http://vocab.nerc.ac.uk/collection/L05/current/101" />
  </rdf:Description>
  <rdf:Description rdf:about="http://vocab.nerc.ac.uk/collection/L22/current/TOOL0674">
    <skos:broader rdf:resource="http://vocab.nerc.ac.uk/collection/L05/current/113" />
  </rdf:Description>
  <rdf:Description rdf:about="http://vocab.nerc.ac.uk/collection/L22/current/TOOL0872/">
    <skos:broader rdf:resource="http://vocab.nerc.ac.uk/collection/L05/current/379" />
  </rdf:Description>
  <rdf:Description rdf:about="http://vocab.nerc.ac.uk/collection/L22/current/TOOL0712">
    <skos:broader rdf:resource="http://vocab.nerc.ac.uk/collection/L05/current/134" />
  </rdf:Description>
  <rdf:Description rdf:about="http://vocab.nerc.ac.uk/collection/L22/current/TOOL0047">
    <skos:broader rdf:resource="http://vocab.nerc.ac.uk/collection/L05/current/134" />
  </rdf:Description>
  <rdf:Description rdf:about="http://vocab.nerc.ac.uk/collection/L22/current/TOOL0056">
    <skos:broader rdf:resource="http://vocab.nerc.ac.uk/collection/L05/current/115" />
  </rdf:Description>
  <rdf:Description rdf:about="http://vocab.nerc.ac.uk/collection/L22/current/TOOL0019">
    <skos:broader rdf:resource="http://vocab.nerc.ac.uk/collection/L05/current/350" />
  </rdf:Description>
  <rdf:Description rdf:about="http://vocab.nerc.ac.uk/collection/L22/current/TOOL0047">
    <skos:broader rdf:resource="http://vocab.nerc.ac.uk/collection/L05/current/130" />
  </rdf:Description>
  <rdf:Description rdf:about="http://vocab.nerc.ac.uk/collection/L22/current/TOOL0294">
    <skos:broader rdf:resource="http://vocab.nerc.ac.uk/collection/L05/current/115" />
  </rdf:Description>
  <rdf:Description rdf:about="http://vocab.nerc.ac.uk/collection/L22/current/TOOL0193">
    <skos:broader rdf:resource="http://vocab.nerc.ac.uk/collection/L05/current/122" />
  </rdf:Description>
  <rdf:Description rdf:about="http://vocab.nerc.ac.uk/collection/L22/current/TOOL0667">
    <skos:broader rdf:resource="http://vocab.nerc.ac.uk/collection/L05/current/350" />
  </rdf:Description>
  <rdf:Description rdf:about="http://vocab.nerc.ac.uk/collection/L22/current/TOOL0053">
    <skos:broader rdf:resource="http://vocab.nerc.ac.uk/collection/L05/current/134" />
  </rdf:Description>
  <rdf:Description rdf:about="http://vocab.nerc.ac.uk/collection/L22/current/TOOL0017">
    <skos:broader rdf:resource="http://vocab.nerc.ac.uk/collection/L05/current/134" />
  </rdf:Description>
  <rdf:Description rdf:about="http://vocab.nerc.ac.uk/collection/L22/current/TOOL0260">
    <skos:broader rdf:resource="http://vocab.nerc.ac.uk/collection/L05/current/101" />
  </rdf:Description>
  <rdf:Description rdf:about="http://vocab.nerc.ac.uk/collection/L22/current/TOOL0685">
    <skos:broader rdf:resource="http://vocab.nerc.ac.uk/collection/L05/current/111" />
  </rdf:Description>
  <rdf:Description rdf:about="http://vocab.nerc.ac.uk/collection/L22/current/TOOL0675">
    <skos:broader rdf:resource="http://vocab.nerc.ac.uk/collection/L05/current/123" />
  </rdf:Description>
  <rdf:Description rdf:about="http://vocab.nerc.ac.uk/collection/L22/current/TOOL0719">
    <skos:broader rdf:resource="http://vocab.nerc.ac.uk/collection/L05/current/134" />
  </rdf:Description>
  <rdf:Description rdf:about="http://vocab.nerc.ac.uk/collection/L22/current/TOOL0878/">
    <skos:broader rdf:resource="http://vocab.nerc.ac.uk/collection/L05/current/382" />
  </rdf:Description>
  <rdf:Description rdf:about="http://vocab.nerc.ac.uk/collection/L22/current/TOOL0729">
    <skos:broader rdf:resource="http://vocab.nerc.ac.uk/collection/L05/current/110" />
    <skos:broader rdf:resource="http://vocab.nerc.ac.uk/collection/L05/current/111" />
  </rdf:Description>
  <rdf:Description rdf:about="http://vocab.nerc.ac.uk/collection/L22/current/TOOL0617">
    <skos:broader rdf:resource="http://vocab.nerc.ac.uk/collection/L05/current/102" />
  </rdf:Description>
  <rdf:Description rdf:about="http://vocab.nerc.ac.uk/collection/L22/current/TOOL0018">
    <skos:broader rdf:resource="http://vocab.nerc.ac.uk/collection/L05/current/134" />
  </rdf:Description>
  <rdf:Description rdf:about="http://vocab.nerc.ac.uk/collection/L22/current/TOOL0100">
    <skos:broader rdf:resource="http://vocab.nerc.ac.uk/collection/L05/current/350" />
  </rdf:Description>
  <rdf:Description rdf:about="http://vocab.nerc.ac.uk/collection/L22/current/TOOL0190">
    <skos:broader rdf:resource="http://vocab.nerc.ac.uk/collection/L05/current/134" />
    <skos:broader rdf:resource="http://vocab.nerc.ac.uk/collection/L05/current/133" />
  </rdf:Description>
  <rdf:Description rdf:about="http://vocab.nerc.ac.uk/collection/L22/current/TOOL0083">
    <skos:broader rdf:resource="http://vocab.nerc.ac.uk/collection/L05/current/122" />
  </rdf:Description>
  <rdf:Description rdf:about="http://vocab.nerc.ac.uk/collection/L22/current/TOOL0675">
    <skos:broader rdf:resource="http://vocab.nerc.ac.uk/collection/L05/current/134" />
  </rdf:Description>
  <rdf:Description rdf:about="http://vocab.nerc.ac.uk/collection/L22/current/NETT0026">
    <skos:broader rdf:resource="http://vocab.nerc.ac.uk/collection/L05/current/21" />
  </rdf:Description>
  <rdf:Description rdf:about="http://vocab.nerc.ac.uk/collection/L22/current/TOOL0121">
    <skos:broader rdf:resource="http://vocab.nerc.ac.uk/collection/L05/current/114" />
  </rdf:Description>
  <rdf:Description rdf:about="http://vocab.nerc.ac.uk/collection/L22/current/TOOL0369">
    <skos:broader rdf:resource="http://vocab.nerc.ac.uk/collection/L05/current/351" />
  </rdf:Description>
  <rdf:Description rdf:about="http://vocab.nerc.ac.uk/collection/L22/current/TOOL0019">
    <skos:broader rdf:resource="http://vocab.nerc.ac.uk/collection/L05/current/134" />
  </rdf:Description>
  <rdf:Description rdf:about="http://vocab.nerc.ac.uk/collection/L22/current/TOOL0665">
    <skos:broader rdf:resource="http://vocab.nerc.ac.uk/collection/L05/current/134" />
  </rdf:Description>
  <rdf:Description rdf:about="http://vocab.nerc.ac.uk/collection/L22/current/TOOL0668">
    <skos:broader rdf:resource="http://vocab.nerc.ac.uk/collection/L05/current/134" />
    <skos:broader rdf:resource="http://vocab.nerc.ac.uk/collection/L05/current/130" />
  </rdf:Description>
  <rdf:Description rdf:about="http://vocab.nerc.ac.uk/collection/L22/current/TOOL0669">
    <skos:broader rdf:resource="http://vocab.nerc.ac.uk/collection/L05/current/130" />
  </rdf:Description>
  <rdf:Description rdf:about="http://vocab.nerc.ac.uk/collection/L22/current/TOOL0446">
    <skos:broader rdf:resource="http://vocab.nerc.ac.uk/collection/L05/current/POS17" />
  </rdf:Description>
  <rdf:Description rdf:about="http://vocab.nerc.ac.uk/collection/L22/current/TOOL0669">
    <skos:broader rdf:resource="http://vocab.nerc.ac.uk/collection/L05/current/134" />
  </rdf:Description>
  <rdf:Description rdf:about="http://vocab.nerc.ac.uk/collection/L22/current/TOOL0293">
    <skos:broader rdf:resource="http://vocab.nerc.ac.uk/collection/L05/current/115" />
  </rdf:Description>
  <rdf:Description rdf:about="http://vocab.nerc.ac.uk/collection/L22/current/TOOL0446">
    <skos:broader rdf:resource="http://vocab.nerc.ac.uk/collection/L05/current/350" />
  </rdf:Description>
  <rdf:Description rdf:about="http://vocab.nerc.ac.uk/collection/L22/current/TOOL0198">
    <skos:broader rdf:resource="http://vocab.nerc.ac.uk/collection/L05/current/FFES" />
  </rdf:Description>
  <rdf:Description rdf:about="http://vocab.nerc.ac.uk/collection/L22/current/TOOL0689">
    <skos:broader rdf:resource="http://vocab.nerc.ac.uk/collection/L05/current/FFES" />
  </rdf:Description>
  <rdf:Description rdf:about="http://vocab.nerc.ac.uk/collection/L22/current/TOOL0058">
    <skos:broader rdf:resource="http://vocab.nerc.ac.uk/collection/L05/current/130" />
  </rdf:Description>
  <rdf:Description rdf:about="http://vocab.nerc.ac.uk/collection/L22/current/TOOL0126">
    <skos:broader rdf:resource="http://vocab.nerc.ac.uk/collection/L05/current/101" />
  </rdf:Description>
  <rdf:Description rdf:about="http://vocab.nerc.ac.uk/collection/L22/current/TOOL0667">
    <skos:broader rdf:resource="http://vocab.nerc.ac.uk/collection/L05/current/134" />
  </rdf:Description>
  <rdf:Description rdf:about="http://vocab.nerc.ac.uk/collection/L22/current/TOOL0058">
    <skos:broader rdf:resource="http://vocab.nerc.ac.uk/collection/L05/current/134" />
  </rdf:Description>
  <rdf:Description rdf:about="http://vocab.aodn.org.au/def/instrument/entity/545">
    <skos:broader rdf:resource="http://vocab.nerc.ac.uk/collection/L05/current/122" />
  </rdf:Description>
  <rdf:Description rdf:about="http://vocab.nerc.ac.uk/collection/L22/current/TOOL0667">
    <skos:broader rdf:resource="http://vocab.nerc.ac.uk/collection/L05/current/133" />
  </rdf:Description>
  <rdf:Description rdf:about="http://vocab.nerc.ac.uk/collection/L22/current/TOOL0190">
    <skos:broader rdf:resource="http://vocab.nerc.ac.uk/collection/L05/current/350" />
  </rdf:Description>
  <rdf:Description rdf:about="http://vocab.nerc.ac.uk/collection/L22/current/TOOL0878/">
    <skos:broader rdf:resource="http://vocab.nerc.ac.uk/collection/L05/current/351" />
  </rdf:Description>
  <rdf:Description rdf:about="http://vocab.nerc.ac.uk/collection/L22/current/TOOL0870/">
    <skos:broader rdf:resource="http://vocab.nerc.ac.uk/collection/L05/current/134" />
  </rdf:Description>
  <rdf:Description rdf:about="http://vocab.nerc.ac.uk/collection/L22/current/TOOL0037">
    <skos:broader rdf:resource="http://vocab.nerc.ac.uk/collection/L05/current/351" />
  </rdf:Description>
  <rdf:Description rdf:about="http://vocab.nerc.ac.uk/collection/L22/current/TOOL0036">
    <skos:broader rdf:resource="http://vocab.nerc.ac.uk/collection/L05/current/351" />
  </rdf:Description>
  <rdf:Description rdf:about="http://vocab.nerc.ac.uk/collection/L22/current/TOOL0675">
    <skos:broader rdf:resource="http://vocab.nerc.ac.uk/collection/L05/current/350" />
  </rdf:Description>
  <rdf:Description rdf:about="http://vocab.nerc.ac.uk/collection/L22/current/TOOL0445">
    <skos:broader rdf:resource="http://vocab.nerc.ac.uk/collection/L05/current/115" />
  </rdf:Description>
  <rdf:Description rdf:about="http://vocab.nerc.ac.uk/collection/L22/current/TOOL0675">
    <skos:broader rdf:resource="http://vocab.nerc.ac.uk/collection/L05/current/351" />
  </rdf:Description>
  <rdf:Description rdf:about="http://vocab.nerc.ac.uk/collection/L22/current/TOOL0786">
    <skos:broader rdf:resource="http://vocab.nerc.ac.uk/collection/L05/current/33" />
  </rdf:Description>
  <rdf:Description rdf:about="http://vocab.nerc.ac.uk/collection/L22/current/TOOL0017">
    <skos:broader rdf:resource="http://vocab.aodn.org.au/def/instrument/entity/365" />
  </rdf:Description>
  <rdf:Description rdf:about="http://vocab.nerc.ac.uk/collection/L22/current/TOOL0100">
    <skos:broader rdf:resource="http://vocab.aodn.org.au/def/instrument/entity/365" />
  </rdf:Description>
  <rdf:Description rdf:about="http://vocab.nerc.ac.uk/collection/L22/current/TOOL0781">
    <skos:broader rdf:resource="http://vocab.nerc.ac.uk/collection/L05/current/110" />
  </rdf:Description>
  <rdf:Description rdf:about="http://vocab.nerc.ac.uk/collection/L22/current/TOOL0625">
    <skos:broader rdf:resource="http://vocab.nerc.ac.uk/collection/L05/current/122" />
  </rdf:Description>
  <rdf:Description rdf:about="http://vocab.nerc.ac.uk/collection/L22/current/TOOL0719">
    <skos:broader rdf:resource="http://vocab.nerc.ac.uk/collection/L05/current/POS17" />
  </rdf:Description>
  <rdf:Description rdf:about="http://vocab.nerc.ac.uk/collection/L22/current/TOOL0670">
    <skos:broader rdf:resource="http://vocab.nerc.ac.uk/collection/L05/current/134" />
  </rdf:Description>
  <rdf:Description rdf:about="http://vocab.nerc.ac.uk/collection/L22/current/TOOL0888/">
    <skos:broader rdf:resource="http://vocab.nerc.ac.uk/collection/L05/current/134" />
  </rdf:Description>
  <rdf:Description rdf:about="http://vocab.nerc.ac.uk/collection/L22/current/TOOL0680">
    <skos:broader rdf:resource="http://vocab.nerc.ac.uk/collection/L05/current/111" />
  </rdf:Description>
  <rdf:Description rdf:about="http://vocab.nerc.ac.uk/collection/L22/current/TOOL0785">
    <skos:broader rdf:resource="http://vocab.nerc.ac.uk/collection/L05/current/33" />
  </rdf:Description>
  <rdf:Description rdf:about="http://vocab.nerc.ac.uk/collection/L22/current/TOOL0181">
    <skos:broader rdf:resource="http://vocab.nerc.ac.uk/collection/L05/current/134" />
  </rdf:Description>
  <rdf:Description rdf:about="http://vocab.nerc.ac.uk/collection/L22/current/TOOL0873/">
    <skos:broader rdf:resource="http://vocab.nerc.ac.uk/collection/L05/current/134" />
  </rdf:Description>
  <rdf:Description rdf:about="http://vocab.nerc.ac.uk/collection/L22/current/TOOL0020">
    <skos:broader rdf:resource="http://vocab.aodn.org.au/def/instrument/entity/365" />
  </rdf:Description>
  <rdf:Description rdf:about="http://vocab.nerc.ac.uk/collection/L22/current/TOOL0682">
    <skos:broader rdf:resource="http://vocab.nerc.ac.uk/collection/L05/current/102" />
  </rdf:Description>
  <rdf:Description rdf:about="http://vocab.nerc.ac.uk/collection/L22/current/TOOL0215">
    <skos:broader rdf:resource="http://vocab.nerc.ac.uk/collection/L05/current/123" />
  </rdf:Description>
  <rdf:Description rdf:about="http://vocab.nerc.ac.uk/collection/L22/current/TOOL0047">
    <skos:broader rdf:resource="http://vocab.nerc.ac.uk/collection/L05/current/350" />
  </rdf:Description>
  <rdf:Description rdf:about="http://vocab.nerc.ac.uk/collection/L22/current/TOOL0680">
    <skos:broader rdf:resource="http://vocab.nerc.ac.uk/collection/L05/current/102" />
  </rdf:Description>
  <rdf:Description rdf:about="http://vocab.nerc.ac.uk/collection/L22/current/TOOL0490">
    <skos:broader rdf:resource="http://vocab.nerc.ac.uk/collection/L05/current/385" />
  </rdf:Description>
  <rdf:Description rdf:about="http://vocab.nerc.ac.uk/collection/L22/current/TOOL0446">
    <skos:broader rdf:resource="http://vocab.nerc.ac.uk/collection/L05/current/134" />
  </rdf:Description>
  <rdf:Description rdf:about="http://vocab.nerc.ac.uk/collection/L22/current/TOOL0674">
    <skos:broader rdf:resource="http://vocab.nerc.ac.uk/collection/L05/current/123" />
  </rdf:Description>
  <rdf:Description rdf:about="http://vocab.nerc.ac.uk/collection/L22/current/TOOL0870/">
    <skos:broader rdf:resource="http://vocab.nerc.ac.uk/collection/L05/current/350" />
  </rdf:Description>
  <rdf:Description rdf:about="http://vocab.nerc.ac.uk/collection/L22/current/TOOL0416">
    <skos:broader rdf:resource="http://vocab.nerc.ac.uk/collection/L05/current/134" />
  </rdf:Description>
  <rdf:Description rdf:about="http://vocab.nerc.ac.uk/collection/L22/current/TOOL0703">
    <skos:broader rdf:resource="http://vocab.nerc.ac.uk/collection/L05/current/308" />
  </rdf:Description>
  <rdf:Description rdf:about="http://vocab.nerc.ac.uk/collection/L22/current/TOOL0683">
    <skos:broader rdf:resource="http://vocab.nerc.ac.uk/collection/L05/current/102" />
  </rdf:Description>
  <rdf:Description rdf:about="http://vocab.nerc.ac.uk/collection/L22/current/TOOL0872/">
    <skos:broader rdf:resource="http://vocab.nerc.ac.uk/collection/L05/current/385" />
  </rdf:Description>
  <rdf:Description rdf:about="http://vocab.nerc.ac.uk/collection/L22/current/TOOL0191">
    <skos:broader rdf:resource="http://vocab.nerc.ac.uk/collection/L05/current/134" />
  </rdf:Description>
  <rdf:Description rdf:about="http://vocab.nerc.ac.uk/collection/L22/current/TOOL0446">
    <skos:broader rdf:resource="http://vocab.nerc.ac.uk/collection/L05/current/130" />
  </rdf:Description>
  <rdf:Description rdf:about="http://vocab.nerc.ac.uk/collection/L22/current/TOOL0705">
    <skos:broader rdf:resource="http://vocab.nerc.ac.uk/collection/L05/current/382" />
  </rdf:Description>
  <rdf:Description rdf:about="http://vocab.nerc.ac.uk/collection/L22/current/TOOL0105">
    <skos:broader rdf:resource="http://vocab.nerc.ac.uk/collection/L05/current/134" />
  </rdf:Description>
  <rdf:Description rdf:about="http://vocab.nerc.ac.uk/collection/L22/current/TOOL0020">
    <skos:broader rdf:resource="http://vocab.nerc.ac.uk/collection/L05/current/134" />
  </rdf:Description>
  <rdf:Description rdf:about="http://vocab.nerc.ac.uk/collection/L22/current/NETT0044">
    <skos:broader rdf:resource="http://vocab.nerc.ac.uk/collection/L05/current/22" />
  </rdf:Description>
  <rdf:Description rdf:about="http://vocab.nerc.ac.uk/collection/L22/current/TOOL0739">
    <skos:broader rdf:resource="http://vocab.nerc.ac.uk/collection/L05/current/351" />
  </rdf:Description>
  <rdf:Description rdf:about="http://vocab.nerc.ac.uk/collection/L22/current/TOOL0706">
    <skos:broader rdf:resource="http://vocab.nerc.ac.uk/collection/L05/current/134" />
  </rdf:Description>
  <rdf:Description rdf:about="http://vocab.nerc.ac.uk/collection/L22/current/TOOL0671">
    <skos:broader rdf:resource="http://vocab.nerc.ac.uk/collection/L05/current/381" />
  </rdf:Description>
  <rdf:Description rdf:about="http://vocab.nerc.ac.uk/collection/L22/current/TOOL0723">
    <skos:broader rdf:resource="http://vocab.nerc.ac.uk/collection/L05/current/308" />
  </rdf:Description>
  <rdf:Description rdf:about="http://vocab.nerc.ac.uk/collection/L22/current/TOOL0873/">
    <skos:broader rdf:resource="http://vocab.nerc.ac.uk/collection/L05/current/POS03" />
  </rdf:Description>
  <rdf:Description rdf:about="http://vocab.nerc.ac.uk/collection/L22/current/TOOL0195">
    <skos:broader rdf:resource="http://vocab.nerc.ac.uk/collection/L05/current/101" />
  </rdf:Description>
  <rdf:Description rdf:about="http://vocab.nerc.ac.uk/collection/L22/current/TOOL0023">
    <skos:broader rdf:resource="http://vocab.aodn.org.au/def/instrument/entity/365" />
  </rdf:Description>
  <rdf:Description rdf:about="http://vocab.nerc.ac.uk/collection/L22/current/TOOL0676">
    <skos:broader rdf:resource="http://vocab.nerc.ac.uk/collection/L05/current/122" />
  </rdf:Description>
  <rdf:Description rdf:about="http://vocab.nerc.ac.uk/collection/L22/current/TOOL0722">
    <skos:broader rdf:resource="http://vocab.nerc.ac.uk/collection/L05/current/308" />
  </rdf:Description>
  <rdf:Description rdf:about="http://vocab.nerc.ac.uk/collection/L22/current/TOOL0053">
    <skos:broader rdf:resource="http://vocab.nerc.ac.uk/collection/L05/current/350" />
  </rdf:Description>
  <rdf:Description rdf:about="http://vocab.nerc.ac.uk/collection/L22/current/TOOL0687">
    <skos:broader rdf:resource="http://vocab.nerc.ac.uk/collection/L05/current/134" />
  </rdf:Description>
  <rdf:Description rdf:about="http://vocab.nerc.ac.uk/collection/L22/current/TOOL0724">
    <skos:broader rdf:resource="http://vocab.nerc.ac.uk/collection/L05/current/382" />
  </rdf:Description>
  <rdf:Description rdf:about="http://vocab.aodn.org.au/def/instrument/entity/37">
    <skos:broader rdf:resource="http://vocab.nerc.ac.uk/collection/L05/current/115" />
  </rdf:Description>
  <rdf:Description rdf:about="http://vocab.nerc.ac.uk/collection/L22/current/TOOL0725">
    <skos:broader rdf:resource="http://vocab.nerc.ac.uk/collection/L05/current/381" />
  </rdf:Description>
  <rdf:Description rdf:about="http://vocab.aodn.org.au/def/instrument/entity/39">
    <skos:broader rdf:resource="http://vocab.nerc.ac.uk/collection/L05/current/134" />
  </rdf:Description>
  <rdf:Description rdf:about="http://vocab.nerc.ac.uk/collection/L22/current/TOOL0688">
    <skos:broader rdf:resource="http://vocab.nerc.ac.uk/collection/L05/current/134" />
  </rdf:Description>
  <rdf:Description rdf:about="http://vocab.nerc.ac.uk/collection/L22/current/TOOL0672">
    <skos:broader rdf:resource="http://vocab.nerc.ac.uk/collection/L05/current/102" />
  </rdf:Description>
  <rdf:Description rdf:about="http://vocab.nerc.ac.uk/collection/L22/current/TOOL0023">
    <skos:broader rdf:resource="http://vocab.nerc.ac.uk/collection/L05/current/350" />
  </rdf:Description>
  <rdf:Description rdf:about="http://vocab.nerc.ac.uk/collection/L22/current/TOOL0679">
    <skos:broader rdf:resource="http://vocab.nerc.ac.uk/collection/L05/current/351" />
  </rdf:Description>
  <rdf:Description rdf:about="http://vocab.nerc.ac.uk/collection/L22/current/TOOL0100">
    <skos:broader rdf:resource="http://vocab.nerc.ac.uk/collection/L05/current/134" />
  </rdf:Description>
  <rdf:Description rdf:about="http://vocab.nerc.ac.uk/collection/L22/current/TOOL0215">
    <skos:broader rdf:resource="http://vocab.aodn.org.au/def/instrument/entity/361" />
  </rdf:Description>
  <rdf:Description rdf:about="http://vocab.aodn.org.au/def/instrument/entity/39">
    <skos:broader rdf:resource="http://vocab.nerc.ac.uk/collection/L05/current/132" />
  </rdf:Description>
  <rdf:Description rdf:about="http://vocab.nerc.ac.uk/collection/L22/current/TOOL0040">
    <skos:broader rdf:resource="http://vocab.nerc.ac.uk/collection/L05/current/130" />
  </rdf:Description>
  <rdf:Description rdf:about="http://vocab.nerc.ac.uk/collection/L22/current/TOOL0053">
    <skos:broader rdf:resource="http://vocab.aodn.org.au/def/instrument/entity/365" />
  </rdf:Description>
  <rdf:Description rdf:about="http://vocab.nerc.ac.uk/collection/L22/current/TOOL0127">
    <skos:broader rdf:resource="http://vocab.nerc.ac.uk/collection/L05/current/101" />
  </rdf:Description>
  <rdf:Description rdf:about="http://vocab.nerc.ac.uk/collection/L22/current/TOOL0022">
    <skos:broader rdf:resource="http://vocab.nerc.ac.uk/collection/L05/current/350" />
  </rdf:Description>
  <rdf:Description rdf:about="http://vocab.nerc.ac.uk/collection/L22/current/TOOL0215">
    <skos:broader rdf:resource="http://vocab.nerc.ac.uk/collection/L05/current/113" />
  </rdf:Description>
  <rdf:Description rdf:about="http://vocab.nerc.ac.uk/collection/L22/current/TOOL0018">
    <skos:broader rdf:resource="http://vocab.aodn.org.au/def/instrument/entity/365" />
  </rdf:Description>
  <rdf:Description rdf:about="http://vocab.nerc.ac.uk/collection/L22/current/TOOL0730">
    <skos:broader rdf:resource="http://vocab.nerc.ac.uk/collection/L05/current/130" />
  </rdf:Description>
  <rdf:Description rdf:about="http://vocab.nerc.ac.uk/collection/L22/current/TOOL0809">
    <skos:broader rdf:resource="http://vocab.nerc.ac.uk/collection/L05/current/111" />
  </rdf:Description>
  <rdf:Description rdf:about="http://vocab.nerc.ac.uk/collection/L22/current/TOOL0673">
    <skos:broader rdf:resource="http://vocab.nerc.ac.uk/collection/L05/current/113" />
  </rdf:Description>
  <rdf:Description rdf:about="http://vocab.nerc.ac.uk/collection/L22/current/TOOL0040">
    <skos:broader rdf:resource="http://vocab.nerc.ac.uk/collection/L05/current/134" />
  </rdf:Description>
  <rdf:Description rdf:about="http://vocab.nerc.ac.uk/collection/L22/current/TOOL0267">
    <skos:broader rdf:resource="http://vocab.nerc.ac.uk/collection/L05/current/134" />
  </rdf:Description>
  <rdf:Description rdf:about="http://vocab.nerc.ac.uk/collection/L22/current/TOOL0720">
    <skos:broader rdf:resource="http://vocab.nerc.ac.uk/collection/L05/current/113" />
  </rdf:Description>
  <rdf:Description rdf:about="http://vocab.nerc.ac.uk/collection/L22/current/TOOL0120">
    <skos:broader rdf:resource="http://vocab.nerc.ac.uk/collection/L05/current/122" />
  </rdf:Description>
  <rdf:Description rdf:about="http://vocab.nerc.ac.uk/collection/L22/current/TOOL0677">
    <skos:broader rdf:resource="http://vocab.nerc.ac.uk/collection/L05/current/102" />
  </rdf:Description>
  <rdf:Description rdf:about="http://vocab.nerc.ac.uk/collection/L22/current/TOOL0673">
    <skos:broader rdf:resource="http://vocab.nerc.ac.uk/collection/L05/current/123" />
  </rdf:Description>
  <rdf:Description rdf:about="http://vocab.nerc.ac.uk/collection/L22/current/TOOL0490">
    <skos:broader rdf:resource="http://vocab.nerc.ac.uk/collection/L05/current/134" />
  </rdf:Description>
  <rdf:Description rdf:about="http://vocab.nerc.ac.uk/collection/L22/current/TOOL0808">
    <skos:broader rdf:resource="http://vocab.nerc.ac.uk/collection/L05/current/102" />
  </rdf:Description>
  <rdf:Description rdf:about="http://vocab.nerc.ac.uk/collection/L22/current/TOOL0477">
    <skos:broader rdf:resource="http://vocab.nerc.ac.uk/collection/L05/current/114" />
  </rdf:Description>
  <rdf:Description rdf:about="http://vocab.nerc.ac.uk/collection/L22/current/TOOL0476">
    <skos:broader rdf:resource="http://vocab.nerc.ac.uk/collection/L05/current/114" />
  </rdf:Description>
  <rdf:Description rdf:about="http://vocab.nerc.ac.uk/collection/L22/current/TOOL0708">
    <skos:broader rdf:resource="http://vocab.nerc.ac.uk/collection/L05/current/111" />
  </rdf:Description>
  <rdf:Description rdf:about="http://vocab.nerc.ac.uk/collection/L22/current/TOOL0898/">
    <skos:broader rdf:resource="http://vocab.nerc.ac.uk/collection/L05/current/134" />
  </rdf:Description>
  <rdf:Description rdf:about="http://vocab.nerc.ac.uk/collection/L22/current/TOOL0263">
    <skos:broader rdf:resource="http://vocab.nerc.ac.uk/collection/L05/current/132" />
  </rdf:Description>
  <rdf:Description rdf:about="http://vocab.nerc.ac.uk/collection/L22/current/TOOL0640">
    <skos:broader rdf:resource="http://vocab.nerc.ac.uk/collection/L05/current/134" />
  </rdf:Description>
  <rdf:Description rdf:about="http://vocab.nerc.ac.uk/collection/L22/current/TOOL0720">
    <skos:broader rdf:resource="http://vocab.nerc.ac.uk/collection/L05/current/POS17" />
  </rdf:Description>
  <rdf:Description rdf:about="http://vocab.nerc.ac.uk/collection/L22/current/TOOL0873/">
    <skos:broader rdf:resource="http://vocab.nerc.ac.uk/collection/L05/current/WPS" />
  </rdf:Description>
  <rdf:Description rdf:about="http://vocab.nerc.ac.uk/collection/L22/current/TOOL0058">
    <skos:broader rdf:resource="http://vocab.nerc.ac.uk/collection/L05/current/350" />
  </rdf:Description>
  <rdf:Description rdf:about="http://vocab.nerc.ac.uk/collection/L22/current/TOOL0023">
    <skos:broader rdf:resource="http://vocab.nerc.ac.uk/collection/L05/current/134" />
  </rdf:Description>
  <rdf:Description rdf:about="http://vocab.nerc.ac.uk/collection/L22/current/TOOL0089">
    <skos:broader rdf:resource="http://vocab.nerc.ac.uk/collection/L05/current/114" />
  </rdf:Description>
  <rdf:Description rdf:about="http://vocab.nerc.ac.uk/collection/L22/current/TOOL0702">
    <skos:broader rdf:resource="http://vocab.nerc.ac.uk/collection/L05/current/308" />
  </rdf:Description>
  <rdf:Description rdf:about="http://vocab.nerc.ac.uk/collection/L22/current/TOOL0780">
    <skos:broader rdf:resource="http://vocab.nerc.ac.uk/collection/L05/current/102" />
  </rdf:Description>
  <rdf:Description rdf:about="http://vocab.nerc.ac.uk/collection/L22/current/TOOL0878/">
    <skos:broader rdf:resource="http://vocab.nerc.ac.uk/collection/L05/current/POS03" />
  </rdf:Description>
  <rdf:Description rdf:about="http://vocab.nerc.ac.uk/collection/L22/current/TOOL0704">
    <skos:broader rdf:resource="http://vocab.nerc.ac.uk/collection/L05/current/101" />
  </rdf:Description>
  <rdf:Description rdf:about="http://vocab.nerc.ac.uk/collection/L22/current/TOOL0724">
    <skos:broader rdf:resource="http://vocab.nerc.ac.uk/collection/L05/current/351" />
  </rdf:Description>
  <rdf:Description rdf:about="http://vocab.nerc.ac.uk/collection/L22/current/TOOL0710">
    <skos:broader rdf:resource="http://vocab.nerc.ac.uk/collection/L05/current/110" />
  </rdf:Description>
  <rdf:Description rdf:about="http://vocab.nerc.ac.uk/collection/L22/current/TOOL0888/">
    <skos:broader rdf:resource="http://vocab.nerc.ac.uk/collection/L05/current/115" />
  </rdf:Description>
  <rdf:Description rdf:about="http://vocab.nerc.ac.uk/collection/L22/current/TOOL0707">
    <skos:broader rdf:resource="http://vocab.nerc.ac.uk/collection/L05/current/134" />
  </rdf:Description>
  <rdf:Description rdf:about="http://vocab.nerc.ac.uk/collection/L22/current/TOOL0173">
    <skos:broader rdf:resource="http://vocab.nerc.ac.uk/collection/L05/current/350" />
  </rdf:Description>
  <rdf:Description rdf:about="http://vocab.nerc.ac.uk/collection/L22/current/TOOL0809">
    <skos:broader rdf:resource="http://vocab.nerc.ac.uk/collection/L05/current/134" />
  </rdf:Description>
  <rdf:Description rdf:about="http://vocab.nerc.ac.uk/collection/L22/current/TOOL0054">
    <skos:broader rdf:resource="http://vocab.nerc.ac.uk/collection/L05/current/134" />
  </rdf:Description>
  <rdf:Description rdf:about="http://vocab.nerc.ac.uk/collection/L22/current/TOOL0684">
    <skos:broader rdf:resource="http://vocab.nerc.ac.uk/collection/L05/current/134" />
  </rdf:Description>
  <rdf:Description rdf:about="http://vocab.nerc.ac.uk/collection/L22/current/TOOL0720">
    <skos:broader rdf:resource="http://vocab.nerc.ac.uk/collection/L05/current/130" />
    <skos:broader rdf:resource="http://vocab.nerc.ac.uk/collection/L05/current/134" />
  </rdf:Description>
  <rdf:Description rdf:about="http://vocab.nerc.ac.uk/collection/L22/current/TOOL0779">
    <skos:broader rdf:resource="http://vocab.nerc.ac.uk/collection/L05/current/102" />
  </rdf:Description>
</rdf:RDF>

